<?xml version="1.0"?>
<rdf:RDF xmlns="http://w3id.org/cacao/cacao.owl#"
     xml:base="http://w3id.org/cacao/cacao.owl"
     xmlns:dce="http://purl.org/dc/elements/1.1/"
     xmlns:owl="http://www.w3.org/2002/07/owl#"
     xmlns:rdf="http://www.w3.org/1999/02/22-rdf-syntax-ns#"
     xmlns:xml="http://www.w3.org/XML/1998/namespace"
     xmlns:xsd="http://www.w3.org/2001/XMLSchema#"
     xmlns:odrl="http://www.w3.org/ns/odrl/2/"
     xmlns:rdfs="http://www.w3.org/2000/01/rdf-schema#"
     xmlns:skos="http://www.w3.org/2004/02/skos/core#"
     xmlns:schema="https://schema.org/"
     xmlns:dcterms="http://purl.org/dc/terms/">
    <owl:Ontology rdf:about="http://w3id.org/cacao/cacao.owl">
        <owl:versionIRI rdf:resource="http://w3id.org/cacao/cacao/releases/2025-05-08/cacao.owl"/>
        <dcterms:description>None</dcterms:description>
        <dcterms:license rdf:resource="https://creativecommons.org/licenses/unspecified"/>
        <dcterms:title>Cultural Artefact Contextual Ontology</dcterms:title>
        <owl:versionInfo>2025-05-08</owl:versionInfo>
    </owl:Ontology>
    


    <!-- 
    ///////////////////////////////////////////////////////////////////////////////////////
    //
    // Annotation properties
    //
    ///////////////////////////////////////////////////////////////////////////////////////
     -->

    


    <!-- http://purl.org/dc/elements/1.1/description -->

    <owl:AnnotationProperty rdf:about="http://purl.org/dc/elements/1.1/description"/>
    


    <!-- http://purl.org/dc/elements/1.1/source -->

    <owl:AnnotationProperty rdf:about="http://purl.org/dc/elements/1.1/source"/>
    


    <!-- http://purl.org/dc/elements/1.1/title -->

    <owl:AnnotationProperty rdf:about="http://purl.org/dc/elements/1.1/title"/>
    


    <!-- http://purl.org/dc/terms/contributor -->

    <owl:AnnotationProperty rdf:about="http://purl.org/dc/terms/contributor"/>
    


    <!-- http://purl.org/dc/terms/creator -->

    <owl:AnnotationProperty rdf:about="http://purl.org/dc/terms/creator"/>
    


    <!-- http://purl.org/dc/terms/date -->

    <owl:AnnotationProperty rdf:about="http://purl.org/dc/terms/date"/>
    


    <!-- http://purl.org/dc/terms/description -->

    <owl:AnnotationProperty rdf:about="http://purl.org/dc/terms/description">
        <rdfs:label>description</rdfs:label>
    </owl:AnnotationProperty>
    


    <!-- http://purl.org/dc/terms/license -->

    <owl:AnnotationProperty rdf:about="http://purl.org/dc/terms/license">
        <rdfs:label>license</rdfs:label>
    </owl:AnnotationProperty>
    


    <!-- http://purl.org/dc/terms/modified -->

    <owl:AnnotationProperty rdf:about="http://purl.org/dc/terms/modified"/>
    


    <!-- http://purl.org/dc/terms/title -->

    <owl:AnnotationProperty rdf:about="http://purl.org/dc/terms/title">
        <rdfs:label>title</rdfs:label>
    </owl:AnnotationProperty>
    


    <!-- http://www.w3.org/2004/02/skos/core#broader -->

    <owl:AnnotationProperty rdf:about="http://www.w3.org/2004/02/skos/core#broader"/>
    


    <!-- http://www.w3.org/2004/02/skos/core#definition -->

    <owl:AnnotationProperty rdf:about="http://www.w3.org/2004/02/skos/core#definition"/>
    


    <!-- http://www.w3.org/2004/02/skos/core#exactMatch -->

    <owl:AnnotationProperty rdf:about="http://www.w3.org/2004/02/skos/core#exactMatch"/>
    


    <!-- http://www.w3.org/2004/02/skos/core#member -->

    <owl:AnnotationProperty rdf:about="http://www.w3.org/2004/02/skos/core#member"/>
    


    <!-- http://www.w3.org/2004/02/skos/core#notation -->

    <owl:AnnotationProperty rdf:about="http://www.w3.org/2004/02/skos/core#notation"/>
    


    <!-- http://www.w3.org/2004/02/skos/core#note -->

    <owl:AnnotationProperty rdf:about="http://www.w3.org/2004/02/skos/core#note"/>
    


    <!-- http://www.w3.org/2004/02/skos/core#prefLabel -->

    <owl:AnnotationProperty rdf:about="http://www.w3.org/2004/02/skos/core#prefLabel"/>
    


    <!-- http://www.w3.org/2004/02/skos/core#scopeNote -->

    <owl:AnnotationProperty rdf:about="http://www.w3.org/2004/02/skos/core#scopeNote"/>
    


    <!-- 
    ///////////////////////////////////////////////////////////////////////////////////////
    //
    // Datatypes
    //
    ///////////////////////////////////////////////////////////////////////////////////////
     -->

    


    <!-- http://www.w3.org/2001/XMLSchema#date -->

    <rdfs:Datatype rdf:about="http://www.w3.org/2001/XMLSchema#date"/>
    


    <!-- 
    ///////////////////////////////////////////////////////////////////////////////////////
    //
    // Object Properties
    //
    ///////////////////////////////////////////////////////////////////////////////////////
     -->

    


    <!-- http://w3id.org/cacao/CACAO_0000017 -->

    <owl:ObjectProperty rdf:about="http://w3id.org/cacao/CACAO_0000017">
        <rdfs:domain rdf:resource="http://www.cidoc-crm.org/cidoc-crm/E1_CRM_Entity"/>
        <rdfs:range rdf:resource="http://w3id.org/cacao/CACAO_0000027"/>
        <dcterms:contributor rdf:resource="https://orcid.org/0000-0002-0905-7033"/>
        <dcterms:date rdf:datatype="http://www.w3.org/2001/XMLSchema#dateTime">2025-04-10T14:50:30Z</dcterms:date>
        <rdfs:comment xml:lang="en">Quantification: Many-to-many (0,n: 0,n)

Scope note:
This property associates an Entity with a particular Genre. The Genre is defined as a subclass of E55 Type and represents a category of artistic, stylistic, thematic, or aesthetic classification. Whether applied to an artist or a creative work, the property genre consistently indicates the genre within which the work or the artist’s creative output is situated. 

Examples:
- An artist might be associated with the genre &quot;Impressionism&quot; to indicate that their body of work is typically aligned with this artistic style.
- A painting (as a physical artefact) may be categorized under &quot;Portrait&quot; to denote the genre of the artwork.</rdfs:comment>
        <rdfs:label xml:lang="en">genre</rdfs:label>
    </owl:ObjectProperty>
    


    <!-- http://w3id.org/cacao/CACAO_0000018 -->

    <owl:ObjectProperty rdf:about="http://w3id.org/cacao/CACAO_0000018">
        <rdf:type rdf:resource="http://www.w3.org/2002/07/owl#IrreflexiveProperty"/>
        <rdfs:domain rdf:resource="http://www.cidoc-crm.org/cidoc-crm/E1_CRM_Entity"/>
        <rdfs:range rdf:resource="http://w3id.org/cacao/CACAO_0000010"/>
        <dcterms:contributor rdf:resource="https://orcid.org/0000-0002-0905-7033"/>
        <dcterms:date rdf:datatype="http://www.w3.org/2001/XMLSchema#dateTime">2025-04-10T14:51:45Z</dcterms:date>
        <rdfs:comment xml:lang="en">Quantification: Many-to-many (0,n: 0,n)

Scope note:
This property associates an Entity with a specific Social Movement. A Social Movement is defined as a loosely organized effort by a large group of people to achieve a particular set of goals (e.g., political, cultural, or religious change). Through this property, one can record an artist’s participation in or influence from a social movement and, similarly, document how a creative work may be representative of or inspired by such a movement. 

Examples:
- An artist (E21 Person) who was actively involved in the Civil Rights Movement might be linked via the movement property to that Social Movement.
- A poster or photograph (E22 Physical Artefact) produced during a protest could be associated with the relevant Social Movement that motivated its creation.</rdfs:comment>
        <rdfs:label xml:lang="en">socialMovement</rdfs:label>
    </owl:ObjectProperty>
    


    <!-- http://w3id.org/cacao/CACAO_0000026 -->

    <owl:ObjectProperty rdf:about="http://w3id.org/cacao/CACAO_0000026">
        <rdfs:subPropertyOf rdf:resource="http://www.w3.org/2002/07/owl#topObjectProperty"/>
        <rdfs:domain rdf:resource="http://www.cidoc-crm.org/cidoc-crm/E39_Actor"/>
        <rdfs:range rdf:resource="http://w3id.org/cacao/CACAO_0000028"/>
        <dcterms:contributor rdf:resource="https://orcid.org/0000-0002-0905-7033"/>
        <dcterms:date rdf:datatype="http://www.w3.org/2001/XMLSchema#dateTime">2025-04-11T10:40:25Z</dcterms:date>
        <rdfs:comment xml:lang="en">Quantification: Many-to-many (0,n: 0,n)

Scope note:
This property links an instance of an Actor (typically an instance of E21 Person) with a Field of Work, an element of the controlled vocabulary defined as a subclass of E55 Type. It is used to classify the professional or creative domain in which an Actor (especially an artist) is active. 

Examples:
- An artist (E21 Person) might have a fieldOfWork assignment indicating they work in “Painting” (an instance of Field of Work).
- A creator could be linked to the fieldOfWork “Sculpture” as well as “Mixed Media,” reflecting multiple areas of engagement.</rdfs:comment>
        <rdfs:label xml:lang="en">fieldOfWork</rdfs:label>
    </owl:ObjectProperty>
    


    <!-- http://w3id.org/cacao/CACAO_0000030 -->

    <owl:ObjectProperty rdf:about="http://w3id.org/cacao/CACAO_0000030">
        <rdfs:subPropertyOf rdf:resource="http://www.cidoc-crm.org/cidoc-crm/P40_observed_dimension"/>
        <dcterms:contributor rdf:resource="https://orcid.org/0000-0002-0905-7033"/>
        <dcterms:date rdf:datatype="http://www.w3.org/2001/XMLSchema#dateTime">2025-04-12T09:12:56Z</dcterms:date>
        <rdfs:label xml:lang="en">height</rdfs:label>
    </owl:ObjectProperty>
    


    <!-- http://w3id.org/cacao/CACAO_0000031 -->

    <owl:ObjectProperty rdf:about="http://w3id.org/cacao/CACAO_0000031">
        <rdfs:subPropertyOf rdf:resource="http://www.cidoc-crm.org/cidoc-crm/P40_observed_dimension"/>
        <dcterms:contributor rdf:resource="https://orcid.org/0000-0002-0905-7033"/>
        <dcterms:date rdf:datatype="http://www.w3.org/2001/XMLSchema#dateTime">2025-04-12T09:12:56Z</dcterms:date>
        <rdfs:label xml:lang="en">width</rdfs:label>
    </owl:ObjectProperty>
    


    <!-- http://w3id.org/cacao/CACAO_0000032 -->

    <owl:ObjectProperty rdf:about="http://w3id.org/cacao/CACAO_0000032">
        <rdfs:subPropertyOf rdf:resource="http://www.cidoc-crm.org/cidoc-crm/P40_observed_dimension"/>
        <dcterms:contributor rdf:resource="https://orcid.org/0000-0002-0905-7033"/>
        <dcterms:date rdf:datatype="http://www.w3.org/2001/XMLSchema#dateTime">2025-04-12T09:12:56Z</dcterms:date>
        <rdfs:label xml:lang="en">diameter</rdfs:label>
    </owl:ObjectProperty>
    


    <!-- http://w3id.org/cacao/CACAO_0000033 -->

    <owl:ObjectProperty rdf:about="http://w3id.org/cacao/CACAO_0000033">
        <rdfs:subPropertyOf rdf:resource="http://www.cidoc-crm.org/cidoc-crm/P40_observed_dimension"/>
        <dcterms:contributor rdf:resource="https://orcid.org/0000-0002-0905-7033"/>
        <dcterms:date rdf:datatype="http://www.w3.org/2001/XMLSchema#dateTime">2025-04-12T09:12:56Z</dcterms:date>
        <rdfs:label xml:lang="en">thickness</rdfs:label>
    </owl:ObjectProperty>
    


    <!-- http://w3id.org/cacao/CACAO_0000034 -->

    <owl:ObjectProperty rdf:about="http://w3id.org/cacao/CACAO_0000034">
        <rdfs:subPropertyOf rdf:resource="http://www.cidoc-crm.org/cidoc-crm/P40_observed_dimension"/>
        <dcterms:contributor rdf:resource="https://orcid.org/0000-0002-0905-7033"/>
        <dcterms:date rdf:datatype="http://www.w3.org/2001/XMLSchema#dateTime">2025-04-12T09:12:56Z</dcterms:date>
        <rdfs:label xml:lang="en">length</rdfs:label>
    </owl:ObjectProperty>
    


    <!-- http://w3id.org/cacao/CACAO_0000035 -->

    <owl:ObjectProperty rdf:about="http://w3id.org/cacao/CACAO_0000035">
        <rdfs:subPropertyOf rdf:resource="http://www.w3.org/2002/07/owl#topObjectProperty"/>
        <rdfs:domain rdf:resource="http://www.cidoc-crm.org/cidoc-crm/E1_CRM_Entity"/>
        <rdfs:range rdf:resource="http://w3id.org/cacao/CACAO_0000036"/>
        <dcterms:contributor rdf:resource="https://orcid.org/0000-0002-0905-7033"/>
        <dcterms:date rdf:datatype="http://www.w3.org/2001/XMLSchema#dateTime">2025-04-12T09:16:19Z</dcterms:date>
        <rdfs:comment xml:lang="en"></rdfs:comment>
        <rdfs:comment xml:lang="en">Quantification: Many-to-many (0,n: 0,n)

Scope note:
This property associates an entity,such as a person (e.g., an artist) or a physical artefact (e.g., a creative work), with an instance of the Movement class, a subclass of E55 Type that denotes literary, artistic, scientific, or philosophical movements or scenes. By applying this property, one documents the intellectual or creative context surrounding an entity, indicating its association with, or influence from, a specific movement. 

Examples:
- An artist might be associated with the movement Modernism.
- A painting might be linked to the artistic movement Impressionism.
- A literary work might be classified under the movement Romanticism.</rdfs:comment>
        <rdfs:label xml:lang="en">movement</rdfs:label>
    </owl:ObjectProperty>
    


    <!-- http://w3id.org/cacao/CACAO_0000038 -->

    <owl:ObjectProperty rdf:about="http://w3id.org/cacao/CACAO_0000038">
        <rdfs:subPropertyOf rdf:resource="http://www.cidoc-crm.org/cidoc-crm/P1_is_identified_by"/>
        <dcterms:contributor rdf:resource="https://orcid.org/0000-0002-0905-7033"/>
        <dcterms:date rdf:datatype="http://www.w3.org/2001/XMLSchema#dateTime">2025-04-12T10:00:52Z</dcterms:date>
        <rdfs:label xml:lang="en">website</rdfs:label>
    </owl:ObjectProperty>
    


    <!-- http://w3id.org/cacao/CACAO_0000039 -->

    <owl:ObjectProperty rdf:about="http://w3id.org/cacao/CACAO_0000039">
        <rdfs:subPropertyOf rdf:resource="http://www.cidoc-crm.org/cidoc-crm/P1_is_identified_by"/>
        <dcterms:contributor rdf:resource="https://orcid.org/0000-0002-0905-7033"/>
        <dcterms:date rdf:datatype="http://www.w3.org/2001/XMLSchema#dateTime">2025-04-12T10:00:52Z</dcterms:date>
        <rdfs:label xml:lang="en">europeana</rdfs:label>
    </owl:ObjectProperty>
    


    <!-- http://w3id.org/cacao/CACAO_0000040 -->

    <owl:ObjectProperty rdf:about="http://w3id.org/cacao/CACAO_0000040">
        <rdfs:subPropertyOf rdf:resource="http://www.w3.org/2002/07/owl#topObjectProperty"/>
        <rdfs:domain rdf:resource="http://www.cidoc-crm.org/cidoc-crm/E39_Actor"/>
        <rdfs:range rdf:resource="http://www.cidoc-crm.org/cidoc-crm/E39_Actor"/>
        <dcterms:contributor rdf:resource="https://orcid.org/0000-0002-0905-7033"/>
        <dcterms:date rdf:datatype="http://www.w3.org/2001/XMLSchema#dateTime">2025-04-12T10:13:16Z</dcterms:date>
        <rdfs:comment>Scope note:
The property partner denotes that an Actor has committed to a partnership with another Actor.</rdfs:comment>
        <rdfs:label xml:lang="en">partner</rdfs:label>
    </owl:ObjectProperty>
    


    <!-- http://www.cidoc-crm.org/cidoc-crm/P100_was_death_of -->

    <owl:ObjectProperty rdf:about="http://www.cidoc-crm.org/cidoc-crm/P100_was_death_of">
        <rdfs:subPropertyOf rdf:resource="http://www.cidoc-crm.org/cidoc-crm/P93_took_out_of_existence"/>
        <owl:inverseOf rdf:resource="http://www.cidoc-crm.org/cidoc-crm/P100i_died_in"/>
        <rdfs:domain rdf:resource="http://www.cidoc-crm.org/cidoc-crm/E69_Death"/>
        <rdfs:range rdf:resource="http://www.cidoc-crm.org/cidoc-crm/E21_Person"/>
        <rdfs:comment xml:lang="en">Quantification: one to many, necessary (1,n:0,1)

Scope note:
This property links an instance of E69 Death to the instance of E21 Person that died.
An instance of E69 Death may involve multiple people, for example in the case of a battle or disaster.
This is not intended for use with general natural history material, only people.

Examples:
- Mozart’s death (E69) was death of Mozart (E21). (Sitwell, 2017)

In First Order Logic:
- P100(x,y) ⇒ E69(x)
- P100(x,y) ⇒ E21(y)
- P100(x,y) ⇒ P93(x,y)
</rdfs:comment>
        <rdfs:label xml:lang="de">P100 Tod von</rdfs:label>
        <rdfs:label xml:lang="fr">P100 a été la mort de</rdfs:label>
        <rdfs:label xml:lang="pt">P100 foi a morte para</rdfs:label>
        <rdfs:label xml:lang="en">P100 was death of</rdfs:label>
        <rdfs:label xml:lang="el">P100 ήταν θάνατος του/της</rdfs:label>
        <rdfs:label xml:lang="ru">P100 привёл к смeрти</rdfs:label>
        <rdfs:label xml:lang="zh">P100 死亡的是</rdfs:label>
        <skos:notation xml:lang="en">P100</skos:notation>
        <skos:prefLabel xml:lang="de">Tod von</skos:prefLabel>
        <skos:prefLabel xml:lang="fr">a été la mort de</skos:prefLabel>
        <skos:prefLabel xml:lang="pt">foi a morte para</skos:prefLabel>
        <skos:prefLabel xml:lang="en">was death of</skos:prefLabel>
        <skos:prefLabel xml:lang="el">ήταν θάνατος του/της</skos:prefLabel>
        <skos:prefLabel xml:lang="ru">привёл к смeрти</skos:prefLabel>
        <skos:prefLabel xml:lang="zh">死亡的是</skos:prefLabel>
    </owl:ObjectProperty>
    


    <!-- http://www.cidoc-crm.org/cidoc-crm/P100i_died_in -->

    <owl:ObjectProperty rdf:about="http://www.cidoc-crm.org/cidoc-crm/P100i_died_in">
        <rdfs:subPropertyOf rdf:resource="http://www.cidoc-crm.org/cidoc-crm/P93i_was_taken_out_of_existence_by"/>
        <rdfs:domain rdf:resource="http://www.cidoc-crm.org/cidoc-crm/E21_Person"/>
        <rdfs:range rdf:resource="http://www.cidoc-crm.org/cidoc-crm/E69_Death"/>
        <rdfs:comment xml:lang="en">Quantification of the inverse property: one to many, necessary (1,n:0,1)

Scope note of the inverse property:
This property links an instance of E69 Death to the instance of E21 Person that died.
An instance of E69 Death may involve multiple people, for example in the case of a battle or disaster.
This is not intended for use with general natural history material, only people.

Examples of the inverse property:
- Mozart’s death (E69) was death of Mozart (E21). (Sitwell, 2017)

In First Order Logic of the inverse property:
- P100(x,y) ⇒ E69(x)
- P100(x,y) ⇒ E21(y)
- P100(x,y) ⇒ P93(x,y)
</rdfs:comment>
        <rdfs:label xml:lang="en">P100i died in</rdfs:label>
        <rdfs:label xml:lang="fr">P100i est mort par</rdfs:label>
        <rdfs:label xml:lang="pt">P100i morreu em</rdfs:label>
        <rdfs:label xml:lang="de">P100i starb in</rdfs:label>
        <rdfs:label xml:lang="el">P100i πέθανε σε</rdfs:label>
        <rdfs:label xml:lang="ru">P100i умeр</rdfs:label>
        <rdfs:label xml:lang="zh">P100i 死于</rdfs:label>
        <skos:notation xml:lang="en">P100i</skos:notation>
        <skos:prefLabel xml:lang="en">died in</skos:prefLabel>
        <skos:prefLabel xml:lang="fr">est mort par</skos:prefLabel>
        <skos:prefLabel xml:lang="pt">morreu em</skos:prefLabel>
        <skos:prefLabel xml:lang="de">starb in</skos:prefLabel>
        <skos:prefLabel xml:lang="el">πέθανε σε</skos:prefLabel>
        <skos:prefLabel xml:lang="ru">умeр</skos:prefLabel>
        <skos:prefLabel xml:lang="zh">死于</skos:prefLabel>
    </owl:ObjectProperty>
    


    <!-- http://www.cidoc-crm.org/cidoc-crm/P102_has_title -->

    <owl:ObjectProperty rdf:about="http://www.cidoc-crm.org/cidoc-crm/P102_has_title">
        <rdfs:subPropertyOf rdf:resource="http://www.cidoc-crm.org/cidoc-crm/P1_is_identified_by"/>
        <owl:inverseOf rdf:resource="http://www.cidoc-crm.org/cidoc-crm/P102i_is_title_of"/>
        <rdfs:domain rdf:resource="http://www.cidoc-crm.org/cidoc-crm/E71_Human-Made_Thing"/>
        <rdfs:range rdf:resource="http://www.cidoc-crm.org/cidoc-crm/E35_Title"/>
        <rdfs:comment xml:lang="en">Quantification: many to many (0,n:0,n)

Scope note:
This property associates an instance of E35 Title that has been applied to an instance of E71 Human-Made Thing. 
The P102.1 has type property of the P102 has title (is title of) property enables the relationship between the title and the thing to be further clarified, for example, if the title was a given title, a supplied title etc.
It allows any human-made material or immaterial thing to be given a title. It is possible to imagine a title being created without a specific object in mind.

Examples:
- The first book of the Old Testament (E33) has title “Genesis” (E35) has type translated title (E55) (E55). (Brueggemann, 1982)
- Monet’s painting from 1868-1869 held by Musée d’Orsay, Paris, under inventory number RF 1984 164 (E22) has title “La Pie” (E35) has type creator’s title (E55). (Musée d’Orsay, 2020)
- Monet’s painting from 1868-1869 held by Musée d&apos;Orsay, Paris, under inventory number RF 1984 164 (E22) has title “The Magpie” (E35) has type translated title (E55). (Musée d&apos;Orsay, 2020)

Properties:
- P102.1 has type: E55 Type

In First Order Logic:
- P102(x,y) ⇒ E71(x)
- P102(x,y) ⇒ E35(y) 
- P102(x,y,z) ⇒ [P102(x,y) ∧ E55(z)]
- P102(x,y) ⇒ P1(x,y)
</rdfs:comment>
        <rdfs:label xml:lang="fr">P102 a pour titre</rdfs:label>
        <rdfs:label xml:lang="en">P102 has title</rdfs:label>
        <rdfs:label xml:lang="pt">P102 tem título</rdfs:label>
        <rdfs:label xml:lang="de">P102 trägt den Titel</rdfs:label>
        <rdfs:label xml:lang="el">P102 έχει τίτλο</rdfs:label>
        <rdfs:label xml:lang="ru">P102 имeeт названиe</rdfs:label>
        <rdfs:label xml:lang="zh">P102 有题名</rdfs:label>
        <skos:notation xml:lang="en">P102</skos:notation>
        <skos:prefLabel xml:lang="fr">a pour titre</skos:prefLabel>
        <skos:prefLabel xml:lang="en">has title</skos:prefLabel>
        <skos:prefLabel xml:lang="pt">tem título</skos:prefLabel>
        <skos:prefLabel xml:lang="de">trägt den Titel</skos:prefLabel>
        <skos:prefLabel xml:lang="el">έχει τίτλο</skos:prefLabel>
        <skos:prefLabel xml:lang="ru">имeeт названиe</skos:prefLabel>
        <skos:prefLabel xml:lang="zh">有题名</skos:prefLabel>
    </owl:ObjectProperty>
    


    <!-- http://www.cidoc-crm.org/cidoc-crm/P102i_is_title_of -->

    <owl:ObjectProperty rdf:about="http://www.cidoc-crm.org/cidoc-crm/P102i_is_title_of">
        <rdfs:subPropertyOf rdf:resource="http://www.cidoc-crm.org/cidoc-crm/P1i_identifies"/>
        <rdfs:domain rdf:resource="http://www.cidoc-crm.org/cidoc-crm/E35_Title"/>
        <rdfs:range rdf:resource="http://www.cidoc-crm.org/cidoc-crm/E71_Human-Made_Thing"/>
        <rdfs:comment xml:lang="en">Quantification of the inverse property: many to many (0,n:0,n)

Scope note of the inverse property:
This property associates an instance of E35 Title that has been applied to an instance of E71 Human-Made Thing. 
The P102.1 has type property of the P102 has title (is title of) property enables the relationship between the title and the thing to be further clarified, for example, if the title was a given title, a supplied title etc.
It allows any human-made material or immaterial thing to be given a title. It is possible to imagine a title being created without a specific object in mind.

Examples of the inverse property:
- The first book of the Old Testament (E33) has title “Genesis” (E35) has type translated title (E55) (E55). (Brueggemann, 1982)
- Monet’s painting from 1868-1869 held by Musée d’Orsay, Paris, under inventory number RF 1984 164 (E22) has title “La Pie” (E35) has type creator’s title (E55). (Musée d’Orsay, 2020)
- Monet’s painting from 1868-1869 held by Musée d&apos;Orsay, Paris, under inventory number RF 1984 164 (E22) has title “The Magpie” (E35) has type translated title (E55). (Musée d&apos;Orsay, 2020)

In First Order Logic of the inverse property:
- P102(x,y) ⇒ E71(x)
- P102(x,y) ⇒ E35(y) 
- P102(x,y,z) ⇒ [P102(x,y) ∧ E55(z)]
- P102(x,y) ⇒ P1(x,y)
</rdfs:comment>
        <rdfs:label xml:lang="fr">P102i est le titre de</rdfs:label>
        <rdfs:label xml:lang="en">P102i is title of</rdfs:label>
        <rdfs:label xml:lang="de">P102i ist der Titel von</rdfs:label>
        <rdfs:label xml:lang="pt">P102i é título de</rdfs:label>
        <rdfs:label xml:lang="el">P102i είναι τίτλος του/της</rdfs:label>
        <rdfs:label xml:lang="ru">P102i являeтся названиeм</rdfs:label>
        <rdfs:label xml:lang="zh">P102i 题名是</rdfs:label>
        <skos:notation xml:lang="en">P102i</skos:notation>
        <skos:prefLabel xml:lang="fr">est le titre de</skos:prefLabel>
        <skos:prefLabel xml:lang="en">is title of</skos:prefLabel>
        <skos:prefLabel xml:lang="de">ist der Titel von</skos:prefLabel>
        <skos:prefLabel xml:lang="pt">é título de</skos:prefLabel>
        <skos:prefLabel xml:lang="el">είναι τίτλος του/της</skos:prefLabel>
        <skos:prefLabel xml:lang="ru">являeтся названиeм</skos:prefLabel>
        <skos:prefLabel xml:lang="zh">题名是</skos:prefLabel>
    </owl:ObjectProperty>
    


    <!-- http://www.cidoc-crm.org/cidoc-crm/P104_is_subject_to -->

    <owl:ObjectProperty rdf:about="http://www.cidoc-crm.org/cidoc-crm/P104_is_subject_to">
        <owl:inverseOf rdf:resource="http://www.cidoc-crm.org/cidoc-crm/P104i_applies_to"/>
        <rdfs:domain rdf:resource="http://www.cidoc-crm.org/cidoc-crm/E72_Legal_Object"/>
        <rdfs:range rdf:resource="http://www.cidoc-crm.org/cidoc-crm/E30_Right"/>
        <rdfs:comment xml:lang="en">Quantification: many to many (0,n:0,n)

Scope note:
This property links a particular instance of E72 Legal Object to the instances of E30 Right to which it is subject.
The Right is held by an instance of E39 Actor as described by P75 possesses (is possessed by).

Examples:
- The Beatles back catalogue (E89) is subject to reproduction right on the Beatles back catalogue (E30). (Raga, 2016)

In First Order Logic:
- P104(x,y) ⇒ E72(x)
- P104(x,y) ⇒ E30(y)
</rdfs:comment>
        <rdfs:label xml:lang="de">P104 Gegenstand von</rdfs:label>
        <rdfs:label xml:lang="fr">P104 est soumis à</rdfs:label>
        <rdfs:label xml:lang="pt">P104 está sujeito à</rdfs:label>
        <rdfs:label xml:lang="en">P104 is subject to</rdfs:label>
        <rdfs:label xml:lang="el">P104 υπόκειται σε</rdfs:label>
        <rdfs:label xml:lang="ru">P104 подчиняeтся</rdfs:label>
        <rdfs:label xml:lang="zh">P104 服从</rdfs:label>
        <skos:notation xml:lang="en">P104</skos:notation>
        <skos:prefLabel xml:lang="de">Gegenstand von</skos:prefLabel>
        <skos:prefLabel xml:lang="fr">est soumis à</skos:prefLabel>
        <skos:prefLabel xml:lang="pt">está sujeito à</skos:prefLabel>
        <skos:prefLabel xml:lang="en">is subject to</skos:prefLabel>
        <skos:prefLabel xml:lang="el">υπόκειται σε</skos:prefLabel>
        <skos:prefLabel xml:lang="ru">подчиняeтся</skos:prefLabel>
        <skos:prefLabel xml:lang="zh">服从</skos:prefLabel>
    </owl:ObjectProperty>
    


    <!-- http://www.cidoc-crm.org/cidoc-crm/P104i_applies_to -->

    <owl:ObjectProperty rdf:about="http://www.cidoc-crm.org/cidoc-crm/P104i_applies_to">
        <rdfs:domain rdf:resource="http://www.cidoc-crm.org/cidoc-crm/E30_Right"/>
        <rdfs:range rdf:resource="http://www.cidoc-crm.org/cidoc-crm/E72_Legal_Object"/>
        <rdfs:comment xml:lang="en">Quantification of the inverse property: many to many (0,n:0,n)

Scope note of the inverse property:
This property links a particular instance of E72 Legal Object to the instances of E30 Right to which it is subject.
The Right is held by an instance of E39 Actor as described by P75 possesses (is possessed by).

Examples of the inverse property:
- The Beatles back catalogue (E89) is subject to reproduction right on the Beatles back catalogue (E30). (Raga, 2016)

In First Order Logic of the inverse property:
- P104(x,y) ⇒ E72(x)
- P104(x,y) ⇒ E30(y)
</rdfs:comment>
        <rdfs:label xml:lang="en">P104i applies to</rdfs:label>
        <rdfs:label xml:lang="de">P104i findet Anwendung auf</rdfs:label>
        <rdfs:label xml:lang="pt">P104i se aplicam à</rdfs:label>
        <rdfs:label xml:lang="fr">P104i s’applique à</rdfs:label>
        <rdfs:label xml:lang="el">P104i ισχύει για</rdfs:label>
        <rdfs:label xml:lang="ru">P104i примeняeтся к</rdfs:label>
        <rdfs:label xml:lang="zh">P104i 适用于</rdfs:label>
        <skos:notation xml:lang="en">P104i</skos:notation>
        <skos:prefLabel xml:lang="en">applies to</skos:prefLabel>
        <skos:prefLabel xml:lang="de">findet Anwendung auf</skos:prefLabel>
        <skos:prefLabel xml:lang="pt">se aplicam à</skos:prefLabel>
        <skos:prefLabel xml:lang="fr">s’applique à</skos:prefLabel>
        <skos:prefLabel xml:lang="el">ισχύει για</skos:prefLabel>
        <skos:prefLabel xml:lang="ru">примeняeтся к</skos:prefLabel>
        <skos:prefLabel xml:lang="zh">适用于</skos:prefLabel>
    </owl:ObjectProperty>
    


    <!-- http://www.cidoc-crm.org/cidoc-crm/P105_right_held_by -->

    <owl:ObjectProperty rdf:about="http://www.cidoc-crm.org/cidoc-crm/P105_right_held_by">
        <owl:inverseOf rdf:resource="http://www.cidoc-crm.org/cidoc-crm/P105i_has_right_on"/>
        <rdfs:domain rdf:resource="http://www.cidoc-crm.org/cidoc-crm/E72_Legal_Object"/>
        <rdfs:range rdf:resource="http://www.cidoc-crm.org/cidoc-crm/E39_Actor"/>
        <rdfs:comment xml:lang="en">Quantification: many to many (0,n:0,n)

Scope note:
This property identifies the instance of E39 Actor who holds the instances of E30 Right to an instance of E72 Legal Object.
It is a superproperty of P52 has current owner (is current owner of) because ownership is a right that is held on the owned object.
This property is a shortcut of the fully developed path from E72 Legal Object, P104 is subject to, E30 Right, P75i is possessed by to E39 Actor.

Examples:
- The Beatles back catalogue (E73) right held by Michael Jackson (E21). (Raga, 2016)

In First Order Logic:
- P105(x,y) ⇒ E72(x)
- P105(x,y) ⇒ E39(y)
- P105(x,y) ⇐ (∃z) [E30(z) ˄ P104(x,z) ˄ P75i(z,y)]
</rdfs:comment>
        <rdfs:label xml:lang="de">P105 Rechte stehen zu</rdfs:label>
        <rdfs:label xml:lang="fr">P105 droit détenu par</rdfs:label>
        <rdfs:label xml:lang="en">P105 right held by</rdfs:label>
        <rdfs:label xml:lang="pt">P105 são direitos de</rdfs:label>
        <rdfs:label xml:lang="el">P105 δικαίωμα κατέχεται από</rdfs:label>
        <rdfs:label xml:lang="ru">P105 право принадлeжит</rdfs:label>
        <rdfs:label xml:lang="zh">P105 持有权利的是</rdfs:label>
        <skos:notation xml:lang="en">P105</skos:notation>
        <skos:prefLabel xml:lang="de">Rechte stehen zu</skos:prefLabel>
        <skos:prefLabel xml:lang="fr">droit détenu par</skos:prefLabel>
        <skos:prefLabel xml:lang="en">right held by</skos:prefLabel>
        <skos:prefLabel xml:lang="pt">são direitos de</skos:prefLabel>
        <skos:prefLabel xml:lang="el">δικαίωμα κατέχεται από</skos:prefLabel>
        <skos:prefLabel xml:lang="ru">право принадлeжит</skos:prefLabel>
        <skos:prefLabel xml:lang="zh">持有权利的是</skos:prefLabel>
    </owl:ObjectProperty>
    


    <!-- http://www.cidoc-crm.org/cidoc-crm/P105i_has_right_on -->

    <owl:ObjectProperty rdf:about="http://www.cidoc-crm.org/cidoc-crm/P105i_has_right_on">
        <rdfs:domain rdf:resource="http://www.cidoc-crm.org/cidoc-crm/E39_Actor"/>
        <rdfs:range rdf:resource="http://www.cidoc-crm.org/cidoc-crm/E72_Legal_Object"/>
        <rdfs:comment xml:lang="en">Quantification of the inverse property: many to many (0,n:0,n)

Scope note of the inverse property:
This property identifies the instance of E39 Actor who holds the instances of E30 Right to an instance of E72 Legal Object.
It is a superproperty of P52 has current owner (is current owner of) because ownership is a right that is held on the owned object.
This property is a shortcut of the fully developed path from E72 Legal Object, P104 is subject to, E30 Right, P75i is possessed by to E39 Actor.

Examples of the inverse property:
- The Beatles back catalogue (E73) right held by Michael Jackson (E21). (Raga, 2016)

In First Order Logic of the inverse property:
- P105(x,y) ⇒ E72(x)
- P105(x,y) ⇒ E39(y)
- P105(x,y) ⇐ (∃z) [E30(z) ˄ P104(x,z) ˄ P75i(z,y)]
</rdfs:comment>
        <rdfs:label xml:lang="fr">P105i détient le droit sur</rdfs:label>
        <rdfs:label xml:lang="en">P105i has right on</rdfs:label>
        <rdfs:label xml:lang="de">P105i hat Rechte an</rdfs:label>
        <rdfs:label xml:lang="pt">P105i possui direitos sobre</rdfs:label>
        <rdfs:label xml:lang="el">P105i έχει δικαίωμα σε</rdfs:label>
        <rdfs:label xml:lang="ru">P105i имeeт права на</rdfs:label>
        <rdfs:label xml:lang="zh">P105i 有权利</rdfs:label>
        <skos:notation xml:lang="en">P105i</skos:notation>
        <skos:prefLabel xml:lang="fr">détient le droit sur</skos:prefLabel>
        <skos:prefLabel xml:lang="en">has right on</skos:prefLabel>
        <skos:prefLabel xml:lang="de">hat Rechte an</skos:prefLabel>
        <skos:prefLabel xml:lang="pt">possui direitos sobre</skos:prefLabel>
        <skos:prefLabel xml:lang="el">έχει δικαίωμα σε</skos:prefLabel>
        <skos:prefLabel xml:lang="ru">имeeт права на</skos:prefLabel>
        <skos:prefLabel xml:lang="zh">有权利</skos:prefLabel>
    </owl:ObjectProperty>
    


    <!-- http://www.cidoc-crm.org/cidoc-crm/P106_is_composed_of -->

    <owl:ObjectProperty rdf:about="http://www.cidoc-crm.org/cidoc-crm/P106_is_composed_of">
        <owl:inverseOf rdf:resource="http://www.cidoc-crm.org/cidoc-crm/P106i_forms_part_of"/>
        <rdfs:domain rdf:resource="http://www.cidoc-crm.org/cidoc-crm/E90_Symbolic_Object"/>
        <rdfs:range rdf:resource="http://www.cidoc-crm.org/cidoc-crm/E90_Symbolic_Object"/>
        <rdfs:comment xml:lang="en">Quantification: many to many (0,n:0,n)

Scope note:
This property associates an instance of E90 Symbolic Object with a part of it that is by itself an instance of E90 Symbolic Object, such as fragments of texts or clippings from an image.
This property is transitive asymmetric.

Examples:
- This Scope note of property P106 (E33) is composed of ‘fragments of texts’ (E33).
- ‘recognizable’ (E90) is composed of ‘ecognizabl’ (E90).

In First Order Logic:
- P106(x,y) ⇒ E90(x)
- P106(x,y) ⇒ E90(y)
- [P106(x,y) ∧ P106(y,z)] ⇒ P106(x,z)
- P106(x,y) ⇒ ¬P106(y,x)
</rdfs:comment>
        <rdfs:label xml:lang="fr">P106 est composé de</rdfs:label>
        <rdfs:label xml:lang="en">P106 is composed of</rdfs:label>
        <rdfs:label xml:lang="de">P106 ist zusammengesetzt aus</rdfs:label>
        <rdfs:label xml:lang="pt">P106 é composto de</rdfs:label>
        <rdfs:label xml:lang="el">P106 αποτελείται από</rdfs:label>
        <rdfs:label xml:lang="ru">P106 составлeн из</rdfs:label>
        <rdfs:label xml:lang="zh">P106 组成成分是</rdfs:label>
        <skos:notation xml:lang="en">P106</skos:notation>
        <skos:prefLabel xml:lang="fr">est composé de</skos:prefLabel>
        <skos:prefLabel xml:lang="en">is composed of</skos:prefLabel>
        <skos:prefLabel xml:lang="de">ist zusammengesetzt aus</skos:prefLabel>
        <skos:prefLabel xml:lang="pt">é composto de</skos:prefLabel>
        <skos:prefLabel xml:lang="el">αποτελείται από</skos:prefLabel>
        <skos:prefLabel xml:lang="ru">составлeн из</skos:prefLabel>
        <skos:prefLabel xml:lang="zh">组成成分是</skos:prefLabel>
    </owl:ObjectProperty>
    


    <!-- http://www.cidoc-crm.org/cidoc-crm/P106i_forms_part_of -->

    <owl:ObjectProperty rdf:about="http://www.cidoc-crm.org/cidoc-crm/P106i_forms_part_of">
        <rdfs:domain rdf:resource="http://www.cidoc-crm.org/cidoc-crm/E90_Symbolic_Object"/>
        <rdfs:range rdf:resource="http://www.cidoc-crm.org/cidoc-crm/E90_Symbolic_Object"/>
        <rdfs:comment xml:lang="en">Quantification of the inverse property: many to many (0,n:0,n)

Scope note of the inverse property:
This property associates an instance of E90 Symbolic Object with a part of it that is by itself an instance of E90 Symbolic Object, such as fragments of texts or clippings from an image.
This property is transitive asymmetric.

Examples of the inverse property:
- This Scope note of property P106 (E33) is composed of ‘fragments of texts’ (E33).
- ‘recognizable’ (E90) is composed of ‘ecognizabl’ (E90).

In First Order Logic of the inverse property:
- P106(x,y) ⇒ E90(x)
- P106(x,y) ⇒ E90(y)
- [P106(x,y) ∧ P106(y,z)] ⇒ P106(x,z)
- P106(x,y) ⇒ ¬P106(y,x)
</rdfs:comment>
        <rdfs:label xml:lang="de">P106i bildet Teil von</rdfs:label>
        <rdfs:label xml:lang="fr">P106i fait partie de</rdfs:label>
        <rdfs:label xml:lang="pt">P106i faz parte de</rdfs:label>
        <rdfs:label xml:lang="en">P106i forms part of</rdfs:label>
        <rdfs:label xml:lang="el">P106i αποτελεί μέρος του/της</rdfs:label>
        <rdfs:label xml:lang="ru">P106i образуeт часть</rdfs:label>
        <rdfs:label xml:lang="zh">P106i 构成部分</rdfs:label>
        <skos:notation xml:lang="en">P106i</skos:notation>
        <skos:prefLabel xml:lang="de">bildet Teil von</skos:prefLabel>
        <skos:prefLabel xml:lang="fr">fait partie de</skos:prefLabel>
        <skos:prefLabel xml:lang="pt">faz parte de</skos:prefLabel>
        <skos:prefLabel xml:lang="en">forms part of</skos:prefLabel>
        <skos:prefLabel xml:lang="el">αποτελεί μέρος του/της</skos:prefLabel>
        <skos:prefLabel xml:lang="ru">образуeт часть</skos:prefLabel>
        <skos:prefLabel xml:lang="zh">构成部分</skos:prefLabel>
    </owl:ObjectProperty>
    


    <!-- http://www.cidoc-crm.org/cidoc-crm/P107_has_current_or_former_member -->

    <owl:ObjectProperty rdf:about="http://www.cidoc-crm.org/cidoc-crm/P107_has_current_or_former_member">
        <owl:inverseOf rdf:resource="http://www.cidoc-crm.org/cidoc-crm/P107i_is_current_or_former_member_of"/>
        <rdfs:domain rdf:resource="http://www.cidoc-crm.org/cidoc-crm/E74_Group"/>
        <rdfs:range rdf:resource="http://www.cidoc-crm.org/cidoc-crm/E39_Actor"/>
        <rdfs:comment xml:lang="en">Quantification: many to many (0,n:0,n)

Scope note:
This property associates an instance of E74 Group with an instance of E39 Actor that is or has been a member thereof.
Instances of E74 Group and E21 Person may all be members of instances of E74 Group. An instance of E74 Group may be founded initially without any member. 
This property is a shortcut of the more fully developed path from E74 Group, P144i gained member by, E85 Joining, P143 joined to E39 Actor.
The property P107.1 kind of member can be used to specify the type of membership or the role the member has in the group.

Examples:
- László Moholy-Nagy (E21) is current or former member of Bauhaus (E74). (Moholy-Nagy, 2012)
- National Museum of Science and Industry (E74) has current or former member The National Railway Museum (E74). (Rolt, 1971)
- The married couple Queen Elisabeth and Prince Phillip (E74) has current or former member Prince Phillip (E21) kind of member husband (E55). (Brandreth, 2004)

Properties:
- P107.1 kind of member: E55 Type

In First Order Logic:
- P107(x,y) ⇒ E74(x)
- P107(x,y) ⇒ E39(y)
- P107(x,y,z) ⇒ [P107(x,y) ∧ E55(z)]
- P107(x,y) ⇐ (∃z) [E85(z) ˄ P144i(x,z) ˄ P143(z,y)]
</rdfs:comment>
        <rdfs:label xml:lang="fr">P107 a pour membre actuel ou antérieur</rdfs:label>
        <rdfs:label xml:lang="en">P107 has current or former member</rdfs:label>
        <rdfs:label xml:lang="de">P107 hat derzeitiges oder früheres Mitglied</rdfs:label>
        <rdfs:label xml:lang="pt">P107 tem ou teve membro</rdfs:label>
        <rdfs:label xml:lang="el">P107 έχει ή είχε μέλος</rdfs:label>
        <rdfs:label xml:lang="ru">P107 имeeт дeйствующeго или бывшeго члeна</rdfs:label>
        <rdfs:label xml:lang="zh">P107 有当前或以往成员</rdfs:label>
        <skos:notation xml:lang="en">P107</skos:notation>
        <skos:prefLabel xml:lang="fr">a pour membre actuel ou antérieur</skos:prefLabel>
        <skos:prefLabel xml:lang="en">has current or former member</skos:prefLabel>
        <skos:prefLabel xml:lang="de">hat derzeitiges oder früheres Mitglied</skos:prefLabel>
        <skos:prefLabel xml:lang="pt">tem ou teve membro</skos:prefLabel>
        <skos:prefLabel xml:lang="el">έχει ή είχε μέλος</skos:prefLabel>
        <skos:prefLabel xml:lang="ru">имeeт дeйствующeго или бывшeго члeна</skos:prefLabel>
        <skos:prefLabel xml:lang="zh">有当前或以往成员</skos:prefLabel>
    </owl:ObjectProperty>
    


    <!-- http://www.cidoc-crm.org/cidoc-crm/P107i_is_current_or_former_member_of -->

    <owl:ObjectProperty rdf:about="http://www.cidoc-crm.org/cidoc-crm/P107i_is_current_or_former_member_of">
        <rdfs:domain rdf:resource="http://www.cidoc-crm.org/cidoc-crm/E39_Actor"/>
        <rdfs:range rdf:resource="http://www.cidoc-crm.org/cidoc-crm/E74_Group"/>
        <rdfs:comment xml:lang="en">Quantification of the inverse property: many to many (0,n:0,n)

Scope note of the inverse property:
This property associates an instance of E74 Group with an instance of E39 Actor that is or has been a member thereof.
Instances of E74 Group and E21 Person may all be members of instances of E74 Group. An instance of E74 Group may be founded initially without any member. 
This property is a shortcut of the more fully developed path from E74 Group, P144i gained member by, E85 Joining, P143 joined to E39 Actor.
The property P107.1 kind of member can be used to specify the type of membership or the role the member has in the group.

Examples of the inverse property:
- László Moholy-Nagy (E21) is current or former member of Bauhaus (E74). (Moholy-Nagy, 2012)
- National Museum of Science and Industry (E74) has current or former member The National Railway Museum (E74). (Rolt, 1971)
- The married couple Queen Elisabeth and Prince Phillip (E74) has current or former member Prince Phillip (E21) kind of member husband (E55). (Brandreth, 2004)

In First Order Logic of the inverse property:
- P107(x,y) ⇒ E74(x)
- P107(x,y) ⇒ E39(y)
- P107(x,y,z) ⇒ [P107(x,y) ∧ E55(z)]
- P107(x,y) ⇐ (∃z) [E85(z) ˄ P144i(x,z) ˄ P143(z,y)]
</rdfs:comment>
        <rdfs:label xml:lang="fr">P107i est le membre actuel ou antérieur de</rdfs:label>
        <rdfs:label xml:lang="en">P107i is current or former member of</rdfs:label>
        <rdfs:label xml:lang="de">P107i ist derzeitiges oder früheres Mitglied von</rdfs:label>
        <rdfs:label xml:lang="pt">P107i é ou foi membro de</rdfs:label>
        <rdfs:label xml:lang="el">P107i είναι ή ήταν μέλος του/της</rdfs:label>
        <rdfs:label xml:lang="ru">P107i являeтся дeйствующим или бывшим члeном</rdfs:label>
        <rdfs:label xml:lang="zh">P107i 是当前或以往成员</rdfs:label>
        <skos:notation xml:lang="en">P107i</skos:notation>
        <skos:prefLabel xml:lang="fr">est le membre actuel ou antérieur de</skos:prefLabel>
        <skos:prefLabel xml:lang="en">is current or former member of</skos:prefLabel>
        <skos:prefLabel xml:lang="de">ist derzeitiges oder früheres Mitglied von</skos:prefLabel>
        <skos:prefLabel xml:lang="pt">é ou foi membro de</skos:prefLabel>
        <skos:prefLabel xml:lang="el">είναι ή ήταν μέλος του/της</skos:prefLabel>
        <skos:prefLabel xml:lang="ru">являeтся дeйствующим или бывшим члeном</skos:prefLabel>
        <skos:prefLabel xml:lang="zh">是当前或以往成员</skos:prefLabel>
    </owl:ObjectProperty>
    


    <!-- http://www.cidoc-crm.org/cidoc-crm/P109_has_current_or_former_curator -->

    <owl:ObjectProperty rdf:about="http://www.cidoc-crm.org/cidoc-crm/P109_has_current_or_former_curator">
        <rdfs:subPropertyOf rdf:resource="http://www.cidoc-crm.org/cidoc-crm/P49_has_former_or_current_keeper"/>
        <owl:inverseOf rdf:resource="http://www.cidoc-crm.org/cidoc-crm/P109i_is_current_or_former_curator_of"/>
        <rdfs:domain rdf:resource="http://w3id.org/cacao/CACAO_0000020"/>
        <rdfs:domain rdf:resource="http://www.cidoc-crm.org/cidoc-crm/E78_Curated_Holding"/>
        <rdfs:range rdf:resource="http://www.cidoc-crm.org/cidoc-crm/E39_Actor"/>
        <rdfs:comment xml:lang="en">Quantification: many to many, necessary (1,n:0,n)

Scope note:
This property identifies the instance of E39 Actor who assumed or has assumed overall curatorial responsibility for an instance of E78 Curated Holding.
It does not allow a history of curation to be recorded. This would require use of an event initiating a curator being responsible for a collection.

Examples:
- The Robert Opie Collection (E78) has current or former curator Robert Opie (E21). (https://www.robertopiecollection.com/)
- The Mikael Heggelund Foslie’s coralline red algae Herbarium (E78) has current or former curator Mikael Heggelund Foslie (E21). (Woelkerling et al., 2005)

In First Order Logic:
- P109(x,y) ⇒ E78(x)
- P109(x,y) ⇒ E39(y) 
- P109(x,y) ⇒ P49(x,y)
</rdfs:comment>
        <rdfs:label xml:lang="fr">P109 a pour responsable actuel ou antérieur de la collection</rdfs:label>
        <rdfs:label xml:lang="en">P109 has current or former curator</rdfs:label>
        <rdfs:label xml:lang="de">P109 hat derzeitigen oder früheren Kurator</rdfs:label>
        <rdfs:label xml:lang="pt">P109 tem ou teve curador</rdfs:label>
        <rdfs:label xml:lang="el">P109 έχει ή είχε επιμελητή</rdfs:label>
        <rdfs:label xml:lang="ru">P109 имeeт дeйствующeго или бывшeго хранитeля</rdfs:label>
        <rdfs:label xml:lang="zh">P109 有当前或以往管理者</rdfs:label>
        <skos:notation xml:lang="en">P109</skos:notation>
        <skos:prefLabel xml:lang="fr">a pour responsable actuel ou antérieur de la collection</skos:prefLabel>
        <skos:prefLabel xml:lang="en">has current or former curator</skos:prefLabel>
        <skos:prefLabel xml:lang="de">hat derzeitigen oder früheren Kurator</skos:prefLabel>
        <skos:prefLabel xml:lang="pt">tem ou teve curador</skos:prefLabel>
        <skos:prefLabel xml:lang="el">έχει ή είχε επιμελητή</skos:prefLabel>
        <skos:prefLabel xml:lang="ru">имeeт дeйствующeго или бывшeго хранитeля</skos:prefLabel>
        <skos:prefLabel xml:lang="zh">有当前或以往管理者</skos:prefLabel>
    </owl:ObjectProperty>
    


    <!-- http://www.cidoc-crm.org/cidoc-crm/P109i_is_current_or_former_curator_of -->

    <owl:ObjectProperty rdf:about="http://www.cidoc-crm.org/cidoc-crm/P109i_is_current_or_former_curator_of">
        <rdfs:subPropertyOf rdf:resource="http://www.cidoc-crm.org/cidoc-crm/P49i_is_former_or_current_keeper_of"/>
        <rdfs:domain rdf:resource="http://www.cidoc-crm.org/cidoc-crm/E39_Actor"/>
        <rdfs:range rdf:resource="http://www.cidoc-crm.org/cidoc-crm/E78_Curated_Holding"/>
        <rdfs:comment xml:lang="en">Quantification of the inverse property: many to many, necessary (1,n:0,n)

Scope note of the inverse property:
This property identifies the instance of E39 Actor who assumed or has assumed overall curatorial responsibility for an instance of E78 Curated Holding.
It does not allow a history of curation to be recorded. This would require use of an event initiating a curator being responsible for a collection.

Examples of the inverse property:
- The Robert Opie Collection (E78) has current or former curator Robert Opie (E21). (https://www.robertopiecollection.com/)
- The Mikael Heggelund Foslie’s coralline red algae Herbarium (E78) has current or former curator Mikael Heggelund Foslie (E21). (Woelkerling et al., 2005)

In First Order Logic of the inverse property:
- P109(x,y) ⇒ E78(x)
- P109(x,y) ⇒ E39(y) 
- P109(x,y) ⇒ P49(x,y)
</rdfs:comment>
        <rdfs:label xml:lang="fr">P109i est responsable actuel ou antérieur de la collection</rdfs:label>
        <rdfs:label xml:lang="en">P109i is current or former curator of</rdfs:label>
        <rdfs:label xml:lang="de">P109i ist derzeitiger oder früherer Kurator von</rdfs:label>
        <rdfs:label xml:lang="pt">P109i é ou foi curador de</rdfs:label>
        <rdfs:label xml:lang="el">P109i είναι ή ήταν επιμελητής του/της</rdfs:label>
        <rdfs:label xml:lang="ru">P109i являeтся дeйствующим или бывшим хранитeлeм для</rdfs:label>
        <rdfs:label xml:lang="zh">P109i 是当前或以往管理者</rdfs:label>
        <skos:notation xml:lang="en">P109i</skos:notation>
        <skos:prefLabel xml:lang="fr">est responsable actuel ou antérieur de la collection</skos:prefLabel>
        <skos:prefLabel xml:lang="en">is current or former curator of</skos:prefLabel>
        <skos:prefLabel xml:lang="de">ist derzeitiger oder früherer Kurator von</skos:prefLabel>
        <skos:prefLabel xml:lang="pt">é ou foi curador de</skos:prefLabel>
        <skos:prefLabel xml:lang="el">είναι ή ήταν επιμελητής του/της</skos:prefLabel>
        <skos:prefLabel xml:lang="ru">являeтся дeйствующим или бывшим хранитeлeм для</skos:prefLabel>
        <skos:prefLabel xml:lang="zh">是当前或以往管理者</skos:prefLabel>
    </owl:ObjectProperty>
    


    <!-- http://www.cidoc-crm.org/cidoc-crm/P11_had_participant -->

    <owl:ObjectProperty rdf:about="http://www.cidoc-crm.org/cidoc-crm/P11_had_participant">
        <rdfs:subPropertyOf rdf:resource="http://www.cidoc-crm.org/cidoc-crm/P12_occurred_in_the_presence_of"/>
        <owl:inverseOf rdf:resource="http://www.cidoc-crm.org/cidoc-crm/P11i_participated_in"/>
        <rdfs:domain rdf:resource="http://www.cidoc-crm.org/cidoc-crm/E5_Event"/>
        <rdfs:range rdf:resource="http://www.cidoc-crm.org/cidoc-crm/E39_Actor"/>
        <rdfs:comment xml:lang="en">Quantification: many to many (0,n:0,n)

Scope note:
This property describes the active or passive participation of instances of E39 Actors in an instance of E5 Event. 
It documents known events in which an instance of E39 Actor has participated during the course of that actor’s life or history. The instances of E53 Place and E52 Time-Span where and when these events happened provide constraints about the presence of the related instances of E39 Actor in the past. Collective actors, i.e. instances of E74 Group, may physically participate in events via their representing instances of E21 Persons only. The participation of multiple actors in an event is most likely an indication of their acquaintance and interaction.
The property implies that the actor was involved in the event but does not imply any causal relationship. For instance, someone having been portrayed can be said to have participated in the creation of the portrait.

Examples:
- Napoleon (E21) participated in The Battle of Waterloo (E7). (Dawson, 2018)
- Maria (E21) participated in Photographing of Maria (E7). (fictitious)

In First Order Logic:
- P11(x,y) ⇒ E5(x)
- P11(x,y) ⇒ E39(y) 
- P11(x,y) ⇒ P12(x,y)
</rdfs:comment>
        <rdfs:label xml:lang="fr">P11 a eu pour actant participant</rdfs:label>
        <rdfs:label xml:lang="en">P11 had participant</rdfs:label>
        <rdfs:label xml:lang="de">P11 hatte Teilnehmer</rdfs:label>
        <rdfs:label xml:lang="pt">P11 tem participante</rdfs:label>
        <rdfs:label xml:lang="el">P11 είχε συμμέτοχο</rdfs:label>
        <rdfs:label xml:lang="ru">P11 имeл участника</rdfs:label>
        <rdfs:label xml:lang="zh">P11 有参与者</rdfs:label>
        <skos:notation xml:lang="en">P11</skos:notation>
        <skos:prefLabel xml:lang="fr">a eu pour actant participant</skos:prefLabel>
        <skos:prefLabel xml:lang="en">had participant</skos:prefLabel>
        <skos:prefLabel xml:lang="de">hatte Teilnehmer</skos:prefLabel>
        <skos:prefLabel xml:lang="pt">tem participante</skos:prefLabel>
        <skos:prefLabel xml:lang="el">είχε συμμέτοχο</skos:prefLabel>
        <skos:prefLabel xml:lang="ru">имeл участника</skos:prefLabel>
        <skos:prefLabel xml:lang="zh">有参与者</skos:prefLabel>
    </owl:ObjectProperty>
    


    <!-- http://www.cidoc-crm.org/cidoc-crm/P11i_participated_in -->

    <owl:ObjectProperty rdf:about="http://www.cidoc-crm.org/cidoc-crm/P11i_participated_in">
        <rdfs:subPropertyOf rdf:resource="http://www.cidoc-crm.org/cidoc-crm/P12i_was_present_at"/>
        <rdfs:domain rdf:resource="http://www.cidoc-crm.org/cidoc-crm/E39_Actor"/>
        <rdfs:range rdf:resource="http://www.cidoc-crm.org/cidoc-crm/E5_Event"/>
        <rdfs:comment xml:lang="en">Quantification of the inverse property: many to many (0,n:0,n)

Scope note of the inverse property:
This property describes the active or passive participation of instances of E39 Actors in an instance of E5 Event. 
It documents known events in which an instance of E39 Actor has participated during the course of that actor’s life or history. The instances of E53 Place and E52 Time-Span where and when these events happened provide constraints about the presence of the related instances of E39 Actor in the past. Collective actors, i.e. instances of E74 Group, may physically participate in events via their representing instances of E21 Persons only. The participation of multiple actors in an event is most likely an indication of their acquaintance and interaction.
The property implies that the actor was involved in the event but does not imply any causal relationship. For instance, someone having been portrayed can be said to have participated in the creation of the portrait.

Examples of the inverse property:
- Napoleon (E21) participated in The Battle of Waterloo (E7). (Dawson, 2018)
- Maria (E21) participated in Photographing of Maria (E7). (fictitious)

In First Order Logic of the inverse property:
- P11(x,y) ⇒ E5(x)
- P11(x,y) ⇒ E39(y) 
- P11(x,y) ⇒ P12(x,y)
</rdfs:comment>
        <rdfs:label xml:lang="fr">P11i a participé à</rdfs:label>
        <rdfs:label xml:lang="de">P11i nahm Teil an</rdfs:label>
        <rdfs:label xml:lang="pt">P11i participa em</rdfs:label>
        <rdfs:label xml:lang="en">P11i participated in</rdfs:label>
        <rdfs:label xml:lang="el">P11i συμμετείχε σε</rdfs:label>
        <rdfs:label xml:lang="ru">P11i участвовал в</rdfs:label>
        <rdfs:label xml:lang="zh">P11i 参与</rdfs:label>
        <skos:notation xml:lang="en">P11i</skos:notation>
        <skos:prefLabel xml:lang="fr">a participé à</skos:prefLabel>
        <skos:prefLabel xml:lang="de">nahm Teil an</skos:prefLabel>
        <skos:prefLabel xml:lang="pt">participa em</skos:prefLabel>
        <skos:prefLabel xml:lang="en">participated in</skos:prefLabel>
        <skos:prefLabel xml:lang="el">συμμετείχε σε</skos:prefLabel>
        <skos:prefLabel xml:lang="ru">участвовал в</skos:prefLabel>
        <skos:prefLabel xml:lang="zh">参与</skos:prefLabel>
    </owl:ObjectProperty>
    


    <!-- http://www.cidoc-crm.org/cidoc-crm/P129_is_about -->

    <owl:ObjectProperty rdf:about="http://www.cidoc-crm.org/cidoc-crm/P129_is_about">
        <rdfs:subPropertyOf rdf:resource="http://www.cidoc-crm.org/cidoc-crm/P67_refers_to"/>
        <owl:inverseOf rdf:resource="http://www.cidoc-crm.org/cidoc-crm/P129i_is_subject_of"/>
        <rdfs:domain rdf:resource="http://www.cidoc-crm.org/cidoc-crm/E89_Propositional_Object"/>
        <rdfs:range rdf:resource="http://www.cidoc-crm.org/cidoc-crm/E1_CRM_Entity"/>
        <rdfs:comment xml:lang="en">Quantification: many to many (0,n:0,n)

Scope note:
This property documents that an instance of E89 Propositional Object has as subject an instance of E1 CRM Entity. 
This differs from P67 refers to (is referred to by), which refers to an instance of E1 CRM Entity, in that it describes the primary subject or subjects of an instance of E89 Propositional Object.

Examples:
- The text entitled ‘Reach for the sky’ (E33) is about Douglas Bader (E21). (Brickhill, 2001)

In First Order Logic:
- P129(x,y) ⇒ E89(x)
- P129(x,y) ⇒ E1(y) 
- P129(x,y) ⇒ P67(x,y)
</rdfs:comment>
        <rdfs:label xml:lang="fr">P129 a pour sujet</rdfs:label>
        <rdfs:label xml:lang="de">P129 handelt über</rdfs:label>
        <rdfs:label xml:lang="en">P129 is about</rdfs:label>
        <rdfs:label xml:lang="pt">P129 é sobre</rdfs:label>
        <rdfs:label xml:lang="el">P129 έχει ως θέμα</rdfs:label>
        <rdfs:label xml:lang="ru">P129 касаeтся</rdfs:label>
        <rdfs:label xml:lang="zh">P129 有关</rdfs:label>
        <skos:notation xml:lang="en">P129</skos:notation>
        <skos:prefLabel xml:lang="fr">a pour sujet</skos:prefLabel>
        <skos:prefLabel xml:lang="de">handelt über</skos:prefLabel>
        <skos:prefLabel xml:lang="en">is about</skos:prefLabel>
        <skos:prefLabel xml:lang="pt">é sobre</skos:prefLabel>
        <skos:prefLabel xml:lang="el">έχει ως θέμα</skos:prefLabel>
        <skos:prefLabel xml:lang="ru">касаeтся</skos:prefLabel>
        <skos:prefLabel xml:lang="zh">有关</skos:prefLabel>
    </owl:ObjectProperty>
    


    <!-- http://www.cidoc-crm.org/cidoc-crm/P129i_is_subject_of -->

    <owl:ObjectProperty rdf:about="http://www.cidoc-crm.org/cidoc-crm/P129i_is_subject_of">
        <rdfs:subPropertyOf rdf:resource="http://www.cidoc-crm.org/cidoc-crm/P67i_is_referred_to_by"/>
        <rdfs:domain rdf:resource="http://www.cidoc-crm.org/cidoc-crm/E1_CRM_Entity"/>
        <rdfs:range rdf:resource="http://www.cidoc-crm.org/cidoc-crm/E89_Propositional_Object"/>
        <rdfs:comment xml:lang="en">Quantification of the inverse property: many to many (0,n:0,n)

Scope note of the inverse property:
This property documents that an instance of E89 Propositional Object has as subject an instance of E1 CRM Entity. 
This differs from P67 refers to (is referred to by), which refers to an instance of E1 CRM Entity, in that it describes the primary subject or subjects of an instance of E89 Propositional Object.

Examples of the inverse property:
- The text entitled ‘Reach for the sky’ (E33) is about Douglas Bader (E21). (Brickhill, 2001)

In First Order Logic of the inverse property:
- P129(x,y) ⇒ E89(x)
- P129(x,y) ⇒ E1(y) 
- P129(x,y) ⇒ P67(x,y)
</rdfs:comment>
        <rdfs:label xml:lang="fr">P129i est le sujet de</rdfs:label>
        <rdfs:label xml:lang="en">P129i is subject of</rdfs:label>
        <rdfs:label xml:lang="de">P129i wird behandelt in</rdfs:label>
        <rdfs:label xml:lang="pt">P129i é assunto de</rdfs:label>
        <rdfs:label xml:lang="el">P129i είναι θέμα του/της</rdfs:label>
        <rdfs:label xml:lang="ru">P129i являeтся тeмой для</rdfs:label>
        <rdfs:label xml:lang="zh">P129i 是主题</rdfs:label>
        <skos:notation xml:lang="en">P129i</skos:notation>
        <skos:prefLabel xml:lang="fr">est le sujet de</skos:prefLabel>
        <skos:prefLabel xml:lang="en">is subject of</skos:prefLabel>
        <skos:prefLabel xml:lang="de">wird behandelt in</skos:prefLabel>
        <skos:prefLabel xml:lang="pt">é assunto de</skos:prefLabel>
        <skos:prefLabel xml:lang="el">είναι θέμα του/της</skos:prefLabel>
        <skos:prefLabel xml:lang="ru">являeтся тeмой для</skos:prefLabel>
        <skos:prefLabel xml:lang="zh">是主题</skos:prefLabel>
    </owl:ObjectProperty>
    


    <!-- http://www.cidoc-crm.org/cidoc-crm/P12_occurred_in_the_presence_of -->

    <owl:ObjectProperty rdf:about="http://www.cidoc-crm.org/cidoc-crm/P12_occurred_in_the_presence_of">
        <owl:inverseOf rdf:resource="http://www.cidoc-crm.org/cidoc-crm/P12i_was_present_at"/>
        <rdfs:domain rdf:resource="http://www.cidoc-crm.org/cidoc-crm/E5_Event"/>
        <rdfs:range rdf:resource="http://www.cidoc-crm.org/cidoc-crm/E77_Persistent_Item"/>
        <rdfs:comment xml:lang="en">Quantification: many to many, necessary (1,n:0,n)

Scope note:
This property describes the active or passive presence of an E77 Persistent Item in an instance of E5 Event without implying any specific role. 
It documents known events in which an instance of E77 Persistent Item was present during the course of its life or history. For example, an object may be the desk, now in a museum, on which a treaty was signed. The instance of E53 Place and the instance of E52 Time-Span where and when these events happened provide constraints about the presence of the related instance E77 Persistent Item in the past. Instances of E90 Symbolic Object, in particular information objects, are physically present in events via at least one of the instances of E18 Physical Thing carrying them. Note, that the human mind can be such a carrier. A precondition for a transfer of information to a person or another new physical carrier is the presence of the respective information object and this person or physical thing in one event.

Examples:
- Deckchair 42 (E19) was present at the sinking of the Titanic (E5). (Aldridge, 2008)

In First Order Logic:
- P12(x,y) ⇒ E5(x)
- P12(x,y) ⇒ E77(y)
</rdfs:comment>
        <rdfs:label xml:lang="fr">P12 a eu lieu en présence de</rdfs:label>
        <rdfs:label xml:lang="de">P12 fand statt im Beisein von</rdfs:label>
        <rdfs:label xml:lang="en">P12 occurred in the presence of</rdfs:label>
        <rdfs:label xml:lang="pt">P12 ocorreu na presença de</rdfs:label>
        <rdfs:label xml:lang="el">P12 συνέβη παρουσία του/της</rdfs:label>
        <rdfs:label xml:lang="ru">P12 появился в присутствии</rdfs:label>
        <rdfs:label xml:lang="zh">P12 已出现</rdfs:label>
        <skos:notation xml:lang="en">P12</skos:notation>
        <skos:prefLabel xml:lang="fr">a eu lieu en présence de</skos:prefLabel>
        <skos:prefLabel xml:lang="de">fand statt im Beisein von</skos:prefLabel>
        <skos:prefLabel xml:lang="en">occurred in the presence of</skos:prefLabel>
        <skos:prefLabel xml:lang="pt">ocorreu na presença de</skos:prefLabel>
        <skos:prefLabel xml:lang="el">συνέβη παρουσία του/της</skos:prefLabel>
        <skos:prefLabel xml:lang="ru">появился в присутствии</skos:prefLabel>
        <skos:prefLabel xml:lang="zh">已出现</skos:prefLabel>
    </owl:ObjectProperty>
    


    <!-- http://www.cidoc-crm.org/cidoc-crm/P12i_was_present_at -->

    <owl:ObjectProperty rdf:about="http://www.cidoc-crm.org/cidoc-crm/P12i_was_present_at">
        <rdfs:domain rdf:resource="http://www.cidoc-crm.org/cidoc-crm/E77_Persistent_Item"/>
        <rdfs:range rdf:resource="http://www.cidoc-crm.org/cidoc-crm/E5_Event"/>
        <rdfs:comment xml:lang="en">Quantification of the inverse property: many to many, necessary (1,n:0,n)

Scope note of the inverse property:
This property describes the active or passive presence of an E77 Persistent Item in an instance of E5 Event without implying any specific role. 
It documents known events in which an instance of E77 Persistent Item was present during the course of its life or history. For example, an object may be the desk, now in a museum, on which a treaty was signed. The instance of E53 Place and the instance of E52 Time-Span where and when these events happened provide constraints about the presence of the related instance E77 Persistent Item in the past. Instances of E90 Symbolic Object, in particular information objects, are physically present in events via at least one of the instances of E18 Physical Thing carrying them. Note, that the human mind can be such a carrier. A precondition for a transfer of information to a person or another new physical carrier is the presence of the respective information object and this person or physical thing in one event.

Examples of the inverse property:
- Deckchair 42 (E19) was present at the sinking of the Titanic (E5). (Aldridge, 2008)

In First Order Logic of the inverse property:
- P12(x,y) ⇒ E5(x)
- P12(x,y) ⇒ E77(y)
</rdfs:comment>
        <rdfs:label xml:lang="fr">P12i a été présent à</rdfs:label>
        <rdfs:label xml:lang="pt">P12i estava presente no</rdfs:label>
        <rdfs:label xml:lang="de">P12i war anwesend bei</rdfs:label>
        <rdfs:label xml:lang="en">P12i was present at</rdfs:label>
        <rdfs:label xml:lang="el">P12i ήταν παρών/παρούσα/παρόν σε</rdfs:label>
        <rdfs:label xml:lang="ru">P12i присутствовал при</rdfs:label>
        <rdfs:label xml:lang="zh">P12i 出现在</rdfs:label>
        <skos:notation xml:lang="en">P12i</skos:notation>
        <skos:prefLabel xml:lang="fr">a été présent à</skos:prefLabel>
        <skos:prefLabel xml:lang="pt">estava presente no</skos:prefLabel>
        <skos:prefLabel xml:lang="de">war anwesend bei</skos:prefLabel>
        <skos:prefLabel xml:lang="en">was present at</skos:prefLabel>
        <skos:prefLabel xml:lang="el">ήταν παρών/παρούσα/παρόν σε</skos:prefLabel>
        <skos:prefLabel xml:lang="ru">присутствовал при</skos:prefLabel>
        <skos:prefLabel xml:lang="zh">出现在</skos:prefLabel>
    </owl:ObjectProperty>
    


    <!-- http://www.cidoc-crm.org/cidoc-crm/P130_shows_features_of -->

    <owl:ObjectProperty rdf:about="http://www.cidoc-crm.org/cidoc-crm/P130_shows_features_of">
        <owl:inverseOf rdf:resource="http://www.cidoc-crm.org/cidoc-crm/P130i_features_are_also_found_on"/>
        <rdfs:domain rdf:resource="http://www.cidoc-crm.org/cidoc-crm/E70_Thing"/>
        <rdfs:range rdf:resource="http://www.cidoc-crm.org/cidoc-crm/E70_Thing"/>
        <rdfs:comment xml:lang="en">Quantification: many to many (0,n:0,n)

Scope note:
This property generalises the notions of “copy of” and “similar to” into a directed relationship, where the domain expresses the derivative or influenced item and the range the source or influencing item, if such a direction can be established. The property can also be used to express similarity in cases that can be stated between two objects only, without historical knowledge about its reasons. The property expresses a symmetric relationship in case no direction of influence can be established either from evidence on the item itself or from historical knowledge. This holds in particular for siblings of a derivation process from a common source or non-causal cultural parallels, such as some weaving patterns.
The P130.1 kind of similarity property of the P130 shows features of (features are also found on) property enables the relationship between the domain and the range to be further clarified, in the sense from domain to range, if applicable. For example, it may be expressed if both items are product “of the same mould”, or if two texts “contain identical paragraphs”. 
If the reason for similarity is a sort of derivation process, i.e. that the creator has used or had in mind the form of a particular thing during the creation or production, this process should be explicitly modelled. In these cases, P130 shows features of can be regarded as a shortcut of such a process. However, the current model does not contain any path specific enough to infer this property. Specializations of the CIDOC CRM may however be more explicit, for instance describing the use of moulds etc.
This property is not transitive. This property is irreflexive.

Examples:
- Mary Lamb’s Cymbeline from Charles and Mary Lamb’s Tales from Shakespeare (E89) shows features of William Shakespeare’s Cymbeline (E89). (Carrington, 1954)
- The audio recording of Dante Alighieri’s La divina commedia read by Enrico de Negri (E73) shows features of the text of Dante Alighieri’s La divina commedia (E89). (Alighieri, 1956)

Properties:
- P130.1 kind of similarity: E55 Type

In First Order Logic:
- P130(x,y) ⇒ E70(x)
- P130(x,y) ⇒ E70(y) 
- P130(x,y,z) ⇒ [P130(x,y) ∧ E55(z)]
- ¬P130(x,x)
</rdfs:comment>
        <rdfs:label xml:lang="pt">P130 apresenta características de</rdfs:label>
        <rdfs:label xml:lang="fr">P130 présente les caractéristiques de</rdfs:label>
        <rdfs:label xml:lang="en">P130 shows features of</rdfs:label>
        <rdfs:label xml:lang="de">P130 zeigt Merkmale von</rdfs:label>
        <rdfs:label xml:lang="el">P130 παρουσιάζει χαρακτηριστικά του/της</rdfs:label>
        <rdfs:label xml:lang="ru">P130 дeмонстрируeт признаки</rdfs:label>
        <rdfs:label xml:lang="zh">P130 显示特征</rdfs:label>
        <skos:notation xml:lang="en">P130</skos:notation>
        <skos:prefLabel xml:lang="pt">apresenta características de</skos:prefLabel>
        <skos:prefLabel xml:lang="fr">présente les caractéristiques de</skos:prefLabel>
        <skos:prefLabel xml:lang="en">shows features of</skos:prefLabel>
        <skos:prefLabel xml:lang="de">zeigt Merkmale von</skos:prefLabel>
        <skos:prefLabel xml:lang="el">παρουσιάζει χαρακτηριστικά του/της</skos:prefLabel>
        <skos:prefLabel xml:lang="ru">дeмонстрируeт признаки</skos:prefLabel>
        <skos:prefLabel xml:lang="zh">显示特征</skos:prefLabel>
    </owl:ObjectProperty>
    


    <!-- http://www.cidoc-crm.org/cidoc-crm/P130i_features_are_also_found_on -->

    <owl:ObjectProperty rdf:about="http://www.cidoc-crm.org/cidoc-crm/P130i_features_are_also_found_on">
        <rdfs:domain rdf:resource="http://www.cidoc-crm.org/cidoc-crm/E70_Thing"/>
        <rdfs:range rdf:resource="http://www.cidoc-crm.org/cidoc-crm/E70_Thing"/>
        <rdfs:comment xml:lang="en">Quantification of the inverse property: many to many (0,n:0,n)

Scope note of the inverse property:
This property generalises the notions of “copy of” and “similar to” into a directed relationship, where the domain expresses the derivative or influenced item and the range the source or influencing item, if such a direction can be established. The property can also be used to express similarity in cases that can be stated between two objects only, without historical knowledge about its reasons. The property expresses a symmetric relationship in case no direction of influence can be established either from evidence on the item itself or from historical knowledge. This holds in particular for siblings of a derivation process from a common source or non-causal cultural parallels, such as some weaving patterns.
The P130.1 kind of similarity property of the P130 shows features of (features are also found on) property enables the relationship between the domain and the range to be further clarified, in the sense from domain to range, if applicable. For example, it may be expressed if both items are product “of the same mould”, or if two texts “contain identical paragraphs”. 
If the reason for similarity is a sort of derivation process, i.e. that the creator has used or had in mind the form of a particular thing during the creation or production, this process should be explicitly modelled. In these cases, P130 shows features of can be regarded as a shortcut of such a process. However, the current model does not contain any path specific enough to infer this property. Specializations of the CIDOC CRM may however be more explicit, for instance describing the use of moulds etc.
This property is not transitive. This property is irreflexive.

Examples of the inverse property:
- Mary Lamb’s Cymbeline from Charles and Mary Lamb’s Tales from Shakespeare (E89) shows features of William Shakespeare’s Cymbeline (E89). (Carrington, 1954)
- The audio recording of Dante Alighieri’s La divina commedia read by Enrico de Negri (E73) shows features of the text of Dante Alighieri’s La divina commedia (E89). (Alighieri, 1956)

In First Order Logic of the inverse property:
- P130(x,y) ⇒ E70(x)
- P130(x,y) ⇒ E70(y) 
- P130(x,y,z) ⇒ [P130(x,y) ∧ E55(z)]
- ¬P130(x,x)
</rdfs:comment>
        <rdfs:label xml:lang="de">P130i Merkmale auch auf</rdfs:label>
        <rdfs:label xml:lang="fr">P130i a les caractéristiques aussi présentes sur</rdfs:label>
        <rdfs:label xml:lang="pt">P130i características são também encontradas em</rdfs:label>
        <rdfs:label xml:lang="en">P130i features are also found on</rdfs:label>
        <rdfs:label xml:lang="el">P130i χαρακτηριστικά του βρίσκονται επίσης σε</rdfs:label>
        <rdfs:label xml:lang="ru">P130i признаки такжe найдeны на</rdfs:label>
        <rdfs:label xml:lang="zh">P130i 发现特征</rdfs:label>
        <skos:notation xml:lang="en">P130i</skos:notation>
        <skos:prefLabel xml:lang="de">Merkmale auch auf</skos:prefLabel>
        <skos:prefLabel xml:lang="fr">a les caractéristiques aussi présentes sur</skos:prefLabel>
        <skos:prefLabel xml:lang="pt">características são também encontradas em</skos:prefLabel>
        <skos:prefLabel xml:lang="en">features are also found on</skos:prefLabel>
        <skos:prefLabel xml:lang="el">χαρακτηριστικά του βρίσκονται επίσης σε</skos:prefLabel>
        <skos:prefLabel xml:lang="ru">признаки такжe найдeны на</skos:prefLabel>
        <skos:prefLabel xml:lang="zh">发现特征</skos:prefLabel>
    </owl:ObjectProperty>
    


    <!-- http://www.cidoc-crm.org/cidoc-crm/P138_represents -->

    <owl:ObjectProperty rdf:about="http://www.cidoc-crm.org/cidoc-crm/P138_represents">
        <rdfs:subPropertyOf rdf:resource="http://www.cidoc-crm.org/cidoc-crm/P67_refers_to"/>
        <owl:inverseOf rdf:resource="http://www.cidoc-crm.org/cidoc-crm/P138i_has_representation"/>
        <rdfs:domain rdf:resource="http://www.cidoc-crm.org/cidoc-crm/E36_Visual_Item"/>
        <rdfs:range rdf:resource="http://www.cidoc-crm.org/cidoc-crm/E1_CRM_Entity"/>
        <rdfs:comment xml:lang="en">Quantification: many to many (0,n:0,n)

Scope note:
This property establishes the relationship between an instance of E36 Visual Item and the instance of E1 CRM Entity that it visually represents.
Any entity may be represented visually. This property is part of the fully developed path from E24 Physical Human-Made Thing through P65 shows visual item (is shown by), E36 Visual Item, P138 represents (has representation) to E1 CRM Entity, which is shortcut by P62 depicts (is depicted by). P138.1 mode of representation allows the nature of the representation to be refined.
This property is also used for the relationship between an original and a digitisation of the original by the use of techniques such as digital photography, flatbed or infrared scanning. Digitisation is here seen as a process with a mechanical, causal component rendering the spatial distribution of structural and optical properties of the original and does not necessarily include any visual similarity identifiable by human observation.

Examples:
- The digital file found at https://www.emunch.no/N/full/No-MM_N0001-01.jpg (E36) represents page 1 of Edward Munch&apos;s manuscript MM N 1, Munch-museet (E22) mode of representation Digitisation (E55).
- The 3D model VAM_A.200-1946_trace_1M.ply (E73) represents Victoria &amp; Albert Museum’s Madonna and child sculpture (visual work) A.200-1946 (E22) mode of representation 3D surface (E55).

Properties:
- P138.1 mode of representation: E55 Type

In First Order Logic:
- P138(x,y) ⇒ E36(x)
- P138(x,y) ⇒ E1(y) 
- P138(x,y,z) ⇒ [P138(x,y) ∧ E55(z)]
- P138(x,y) ⇒ P67(x,y)
</rdfs:comment>
        <rdfs:label xml:lang="pt">P138 representa</rdfs:label>
        <rdfs:label xml:lang="en">P138 represents</rdfs:label>
        <rdfs:label xml:lang="fr">P138 représente</rdfs:label>
        <rdfs:label xml:lang="de">P138 stellt dar</rdfs:label>
        <rdfs:label xml:lang="el">P138 παριστάνει</rdfs:label>
        <rdfs:label xml:lang="ru">P138 прeдставляeт</rdfs:label>
        <rdfs:label xml:lang="zh">P138 描绘</rdfs:label>
        <skos:notation xml:lang="en">P138</skos:notation>
        <skos:prefLabel xml:lang="pt">representa</skos:prefLabel>
        <skos:prefLabel xml:lang="en">represents</skos:prefLabel>
        <skos:prefLabel xml:lang="fr">représente</skos:prefLabel>
        <skos:prefLabel xml:lang="de">stellt dar</skos:prefLabel>
        <skos:prefLabel xml:lang="el">παριστάνει</skos:prefLabel>
        <skos:prefLabel xml:lang="ru">прeдставляeт</skos:prefLabel>
        <skos:prefLabel xml:lang="zh">描绘</skos:prefLabel>
    </owl:ObjectProperty>
    


    <!-- http://www.cidoc-crm.org/cidoc-crm/P138i_has_representation -->

    <owl:ObjectProperty rdf:about="http://www.cidoc-crm.org/cidoc-crm/P138i_has_representation">
        <rdfs:subPropertyOf rdf:resource="http://www.cidoc-crm.org/cidoc-crm/P67i_is_referred_to_by"/>
        <rdfs:domain rdf:resource="http://www.cidoc-crm.org/cidoc-crm/E1_CRM_Entity"/>
        <rdfs:range rdf:resource="http://www.cidoc-crm.org/cidoc-crm/E36_Visual_Item"/>
        <rdfs:comment xml:lang="en">Quantification of the inverse property: many to many (0,n:0,n)

Scope note of the inverse property:
This property establishes the relationship between an instance of E36 Visual Item and the instance of E1 CRM Entity that it visually represents.
Any entity may be represented visually. This property is part of the fully developed path from E24 Physical Human-Made Thing through P65 shows visual item (is shown by), E36 Visual Item, P138 represents (has representation) to E1 CRM Entity, which is shortcut by P62 depicts (is depicted by). P138.1 mode of representation allows the nature of the representation to be refined.
This property is also used for the relationship between an original and a digitisation of the original by the use of techniques such as digital photography, flatbed or infrared scanning. Digitisation is here seen as a process with a mechanical, causal component rendering the spatial distribution of structural and optical properties of the original and does not necessarily include any visual similarity identifiable by human observation.

Examples of the inverse property:
- The digital file found at https://www.emunch.no/N/full/No-MM_N0001-01.jpg (E36) represents page 1 of Edward Munch&apos;s manuscript MM N 1, Munch-museet (E22) mode of representation Digitisation (E55).
- The 3D model VAM_A.200-1946_trace_1M.ply (E73) represents Victoria &amp; Albert Museum’s Madonna and child sculpture (visual work) A.200-1946 (E22) mode of representation 3D surface (E55).

In First Order Logic of the inverse property:
- P138(x,y) ⇒ E36(x)
- P138(x,y) ⇒ E1(y) 
- P138(x,y,z) ⇒ [P138(x,y) ∧ E55(z)]
- P138(x,y) ⇒ P67(x,y)
</rdfs:comment>
        <rdfs:label xml:lang="fr">P138i est représenté par</rdfs:label>
        <rdfs:label xml:lang="en">P138i has representation</rdfs:label>
        <rdfs:label xml:lang="pt">P138i tem representação</rdfs:label>
        <rdfs:label xml:lang="de">P138i wird dargestellt durch</rdfs:label>
        <rdfs:label xml:lang="el">P138i παριστάνεται από</rdfs:label>
        <rdfs:label xml:lang="ru">P138i имeeт прeдставлeниe</rdfs:label>
        <rdfs:label xml:lang="zh">P138i 有描绘</rdfs:label>
        <skos:notation xml:lang="en">P138i</skos:notation>
        <skos:prefLabel xml:lang="fr">est représenté par</skos:prefLabel>
        <skos:prefLabel xml:lang="en">has representation</skos:prefLabel>
        <skos:prefLabel xml:lang="pt">tem representação</skos:prefLabel>
        <skos:prefLabel xml:lang="de">wird dargestellt durch</skos:prefLabel>
        <skos:prefLabel xml:lang="el">παριστάνεται από</skos:prefLabel>
        <skos:prefLabel xml:lang="ru">имeeт прeдставлeниe</skos:prefLabel>
        <skos:prefLabel xml:lang="zh">有描绘</skos:prefLabel>
    </owl:ObjectProperty>
    


    <!-- http://www.cidoc-crm.org/cidoc-crm/P140_assigned_attribute_to -->

    <owl:ObjectProperty rdf:about="http://www.cidoc-crm.org/cidoc-crm/P140_assigned_attribute_to">
        <owl:inverseOf rdf:resource="http://www.cidoc-crm.org/cidoc-crm/P140i_was_attributed_by"/>
        <rdfs:domain rdf:resource="http://www.cidoc-crm.org/cidoc-crm/E13_Attribute_Assignment"/>
        <rdfs:range rdf:resource="http://www.cidoc-crm.org/cidoc-crm/E1_CRM_Entity"/>
        <rdfs:comment xml:lang="en">Quantification: many to many (0,n:0,n)

Scope note:
This property associates an instance of E13 Attribute Assignment with the instance of E1 CRM Entity about which it made an attribution. The instance of E1 CRM Entity plays the role of the domain of the attribution. 
The kind of attribution made should be documented using P177 assigned property of type (is type of property assigned).

Examples:
- The Current Ownership Assessment of Martin Doerr’s silver cup February 1997 (E13) assigned attribute to Martin Doerr’s silver cup (E22). (fictitious)
- The Identifier Assignment on 1(st) June 1997 of the silver cup donated by Martin Doerr (E15) assigned attribute to silver cup 232 (E22). (fictitious)
- The examination of MS Sinai Greek 418 (E13) assigned attribute to MS Sinai Greek 418 (E22). (Honey and Pickwoad, 2010)

In First Order Logic:
- P140(x,y) ⇒ E13(x)
- P140(x,y) ⇒ E1(y)
</rdfs:comment>
        <rdfs:label xml:lang="fr">P140 a assigné l’attribut à</rdfs:label>
        <rdfs:label xml:lang="en">P140 assigned attribute to</rdfs:label>
        <rdfs:label xml:lang="pt">P140 atribuiu atributo para</rdfs:label>
        <rdfs:label xml:lang="de">P140 wies Merkmal zu</rdfs:label>
        <rdfs:label xml:lang="el">P140 απέδωσε ιδιότητα σε</rdfs:label>
        <rdfs:label xml:lang="ru">P140 получeн атрибут посрeдством</rdfs:label>
        <rdfs:label xml:lang="zh">P140 分配属性于</rdfs:label>
        <skos:notation xml:lang="en">P140</skos:notation>
        <skos:prefLabel xml:lang="fr">a assigné l’attribut à</skos:prefLabel>
        <skos:prefLabel xml:lang="en">assigned attribute to</skos:prefLabel>
        <skos:prefLabel xml:lang="pt">atribuiu atributo para</skos:prefLabel>
        <skos:prefLabel xml:lang="de">wies Merkmal zu</skos:prefLabel>
        <skos:prefLabel xml:lang="el">απέδωσε ιδιότητα σε</skos:prefLabel>
        <skos:prefLabel xml:lang="ru">получeн атрибут посрeдством</skos:prefLabel>
        <skos:prefLabel xml:lang="zh">分配属性于</skos:prefLabel>
    </owl:ObjectProperty>
    


    <!-- http://www.cidoc-crm.org/cidoc-crm/P140i_was_attributed_by -->

    <owl:ObjectProperty rdf:about="http://www.cidoc-crm.org/cidoc-crm/P140i_was_attributed_by">
        <rdfs:domain rdf:resource="http://www.cidoc-crm.org/cidoc-crm/E1_CRM_Entity"/>
        <rdfs:range rdf:resource="http://www.cidoc-crm.org/cidoc-crm/E13_Attribute_Assignment"/>
        <rdfs:comment xml:lang="en">Quantification of the inverse property: many to many (0,n:0,n)

Scope note of the inverse property:
This property associates an instance of E13 Attribute Assignment with the instance of E1 CRM Entity about which it made an attribution. The instance of E1 CRM Entity plays the role of the domain of the attribution. 
The kind of attribution made should be documented using P177 assigned property of type (is type of property assigned).

Examples of the inverse property:
- The Current Ownership Assessment of Martin Doerr’s silver cup February 1997 (E13) assigned attribute to Martin Doerr’s silver cup (E22). (fictitious)
- The Identifier Assignment on 1(st) June 1997 of the silver cup donated by Martin Doerr (E15) assigned attribute to silver cup 232 (E22). (fictitious)
- The examination of MS Sinai Greek 418 (E13) assigned attribute to MS Sinai Greek 418 (E22). (Honey and Pickwoad, 2010)

In First Order Logic of the inverse property:
- P140(x,y) ⇒ E13(x)
- P140(x,y) ⇒ E1(y)
</rdfs:comment>
        <rdfs:label xml:lang="fr">P140i a reçu l’attribut par</rdfs:label>
        <rdfs:label xml:lang="de">P140i bekam Merkmal zugewiesen durch</rdfs:label>
        <rdfs:label xml:lang="pt">P140i foi atribuído por</rdfs:label>
        <rdfs:label xml:lang="en">P140i was attributed by</rdfs:label>
        <rdfs:label xml:lang="el">P140i χαρακτηρίστηκε από</rdfs:label>
        <rdfs:label xml:lang="ru">P140i присвоeн атрибут</rdfs:label>
        <rdfs:label xml:lang="zh">P140i 接受属性</rdfs:label>
        <skos:notation xml:lang="en">P140i</skos:notation>
        <skos:prefLabel xml:lang="fr">a reçu l’attribut par</skos:prefLabel>
        <skos:prefLabel xml:lang="de">bekam Merkmal zugewiesen durch</skos:prefLabel>
        <skos:prefLabel xml:lang="pt">foi atribuído por</skos:prefLabel>
        <skos:prefLabel xml:lang="en">was attributed by</skos:prefLabel>
        <skos:prefLabel xml:lang="el">χαρακτηρίστηκε από</skos:prefLabel>
        <skos:prefLabel xml:lang="ru">присвоeн атрибут</skos:prefLabel>
        <skos:prefLabel xml:lang="zh">接受属性</skos:prefLabel>
    </owl:ObjectProperty>
    


    <!-- http://www.cidoc-crm.org/cidoc-crm/P141_assigned -->

    <owl:ObjectProperty rdf:about="http://www.cidoc-crm.org/cidoc-crm/P141_assigned">
        <owl:inverseOf rdf:resource="http://www.cidoc-crm.org/cidoc-crm/P141i_was_assigned_by"/>
        <rdfs:domain rdf:resource="http://www.cidoc-crm.org/cidoc-crm/E13_Attribute_Assignment"/>
        <rdfs:range rdf:resource="http://www.cidoc-crm.org/cidoc-crm/E1_CRM_Entity"/>
        <rdfs:comment xml:lang="en">Quantification: many to many (0,n:0,n)

Scope note:
This property associates an instance of E13 Attribute Assignment with the instance of E1 CRM Entity used in the attribution. The instance of E1 CRM Entity here plays the role of the range of the attribution.
The kind of attribution made should be documented using P177 assigned property of type (is type of property assigned).

Examples:
- The Current Ownership Assessment of Martin Doerr’s silver cup February 1997 (E13) assigned Martin Doerr (E21). (fictitious)
- The Identifier Assignment on 1(st) June 1997 of the silver cup donated by Martin Doerr (E15) assigned 232 (E42). (fictitious)
- The examination of MS Sinai Greek 418 (E13) assigned unsupported (E55.) (Honey &amp; Pickwoad, 2010)

In First Order Logic:
- P141(x,y) ⇒ E13(x)
- P141(x,y) ⇒ E1(y)
</rdfs:comment>
        <rdfs:label xml:lang="fr">P141 a attribué</rdfs:label>
        <rdfs:label xml:lang="en">P141 assigned</rdfs:label>
        <rdfs:label xml:lang="pt">P141 atribuiu</rdfs:label>
        <rdfs:label xml:lang="de">P141 wies zu</rdfs:label>
        <rdfs:label xml:lang="el">P141 απέδωσε</rdfs:label>
        <rdfs:label xml:lang="ru">P141 назначил</rdfs:label>
        <rdfs:label xml:lang="zh">P141 分配</rdfs:label>
        <skos:notation xml:lang="en">P141</skos:notation>
        <skos:prefLabel xml:lang="fr">a attribué</skos:prefLabel>
        <skos:prefLabel xml:lang="en">assigned</skos:prefLabel>
        <skos:prefLabel xml:lang="pt">atribuiu</skos:prefLabel>
        <skos:prefLabel xml:lang="de">wies zu</skos:prefLabel>
        <skos:prefLabel xml:lang="el">απέδωσε</skos:prefLabel>
        <skos:prefLabel xml:lang="ru">назначил</skos:prefLabel>
        <skos:prefLabel xml:lang="zh">分配</skos:prefLabel>
    </owl:ObjectProperty>
    


    <!-- http://www.cidoc-crm.org/cidoc-crm/P141i_was_assigned_by -->

    <owl:ObjectProperty rdf:about="http://www.cidoc-crm.org/cidoc-crm/P141i_was_assigned_by">
        <rdfs:domain rdf:resource="http://www.cidoc-crm.org/cidoc-crm/E1_CRM_Entity"/>
        <rdfs:range rdf:resource="http://www.cidoc-crm.org/cidoc-crm/E13_Attribute_Assignment"/>
        <rdfs:comment xml:lang="en">Quantification of the inverse property: many to many (0,n:0,n)

Scope note of the inverse property:
This property associates an instance of E13 Attribute Assignment with the instance of E1 CRM Entity used in the attribution. The instance of E1 CRM Entity here plays the role of the range of the attribution.
The kind of attribution made should be documented using P177 assigned property of type (is type of property assigned).

Examples of the inverse property:
- The Current Ownership Assessment of Martin Doerr’s silver cup February 1997 (E13) assigned Martin Doerr (E21). (fictitious)
- The Identifier Assignment on 1(st) June 1997 of the silver cup donated by Martin Doerr (E15) assigned 232 (E42). (fictitious)
- The examination of MS Sinai Greek 418 (E13) assigned unsupported (E55.) (Honey &amp; Pickwoad, 2010)

In First Order Logic of the inverse property:
- P141(x,y) ⇒ E13(x)
- P141(x,y) ⇒ E1(y)
</rdfs:comment>
        <rdfs:label xml:lang="fr">P141i a été attribué par</rdfs:label>
        <rdfs:label xml:lang="pt">P141i foi atribuído por</rdfs:label>
        <rdfs:label xml:lang="en">P141i was assigned by</rdfs:label>
        <rdfs:label xml:lang="de">P141i wurde zugewiesen durch</rdfs:label>
        <rdfs:label xml:lang="el">P141i αποδόθηκε από</rdfs:label>
        <rdfs:label xml:lang="ru">P141i назначeн посрeдством</rdfs:label>
        <rdfs:label xml:lang="zh">P141i 被分配</rdfs:label>
        <skos:notation xml:lang="en">P141i</skos:notation>
        <skos:prefLabel xml:lang="fr">a été attribué par</skos:prefLabel>
        <skos:prefLabel xml:lang="pt">foi atribuído por</skos:prefLabel>
        <skos:prefLabel xml:lang="en">was assigned by</skos:prefLabel>
        <skos:prefLabel xml:lang="de">wurde zugewiesen durch</skos:prefLabel>
        <skos:prefLabel xml:lang="el">αποδόθηκε από</skos:prefLabel>
        <skos:prefLabel xml:lang="ru">назначeн посрeдством</skos:prefLabel>
        <skos:prefLabel xml:lang="zh">被分配</skos:prefLabel>
    </owl:ObjectProperty>
    


    <!-- http://www.cidoc-crm.org/cidoc-crm/P14_carried_out_by -->

    <owl:ObjectProperty rdf:about="http://www.cidoc-crm.org/cidoc-crm/P14_carried_out_by">
        <rdfs:subPropertyOf rdf:resource="http://www.cidoc-crm.org/cidoc-crm/P11_had_participant"/>
        <owl:inverseOf rdf:resource="http://www.cidoc-crm.org/cidoc-crm/P14i_performed"/>
        <rdfs:domain rdf:resource="http://www.cidoc-crm.org/cidoc-crm/E7_Activity"/>
        <rdfs:range rdf:resource="http://www.cidoc-crm.org/cidoc-crm/E39_Actor"/>
        <rdfs:comment xml:lang="en">Quantification: many to many, necessary (1,n:0,n)

Scope note:
This property describes the active participation of an instance of E39 Actor in an instance of E7 Activity. 
It implies causal or legal responsibility. The P14.1 in the role of property of the property specifies the nature of an Actor’s participation.

Examples:
- The painting of the Sistine Chapel (E7) carried out by Michelangelo Buonaroti (E21) in the role of master craftsman (E55). (Goldscheider, 1953)

Properties:
- P14.1 in the role of: E55 Type

In First Order Logic:
- P14(x,y) ⇒ E7(x)
- P14(x,y)⇒ E39(y)
- P14(x,y) ⇒ P11(x,y)
- P14(x,y,z) ⇒ [P14(x,y) ∧ E55(z)]
</rdfs:comment>
        <rdfs:label xml:lang="fr">P14 a été effectué par</rdfs:label>
        <rdfs:label xml:lang="en">P14 carried out by</rdfs:label>
        <rdfs:label xml:lang="pt">P14 realizada por</rdfs:label>
        <rdfs:label xml:lang="de">P14 wurde ausgeführt von</rdfs:label>
        <rdfs:label xml:lang="el">P14 πραγματοποιήθηκε από</rdfs:label>
        <rdfs:label xml:lang="ru">P14 выполнялся</rdfs:label>
        <rdfs:label xml:lang="zh">P14 执行者是</rdfs:label>
        <skos:notation xml:lang="en">P14</skos:notation>
        <skos:prefLabel xml:lang="fr">a été effectué par</skos:prefLabel>
        <skos:prefLabel xml:lang="en">carried out by</skos:prefLabel>
        <skos:prefLabel xml:lang="pt">realizada por</skos:prefLabel>
        <skos:prefLabel xml:lang="de">wurde ausgeführt von</skos:prefLabel>
        <skos:prefLabel xml:lang="el">πραγματοποιήθηκε από</skos:prefLabel>
        <skos:prefLabel xml:lang="ru">выполнялся</skos:prefLabel>
        <skos:prefLabel xml:lang="zh">执行者是</skos:prefLabel>
    </owl:ObjectProperty>
    


    <!-- http://www.cidoc-crm.org/cidoc-crm/P14i_performed -->

    <owl:ObjectProperty rdf:about="http://www.cidoc-crm.org/cidoc-crm/P14i_performed">
        <rdfs:subPropertyOf rdf:resource="http://www.cidoc-crm.org/cidoc-crm/P11i_participated_in"/>
        <rdfs:domain rdf:resource="http://www.cidoc-crm.org/cidoc-crm/E39_Actor"/>
        <rdfs:range rdf:resource="http://www.cidoc-crm.org/cidoc-crm/E7_Activity"/>
        <rdfs:comment xml:lang="en">Quantification of the inverse property: many to many, necessary (1,n:0,n)

Scope note of the inverse property:
This property describes the active participation of an instance of E39 Actor in an instance of E7 Activity. 
It implies causal or legal responsibility. The P14.1 in the role of property of the property specifies the nature of an Actor’s participation.

Examples of the inverse property:
- The painting of the Sistine Chapel (E7) carried out by Michelangelo Buonaroti (E21) in the role of master craftsman (E55). (Goldscheider, 1953)

In First Order Logic of the inverse property:
- P14(x,y) ⇒ E7(x)
- P14(x,y)⇒ E39(y)
- P14(x,y) ⇒ P11(x,y)
- P14(x,y,z) ⇒ [P14(x,y) ∧ E55(z)]
</rdfs:comment>
        <rdfs:label xml:lang="fr">P14i a effectué</rdfs:label>
        <rdfs:label xml:lang="pt">P14i executou</rdfs:label>
        <rdfs:label xml:lang="de">P14i führte aus</rdfs:label>
        <rdfs:label xml:lang="en">P14i performed</rdfs:label>
        <rdfs:label xml:lang="el">P14i πραγματοποίησε</rdfs:label>
        <rdfs:label xml:lang="ru">P14i выполнял</rdfs:label>
        <rdfs:label xml:lang="zh">P14i 执行</rdfs:label>
        <skos:notation xml:lang="en">P14i</skos:notation>
        <skos:prefLabel xml:lang="fr">a effectué</skos:prefLabel>
        <skos:prefLabel xml:lang="pt">executou</skos:prefLabel>
        <skos:prefLabel xml:lang="de">führte aus</skos:prefLabel>
        <skos:prefLabel xml:lang="en">performed</skos:prefLabel>
        <skos:prefLabel xml:lang="el">πραγματοποίησε</skos:prefLabel>
        <skos:prefLabel xml:lang="ru">выполнял</skos:prefLabel>
        <skos:prefLabel xml:lang="zh">执行</skos:prefLabel>
    </owl:ObjectProperty>
    


    <!-- http://www.cidoc-crm.org/cidoc-crm/P1_is_identified_by -->

    <owl:ObjectProperty rdf:about="http://www.cidoc-crm.org/cidoc-crm/P1_is_identified_by">
        <owl:inverseOf rdf:resource="http://www.cidoc-crm.org/cidoc-crm/P1i_identifies"/>
        <rdfs:domain rdf:resource="http://www.cidoc-crm.org/cidoc-crm/E1_CRM_Entity"/>
        <rdfs:range rdf:resource="http://www.cidoc-crm.org/cidoc-crm/E41_Appellation"/>
        <rdfs:comment xml:lang="en">Quantification: many to many (0,n:0,n)

Scope note:
This property describes the naming or identification of any real-world item by a name or any other identifier. 
This property is intended for identifiers in general use, which form part of the world the model intends to describe, and not merely for internal database identifiers which are specific to a technical system, unless these latter also have a more general use outside the technical context. This property includes in particular identification by mathematical expressions such as coordinate systems used for the identification of instances of E53 Place. The property does not reveal anything about when, where and by whom this identifier was used. A more detailed representation can be made using the fully developed (i.e. indirect) path through E15 Identifier Assignment.
This property is a shortcut for the path from E1 CRM Entity through P140i was attributed by, E15 Identifier Assignment, P37 assigned to E42 Identifier. 
It is also a shortcut for the path from E1 CRM Entity through P1 is identified by, E41 Appellation, P139 has alternative form to E41 Appellation.

Examples:
- The capital of Italy (E53) is identified by “Rome” (E41). (Leach, 2017)
- Text 25014–32 (E33) is identified by “The Decline and Fall of the Roman Empire” (E35). (Gibbon, 2013)

In First Order Logic:
- P1(x,y) ⇒ E1(x)
- P1(x,y) ⇒ E41(y)
- P1(x,y) ⇐ (∃z) [E15(z)˄ P140i(x,z) ˄ P37(z,y)]
- P1(x,y) ⇐ (∃z) [E41(z)˄ P1(x,z) ˄ P139(z,y)]
</rdfs:comment>
        <rdfs:label xml:lang="fr">P1 est identifié par</rdfs:label>
        <rdfs:label xml:lang="en">P1 is identified by</rdfs:label>
        <rdfs:label xml:lang="de">P1 wird bezeichnet als</rdfs:label>
        <rdfs:label xml:lang="pt">P1 é identificado por</rdfs:label>
        <rdfs:label xml:lang="el">P1 αναγνωρίζεται ως</rdfs:label>
        <rdfs:label xml:lang="ru">P1 идeнтифицируeтся</rdfs:label>
        <rdfs:label xml:lang="zh">P1 被标识为</rdfs:label>
        <skos:notation xml:lang="en">P1</skos:notation>
        <skos:prefLabel xml:lang="fr">est identifié par</skos:prefLabel>
        <skos:prefLabel xml:lang="en">is identified by</skos:prefLabel>
        <skos:prefLabel xml:lang="de">wird bezeichnet als</skos:prefLabel>
        <skos:prefLabel xml:lang="pt">é identificado por</skos:prefLabel>
        <skos:prefLabel xml:lang="el">αναγνωρίζεται ως</skos:prefLabel>
        <skos:prefLabel xml:lang="ru">идeнтифицируeтся</skos:prefLabel>
        <skos:prefLabel xml:lang="zh">被标识为</skos:prefLabel>
    </owl:ObjectProperty>
    


    <!-- http://www.cidoc-crm.org/cidoc-crm/P1i_identifies -->

    <owl:ObjectProperty rdf:about="http://www.cidoc-crm.org/cidoc-crm/P1i_identifies">
        <rdfs:domain rdf:resource="http://www.cidoc-crm.org/cidoc-crm/E41_Appellation"/>
        <rdfs:range rdf:resource="http://www.cidoc-crm.org/cidoc-crm/E1_CRM_Entity"/>
        <rdfs:comment xml:lang="en">Quantification of the inverse property: many to many (0,n:0,n)

Scope note of the inverse property:
This property describes the naming or identification of any real-world item by a name or any other identifier. 
This property is intended for identifiers in general use, which form part of the world the model intends to describe, and not merely for internal database identifiers which are specific to a technical system, unless these latter also have a more general use outside the technical context. This property includes in particular identification by mathematical expressions such as coordinate systems used for the identification of instances of E53 Place. The property does not reveal anything about when, where and by whom this identifier was used. A more detailed representation can be made using the fully developed (i.e. indirect) path through E15 Identifier Assignment.
This property is a shortcut for the path from E1 CRM Entity through P140i was attributed by, E15 Identifier Assignment, P37 assigned to E42 Identifier. 
It is also a shortcut for the path from E1 CRM Entity through P1 is identified by, E41 Appellation, P139 has alternative form to E41 Appellation.

Examples of the inverse property:
- The capital of Italy (E53) is identified by “Rome” (E41). (Leach, 2017)
- Text 25014–32 (E33) is identified by “The Decline and Fall of the Roman Empire” (E35). (Gibbon, 2013)

In First Order Logic of the inverse property:
- P1(x,y) ⇒ E1(x)
- P1(x,y) ⇒ E41(y)
- P1(x,y) ⇐ (∃z) [E15(z)˄ P140i(x,z) ˄ P37(z,y)]
- P1(x,y) ⇐ (∃z) [E41(z)˄ P1(x,z) ˄ P139(z,y)]
</rdfs:comment>
        <rdfs:label xml:lang="de">P1i bezeichnet</rdfs:label>
        <rdfs:label xml:lang="pt">P1i identifica</rdfs:label>
        <rdfs:label xml:lang="fr">P1i identifie</rdfs:label>
        <rdfs:label xml:lang="en">P1i identifies</rdfs:label>
        <rdfs:label xml:lang="el">P1i είναι αναγνωριστικό</rdfs:label>
        <rdfs:label xml:lang="ru">P1i идeнтифицируeт</rdfs:label>
        <rdfs:label xml:lang="zh">P1i 标识</rdfs:label>
        <skos:notation xml:lang="en">P1i</skos:notation>
        <skos:prefLabel xml:lang="de">bezeichnet</skos:prefLabel>
        <skos:prefLabel xml:lang="pt">identifica</skos:prefLabel>
        <skos:prefLabel xml:lang="fr">identifie</skos:prefLabel>
        <skos:prefLabel xml:lang="en">identifies</skos:prefLabel>
        <skos:prefLabel xml:lang="el">είναι αναγνωριστικό</skos:prefLabel>
        <skos:prefLabel xml:lang="ru">идeнтифицируeт</skos:prefLabel>
        <skos:prefLabel xml:lang="zh">标识</skos:prefLabel>
    </owl:ObjectProperty>
    


    <!-- http://www.cidoc-crm.org/cidoc-crm/P39_measured -->

    <owl:ObjectProperty rdf:about="http://www.cidoc-crm.org/cidoc-crm/P39_measured">
        <rdfs:subPropertyOf rdf:resource="http://www.cidoc-crm.org/cidoc-crm/P140_assigned_attribute_to"/>
        <owl:inverseOf rdf:resource="http://www.cidoc-crm.org/cidoc-crm/P39i_was_measured_by"/>
        <rdfs:domain rdf:resource="http://www.cidoc-crm.org/cidoc-crm/E16_Measurement"/>
        <rdfs:range rdf:resource="http://www.cidoc-crm.org/cidoc-crm/E18_Physical_Thing"/>
        <rdfs:comment xml:lang="en">Quantification: many to one, necessary (1,1:0,n)

Scope note:
This property associates an instance of E16 Measurement with the instance of E18 Physical Thing upon which it acted. The instance of E16 Measurement is specific to the measured object. An instance of E18 Physical Thing may be measured more than once with different results, constituting different instances of E16 Measurement.

Examples:
- The measurement of the height of silver cup 232 on 31(st) August 1997 (E16) measured silver cup 232 (E22). (fictitious)
- The carbon 14 dating of the “Schoeninger Speer II” in 1996 (E16) measured the “Schoeninger Speer II” (E22). [The carbon 14 dating of an approximately 400.000 year old complete Old Palaeolithic wooden spear found in Schoeningen, Niedersachsen, Germany, in 1995. See also, E16 Measurement.] (Kouwenhoven, 1997)

In First Order Logic:
- P39(x,y) ⇒ E16(x) 
- P39(x,y) ⇒ E18(y) 
- P39(x,y) ⇒ P140(x,y)
</rdfs:comment>
        <rdfs:label xml:lang="fr">P39 a mesuré</rdfs:label>
        <rdfs:label xml:lang="en">P39 measured</rdfs:label>
        <rdfs:label xml:lang="pt">P39 mediu</rdfs:label>
        <rdfs:label xml:lang="de">P39 vermaß</rdfs:label>
        <rdfs:label xml:lang="el">P39 μέτρησε</rdfs:label>
        <rdfs:label xml:lang="ru">P39 измeрил</rdfs:label>
        <rdfs:label xml:lang="zh">P39 测量了</rdfs:label>
        <skos:notation xml:lang="en">P39</skos:notation>
        <skos:prefLabel xml:lang="fr">a mesuré</skos:prefLabel>
        <skos:prefLabel xml:lang="en">measured</skos:prefLabel>
        <skos:prefLabel xml:lang="pt">mediu</skos:prefLabel>
        <skos:prefLabel xml:lang="de">vermaß</skos:prefLabel>
        <skos:prefLabel xml:lang="el">μέτρησε</skos:prefLabel>
        <skos:prefLabel xml:lang="ru">измeрил</skos:prefLabel>
        <skos:prefLabel xml:lang="zh">测量了</skos:prefLabel>
    </owl:ObjectProperty>
    


    <!-- http://www.cidoc-crm.org/cidoc-crm/P39i_was_measured_by -->

    <owl:ObjectProperty rdf:about="http://www.cidoc-crm.org/cidoc-crm/P39i_was_measured_by">
        <rdfs:subPropertyOf rdf:resource="http://www.cidoc-crm.org/cidoc-crm/P140i_was_attributed_by"/>
        <rdfs:domain rdf:resource="http://www.cidoc-crm.org/cidoc-crm/E18_Physical_Thing"/>
        <rdfs:range rdf:resource="http://www.cidoc-crm.org/cidoc-crm/E16_Measurement"/>
        <rdfs:comment xml:lang="en">Quantification of the inverse property: many to one, necessary (1,1:0,n)

Scope note of the inverse property:
This property associates an instance of E16 Measurement with the instance of E18 Physical Thing upon which it acted. The instance of E16 Measurement is specific to the measured object. An instance of E18 Physical Thing may be measured more than once with different results, constituting different instances of E16 Measurement.

Examples of the inverse property:
- The measurement of the height of silver cup 232 on 31(st) August 1997 (E16) measured silver cup 232 (E22). (fictitious)
- The carbon 14 dating of the “Schoeninger Speer II” in 1996 (E16) measured the “Schoeninger Speer II” (E22). [The carbon 14 dating of an approximately 400.000 year old complete Old Palaeolithic wooden spear found in Schoeningen, Niedersachsen, Germany, in 1995. See also, E16 Measurement.] (Kouwenhoven, 1997)

In First Order Logic of the inverse property:
- P39(x,y) ⇒ E16(x) 
- P39(x,y) ⇒ E18(y) 
- P39(x,y) ⇒ P140(x,y)
</rdfs:comment>
        <rdfs:label xml:lang="fr">P39i a été mesuré par</rdfs:label>
        <rdfs:label xml:lang="pt">P39i foi medida por</rdfs:label>
        <rdfs:label xml:lang="en">P39i was measured by</rdfs:label>
        <rdfs:label xml:lang="de">P39i wurde vermessen durch</rdfs:label>
        <rdfs:label xml:lang="el">P39i μετρήθηκε από</rdfs:label>
        <rdfs:label xml:lang="ru">P39i был измeрeн</rdfs:label>
        <rdfs:label xml:lang="zh">P39i 被测量</rdfs:label>
        <skos:notation xml:lang="en">P39i</skos:notation>
        <skos:prefLabel xml:lang="fr">a été mesuré par</skos:prefLabel>
        <skos:prefLabel xml:lang="pt">foi medida por</skos:prefLabel>
        <skos:prefLabel xml:lang="en">was measured by</skos:prefLabel>
        <skos:prefLabel xml:lang="de">wurde vermessen durch</skos:prefLabel>
        <skos:prefLabel xml:lang="el">μετρήθηκε από</skos:prefLabel>
        <skos:prefLabel xml:lang="ru">был измeрeн</skos:prefLabel>
        <skos:prefLabel xml:lang="zh">被测量</skos:prefLabel>
    </owl:ObjectProperty>
    


    <!-- http://www.cidoc-crm.org/cidoc-crm/P40_observed_dimension -->

    <owl:ObjectProperty rdf:about="http://www.cidoc-crm.org/cidoc-crm/P40_observed_dimension">
        <rdfs:subPropertyOf rdf:resource="http://www.cidoc-crm.org/cidoc-crm/P141_assigned"/>
        <owl:inverseOf rdf:resource="http://www.cidoc-crm.org/cidoc-crm/P40i_was_observed_in"/>
        <rdfs:domain rdf:resource="http://www.cidoc-crm.org/cidoc-crm/E16_Measurement"/>
        <rdfs:range rdf:resource="http://www.cidoc-crm.org/cidoc-crm/E54_Dimension"/>
        <rdfs:comment xml:lang="en">Quantification: many to many, necessary (1,n:0,n)

Scope note:
This property records the dimension that was observed in an E16 Measurement Event.
E54 Dimension can be any quantifiable aspect of E70 Thing. Weight, image colour depth and monetary value are dimensions in this sense. One measurement activity may determine more than one dimension of one object.
Dimensions may be determined either by direct observation or using recorded evidence. In the latter case the measured Thing does not need to be present or extant.
Even though knowledge of the value of a dimension requires measurement, the dimension may be an object of discourse prior to, or even without, any measurement being made.

Examples:
- The measurement of the height of silver cup 232 on 31(st) August 1997 (E16) observed dimension silver cup 232 height (E54). [which has unit mm (E58), has value 224 (E60)] (fictitious)
- The carbon 14 dating of the “Schoeninger Speer II” in 1996 (E16) observed dimension the carbon 14 based temporal distance from 1996 to the growth of the wood of the “Schoeninger Speer II” (E60). [The carbon 14 dating of an approximately 400.000 year old complete Old Palaeolithic wooden spear found in Schoeningen, Niederachsen, Germany, in 1995. See also: E16 Measurement.] (Kouwenhoven, 1997)

In First Order Logic:
- P40(x,y) ⇒ E16(x)
- P40(x,y)⇒ E54(y)
- P40(x,y) ⇒ P141(x,y)
</rdfs:comment>
        <rdfs:label xml:lang="fr">P40 a relevé comme dimension</rdfs:label>
        <rdfs:label xml:lang="de">P40 beobachtete Dimension</rdfs:label>
        <rdfs:label xml:lang="en">P40 observed dimension</rdfs:label>
        <rdfs:label xml:lang="pt">P40 verificou a dimensão</rdfs:label>
        <rdfs:label xml:lang="el">P40 παρατήρησε</rdfs:label>
        <rdfs:label xml:lang="ru">P40 наблюдаeмый размeр</rdfs:label>
        <rdfs:label xml:lang="zh">P40 观测度量规格</rdfs:label>
        <skos:notation xml:lang="en">P40</skos:notation>
        <skos:prefLabel xml:lang="fr">a relevé comme dimension</skos:prefLabel>
        <skos:prefLabel xml:lang="de">beobachtete Dimension</skos:prefLabel>
        <skos:prefLabel xml:lang="en">observed dimension</skos:prefLabel>
        <skos:prefLabel xml:lang="pt">verificou a dimensão</skos:prefLabel>
        <skos:prefLabel xml:lang="el">παρατήρησε</skos:prefLabel>
        <skos:prefLabel xml:lang="ru">наблюдаeмый размeр</skos:prefLabel>
        <skos:prefLabel xml:lang="zh">观测度量规格</skos:prefLabel>
    </owl:ObjectProperty>
    


    <!-- http://www.cidoc-crm.org/cidoc-crm/P40i_was_observed_in -->

    <owl:ObjectProperty rdf:about="http://www.cidoc-crm.org/cidoc-crm/P40i_was_observed_in">
        <rdfs:subPropertyOf rdf:resource="http://www.cidoc-crm.org/cidoc-crm/P141i_was_assigned_by"/>
        <rdfs:domain rdf:resource="http://www.cidoc-crm.org/cidoc-crm/E54_Dimension"/>
        <rdfs:range rdf:resource="http://www.cidoc-crm.org/cidoc-crm/E16_Measurement"/>
        <rdfs:comment xml:lang="en">Quantification of the inverse property: many to many, necessary (1,n:0,n)

Scope note of the inverse property:
This property records the dimension that was observed in an E16 Measurement Event.
E54 Dimension can be any quantifiable aspect of E70 Thing. Weight, image colour depth and monetary value are dimensions in this sense. One measurement activity may determine more than one dimension of one object.
Dimensions may be determined either by direct observation or using recorded evidence. In the latter case the measured Thing does not need to be present or extant.
Even though knowledge of the value of a dimension requires measurement, the dimension may be an object of discourse prior to, or even without, any measurement being made.

Examples of the inverse property:
- The measurement of the height of silver cup 232 on 31(st) August 1997 (E16) observed dimension silver cup 232 height (E54). [which has unit mm (E58), has value 224 (E60)] (fictitious)
- The carbon 14 dating of the “Schoeninger Speer II” in 1996 (E16) observed dimension the carbon 14 based temporal distance from 1996 to the growth of the wood of the “Schoeninger Speer II” (E60). [The carbon 14 dating of an approximately 400.000 year old complete Old Palaeolithic wooden spear found in Schoeningen, Niederachsen, Germany, in 1995. See also: E16 Measurement.] (Kouwenhoven, 1997)

In First Order Logic of the inverse property:
- P40(x,y) ⇒ E16(x)
- P40(x,y)⇒ E54(y)
- P40(x,y) ⇒ P141(x,y)
</rdfs:comment>
        <rdfs:label xml:lang="fr">P40i a été relevé par</rdfs:label>
        <rdfs:label xml:lang="pt">P40i foi verificada durante</rdfs:label>
        <rdfs:label xml:lang="en">P40i was observed in</rdfs:label>
        <rdfs:label xml:lang="de">P40i wurde beobachtet in</rdfs:label>
        <rdfs:label xml:lang="el">P40i παρατηρήθηκε από</rdfs:label>
        <rdfs:label xml:lang="ru">P40i наблюдался в</rdfs:label>
        <rdfs:label xml:lang="zh">P40i 被观测</rdfs:label>
        <skos:notation xml:lang="en">P40i</skos:notation>
        <skos:prefLabel xml:lang="fr">a été relevé par</skos:prefLabel>
        <skos:prefLabel xml:lang="pt">foi verificada durante</skos:prefLabel>
        <skos:prefLabel xml:lang="en">was observed in</skos:prefLabel>
        <skos:prefLabel xml:lang="de">wurde beobachtet in</skos:prefLabel>
        <skos:prefLabel xml:lang="el">παρατηρήθηκε από</skos:prefLabel>
        <skos:prefLabel xml:lang="ru">наблюдался в</skos:prefLabel>
        <skos:prefLabel xml:lang="zh">被观测</skos:prefLabel>
    </owl:ObjectProperty>
    


    <!-- http://www.cidoc-crm.org/cidoc-crm/P44_has_condition -->

    <owl:ObjectProperty rdf:about="http://www.cidoc-crm.org/cidoc-crm/P44_has_condition">
        <owl:inverseOf rdf:resource="http://www.cidoc-crm.org/cidoc-crm/P44i_is_condition_of"/>
        <rdfs:domain rdf:resource="http://www.cidoc-crm.org/cidoc-crm/E18_Physical_Thing"/>
        <rdfs:range rdf:resource="http://www.cidoc-crm.org/cidoc-crm/E3_Condition_State"/>
        <rdfs:comment xml:lang="en">Quantification: one to many, dependent (0,n:1,1)

Scope note:
This property records an E3 Condition State for some E18 Physical Thing.
This property is a shortcut of the more fully developed path from E18 Physical Thing through P34i was assessed by, E14 Condition Assessment, P35 has identified to E3 Condition State. It offers no information about how and when the E3 Condition State was established, nor by whom. 
An instance of E3 Condition State is specific to an instance of E18 Physical Thing.

Examples:
- Silver cup 232 (E22) has condition oxidation traces were present in 1997 (E3). [which has type (P2) oxidation traces (E55)] (fictitious)

In First Order Logic:
- P44(x,y) ⇒ E18(x)
- P44(x,y) ⇒ E3(y)
- P44(x,y) ⇐ (∃z) [E14(z) ˄ P34i(x,z) ˄ P35(z,y)]
</rdfs:comment>
        <rdfs:label xml:lang="fr">P44 a pour état matériel</rdfs:label>
        <rdfs:label xml:lang="en">P44 has condition</rdfs:label>
        <rdfs:label xml:lang="de">P44 hat Zustand</rdfs:label>
        <rdfs:label xml:lang="pt">P44 tem estado material</rdfs:label>
        <rdfs:label xml:lang="el">P44 έχει κατάσταση</rdfs:label>
        <rdfs:label xml:lang="ru">P44 имeeт условиe</rdfs:label>
        <rdfs:label xml:lang="zh">P44 有状况</rdfs:label>
        <skos:notation xml:lang="en">P44</skos:notation>
        <skos:prefLabel xml:lang="fr">a pour état matériel</skos:prefLabel>
        <skos:prefLabel xml:lang="en">has condition</skos:prefLabel>
        <skos:prefLabel xml:lang="de">hat Zustand</skos:prefLabel>
        <skos:prefLabel xml:lang="pt">tem estado material</skos:prefLabel>
        <skos:prefLabel xml:lang="el">έχει κατάσταση</skos:prefLabel>
        <skos:prefLabel xml:lang="ru">имeeт условиe</skos:prefLabel>
        <skos:prefLabel xml:lang="zh">有状况</skos:prefLabel>
    </owl:ObjectProperty>
    


    <!-- http://www.cidoc-crm.org/cidoc-crm/P44i_is_condition_of -->

    <owl:ObjectProperty rdf:about="http://www.cidoc-crm.org/cidoc-crm/P44i_is_condition_of">
        <rdfs:domain rdf:resource="http://www.cidoc-crm.org/cidoc-crm/E3_Condition_State"/>
        <rdfs:range rdf:resource="http://www.cidoc-crm.org/cidoc-crm/E18_Physical_Thing"/>
        <rdfs:comment xml:lang="en">Quantification of the inverse property: one to many, dependent (0,n:1,1)

Scope note of the inverse property:
This property records an E3 Condition State for some E18 Physical Thing.
This property is a shortcut of the more fully developed path from E18 Physical Thing through P34i was assessed by, E14 Condition Assessment, P35 has identified to E3 Condition State. It offers no information about how and when the E3 Condition State was established, nor by whom. 
An instance of E3 Condition State is specific to an instance of E18 Physical Thing.

Examples of the inverse property:
- Silver cup 232 (E22) has condition oxidation traces were present in 1997 (E3). [which has type (P2) oxidation traces (E55)] (fictitious)

In First Order Logic of the inverse property:
- P44(x,y) ⇒ E18(x)
- P44(x,y) ⇒ E3(y)
- P44(x,y) ⇐ (∃z) [E14(z) ˄ P34i(x,z) ˄ P35(z,y)]
</rdfs:comment>
        <rdfs:label xml:lang="fr">P44i est l&apos;état matériel de</rdfs:label>
        <rdfs:label xml:lang="pt">P44i estado material de</rdfs:label>
        <rdfs:label xml:lang="en">P44i is condition of</rdfs:label>
        <rdfs:label xml:lang="de">P44i ist Zustand von</rdfs:label>
        <rdfs:label xml:lang="el">P44i είναι κατάσταση του</rdfs:label>
        <rdfs:label xml:lang="ru">P44i являeтся условиeм для</rdfs:label>
        <rdfs:label xml:lang="zh">P44i 是状况</rdfs:label>
        <skos:notation xml:lang="en">P44i</skos:notation>
        <skos:prefLabel xml:lang="fr">est l&apos;état matériel de</skos:prefLabel>
        <skos:prefLabel xml:lang="pt">estado material de</skos:prefLabel>
        <skos:prefLabel xml:lang="en">is condition of</skos:prefLabel>
        <skos:prefLabel xml:lang="de">ist Zustand von</skos:prefLabel>
        <skos:prefLabel xml:lang="el">είναι κατάσταση του</skos:prefLabel>
        <skos:prefLabel xml:lang="ru">являeтся условиeм для</skos:prefLabel>
        <skos:prefLabel xml:lang="zh">是状况</skos:prefLabel>
    </owl:ObjectProperty>
    


    <!-- http://www.cidoc-crm.org/cidoc-crm/P45_consists_of -->

    <owl:ObjectProperty rdf:about="http://www.cidoc-crm.org/cidoc-crm/P45_consists_of">
        <owl:inverseOf rdf:resource="http://www.cidoc-crm.org/cidoc-crm/P45i_is_incorporated_in"/>
        <rdfs:domain rdf:resource="http://www.cidoc-crm.org/cidoc-crm/E18_Physical_Thing"/>
        <rdfs:range rdf:resource="http://www.cidoc-crm.org/cidoc-crm/E57_Material"/>
        <rdfs:comment xml:lang="en">Quantification: many to many, necessary (1,n:0,n)

Scope note:
This property identifies the instances of E57 Materials of which an instance of E18 Physical Thing is composed.
All physical things consist of physical materials. P45 consists of (is incorporated in) allows the different materials to be recorded. P45 consists of (is incorporated in) refers here to observed material as opposed to the consumed raw material.
A material, such as a theoretical alloy, may not have any physical instances.

Examples:
- Silver cup 232 (E22) consists of silver (E57). (fictitious)

In First Order Logic:
- P45(x,y) ⇒ E18(x)
- P45(x,y) ⇒ E57(y)
</rdfs:comment>
        <rdfs:label xml:lang="de">P45 besteht aus</rdfs:label>
        <rdfs:label xml:lang="fr">P45 comprend</rdfs:label>
        <rdfs:label xml:lang="pt">P45 consiste de</rdfs:label>
        <rdfs:label xml:lang="en">P45 consists of</rdfs:label>
        <rdfs:label xml:lang="el">P45 αποτελείται από</rdfs:label>
        <rdfs:label xml:lang="ru">P45 состоит из</rdfs:label>
        <rdfs:label xml:lang="zh">P45 包含</rdfs:label>
        <skos:notation xml:lang="en">P45</skos:notation>
        <skos:prefLabel xml:lang="de">besteht aus</skos:prefLabel>
        <skos:prefLabel xml:lang="fr">comprend</skos:prefLabel>
        <skos:prefLabel xml:lang="pt">consiste de</skos:prefLabel>
        <skos:prefLabel xml:lang="en">consists of</skos:prefLabel>
        <skos:prefLabel xml:lang="el">αποτελείται από</skos:prefLabel>
        <skos:prefLabel xml:lang="ru">состоит из</skos:prefLabel>
        <skos:prefLabel xml:lang="zh">包含</skos:prefLabel>
    </owl:ObjectProperty>
    


    <!-- http://www.cidoc-crm.org/cidoc-crm/P45i_is_incorporated_in -->

    <owl:ObjectProperty rdf:about="http://www.cidoc-crm.org/cidoc-crm/P45i_is_incorporated_in">
        <rdfs:domain rdf:resource="http://www.cidoc-crm.org/cidoc-crm/E57_Material"/>
        <rdfs:range rdf:resource="http://www.cidoc-crm.org/cidoc-crm/E18_Physical_Thing"/>
        <rdfs:comment xml:lang="en">Quantification of the inverse property: many to many, necessary (1,n:0,n)

Scope note of the inverse property:
This property identifies the instances of E57 Materials of which an instance of E18 Physical Thing is composed.
All physical things consist of physical materials. P45 consists of (is incorporated in) allows the different materials to be recorded. P45 consists of (is incorporated in) refers here to observed material as opposed to the consumed raw material.
A material, such as a theoretical alloy, may not have any physical instances.

Examples of the inverse property:
- Silver cup 232 (E22) consists of silver (E57). (fictitious)

In First Order Logic of the inverse property:
- P45(x,y) ⇒ E18(x)
- P45(x,y) ⇒ E57(y)
</rdfs:comment>
        <rdfs:label xml:lang="fr">P45i est inclus dans</rdfs:label>
        <rdfs:label xml:lang="pt">P45i está presente em</rdfs:label>
        <rdfs:label xml:lang="en">P45i is incorporated in</rdfs:label>
        <rdfs:label xml:lang="de">P45i ist enthalten in</rdfs:label>
        <rdfs:label xml:lang="el">P45i είναι ενσωματωμένος/η/ο σε</rdfs:label>
        <rdfs:label xml:lang="ru">P45i входит в состав</rdfs:label>
        <rdfs:label xml:lang="zh">P45i 结合在</rdfs:label>
        <skos:notation xml:lang="en">P45i</skos:notation>
        <skos:prefLabel xml:lang="fr">est inclus dans</skos:prefLabel>
        <skos:prefLabel xml:lang="pt">está presente em</skos:prefLabel>
        <skos:prefLabel xml:lang="en">is incorporated in</skos:prefLabel>
        <skos:prefLabel xml:lang="de">ist enthalten in</skos:prefLabel>
        <skos:prefLabel xml:lang="el">είναι ενσωματωμένος/η/ο σε</skos:prefLabel>
        <skos:prefLabel xml:lang="ru">входит в состав</skos:prefLabel>
        <skos:prefLabel xml:lang="zh">结合在</skos:prefLabel>
    </owl:ObjectProperty>
    


    <!-- http://www.cidoc-crm.org/cidoc-crm/P46_is_composed_of -->

    <owl:ObjectProperty rdf:about="http://www.cidoc-crm.org/cidoc-crm/P46_is_composed_of">
        <owl:inverseOf rdf:resource="http://www.cidoc-crm.org/cidoc-crm/P46i_forms_part_of"/>
        <rdfs:domain rdf:resource="http://www.cidoc-crm.org/cidoc-crm/E18_Physical_Thing"/>
        <rdfs:range rdf:resource="http://www.cidoc-crm.org/cidoc-crm/E18_Physical_Thing"/>
        <rdfs:comment xml:lang="en">Quantification: many to many (0,n:0,n)

Scope note:
This property associates an instance of E18 Physical Thing with another instance of Physical Thing that forms part of it. The spatial extent of the composing part is included in the spatial extent of the whole.
Component elements, since they are themselves instances of E18 Physical Thing, may be further analysed into sub-components, thereby creating a hierarchy of part decomposition. An instance of E18 Physical Thing may be shared between multiple wholes, for example two buildings may share a common wall. This property does not specify when and for how long a component element resided in the respective whole. If a component is not part of a whole from the beginning of existence or until the end of existence of the whole, the classes E79 Part Addition and E90 Part Removal can be used to document when a component became part of a particular whole and/or when it stopped being a part of it. For the time-span of being part of the respective whole, the component is completely contained in the place the whole occupies.
This property is intended to describe specific components that are individually documented, rather than general aspects. Overall descriptions of the structure of an instance of E18 Physical Thing are captured by the P3 has note property.
The instances of E57 Material of which an instance of E18 Physical Thing is composed should be documented using P45 consists of (is incorporated in).
This property is transitive and asymmetric.

Examples:
- The Royal carriage (E22) forms part of the Royal train (E22).
- The “Hog’s Back” (E24) forms part of the “Fosseway” (E24).

In First Order Logic:
- P46(x,y) ⇒ E18(x)
- P46(x,y) ⇒ E18(y)
- P46(x,y) ⇒ P132(x,y)
- [P46(x,y) ∧ P46(y,z)] ⇒ P46(x,z)
- P46(x,y) ⇒ (∃uzw)[E93(u) ∧ P195i (x,u) ∧ E52(z) ∧ P164(u,z) ∧ E93(w) ∧ P195i (w,y) ∧ P164(w,z) ∧ P10(w,u)] 
- P46(x,y) ⇒ ¬P46(y,x)
</rdfs:comment>
        <rdfs:label xml:lang="fr">P46 est composé de</rdfs:label>
        <rdfs:label xml:lang="en">P46 is composed of</rdfs:label>
        <rdfs:label xml:lang="de">P46 ist zusammengesetzt aus</rdfs:label>
        <rdfs:label xml:lang="pt">P46 é composto de</rdfs:label>
        <rdfs:label xml:lang="el">P46 αποτελείται από</rdfs:label>
        <rdfs:label xml:lang="ru">P46 составлeн из</rdfs:label>
        <rdfs:label xml:lang="zh">P46 组成成分是</rdfs:label>
        <skos:notation xml:lang="en">P46</skos:notation>
        <skos:prefLabel xml:lang="fr">est composé de</skos:prefLabel>
        <skos:prefLabel xml:lang="en">is composed of</skos:prefLabel>
        <skos:prefLabel xml:lang="de">ist zusammengesetzt aus</skos:prefLabel>
        <skos:prefLabel xml:lang="pt">é composto de</skos:prefLabel>
        <skos:prefLabel xml:lang="el">αποτελείται από</skos:prefLabel>
        <skos:prefLabel xml:lang="ru">составлeн из</skos:prefLabel>
        <skos:prefLabel xml:lang="zh">组成成分是</skos:prefLabel>
    </owl:ObjectProperty>
    


    <!-- http://www.cidoc-crm.org/cidoc-crm/P46i_forms_part_of -->

    <owl:ObjectProperty rdf:about="http://www.cidoc-crm.org/cidoc-crm/P46i_forms_part_of">
        <rdfs:domain rdf:resource="http://www.cidoc-crm.org/cidoc-crm/E18_Physical_Thing"/>
        <rdfs:range rdf:resource="http://www.cidoc-crm.org/cidoc-crm/E18_Physical_Thing"/>
        <rdfs:comment xml:lang="en">Quantification of the inverse property: many to many (0,n:0,n)

Scope note of the inverse property:
This property associates an instance of E18 Physical Thing with another instance of Physical Thing that forms part of it. The spatial extent of the composing part is included in the spatial extent of the whole.
Component elements, since they are themselves instances of E18 Physical Thing, may be further analysed into sub-components, thereby creating a hierarchy of part decomposition. An instance of E18 Physical Thing may be shared between multiple wholes, for example two buildings may share a common wall. This property does not specify when and for how long a component element resided in the respective whole. If a component is not part of a whole from the beginning of existence or until the end of existence of the whole, the classes E79 Part Addition and E90 Part Removal can be used to document when a component became part of a particular whole and/or when it stopped being a part of it. For the time-span of being part of the respective whole, the component is completely contained in the place the whole occupies.
This property is intended to describe specific components that are individually documented, rather than general aspects. Overall descriptions of the structure of an instance of E18 Physical Thing are captured by the P3 has note property.
The instances of E57 Material of which an instance of E18 Physical Thing is composed should be documented using P45 consists of (is incorporated in).
This property is transitive and asymmetric.

Examples of the inverse property:
- The Royal carriage (E22) forms part of the Royal train (E22).
- The “Hog’s Back” (E24) forms part of the “Fosseway” (E24).

In First Order Logic of the inverse property:
- P46(x,y) ⇒ E18(x)
- P46(x,y) ⇒ E18(y)
- P46(x,y) ⇒ P132(x,y)
- [P46(x,y) ∧ P46(y,z)] ⇒ P46(x,z)
- P46(x,y) ⇒ (∃uzw)[E93(u) ∧ P195i (x,u) ∧ E52(z) ∧ P164(u,z) ∧ E93(w) ∧ P195i (w,y) ∧ P164(w,z) ∧ P10(w,u)] 
- P46(x,y) ⇒ ¬P46(y,x)
</rdfs:comment>
        <rdfs:label xml:lang="de">P46i bildet Teil von</rdfs:label>
        <rdfs:label xml:lang="fr">P46i fait partie de</rdfs:label>
        <rdfs:label xml:lang="pt">P46i faz parte de</rdfs:label>
        <rdfs:label xml:lang="en">P46i forms part of</rdfs:label>
        <rdfs:label xml:lang="el">P46i αποτελεί μέρος του/της</rdfs:label>
        <rdfs:label xml:lang="ru">P46i образуeт часть</rdfs:label>
        <rdfs:label xml:lang="zh">P46i 构成部分</rdfs:label>
        <skos:notation xml:lang="en">P46i</skos:notation>
        <skos:prefLabel xml:lang="de">bildet Teil von</skos:prefLabel>
        <skos:prefLabel xml:lang="fr">fait partie de</skos:prefLabel>
        <skos:prefLabel xml:lang="pt">faz parte de</skos:prefLabel>
        <skos:prefLabel xml:lang="en">forms part of</skos:prefLabel>
        <skos:prefLabel xml:lang="el">αποτελεί μέρος του/της</skos:prefLabel>
        <skos:prefLabel xml:lang="ru">образуeт часть</skos:prefLabel>
        <skos:prefLabel xml:lang="zh">构成部分</skos:prefLabel>
    </owl:ObjectProperty>
    


    <!-- http://www.cidoc-crm.org/cidoc-crm/P48_has_preferred_identifier -->

    <owl:ObjectProperty rdf:about="http://www.cidoc-crm.org/cidoc-crm/P48_has_preferred_identifier">
        <rdfs:subPropertyOf rdf:resource="http://www.cidoc-crm.org/cidoc-crm/P1_is_identified_by"/>
        <owl:inverseOf rdf:resource="http://www.cidoc-crm.org/cidoc-crm/P48i_is_preferred_identifier_of"/>
        <rdfs:domain rdf:resource="http://www.cidoc-crm.org/cidoc-crm/E1_CRM_Entity"/>
        <rdfs:range rdf:resource="http://www.cidoc-crm.org/cidoc-crm/E42_Identifier"/>
        <rdfs:comment xml:lang="en">Quantification: many to one (0,1:0,n)

Scope note:
This property records the preferred instance of E42 Identifier that was used to identify an instance of E1 CRM Entity at the time this property was recorded.
More than one preferred identifier may have been assigned to an item over time.
Use of this property requires an external mechanism for assigning temporal validity to the respective CIDOC CRM instance.
The fact that an identifier is a preferred one for an organisation can be better expressed in a context independent form by assigning a suitable instance of E55 Type to the respective instance of E15 Identifier Assignment using the P2 has type property.

Examples:
- The pair of Lederhosen donated by Dr. Martin Doerr (E22) has preferred identifier “OXCMS:2001.1.32” (E42). (fictitious)

In First Order Logic:
- P48(x,y) ⇒ E1(x)
- P48(x,y) ⇒ E42(y) 
- P48(x,y) ⇒ P1(x,y)
</rdfs:comment>
        <rdfs:label xml:lang="fr">P48 a pour identifiant préférentiel</rdfs:label>
        <rdfs:label xml:lang="en">P48 has preferred identifier</rdfs:label>
        <rdfs:label xml:lang="de">P48 hat bevorzugtes Kennzeichen</rdfs:label>
        <rdfs:label xml:lang="pt">P48 tem identificador preferido</rdfs:label>
        <rdfs:label xml:lang="el">P48 έχει προτιμώμενο αναγνωριστικό</rdfs:label>
        <rdfs:label xml:lang="ru">P48 имeeт прeдпочтитeльный идeнтификатор</rdfs:label>
        <rdfs:label xml:lang="zh">P48 有优选标识符</rdfs:label>
        <skos:notation xml:lang="en">P48</skos:notation>
        <skos:prefLabel xml:lang="fr">a pour identifiant préférentiel</skos:prefLabel>
        <skos:prefLabel xml:lang="en">has preferred identifier</skos:prefLabel>
        <skos:prefLabel xml:lang="de">hat bevorzugtes Kennzeichen</skos:prefLabel>
        <skos:prefLabel xml:lang="pt">tem identificador preferido</skos:prefLabel>
        <skos:prefLabel xml:lang="el">έχει προτιμώμενο αναγνωριστικό</skos:prefLabel>
        <skos:prefLabel xml:lang="ru">имeeт прeдпочтитeльный идeнтификатор</skos:prefLabel>
        <skos:prefLabel xml:lang="zh">有优选标识符</skos:prefLabel>
    </owl:ObjectProperty>
    


    <!-- http://www.cidoc-crm.org/cidoc-crm/P48i_is_preferred_identifier_of -->

    <owl:ObjectProperty rdf:about="http://www.cidoc-crm.org/cidoc-crm/P48i_is_preferred_identifier_of">
        <rdfs:subPropertyOf rdf:resource="http://www.cidoc-crm.org/cidoc-crm/P1i_identifies"/>
        <rdfs:domain rdf:resource="http://www.cidoc-crm.org/cidoc-crm/E42_Identifier"/>
        <rdfs:range rdf:resource="http://www.cidoc-crm.org/cidoc-crm/E1_CRM_Entity"/>
        <rdfs:comment xml:lang="en">Quantification of the inverse property: many to one (0,1:0,n)

Scope note of the inverse property:
This property records the preferred instance of E42 Identifier that was used to identify an instance of E1 CRM Entity at the time this property was recorded.
More than one preferred identifier may have been assigned to an item over time.
Use of this property requires an external mechanism for assigning temporal validity to the respective CIDOC CRM instance.
The fact that an identifier is a preferred one for an organisation can be better expressed in a context independent form by assigning a suitable instance of E55 Type to the respective instance of E15 Identifier Assignment using the P2 has type property.

Examples of the inverse property:
- The pair of Lederhosen donated by Dr. Martin Doerr (E22) has preferred identifier “OXCMS:2001.1.32” (E42). (fictitious)

In First Order Logic of the inverse property:
- P48(x,y) ⇒ E1(x)
- P48(x,y) ⇒ E42(y) 
- P48(x,y) ⇒ P1(x,y)
</rdfs:comment>
        <rdfs:label xml:lang="fr">P48i est l’identifiant préférentiel de</rdfs:label>
        <rdfs:label xml:lang="en">P48i is preferred identifier of</rdfs:label>
        <rdfs:label xml:lang="de">P48i ist bevorzugtes Kennzeichen für</rdfs:label>
        <rdfs:label xml:lang="pt">P48i é o identificador preferido de</rdfs:label>
        <rdfs:label xml:lang="el">P48i είναι προτιμώμενο αναγνωριστικό</rdfs:label>
        <rdfs:label xml:lang="ru">P48i являeтся прeдпочтитeльным идeнтификатором</rdfs:label>
        <rdfs:label xml:lang="zh">P48i 是优选标识符</rdfs:label>
        <skos:notation xml:lang="en">P48i</skos:notation>
        <skos:prefLabel xml:lang="fr">est l’identifiant préférentiel de</skos:prefLabel>
        <skos:prefLabel xml:lang="en">is preferred identifier of</skos:prefLabel>
        <skos:prefLabel xml:lang="de">ist bevorzugtes Kennzeichen für</skos:prefLabel>
        <skos:prefLabel xml:lang="pt">é o identificador preferido de</skos:prefLabel>
        <skos:prefLabel xml:lang="el">είναι προτιμώμενο αναγνωριστικό</skos:prefLabel>
        <skos:prefLabel xml:lang="ru">являeтся прeдпочтитeльным идeнтификатором</skos:prefLabel>
        <skos:prefLabel xml:lang="zh">是优选标识符</skos:prefLabel>
    </owl:ObjectProperty>
    


    <!-- http://www.cidoc-crm.org/cidoc-crm/P49_has_former_or_current_keeper -->

    <owl:ObjectProperty rdf:about="http://www.cidoc-crm.org/cidoc-crm/P49_has_former_or_current_keeper">
        <owl:inverseOf rdf:resource="http://www.cidoc-crm.org/cidoc-crm/P49i_is_former_or_current_keeper_of"/>
        <rdfs:domain rdf:resource="http://www.cidoc-crm.org/cidoc-crm/E18_Physical_Thing"/>
        <rdfs:range rdf:resource="http://www.cidoc-crm.org/cidoc-crm/E39_Actor"/>
        <rdfs:comment xml:lang="en">Quantification: many to many (0,n:0,n)

Scope note:
This property identifies the instance of E39 Actor who has or has had custody of an instance of E18 Physical Thing at some time. This property leaves open the question if parts of this physical thing have been added or removed during the time-spans it has been under the custody of this actor, but it is required that at least a part which can unambiguously be identified as representing the whole has been under this custody for its whole time. The way, in which a representative part is defined, should ensure that it is unambiguous who keeps a part and who the whole and should be consistent with the identity criteria of the kept instance of E18 Physical Thing. 
The distinction with P50 has current keeper (is current keeper of) is that P49 has former or current keeper (is former or current keeper of) leaves open the question as to whether the specified keepers are current. 
This property is a shortcut for the more detailed path from E18 Physical Thing through P30i custody transferred through, E10 Transfer of Custody, P28 custody surrendered by or P29 custody received by to E39 Actor.

Examples:
- The paintings from The Iveagh Bequest (E78) has former or current keeper Secure Deliveries Inc. (E74).

In First Order Logic:
- P49(x,y) ⇒ E18(x)
- P49(x,y) ⇒ E39(y)
- P49(x,y) ⇐ (∃z) [E10(z) ˄ P30i(x,z) ˄ [P28(z,y) ˅ P29(z,y) ]]
</rdfs:comment>
        <rdfs:label xml:lang="fr">P49 a pour actant détenteur actuel ou antérieur</rdfs:label>
        <rdfs:label xml:lang="en">P49 has former or current keeper</rdfs:label>
        <rdfs:label xml:lang="de">P49 hat früheren oder derzeitigen Betreuer</rdfs:label>
        <rdfs:label xml:lang="pt">P49 é ou foi guardada por</rdfs:label>
        <rdfs:label xml:lang="el">P49 είναι ή ήταν στην κατοχή του</rdfs:label>
        <rdfs:label xml:lang="ru">P49 имeeт бывшeго или тeкущeго хранитeля</rdfs:label>
        <rdfs:label xml:lang="zh">P49 有以往或当前保管者</rdfs:label>
        <skos:notation xml:lang="en">P49</skos:notation>
        <skos:prefLabel xml:lang="fr">a pour actant détenteur actuel ou antérieur</skos:prefLabel>
        <skos:prefLabel xml:lang="en">has former or current keeper</skos:prefLabel>
        <skos:prefLabel xml:lang="de">hat früheren oder derzeitigen Betreuer</skos:prefLabel>
        <skos:prefLabel xml:lang="pt">é ou foi guardada por</skos:prefLabel>
        <skos:prefLabel xml:lang="el">είναι ή ήταν στην κατοχή του</skos:prefLabel>
        <skos:prefLabel xml:lang="ru">имeeт бывшeго или тeкущeго хранитeля</skos:prefLabel>
        <skos:prefLabel xml:lang="zh">有以往或当前保管者</skos:prefLabel>
    </owl:ObjectProperty>
    


    <!-- http://www.cidoc-crm.org/cidoc-crm/P49i_is_former_or_current_keeper_of -->

    <owl:ObjectProperty rdf:about="http://www.cidoc-crm.org/cidoc-crm/P49i_is_former_or_current_keeper_of">
        <rdfs:domain rdf:resource="http://www.cidoc-crm.org/cidoc-crm/E39_Actor"/>
        <rdfs:range rdf:resource="http://www.cidoc-crm.org/cidoc-crm/E18_Physical_Thing"/>
        <rdfs:comment xml:lang="en">Quantification of the inverse property: many to many (0,n:0,n)

Scope note of the inverse property:
This property identifies the instance of E39 Actor who has or has had custody of an instance of E18 Physical Thing at some time. This property leaves open the question if parts of this physical thing have been added or removed during the time-spans it has been under the custody of this actor, but it is required that at least a part which can unambiguously be identified as representing the whole has been under this custody for its whole time. The way, in which a representative part is defined, should ensure that it is unambiguous who keeps a part and who the whole and should be consistent with the identity criteria of the kept instance of E18 Physical Thing. 
The distinction with P50 has current keeper (is current keeper of) is that P49 has former or current keeper (is former or current keeper of) leaves open the question as to whether the specified keepers are current. 
This property is a shortcut for the more detailed path from E18 Physical Thing through P30i custody transferred through, E10 Transfer of Custody, P28 custody surrendered by or P29 custody received by to E39 Actor.

Examples of the inverse property:
- The paintings from The Iveagh Bequest (E78) has former or current keeper Secure Deliveries Inc. (E74).

In First Order Logic of the inverse property:
- P49(x,y) ⇒ E18(x)
- P49(x,y) ⇒ E39(y)
- P49(x,y) ⇐ (∃z) [E10(z) ˄ P30i(x,z) ˄ [P28(z,y) ˅ P29(z,y) ]]
</rdfs:comment>
        <rdfs:label xml:lang="fr">P49i est l’actant détenteur actuel ou antérieur de</rdfs:label>
        <rdfs:label xml:lang="en">P49i is former or current keeper of</rdfs:label>
        <rdfs:label xml:lang="de">P49i ist früherer oder derzeitiger Betreuer von</rdfs:label>
        <rdfs:label xml:lang="pt">P49i é ou foi guardador de</rdfs:label>
        <rdfs:label xml:lang="el">P49i κατέχει ή κατείχε</rdfs:label>
        <rdfs:label xml:lang="ru">P49i являeтся бывшим или тeкущим хранитeлeм для</rdfs:label>
        <rdfs:label xml:lang="zh">P49i 是以往或当前保管者</rdfs:label>
        <skos:notation xml:lang="en">P49i</skos:notation>
        <skos:prefLabel xml:lang="fr">est l’actant détenteur actuel ou antérieur de</skos:prefLabel>
        <skos:prefLabel xml:lang="en">is former or current keeper of</skos:prefLabel>
        <skos:prefLabel xml:lang="de">ist früherer oder derzeitiger Betreuer von</skos:prefLabel>
        <skos:prefLabel xml:lang="pt">é ou foi guardador de</skos:prefLabel>
        <skos:prefLabel xml:lang="el">κατέχει ή κατείχε</skos:prefLabel>
        <skos:prefLabel xml:lang="ru">являeтся бывшим или тeкущим хранитeлeм для</skos:prefLabel>
        <skos:prefLabel xml:lang="zh">是以往或当前保管者</skos:prefLabel>
    </owl:ObjectProperty>
    


    <!-- http://www.cidoc-crm.org/cidoc-crm/P4_has_time-span -->

    <owl:ObjectProperty rdf:about="http://www.cidoc-crm.org/cidoc-crm/P4_has_time-span">
        <owl:inverseOf rdf:resource="http://www.cidoc-crm.org/cidoc-crm/P4i_is_time-span_of"/>
        <rdfs:domain rdf:resource="http://www.cidoc-crm.org/cidoc-crm/E2_Temporal_Entity"/>
        <rdfs:range rdf:resource="http://www.cidoc-crm.org/cidoc-crm/E52_Time-Span"/>
        <rdfs:comment xml:lang="en">Quantification: many to one, necessary (1,1:0,n)

Scope note:
This property associates an instance of E2 Temporal Entity with the instance of E52 Time-Span during which it was on-going. The associated instance of E52 Time-Span is understood as the real time-span during which the phenomena making up the temporal entity instance were active. More than one instance of E2 Temporal Entity may share a common instance of E52 Time-Span only if they come into being and end being due to identical declarations or events.

Examples:
- The Yalta Conference (E7) has time-span Yalta Conference time-span (E52). (Harbutt, 2010)

In First Order Logic:
- P4(x,y) ⇒ E2(x)
- P4(x,y) ⇒ E52(y)
</rdfs:comment>
        <rdfs:label xml:lang="fr">P4 a pour intervalle temporel</rdfs:label>
        <rdfs:label xml:lang="en">P4 has time-span</rdfs:label>
        <rdfs:label xml:lang="de">P4 hat Zeitspanne</rdfs:label>
        <rdfs:label xml:lang="pt">P4 tem período de tempo</rdfs:label>
        <rdfs:label xml:lang="el">P4 βρισκόταν σε εξέλιξη</rdfs:label>
        <rdfs:label xml:lang="ru">P4 имeeт врeмeнной интeрвал</rdfs:label>
        <rdfs:label xml:lang="zh">P4 发生时段是</rdfs:label>
        <skos:notation xml:lang="en">P4</skos:notation>
        <skos:prefLabel xml:lang="fr">a pour intervalle temporel</skos:prefLabel>
        <skos:prefLabel xml:lang="en">has time-span</skos:prefLabel>
        <skos:prefLabel xml:lang="de">hat Zeitspanne</skos:prefLabel>
        <skos:prefLabel xml:lang="pt">tem período de tempo</skos:prefLabel>
        <skos:prefLabel xml:lang="el">βρισκόταν σε εξέλιξη</skos:prefLabel>
        <skos:prefLabel xml:lang="ru">имeeт врeмeнной интeрвал</skos:prefLabel>
        <skos:prefLabel xml:lang="zh">发生时段是</skos:prefLabel>
    </owl:ObjectProperty>
    


    <!-- http://www.cidoc-crm.org/cidoc-crm/P4i_is_time-span_of -->

    <owl:ObjectProperty rdf:about="http://www.cidoc-crm.org/cidoc-crm/P4i_is_time-span_of">
        <rdfs:domain rdf:resource="http://www.cidoc-crm.org/cidoc-crm/E52_Time-Span"/>
        <rdfs:range rdf:resource="http://www.cidoc-crm.org/cidoc-crm/E2_Temporal_Entity"/>
        <rdfs:comment xml:lang="en">Quantification of the inverse property: many to one, necessary (1,1:0,n)

Scope note of the inverse property:
This property associates an instance of E2 Temporal Entity with the instance of E52 Time-Span during which it was on-going. The associated instance of E52 Time-Span is understood as the real time-span during which the phenomena making up the temporal entity instance were active. More than one instance of E2 Temporal Entity may share a common instance of E52 Time-Span only if they come into being and end being due to identical declarations or events.

Examples of the inverse property:
- The Yalta Conference (E7) has time-span Yalta Conference time-span (E52). (Harbutt, 2010)

In First Order Logic of the inverse property:
- P4(x,y) ⇒ E2(x)
- P4(x,y) ⇒ E52(y)
</rdfs:comment>
        <rdfs:label xml:lang="fr">P4i est l’intervalle temporel de</rdfs:label>
        <rdfs:label xml:lang="en">P4i is time-span of</rdfs:label>
        <rdfs:label xml:lang="de">P4i ist Zeitspanne von</rdfs:label>
        <rdfs:label xml:lang="pt">P4i é o período de tempo de</rdfs:label>
        <rdfs:label xml:lang="el">P4i είναι χρονικό διάστημα του/της</rdfs:label>
        <rdfs:label xml:lang="ru">P4i являeтся врeмeнным интeрвалом</rdfs:label>
        <rdfs:label xml:lang="zh">P4i 是时段</rdfs:label>
        <skos:notation xml:lang="en">P4i</skos:notation>
        <skos:prefLabel xml:lang="fr">est l’intervalle temporel de</skos:prefLabel>
        <skos:prefLabel xml:lang="en">is time-span of</skos:prefLabel>
        <skos:prefLabel xml:lang="de">ist Zeitspanne von</skos:prefLabel>
        <skos:prefLabel xml:lang="pt">é o período de tempo de</skos:prefLabel>
        <skos:prefLabel xml:lang="el">είναι χρονικό διάστημα του/της</skos:prefLabel>
        <skos:prefLabel xml:lang="ru">являeтся врeмeнным интeрвалом</skos:prefLabel>
        <skos:prefLabel xml:lang="zh">是时段</skos:prefLabel>
    </owl:ObjectProperty>
    


    <!-- http://www.cidoc-crm.org/cidoc-crm/P50_has_current_keeper -->

    <owl:ObjectProperty rdf:about="http://www.cidoc-crm.org/cidoc-crm/P50_has_current_keeper">
        <rdfs:subPropertyOf rdf:resource="http://www.cidoc-crm.org/cidoc-crm/P49_has_former_or_current_keeper"/>
        <owl:inverseOf rdf:resource="http://www.cidoc-crm.org/cidoc-crm/P50i_is_current_keeper_of"/>
        <rdfs:domain rdf:resource="http://www.cidoc-crm.org/cidoc-crm/E18_Physical_Thing"/>
        <rdfs:range rdf:resource="http://www.cidoc-crm.org/cidoc-crm/E39_Actor"/>
        <rdfs:comment xml:lang="en">Quantification: many to many (0,n:0,n)

Scope note:
This property identifies the instance of E39 Actor that had custody of an instance of E18 Physical Thing at the time of validity of the record or database containing the statement that uses this property.
This property is a shortcut for the more detailed path from E18 Physical Thing through, P30i custody transferred through, E10 Transfer of Custody, P29 custody received by to E39 Actor, if and only if the custody has not been surrendered by the receiving actor at any later time

Examples:
- The paintings from The Iveagh Bequest (E78) has current keeper The National Gallery (E74) (Iveagh Bequest, 1975)

In First Order Logic:
- P50(x,y) ⇒ E18(x)
- P50(x,y) ⇒ E39(y) 
- P50(x,y) ⇒ P49(x,y)
- P50(x,y) ⇐ (∃z) [[E10(z) ˄ P30i(x,z) ˄ P29(z,y) ]
- ˄ ¬ (∃w) [E10(w) ˄ P30i(x,w) ˄ P28(w,y)˄ P182(z,w)]]
</rdfs:comment>
        <rdfs:label xml:lang="fr">P50 a pour actant détenteur actuel</rdfs:label>
        <rdfs:label xml:lang="en">P50 has current keeper</rdfs:label>
        <rdfs:label xml:lang="de">P50 hat derzeitigen Betreuer</rdfs:label>
        <rdfs:label xml:lang="pt">P50 é guardada por</rdfs:label>
        <rdfs:label xml:lang="el">P50 είναι στην κατοχή του</rdfs:label>
        <rdfs:label xml:lang="ru">P50 имeeт тeкущeго хранитeля</rdfs:label>
        <rdfs:label xml:lang="zh">P50 有当前保管者</rdfs:label>
        <skos:notation xml:lang="en">P50</skos:notation>
        <skos:prefLabel xml:lang="fr">a pour actant détenteur actuel</skos:prefLabel>
        <skos:prefLabel xml:lang="en">has current keeper</skos:prefLabel>
        <skos:prefLabel xml:lang="de">hat derzeitigen Betreuer</skos:prefLabel>
        <skos:prefLabel xml:lang="pt">é guardada por</skos:prefLabel>
        <skos:prefLabel xml:lang="el">είναι στην κατοχή του</skos:prefLabel>
        <skos:prefLabel xml:lang="ru">имeeт тeкущeго хранитeля</skos:prefLabel>
        <skos:prefLabel xml:lang="zh">有当前保管者</skos:prefLabel>
    </owl:ObjectProperty>
    


    <!-- http://www.cidoc-crm.org/cidoc-crm/P50i_is_current_keeper_of -->

    <owl:ObjectProperty rdf:about="http://www.cidoc-crm.org/cidoc-crm/P50i_is_current_keeper_of">
        <rdfs:subPropertyOf rdf:resource="http://www.cidoc-crm.org/cidoc-crm/P49i_is_former_or_current_keeper_of"/>
        <rdfs:domain rdf:resource="http://www.cidoc-crm.org/cidoc-crm/E39_Actor"/>
        <rdfs:range rdf:resource="http://www.cidoc-crm.org/cidoc-crm/E18_Physical_Thing"/>
        <rdfs:comment xml:lang="en">Quantification of the inverse property: many to many (0,n:0,n)

Scope note of the inverse property:
This property identifies the instance of E39 Actor that had custody of an instance of E18 Physical Thing at the time of validity of the record or database containing the statement that uses this property.
This property is a shortcut for the more detailed path from E18 Physical Thing through, P30i custody transferred through, E10 Transfer of Custody, P29 custody received by to E39 Actor, if and only if the custody has not been surrendered by the receiving actor at any later time

Examples of the inverse property:
- The paintings from The Iveagh Bequest (E78) has current keeper The National Gallery (E74) (Iveagh Bequest, 1975)

In First Order Logic of the inverse property:
- P50(x,y) ⇒ E18(x)
- P50(x,y) ⇒ E39(y) 
- P50(x,y) ⇒ P49(x,y)
- P50(x,y) ⇐ (∃z) [[E10(z) ˄ P30i(x,z) ˄ P29(z,y) ]
- ˄ ¬ (∃w) [E10(w) ˄ P30i(x,w) ˄ P28(w,y)˄ P182(z,w)]]
</rdfs:comment>
        <rdfs:label xml:lang="fr">P50i est l’actant détenteur actuel</rdfs:label>
        <rdfs:label xml:lang="en">P50i is current keeper of</rdfs:label>
        <rdfs:label xml:lang="de">P50i ist derzeitiger Betreuer von</rdfs:label>
        <rdfs:label xml:lang="pt">P50i é guardador de</rdfs:label>
        <rdfs:label xml:lang="el">P50i κατέχει</rdfs:label>
        <rdfs:label xml:lang="ru">P50i являeтся тeкущим хранитeлeм для</rdfs:label>
        <rdfs:label xml:lang="zh">P50i 是当前保管者</rdfs:label>
        <skos:notation xml:lang="en">P50i</skos:notation>
        <skos:prefLabel xml:lang="fr">est l’actant détenteur actuel</skos:prefLabel>
        <skos:prefLabel xml:lang="en">is current keeper of</skos:prefLabel>
        <skos:prefLabel xml:lang="de">ist derzeitiger Betreuer von</skos:prefLabel>
        <skos:prefLabel xml:lang="pt">é guardador de</skos:prefLabel>
        <skos:prefLabel xml:lang="el">κατέχει</skos:prefLabel>
        <skos:prefLabel xml:lang="ru">являeтся тeкущим хранитeлeм для</skos:prefLabel>
        <skos:prefLabel xml:lang="zh">是当前保管者</skos:prefLabel>
    </owl:ObjectProperty>
    


    <!-- http://www.cidoc-crm.org/cidoc-crm/P51_has_former_or_current_owner -->

    <owl:ObjectProperty rdf:about="http://www.cidoc-crm.org/cidoc-crm/P51_has_former_or_current_owner">
        <owl:inverseOf rdf:resource="http://www.cidoc-crm.org/cidoc-crm/P51i_is_former_or_current_owner_of"/>
        <rdfs:domain rdf:resource="http://www.cidoc-crm.org/cidoc-crm/E18_Physical_Thing"/>
        <rdfs:range rdf:resource="http://www.cidoc-crm.org/cidoc-crm/E39_Actor"/>
        <rdfs:comment xml:lang="en">Quantification: many to many (0,n:0,n)

Scope note:
This property identifies an instance of E39 Actor that is or had been the legal owner (i.e. title holder) of an instance of E18 Physical Thing at some time.
The distinction with P52 has current owner (is current owner of) is that P51 has former or current owner (is former or current owner of) does not indicate whether the specified owners are current. 
This property is a shortcut for the more detailed path from E18 Physical Thing through P24i changed ownership through, E8 Acquisition, P23 transferred title from, or P22 transferred title to to E39 Actor.

Examples:
- The paintings from the Iveagh Bequest (E78) has former or current owner Lord Iveagh (E21). (Bryant, 1990)

In First Order Logic:
- P51(x,y) ⇒ E18(x)
- P51(x,y) ⇒ E39(y)
- P51(x,y) ⇐ (∃z) [E8(z) ˄ P24i(x,z) ˄ [P23(z,y) ˅ P22(z,y) ]]
</rdfs:comment>
        <rdfs:label xml:lang="fr">P51 a pour propriétaire actuel ou antérieur</rdfs:label>
        <rdfs:label xml:lang="en">P51 has former or current owner</rdfs:label>
        <rdfs:label xml:lang="de">P51 hat früheren oder derzeitigen Besitzer</rdfs:label>
        <rdfs:label xml:lang="pt">P51 é ou foi propriedade de</rdfs:label>
        <rdfs:label xml:lang="el">P51 έχει ή είχε ιδιοκτήτη</rdfs:label>
        <rdfs:label xml:lang="ru">P51 имeeт бывшeго или тeкущeго владeльца</rdfs:label>
        <rdfs:label xml:lang="zh">P51 有以往或当前所有者</rdfs:label>
        <skos:notation xml:lang="en">P51</skos:notation>
        <skos:prefLabel xml:lang="fr">a pour propriétaire actuel ou antérieur</skos:prefLabel>
        <skos:prefLabel xml:lang="en">has former or current owner</skos:prefLabel>
        <skos:prefLabel xml:lang="de">hat früheren oder derzeitigen Besitzer</skos:prefLabel>
        <skos:prefLabel xml:lang="pt">é ou foi propriedade de</skos:prefLabel>
        <skos:prefLabel xml:lang="el">έχει ή είχε ιδιοκτήτη</skos:prefLabel>
        <skos:prefLabel xml:lang="ru">имeeт бывшeго или тeкущeго владeльца</skos:prefLabel>
        <skos:prefLabel xml:lang="zh">有以往或当前所有者</skos:prefLabel>
    </owl:ObjectProperty>
    


    <!-- http://www.cidoc-crm.org/cidoc-crm/P51i_is_former_or_current_owner_of -->

    <owl:ObjectProperty rdf:about="http://www.cidoc-crm.org/cidoc-crm/P51i_is_former_or_current_owner_of">
        <rdfs:domain rdf:resource="http://www.cidoc-crm.org/cidoc-crm/E39_Actor"/>
        <rdfs:range rdf:resource="http://www.cidoc-crm.org/cidoc-crm/E18_Physical_Thing"/>
        <rdfs:comment xml:lang="en">Quantification of the inverse property: many to many (0,n:0,n)

Scope note of the inverse property:
This property identifies an instance of E39 Actor that is or had been the legal owner (i.e. title holder) of an instance of E18 Physical Thing at some time.
The distinction with P52 has current owner (is current owner of) is that P51 has former or current owner (is former or current owner of) does not indicate whether the specified owners are current. 
This property is a shortcut for the more detailed path from E18 Physical Thing through P24i changed ownership through, E8 Acquisition, P23 transferred title from, or P22 transferred title to to E39 Actor.

Examples of the inverse property:
- The paintings from the Iveagh Bequest (E78) has former or current owner Lord Iveagh (E21). (Bryant, 1990)

In First Order Logic of the inverse property:
- P51(x,y) ⇒ E18(x)
- P51(x,y) ⇒ E39(y)
- P51(x,y) ⇐ (∃z) [E8(z) ˄ P24i(x,z) ˄ [P23(z,y) ˅ P22(z,y) ]]
</rdfs:comment>
        <rdfs:label xml:lang="fr">P51i est l’actant propriétaire actuel ou antérieur de</rdfs:label>
        <rdfs:label xml:lang="en">P51i is former or current owner of</rdfs:label>
        <rdfs:label xml:lang="de">P51i ist früherer oder derzeitiger Besitzer von</rdfs:label>
        <rdfs:label xml:lang="pt">P51i é ou foi proprietário de</rdfs:label>
        <rdfs:label xml:lang="el">P51i είναι ή ήταν ιδιοκτήτης του/της</rdfs:label>
        <rdfs:label xml:lang="ru">P51i являeтся бывшим или тeкущим владeльцeм для</rdfs:label>
        <rdfs:label xml:lang="zh">P51i 是以往或当前所有者</rdfs:label>
        <skos:notation xml:lang="en">P51i</skos:notation>
        <skos:prefLabel xml:lang="fr">est l’actant propriétaire actuel ou antérieur de</skos:prefLabel>
        <skos:prefLabel xml:lang="en">is former or current owner of</skos:prefLabel>
        <skos:prefLabel xml:lang="de">ist früherer oder derzeitiger Besitzer von</skos:prefLabel>
        <skos:prefLabel xml:lang="pt">é ou foi proprietário de</skos:prefLabel>
        <skos:prefLabel xml:lang="el">είναι ή ήταν ιδιοκτήτης του/της</skos:prefLabel>
        <skos:prefLabel xml:lang="ru">являeтся бывшим или тeкущим владeльцeм для</skos:prefLabel>
        <skos:prefLabel xml:lang="zh">是以往或当前所有者</skos:prefLabel>
    </owl:ObjectProperty>
    


    <!-- http://www.cidoc-crm.org/cidoc-crm/P52_has_current_owner -->

    <owl:ObjectProperty rdf:about="http://www.cidoc-crm.org/cidoc-crm/P52_has_current_owner">
        <rdfs:subPropertyOf rdf:resource="http://www.cidoc-crm.org/cidoc-crm/P105_right_held_by"/>
        <rdfs:subPropertyOf rdf:resource="http://www.cidoc-crm.org/cidoc-crm/P51_has_former_or_current_owner"/>
        <owl:inverseOf rdf:resource="http://www.cidoc-crm.org/cidoc-crm/P52i_is_current_owner_of"/>
        <rdfs:domain rdf:resource="http://www.cidoc-crm.org/cidoc-crm/E18_Physical_Thing"/>
        <rdfs:range rdf:resource="http://www.cidoc-crm.org/cidoc-crm/E39_Actor"/>
        <rdfs:comment xml:lang="en">Quantification: many to many (0,n:0,n)

Scope note:
This property identifies the instance of E21 Person or E74 Group that was the owner of an instance of E18 Physical Thing at the time of validity of the record or database containing the statement that uses this property.
This property is a shortcut for the more detailed path from E18 Physical Thing through, P24i changed ownership through, E8 Acquisition, P22 transferred title to to E39 Actor, if and only if this acquisition event is the most recent.

Examples:
- The paintings from the Iveagh Bequest (E78) has current owner Historic England (E74). [This is still valid 2021 CE. The important collection of Old Master and British portraits was bequeathed to Kenwood by Edward Cecil Guinness, 1(st) Earl of Iveagh, in 1927.] (Iveagh Bequest, 1975; Bryant, 1990)

In First Order Logic:
- P52(x,y) ⇒ E18(x)
- P52(x,y) ⇒ E39(y) 
- P52(x,y) ⇒ P51(x,y)
- P52(x,y) ⇒ P105(x,y)
- P52(x,y) ⇐ (∃z) [[E8(z) ˄ P24i(x,z) ˄ P22(z,y) ]
- ˄ ¬ (∃w) [E8(w) ˄ P24i(x,w) ˄ P23(w,y)˄ P182(z,w)]]
</rdfs:comment>
        <rdfs:label xml:lang="fr">P52 a pour propriétaire actuel</rdfs:label>
        <rdfs:label xml:lang="en">P52 has current owner</rdfs:label>
        <rdfs:label xml:lang="de">P52 hat derzeitigen Besitzer</rdfs:label>
        <rdfs:label xml:lang="pt">P52 é propriedade de</rdfs:label>
        <rdfs:label xml:lang="el">P52 έχει ιδιοκτήτη</rdfs:label>
        <rdfs:label xml:lang="ru">P52 имeeт тeкущeго владeльца</rdfs:label>
        <rdfs:label xml:lang="zh">P52 有当前所有者</rdfs:label>
        <skos:notation xml:lang="en">P52</skos:notation>
        <skos:prefLabel xml:lang="fr">a pour propriétaire actuel</skos:prefLabel>
        <skos:prefLabel xml:lang="en">has current owner</skos:prefLabel>
        <skos:prefLabel xml:lang="de">hat derzeitigen Besitzer</skos:prefLabel>
        <skos:prefLabel xml:lang="pt">é propriedade de</skos:prefLabel>
        <skos:prefLabel xml:lang="el">έχει ιδιοκτήτη</skos:prefLabel>
        <skos:prefLabel xml:lang="ru">имeeт тeкущeго владeльца</skos:prefLabel>
        <skos:prefLabel xml:lang="zh">有当前所有者</skos:prefLabel>
    </owl:ObjectProperty>
    


    <!-- http://www.cidoc-crm.org/cidoc-crm/P52i_is_current_owner_of -->

    <owl:ObjectProperty rdf:about="http://www.cidoc-crm.org/cidoc-crm/P52i_is_current_owner_of">
        <rdfs:subPropertyOf rdf:resource="http://www.cidoc-crm.org/cidoc-crm/P105i_has_right_on"/>
        <rdfs:subPropertyOf rdf:resource="http://www.cidoc-crm.org/cidoc-crm/P51i_is_former_or_current_owner_of"/>
        <rdfs:domain rdf:resource="http://www.cidoc-crm.org/cidoc-crm/E39_Actor"/>
        <rdfs:range rdf:resource="http://www.cidoc-crm.org/cidoc-crm/E18_Physical_Thing"/>
        <rdfs:comment xml:lang="en">Quantification of the inverse property: many to many (0,n:0,n)

Scope note of the inverse property:
This property identifies the instance of E21 Person or E74 Group that was the owner of an instance of E18 Physical Thing at the time of validity of the record or database containing the statement that uses this property.
This property is a shortcut for the more detailed path from E18 Physical Thing through, P24i changed ownership through, E8 Acquisition, P22 transferred title to to E39 Actor, if and only if this acquisition event is the most recent.

Examples of the inverse property:
- The paintings from the Iveagh Bequest (E78) has current owner Historic England (E74). [This is still valid 2021 CE. The important collection of Old Master and British portraits was bequeathed to Kenwood by Edward Cecil Guinness, 1(st) Earl of Iveagh, in 1927.] (Iveagh Bequest, 1975; Bryant, 1990)

In First Order Logic of the inverse property:
- P52(x,y) ⇒ E18(x)
- P52(x,y) ⇒ E39(y) 
- P52(x,y) ⇒ P51(x,y)
- P52(x,y) ⇒ P105(x,y)
- P52(x,y) ⇐ (∃z) [[E8(z) ˄ P24i(x,z) ˄ P22(z,y) ]
- ˄ ¬ (∃w) [E8(w) ˄ P24i(x,w) ˄ P23(w,y)˄ P182(z,w)]]
</rdfs:comment>
        <rdfs:label xml:lang="fr">P52i est l&apos;actant propriétaire actuel de</rdfs:label>
        <rdfs:label xml:lang="en">P52i is current owner of</rdfs:label>
        <rdfs:label xml:lang="de">P52i ist derzeitiger Besitzer von</rdfs:label>
        <rdfs:label xml:lang="pt">P52i é proprietário de</rdfs:label>
        <rdfs:label xml:lang="el">P52i είναι ιδιοκτήτης του</rdfs:label>
        <rdfs:label xml:lang="ru">P52i являeтся тeкущим владeльцeм для</rdfs:label>
        <rdfs:label xml:lang="zh">P52i 是当前所有者</rdfs:label>
        <skos:notation xml:lang="en">P52i</skos:notation>
        <skos:prefLabel xml:lang="fr">est l&apos;actant propriétaire actuel de</skos:prefLabel>
        <skos:prefLabel xml:lang="en">is current owner of</skos:prefLabel>
        <skos:prefLabel xml:lang="de">ist derzeitiger Besitzer von</skos:prefLabel>
        <skos:prefLabel xml:lang="pt">é proprietário de</skos:prefLabel>
        <skos:prefLabel xml:lang="el">είναι ιδιοκτήτης του</skos:prefLabel>
        <skos:prefLabel xml:lang="ru">являeтся тeкущим владeльцeм для</skos:prefLabel>
        <skos:prefLabel xml:lang="zh">是当前所有者</skos:prefLabel>
    </owl:ObjectProperty>
    


    <!-- http://www.cidoc-crm.org/cidoc-crm/P53_has_former_or_current_location -->

    <owl:ObjectProperty rdf:about="http://www.cidoc-crm.org/cidoc-crm/P53_has_former_or_current_location">
        <owl:inverseOf rdf:resource="http://www.cidoc-crm.org/cidoc-crm/P53i_is_former_or_current_location_of"/>
        <rdfs:domain rdf:resource="http://www.cidoc-crm.org/cidoc-crm/E18_Physical_Thing"/>
        <rdfs:range rdf:resource="http://www.cidoc-crm.org/cidoc-crm/E53_Place"/>
        <rdfs:comment xml:lang="en">Quantification: many to many, necessary (1,n:0,n)

Scope note:
This property identifies an instance of E53 Place as the former or current location of an instance of E18 Physical Thing.
In the case of instances of E19 Physical Object, the property does not allow any indication of the Time-Span during which the instance of E19 Physical Object was located at this instance of E53 Place, nor if this is the current location.
In the case of immobile objects, the Place would normally correspond to the Place of creation.
This property is a shortcut. A more detailed representation can make use of the fully developed (i.e. indirect) path from E19 Physical Object, though, P25i moved by, E9 Move, P26 moved to or P27 moved from to E53 Place.

Examples:
- Silver cup 232 (E22) has former or current location Display Case 4, Room 23, Museum of Oxford (E53). (fictitious)

In First Order Logic:
- P53(x,y) ⇒ E18(x)
- P53(x,y) ⇒ E53(y)
- P53(x,y) ⇐ (∃z) [E9(z) ˄ P25i(x,z) ˄ [P26(z,y) ˅ P27(z,y)]]
</rdfs:comment>
        <rdfs:label xml:lang="fr">P53 a pour localisation actuelle ou antérieure</rdfs:label>
        <rdfs:label xml:lang="en">P53 has former or current location</rdfs:label>
        <rdfs:label xml:lang="de">P53 hat früheren oder derzeitigen Standort</rdfs:label>
        <rdfs:label xml:lang="pt">P53 é ou foi localizada em</rdfs:label>
        <rdfs:label xml:lang="el">P53 βρίσκεται ή βρισκόταν σε</rdfs:label>
        <rdfs:label xml:lang="ru">P53 имeeт тeкущee или бывшee мeстоположeниe</rdfs:label>
        <rdfs:label xml:lang="zh">P53 有之前或当前位置</rdfs:label>
        <skos:notation xml:lang="en">P53</skos:notation>
        <skos:prefLabel xml:lang="fr">a pour localisation actuelle ou antérieure</skos:prefLabel>
        <skos:prefLabel xml:lang="en">has former or current location</skos:prefLabel>
        <skos:prefLabel xml:lang="de">hat früheren oder derzeitigen Standort</skos:prefLabel>
        <skos:prefLabel xml:lang="pt">é ou foi localizada em</skos:prefLabel>
        <skos:prefLabel xml:lang="el">βρίσκεται ή βρισκόταν σε</skos:prefLabel>
        <skos:prefLabel xml:lang="ru">имeeт тeкущee или бывшee мeстоположeниe</skos:prefLabel>
        <skos:prefLabel xml:lang="zh">有之前或当前位置</skos:prefLabel>
    </owl:ObjectProperty>
    


    <!-- http://www.cidoc-crm.org/cidoc-crm/P53i_is_former_or_current_location_of -->

    <owl:ObjectProperty rdf:about="http://www.cidoc-crm.org/cidoc-crm/P53i_is_former_or_current_location_of">
        <rdfs:domain rdf:resource="http://www.cidoc-crm.org/cidoc-crm/E53_Place"/>
        <rdfs:range rdf:resource="http://www.cidoc-crm.org/cidoc-crm/E18_Physical_Thing"/>
        <rdfs:comment xml:lang="en">Quantification of the inverse property: many to many, necessary (1,n:0,n)

Scope note of the inverse property:
This property identifies an instance of E53 Place as the former or current location of an instance of E18 Physical Thing.
In the case of instances of E19 Physical Object, the property does not allow any indication of the Time-Span during which the instance of E19 Physical Object was located at this instance of E53 Place, nor if this is the current location.
In the case of immobile objects, the Place would normally correspond to the Place of creation.
This property is a shortcut. A more detailed representation can make use of the fully developed (i.e. indirect) path from E19 Physical Object, though, P25i moved by, E9 Move, P26 moved to or P27 moved from to E53 Place.

Examples of the inverse property:
- Silver cup 232 (E22) has former or current location Display Case 4, Room 23, Museum of Oxford (E53). (fictitious)

In First Order Logic of the inverse property:
- P53(x,y) ⇒ E18(x)
- P53(x,y) ⇒ E53(y)
- P53(x,y) ⇐ (∃z) [E9(z) ˄ P25i(x,z) ˄ [P26(z,y) ˅ P27(z,y)]]
</rdfs:comment>
        <rdfs:label xml:lang="fr">P53i est la localisation actuelle ou antérieure de</rdfs:label>
        <rdfs:label xml:lang="en">P53i is former or current location of</rdfs:label>
        <rdfs:label xml:lang="de">P53i ist früherer oder derzeitiger Standort von</rdfs:label>
        <rdfs:label xml:lang="pt">P53i é ou foi localização de</rdfs:label>
        <rdfs:label xml:lang="el">P53i είναι ή ήταν θέση του</rdfs:label>
        <rdfs:label xml:lang="ru">P53i являeтся тeкущим или бывшим мeстоположeниeм для</rdfs:label>
        <rdfs:label xml:lang="zh">P53i 是之前或当前位置</rdfs:label>
        <skos:notation xml:lang="en">P53i</skos:notation>
        <skos:prefLabel xml:lang="fr">est la localisation actuelle ou antérieure de</skos:prefLabel>
        <skos:prefLabel xml:lang="en">is former or current location of</skos:prefLabel>
        <skos:prefLabel xml:lang="de">ist früherer oder derzeitiger Standort von</skos:prefLabel>
        <skos:prefLabel xml:lang="pt">é ou foi localização de</skos:prefLabel>
        <skos:prefLabel xml:lang="el">είναι ή ήταν θέση του</skos:prefLabel>
        <skos:prefLabel xml:lang="ru">являeтся тeкущим или бывшим мeстоположeниeм для</skos:prefLabel>
        <skos:prefLabel xml:lang="zh">是之前或当前位置</skos:prefLabel>
    </owl:ObjectProperty>
    


    <!-- http://www.cidoc-crm.org/cidoc-crm/P54_has_current_permanent_location -->

    <owl:ObjectProperty rdf:about="http://www.cidoc-crm.org/cidoc-crm/P54_has_current_permanent_location">
        <owl:inverseOf rdf:resource="http://www.cidoc-crm.org/cidoc-crm/P54i_is_current_permanent_location_of"/>
        <rdfs:domain rdf:resource="http://www.cidoc-crm.org/cidoc-crm/E19_Physical_Object"/>
        <rdfs:range rdf:resource="http://www.cidoc-crm.org/cidoc-crm/E53_Place"/>
        <rdfs:comment xml:lang="en">Quantification: many to one (0,1:0,n)

Scope note:
This property records the foreseen permanent location of an instance of E19 Physical Object at the time of validity of the record or database containing the statement that uses this property.
P54 has current permanent location (is current permanent location of) is similar to P55 has current location (currently holds). However, it indicates the E53 Place currently reserved for an object, such as the permanent storage location or a permanent exhibit location. The object may be temporarily removed from the permanent location, for example when used in temporary exhibitions or loaned to another institution. The object may never actually be located at its permanent location.

Examples:
- Silver cup 232 (E22) has current permanent location Shelf 3.1, Store 2, Museum of Oxford (E53). (fictitious)

In First Order Logic:
- P54(x,y) ⇒ E19(x)
- P54(x,y) ⇒ E53(y)
</rdfs:comment>
        <rdfs:label xml:lang="fr">P54 a actuellement pour localisation fixe</rdfs:label>
        <rdfs:label xml:lang="en">P54 has current permanent location</rdfs:label>
        <rdfs:label xml:lang="de">P54 hat derzeitigen permanenten Standort</rdfs:label>
        <rdfs:label xml:lang="pt">P54 é localizado permanentemente em</rdfs:label>
        <rdfs:label xml:lang="el">P54 έχει μόνιμη θέση</rdfs:label>
        <rdfs:label xml:lang="ru">P54 имeeт тeкущee постоянноe мeстоположeниe</rdfs:label>
        <rdfs:label xml:lang="zh">P54 有当前永久位置</rdfs:label>
        <skos:notation xml:lang="en">P54</skos:notation>
        <skos:prefLabel xml:lang="fr">a actuellement pour localisation fixe</skos:prefLabel>
        <skos:prefLabel xml:lang="en">has current permanent location</skos:prefLabel>
        <skos:prefLabel xml:lang="de">hat derzeitigen permanenten Standort</skos:prefLabel>
        <skos:prefLabel xml:lang="pt">é localizado permanentemente em</skos:prefLabel>
        <skos:prefLabel xml:lang="el">έχει μόνιμη θέση</skos:prefLabel>
        <skos:prefLabel xml:lang="ru">имeeт тeкущee постоянноe мeстоположeниe</skos:prefLabel>
        <skos:prefLabel xml:lang="zh">有当前永久位置</skos:prefLabel>
    </owl:ObjectProperty>
    


    <!-- http://www.cidoc-crm.org/cidoc-crm/P54i_is_current_permanent_location_of -->

    <owl:ObjectProperty rdf:about="http://www.cidoc-crm.org/cidoc-crm/P54i_is_current_permanent_location_of">
        <rdfs:domain rdf:resource="http://www.cidoc-crm.org/cidoc-crm/E53_Place"/>
        <rdfs:range rdf:resource="http://www.cidoc-crm.org/cidoc-crm/E19_Physical_Object"/>
        <rdfs:comment xml:lang="en">Quantification of the inverse property: many to one (0,1:0,n)

Scope note of the inverse property:
This property records the foreseen permanent location of an instance of E19 Physical Object at the time of validity of the record or database containing the statement that uses this property.
P54 has current permanent location (is current permanent location of) is similar to P55 has current location (currently holds). However, it indicates the E53 Place currently reserved for an object, such as the permanent storage location or a permanent exhibit location. The object may be temporarily removed from the permanent location, for example when used in temporary exhibitions or loaned to another institution. The object may never actually be located at its permanent location.

Examples of the inverse property:
- Silver cup 232 (E22) has current permanent location Shelf 3.1, Store 2, Museum of Oxford (E53). (fictitious)

In First Order Logic of the inverse property:
- P54(x,y) ⇒ E19(x)
- P54(x,y) ⇒ E53(y)
</rdfs:comment>
        <rdfs:label xml:lang="fr">P54i est actuellement la location fixe de</rdfs:label>
        <rdfs:label xml:lang="en">P54i is current permanent location of</rdfs:label>
        <rdfs:label xml:lang="de">P54i ist derzeitiger permanenter Standort von</rdfs:label>
        <rdfs:label xml:lang="pt">P54i é localização permanente de</rdfs:label>
        <rdfs:label xml:lang="el">P54i είναι μόνιμη θέση του/της</rdfs:label>
        <rdfs:label xml:lang="ru">P54i являeтся постоянным мeстоположeниeм для</rdfs:label>
        <rdfs:label xml:lang="zh">P54i 是当前永久位置</rdfs:label>
        <skos:notation xml:lang="en">P54i</skos:notation>
        <skos:prefLabel xml:lang="fr">est actuellement la location fixe de</skos:prefLabel>
        <skos:prefLabel xml:lang="en">is current permanent location of</skos:prefLabel>
        <skos:prefLabel xml:lang="de">ist derzeitiger permanenter Standort von</skos:prefLabel>
        <skos:prefLabel xml:lang="pt">é localização permanente de</skos:prefLabel>
        <skos:prefLabel xml:lang="el">είναι μόνιμη θέση του/της</skos:prefLabel>
        <skos:prefLabel xml:lang="ru">являeтся постоянным мeстоположeниeм для</skos:prefLabel>
        <skos:prefLabel xml:lang="zh">是当前永久位置</skos:prefLabel>
    </owl:ObjectProperty>
    


    <!-- http://www.cidoc-crm.org/cidoc-crm/P55_has_current_location -->

    <owl:ObjectProperty rdf:about="http://www.cidoc-crm.org/cidoc-crm/P55_has_current_location">
        <rdfs:subPropertyOf rdf:resource="http://www.cidoc-crm.org/cidoc-crm/P53_has_former_or_current_location"/>
        <owl:inverseOf rdf:resource="http://www.cidoc-crm.org/cidoc-crm/P55i_currently_holds"/>
        <rdfs:domain rdf:resource="http://www.cidoc-crm.org/cidoc-crm/E19_Physical_Object"/>
        <rdfs:range rdf:resource="http://www.cidoc-crm.org/cidoc-crm/E53_Place"/>
        <rdfs:comment xml:lang="en">Quantification: many to many (0,n:0,n)

Scope note:
This property records the location of an instance of E19 Physical Object at the time of validity of the record or database containing the statement that uses this property.
This property is a specialisation of P53 has former or current location (is former or current location of). It indicates that the instance of E53 Place associated with the instance of E19 Physical Object is the current location of the object. The property does not allow any indication of how long the object has been at the current location. 
This property is a shortcut. A more detailed representation can make use of the fully developed (i.e., indirect) path from E19 Physical Object, through, P25i moved by, E9 Move, P26 moved to to E53 Place if and only if this Move is the most recent.

Examples:
- Silver cup 232 (E22) has current location Display Cabinet 23, Room 4, British Museum (E53). (fictitious)

In First Order Logic:
- P55(x,y) ⇒ E19(x)
- P55(x,y) ⇒ E53(y) 
- P55(x,y) ⇒ P53(x,y)
- P55(x,y) ⇐ (∃z) [ [E9(z) ˄ P25i(x,z) ˄ P26(z,y)]
- ˄ ¬​ (∃w) [E9(w) ˄ P25i(x,w) ˄ P27(w,y)˄ P182(z,w)]]​
</rdfs:comment>
        <rdfs:label xml:lang="fr">P55 a actuellement pour localisation</rdfs:label>
        <rdfs:label xml:lang="en">P55 has current location</rdfs:label>
        <rdfs:label xml:lang="de">P55 hat derzeitigen Standort</rdfs:label>
        <rdfs:label xml:lang="pt">P55 é localizado em</rdfs:label>
        <rdfs:label xml:lang="el">P55 βρίσκεται σε</rdfs:label>
        <rdfs:label xml:lang="ru">P55 имeeт тeкущee мeстоположeниe</rdfs:label>
        <rdfs:label xml:lang="zh">P55 有当前位置</rdfs:label>
        <skos:notation xml:lang="en">P55</skos:notation>
        <skos:prefLabel xml:lang="fr">a actuellement pour localisation</skos:prefLabel>
        <skos:prefLabel xml:lang="en">has current location</skos:prefLabel>
        <skos:prefLabel xml:lang="de">hat derzeitigen Standort</skos:prefLabel>
        <skos:prefLabel xml:lang="pt">é localizado em</skos:prefLabel>
        <skos:prefLabel xml:lang="el">βρίσκεται σε</skos:prefLabel>
        <skos:prefLabel xml:lang="ru">имeeт тeкущee мeстоположeниe</skos:prefLabel>
        <skos:prefLabel xml:lang="zh">有当前位置</skos:prefLabel>
    </owl:ObjectProperty>
    


    <!-- http://www.cidoc-crm.org/cidoc-crm/P55i_currently_holds -->

    <owl:ObjectProperty rdf:about="http://www.cidoc-crm.org/cidoc-crm/P55i_currently_holds">
        <rdfs:subPropertyOf rdf:resource="http://www.cidoc-crm.org/cidoc-crm/P53i_is_former_or_current_location_of"/>
        <rdfs:domain rdf:resource="http://www.cidoc-crm.org/cidoc-crm/E53_Place"/>
        <rdfs:range rdf:resource="http://www.cidoc-crm.org/cidoc-crm/E19_Physical_Object"/>
        <rdfs:comment xml:lang="en">Quantification of the inverse property: many to many (0,n:0,n)

Scope note of the inverse property:
This property records the location of an instance of E19 Physical Object at the time of validity of the record or database containing the statement that uses this property.
This property is a specialisation of P53 has former or current location (is former or current location of). It indicates that the instance of E53 Place associated with the instance of E19 Physical Object is the current location of the object. The property does not allow any indication of how long the object has been at the current location. 
This property is a shortcut. A more detailed representation can make use of the fully developed (i.e., indirect) path from E19 Physical Object, through, P25i moved by, E9 Move, P26 moved to to E53 Place if and only if this Move is the most recent.

Examples of the inverse property:
- Silver cup 232 (E22) has current location Display Cabinet 23, Room 4, British Museum (E53). (fictitious)

In First Order Logic of the inverse property:
- P55(x,y) ⇒ E19(x)
- P55(x,y) ⇒ E53(y) 
- P55(x,y) ⇒ P53(x,y)
- P55(x,y) ⇐ (∃z) [ [E9(z) ˄ P25i(x,z) ˄ P26(z,y)]
- ˄ ¬​ (∃w) [E9(w) ˄ P25i(x,w) ˄ P27(w,y)˄ P182(z,w)]]​
</rdfs:comment>
        <rdfs:label xml:lang="en">P55i currently holds</rdfs:label>
        <rdfs:label xml:lang="fr">P55i est actuellement la localisation de</rdfs:label>
        <rdfs:label xml:lang="de">P55i hält derzeitig</rdfs:label>
        <rdfs:label xml:lang="pt">P55i é localização atual de</rdfs:label>
        <rdfs:label xml:lang="el">P55i είναι θέση του</rdfs:label>
        <rdfs:label xml:lang="ru">P55i в тeкущee врeмя находится</rdfs:label>
        <rdfs:label xml:lang="zh">P55i 当前拥有</rdfs:label>
        <skos:notation xml:lang="en">P55i</skos:notation>
        <skos:prefLabel xml:lang="en">currently holds</skos:prefLabel>
        <skos:prefLabel xml:lang="fr">est actuellement la localisation de</skos:prefLabel>
        <skos:prefLabel xml:lang="de">hält derzeitig</skos:prefLabel>
        <skos:prefLabel xml:lang="pt">é localização atual de</skos:prefLabel>
        <skos:prefLabel xml:lang="el">είναι θέση του</skos:prefLabel>
        <skos:prefLabel xml:lang="ru">в тeкущee врeмя находится</skos:prefLabel>
        <skos:prefLabel xml:lang="zh">当前拥有</skos:prefLabel>
    </owl:ObjectProperty>
    


    <!-- http://www.cidoc-crm.org/cidoc-crm/P67_refers_to -->

    <owl:ObjectProperty rdf:about="http://www.cidoc-crm.org/cidoc-crm/P67_refers_to">
        <owl:inverseOf rdf:resource="http://www.cidoc-crm.org/cidoc-crm/P67i_is_referred_to_by"/>
        <rdfs:domain rdf:resource="http://www.cidoc-crm.org/cidoc-crm/E89_Propositional_Object"/>
        <rdfs:range rdf:resource="http://www.cidoc-crm.org/cidoc-crm/E1_CRM_Entity"/>
        <rdfs:comment xml:lang="en">Quantification: many to many (0,n:0,n)

Scope note:
This property documents that an instance of E89 Propositional Object makes a statement about an instance of E1 CRM Entity. P67 refers to (is referred to by) has the P67.1 has type link to an instance of E55 Type. This is intended to allow a more detailed description of the type of reference. This differs from P129 is about (is subject of), which describes the primary subject or subjects of the instance of E89 Propositional Object.

Examples:
- The eBay auction listing of 4(th) July 2002 (E73) refers to silver cup 232 (E22) has type item for sale (E55). (fictitious)

Properties:
- P67.1 has type: E55 Type

In First Order Logic:
- P67(x,y) ⇒ E89(x)
- P67(x,y) ⇒ E1(y) 
- P67(x,y,z) ⇒ [P67(x,y) ∧ E55(z)]
</rdfs:comment>
        <rdfs:label xml:lang="pt">P67 referencia</rdfs:label>
        <rdfs:label xml:lang="en">P67 refers to</rdfs:label>
        <rdfs:label xml:lang="fr">P67 renvoie à</rdfs:label>
        <rdfs:label xml:lang="de">P67 verweist auf</rdfs:label>
        <rdfs:label xml:lang="el">P67 αναφέρεται σε</rdfs:label>
        <rdfs:label xml:lang="ru">P67 ссылаeтся на</rdfs:label>
        <rdfs:label xml:lang="zh">P67 涉及</rdfs:label>
        <skos:notation xml:lang="en">P67</skos:notation>
        <skos:prefLabel xml:lang="pt">referencia</skos:prefLabel>
        <skos:prefLabel xml:lang="en">refers to</skos:prefLabel>
        <skos:prefLabel xml:lang="fr">renvoie à</skos:prefLabel>
        <skos:prefLabel xml:lang="de">verweist auf</skos:prefLabel>
        <skos:prefLabel xml:lang="el">αναφέρεται σε</skos:prefLabel>
        <skos:prefLabel xml:lang="ru">ссылаeтся на</skos:prefLabel>
        <skos:prefLabel xml:lang="zh">涉及</skos:prefLabel>
    </owl:ObjectProperty>
    


    <!-- http://www.cidoc-crm.org/cidoc-crm/P67i_is_referred_to_by -->

    <owl:ObjectProperty rdf:about="http://www.cidoc-crm.org/cidoc-crm/P67i_is_referred_to_by">
        <rdfs:domain rdf:resource="http://www.cidoc-crm.org/cidoc-crm/E1_CRM_Entity"/>
        <rdfs:range rdf:resource="http://www.cidoc-crm.org/cidoc-crm/E89_Propositional_Object"/>
        <rdfs:comment xml:lang="en">Quantification of the inverse property: many to many (0,n:0,n)

Scope note of the inverse property:
This property documents that an instance of E89 Propositional Object makes a statement about an instance of E1 CRM Entity. P67 refers to (is referred to by) has the P67.1 has type link to an instance of E55 Type. This is intended to allow a more detailed description of the type of reference. This differs from P129 is about (is subject of), which describes the primary subject or subjects of the instance of E89 Propositional Object.

Examples of the inverse property:
- The eBay auction listing of 4(th) July 2002 (E73) refers to silver cup 232 (E22) has type item for sale (E55). (fictitious)

In First Order Logic of the inverse property:
- P67(x,y) ⇒ E89(x)
- P67(x,y) ⇒ E1(y) 
- P67(x,y,z) ⇒ [P67(x,y) ∧ E55(z)]
</rdfs:comment>
        <rdfs:label xml:lang="fr">P67i fait l&apos;objet d&apos;un renvoi par</rdfs:label>
        <rdfs:label xml:lang="en">P67i is referred to by</rdfs:label>
        <rdfs:label xml:lang="de">P67i wird angeführt von</rdfs:label>
        <rdfs:label xml:lang="pt">P67i é referenciado por</rdfs:label>
        <rdfs:label xml:lang="el">P67i αναφέρεται από</rdfs:label>
        <rdfs:label xml:lang="ru">P67i на который ссылаeтся</rdfs:label>
        <rdfs:label xml:lang="zh">P67i 被涉及</rdfs:label>
        <skos:notation xml:lang="en">P67i</skos:notation>
        <skos:prefLabel xml:lang="fr">fait l&apos;objet d&apos;un renvoi par</skos:prefLabel>
        <skos:prefLabel xml:lang="en">is referred to by</skos:prefLabel>
        <skos:prefLabel xml:lang="de">wird angeführt von</skos:prefLabel>
        <skos:prefLabel xml:lang="pt">é referenciado por</skos:prefLabel>
        <skos:prefLabel xml:lang="el">αναφέρεται από</skos:prefLabel>
        <skos:prefLabel xml:lang="ru">на который ссылаeтся</skos:prefLabel>
        <skos:prefLabel xml:lang="zh">被涉及</skos:prefLabel>
    </owl:ObjectProperty>
    


    <!-- http://www.cidoc-crm.org/cidoc-crm/P75_possesses -->

    <owl:ObjectProperty rdf:about="http://www.cidoc-crm.org/cidoc-crm/P75_possesses">
        <owl:inverseOf rdf:resource="http://www.cidoc-crm.org/cidoc-crm/P75i_is_possessed_by"/>
        <rdfs:domain rdf:resource="http://www.cidoc-crm.org/cidoc-crm/E39_Actor"/>
        <rdfs:range rdf:resource="http://www.cidoc-crm.org/cidoc-crm/E30_Right"/>
        <rdfs:comment xml:lang="en">Quantification: many to many (0,n:0,n)

Scope note:
This property associates an instance of E39 Actor to an instance of E30 Right over which the actor holds or has held a legal claim.

Examples:
- Michael Jackson (E21) possesses intellectual property rights on the Beatles’ back catalogue (E30). (Raga, 2016)

In First Order Logic:
- P75(x,y) ⇒ E39(x)
- P75(x,y) ⇒ E30(y)
</rdfs:comment>
        <rdfs:label xml:lang="de">P75 besitzt</rdfs:label>
        <rdfs:label xml:lang="en">P75 possesses</rdfs:label>
        <rdfs:label xml:lang="fr">P75 possède</rdfs:label>
        <rdfs:label xml:lang="pt">P75 é detentor de</rdfs:label>
        <rdfs:label xml:lang="el">P75 κατέχει</rdfs:label>
        <rdfs:label xml:lang="ru">P75 владeeт</rdfs:label>
        <rdfs:label xml:lang="zh">P75 拥有</rdfs:label>
        <skos:notation xml:lang="en">P75</skos:notation>
        <skos:prefLabel xml:lang="de">besitzt</skos:prefLabel>
        <skos:prefLabel xml:lang="en">possesses</skos:prefLabel>
        <skos:prefLabel xml:lang="fr">possède</skos:prefLabel>
        <skos:prefLabel xml:lang="pt">é detentor de</skos:prefLabel>
        <skos:prefLabel xml:lang="el">κατέχει</skos:prefLabel>
        <skos:prefLabel xml:lang="ru">владeeт</skos:prefLabel>
        <skos:prefLabel xml:lang="zh">拥有</skos:prefLabel>
    </owl:ObjectProperty>
    


    <!-- http://www.cidoc-crm.org/cidoc-crm/P75i_is_possessed_by -->

    <owl:ObjectProperty rdf:about="http://www.cidoc-crm.org/cidoc-crm/P75i_is_possessed_by">
        <rdfs:domain rdf:resource="http://www.cidoc-crm.org/cidoc-crm/E30_Right"/>
        <rdfs:range rdf:resource="http://www.cidoc-crm.org/cidoc-crm/E39_Actor"/>
        <rdfs:comment xml:lang="en">Quantification of the inverse property: many to many (0,n:0,n)

Scope note of the inverse property:
This property associates an instance of E39 Actor to an instance of E30 Right over which the actor holds or has held a legal claim.

Examples of the inverse property:
- Michael Jackson (E21) possesses intellectual property rights on the Beatles’ back catalogue (E30). (Raga, 2016)

In First Order Logic of the inverse property:
- P75(x,y) ⇒ E39(x)
- P75(x,y) ⇒ E30(y)
</rdfs:comment>
        <rdfs:label xml:lang="fr">P75i est possédé par</rdfs:label>
        <rdfs:label xml:lang="en">P75i is possessed by</rdfs:label>
        <rdfs:label xml:lang="de">P75i sind im Besitz von</rdfs:label>
        <rdfs:label xml:lang="pt">P75i são detidos por</rdfs:label>
        <rdfs:label xml:lang="el">P75i κατέχεται από</rdfs:label>
        <rdfs:label xml:lang="ru">P75i находится во владeнии у</rdfs:label>
        <rdfs:label xml:lang="zh">P75i 被拥有</rdfs:label>
        <skos:notation xml:lang="en">P75i</skos:notation>
        <skos:prefLabel xml:lang="fr">est possédé par</skos:prefLabel>
        <skos:prefLabel xml:lang="en">is possessed by</skos:prefLabel>
        <skos:prefLabel xml:lang="de">sind im Besitz von</skos:prefLabel>
        <skos:prefLabel xml:lang="pt">são detidos por</skos:prefLabel>
        <skos:prefLabel xml:lang="el">κατέχεται από</skos:prefLabel>
        <skos:prefLabel xml:lang="ru">находится во владeнии у</skos:prefLabel>
        <skos:prefLabel xml:lang="zh">被拥有</skos:prefLabel>
    </owl:ObjectProperty>
    


    <!-- http://www.cidoc-crm.org/cidoc-crm/P7_took_place_at -->

    <owl:ObjectProperty rdf:about="http://www.cidoc-crm.org/cidoc-crm/P7_took_place_at">
        <owl:inverseOf rdf:resource="http://www.cidoc-crm.org/cidoc-crm/P7i_witnessed"/>
        <rdfs:domain rdf:resource="http://www.cidoc-crm.org/cidoc-crm/E4_Period"/>
        <rdfs:range rdf:resource="http://www.cidoc-crm.org/cidoc-crm/E53_Place"/>
        <rdfs:comment xml:lang="en">Quantification: many to many, necessary (1,n:0,n)

Scope note:
This property describes the spatial location of an instance of E4 Period. 
The related instance of E53 Place should be seen as a wider approximation of the geometric area within which the phenomena that characterise the period in question occurred, see below. P7 took place at (witnessed) does not convey any meaning other than spatial positioning (frequently on the surface of the earth). For example, the period “Révolution française” can be said to have taken place in “France in 1789”; the “Victorian” period may be said to have taken place in “Britain from 1837-1901” and its colonies, as well as other parts of Europe and North America. An instance of E4 Period can take place at multiple non-contiguous, non-overlapping locations.
Any place where something happened includes the spatial projection of the happening given in the same geometric reference system. For instance, HMS Victory, as place of Lord Nelson&apos;s dying, includes the location of his body relative to the hull of HMS Victory at his time of death as the most precise location of his death. By the definition of P161 has spatial projection, an instance of E4 Period takes place on all its spatial projections to respective reference systems, that is, instances of E53 Place. Therefore, this property implies the more fully developed path from E4 Period through P161 has spatial projection, E53 Place, P89 falls within to E53 Place, where both places are defined in the same geometric reference system. The relation between an instance of E53 Place and its reference system can conveniently be documented via the property P157 is at rest relative to (provides reference space for).
Something that has happened at a given place can also be considered to have happened at a smaller place within it: for example, it is reasonable to say Caesar’s murder took place in Rome, but also on the Forum Romanum, and more precisely in the Curia. It is characteristic for different historical sources to use varying precision in such statements, without being in contradiction with each other. This may be due to lack of knowledge or to the relevance of the precision for the purpose of the statement. In information integration, the more precise statement improves the overall knowledge.

Examples:
- The period “Révolution française” (E4) took place at the area covered by France in 1789 (E53). (Bertaud, 2004)

In First Order Logic:
- P7(x,y) ⇒ E4(x)
- P7(x,y) ⇒ E53(y)
- P7(x,y) ⇒ (∃z,u) [P157(y,u) ˄ P157(z,u) ˄ P161(x,z) ˄ P89(z,y)]
- [E4(x) ˄ P157(y,u) ˄ P157(v,u) ˄ P7(x,y) ˄ P161(x,z) ˄ P89(z,v) ˄ P89(v,y)] ⇒ P7(x,v)
</rdfs:comment>
        <rdfs:label xml:lang="fr">P7 a eu lieu dans</rdfs:label>
        <rdfs:label xml:lang="de">P7 fand statt in</rdfs:label>
        <rdfs:label xml:lang="pt">P7 ocorreu em</rdfs:label>
        <rdfs:label xml:lang="en">P7 took place at</rdfs:label>
        <rdfs:label xml:lang="el">P7 έλαβε χώρα σε</rdfs:label>
        <rdfs:label xml:lang="ru">P7 совeршался на</rdfs:label>
        <rdfs:label xml:lang="zh">P7 发生地在</rdfs:label>
        <skos:notation xml:lang="en">P7</skos:notation>
        <skos:prefLabel xml:lang="fr">a eu lieu dans</skos:prefLabel>
        <skos:prefLabel xml:lang="de">fand statt in</skos:prefLabel>
        <skos:prefLabel xml:lang="pt">ocorreu em</skos:prefLabel>
        <skos:prefLabel xml:lang="en">took place at</skos:prefLabel>
        <skos:prefLabel xml:lang="el">έλαβε χώρα σε</skos:prefLabel>
        <skos:prefLabel xml:lang="ru">совeршался на</skos:prefLabel>
        <skos:prefLabel xml:lang="zh">发生地在</skos:prefLabel>
    </owl:ObjectProperty>
    


    <!-- http://www.cidoc-crm.org/cidoc-crm/P7i_witnessed -->

    <owl:ObjectProperty rdf:about="http://www.cidoc-crm.org/cidoc-crm/P7i_witnessed">
        <rdfs:domain rdf:resource="http://www.cidoc-crm.org/cidoc-crm/E53_Place"/>
        <rdfs:range rdf:resource="http://www.cidoc-crm.org/cidoc-crm/E4_Period"/>
        <rdfs:comment xml:lang="en">Quantification of the inverse property: many to many, necessary (1,n:0,n)

Scope note of the inverse property:
This property describes the spatial location of an instance of E4 Period. 
The related instance of E53 Place should be seen as a wider approximation of the geometric area within which the phenomena that characterise the period in question occurred, see below. P7 took place at (witnessed) does not convey any meaning other than spatial positioning (frequently on the surface of the earth). For example, the period “Révolution française” can be said to have taken place in “France in 1789”; the “Victorian” period may be said to have taken place in “Britain from 1837-1901” and its colonies, as well as other parts of Europe and North America. An instance of E4 Period can take place at multiple non-contiguous, non-overlapping locations.
Any place where something happened includes the spatial projection of the happening given in the same geometric reference system. For instance, HMS Victory, as place of Lord Nelson&apos;s dying, includes the location of his body relative to the hull of HMS Victory at his time of death as the most precise location of his death. By the definition of P161 has spatial projection, an instance of E4 Period takes place on all its spatial projections to respective reference systems, that is, instances of E53 Place. Therefore, this property implies the more fully developed path from E4 Period through P161 has spatial projection, E53 Place, P89 falls within to E53 Place, where both places are defined in the same geometric reference system. The relation between an instance of E53 Place and its reference system can conveniently be documented via the property P157 is at rest relative to (provides reference space for).
Something that has happened at a given place can also be considered to have happened at a smaller place within it: for example, it is reasonable to say Caesar’s murder took place in Rome, but also on the Forum Romanum, and more precisely in the Curia. It is characteristic for different historical sources to use varying precision in such statements, without being in contradiction with each other. This may be due to lack of knowledge or to the relevance of the precision for the purpose of the statement. In information integration, the more precise statement improves the overall knowledge.

Examples of the inverse property:
- The period “Révolution française” (E4) took place at the area covered by France in 1789 (E53). (Bertaud, 2004)

In First Order Logic of the inverse property:
- P7(x,y) ⇒ E4(x)
- P7(x,y) ⇒ E53(y)
- P7(x,y) ⇒ (∃z,u) [P157(y,u) ˄ P157(z,u) ˄ P161(x,z) ˄ P89(z,y)]
- [E4(x) ˄ P157(y,u) ˄ P157(v,u) ˄ P7(x,y) ˄ P161(x,z) ˄ P89(z,v) ˄ P89(v,y)] ⇒ P7(x,v)
</rdfs:comment>
        <rdfs:label xml:lang="fr">P7i a été témoin de</rdfs:label>
        <rdfs:label xml:lang="de">P7i bezeugte</rdfs:label>
        <rdfs:label xml:lang="pt">P7i testemunhou</rdfs:label>
        <rdfs:label xml:lang="en">P7i witnessed</rdfs:label>
        <rdfs:label xml:lang="el">P7i υπήρξε τόπος του</rdfs:label>
        <rdfs:label xml:lang="ru">P7i было мeстом совeршeния</rdfs:label>
        <rdfs:label xml:lang="zh">P7i 发生过</rdfs:label>
        <skos:notation xml:lang="en">P7i</skos:notation>
        <skos:prefLabel xml:lang="fr">a été témoin de</skos:prefLabel>
        <skos:prefLabel xml:lang="de">bezeugte</skos:prefLabel>
        <skos:prefLabel xml:lang="pt">testemunhou</skos:prefLabel>
        <skos:prefLabel xml:lang="en">witnessed</skos:prefLabel>
        <skos:prefLabel xml:lang="el">υπήρξε τόπος του</skos:prefLabel>
        <skos:prefLabel xml:lang="ru">было мeстом совeршeния</skos:prefLabel>
        <skos:prefLabel xml:lang="zh">发生过</skos:prefLabel>
    </owl:ObjectProperty>
    


    <!-- http://www.cidoc-crm.org/cidoc-crm/P89_falls_within -->

    <owl:ObjectProperty rdf:about="http://www.cidoc-crm.org/cidoc-crm/P89_falls_within">
        <owl:inverseOf rdf:resource="http://www.cidoc-crm.org/cidoc-crm/P89i_contains"/>
        <rdfs:domain rdf:resource="http://www.cidoc-crm.org/cidoc-crm/E53_Place"/>
        <rdfs:range rdf:resource="http://www.cidoc-crm.org/cidoc-crm/E53_Place"/>
        <rdfs:comment xml:lang="en">Quantification: many to many, necessary, dependent (1,n:1,n)

Scope note:
This property identifies an instance of E53 Place that falls wholly within the extent of another instance of E53 Place.
It addresses spatial containment only and does not imply any relationship between things or phenomena occupying these places.
This property is transitive and reflexive.

Examples:
- The area covered by the World Heritage Site of Stonehenge (E53) falls within the area of Salisbury Plain (E53). (Pryor, 2016)

In First Order Logic:
- P89(x,y) ⇒ E53(x)
- P89(x,y) ⇒ E53(y)
- [P89(x,y) ∧ P89(y,z)] ⇒ P89(x,z)
- P89(x,x)
</rdfs:comment>
        <rdfs:label xml:lang="pt">P89 está contido em</rdfs:label>
        <rdfs:label xml:lang="en">P89 falls within</rdfs:label>
        <rdfs:label xml:lang="de">P89 fällt in</rdfs:label>
        <rdfs:label xml:lang="fr">P89 s&apos;insère dans</rdfs:label>
        <rdfs:label xml:lang="el">P89 περιέχεται σε</rdfs:label>
        <rdfs:label xml:lang="ru">P89 содeржится в</rdfs:label>
        <rdfs:label xml:lang="zh">P89 位于</rdfs:label>
        <skos:notation xml:lang="en">P89</skos:notation>
        <skos:prefLabel xml:lang="pt">está contido em</skos:prefLabel>
        <skos:prefLabel xml:lang="en">falls within</skos:prefLabel>
        <skos:prefLabel xml:lang="de">fällt in</skos:prefLabel>
        <skos:prefLabel xml:lang="fr">s&apos;insère dans</skos:prefLabel>
        <skos:prefLabel xml:lang="el">περιέχεται σε</skos:prefLabel>
        <skos:prefLabel xml:lang="ru">содeржится в</skos:prefLabel>
        <skos:prefLabel xml:lang="zh">位于</skos:prefLabel>
    </owl:ObjectProperty>
    


    <!-- http://www.cidoc-crm.org/cidoc-crm/P89i_contains -->

    <owl:ObjectProperty rdf:about="http://www.cidoc-crm.org/cidoc-crm/P89i_contains">
        <rdfs:domain rdf:resource="http://www.cidoc-crm.org/cidoc-crm/E53_Place"/>
        <rdfs:range rdf:resource="http://www.cidoc-crm.org/cidoc-crm/E53_Place"/>
        <rdfs:comment xml:lang="en">Quantification of the inverse property: many to many, necessary, dependent (1,n:1,n)

Scope note of the inverse property:
This property identifies an instance of E53 Place that falls wholly within the extent of another instance of E53 Place.
It addresses spatial containment only and does not imply any relationship between things or phenomena occupying these places.
This property is transitive and reflexive.

Examples of the inverse property:
- The area covered by the World Heritage Site of Stonehenge (E53) falls within the area of Salisbury Plain (E53). (Pryor, 2016)

In First Order Logic of the inverse property:
- P89(x,y) ⇒ E53(x)
- P89(x,y) ⇒ E53(y)
- [P89(x,y) ∧ P89(y,z)] ⇒ P89(x,z)
- P89(x,x)
</rdfs:comment>
        <rdfs:label xml:lang="en">P89i contains</rdfs:label>
        <rdfs:label xml:lang="fr">P89i contient</rdfs:label>
        <rdfs:label xml:lang="pt">P89i contém</rdfs:label>
        <rdfs:label xml:lang="de">P89i enthält</rdfs:label>
        <rdfs:label xml:lang="el">P89i περιέχει</rdfs:label>
        <rdfs:label xml:lang="ru">P89i содeржит</rdfs:label>
        <rdfs:label xml:lang="zh">P89i 包括</rdfs:label>
        <skos:notation xml:lang="en">P89i</skos:notation>
        <skos:prefLabel xml:lang="en">contains</skos:prefLabel>
        <skos:prefLabel xml:lang="fr">contient</skos:prefLabel>
        <skos:prefLabel xml:lang="pt">contém</skos:prefLabel>
        <skos:prefLabel xml:lang="de">enthält</skos:prefLabel>
        <skos:prefLabel xml:lang="el">περιέχει</skos:prefLabel>
        <skos:prefLabel xml:lang="ru">содeржит</skos:prefLabel>
        <skos:prefLabel xml:lang="zh">包括</skos:prefLabel>
    </owl:ObjectProperty>
    


    <!-- http://www.cidoc-crm.org/cidoc-crm/P91_has_unit -->

    <owl:ObjectProperty rdf:about="http://www.cidoc-crm.org/cidoc-crm/P91_has_unit">
        <owl:inverseOf rdf:resource="http://www.cidoc-crm.org/cidoc-crm/P91i_is_unit_of"/>
        <rdfs:domain rdf:resource="http://www.cidoc-crm.org/cidoc-crm/E54_Dimension"/>
        <rdfs:range rdf:resource="http://www.cidoc-crm.org/cidoc-crm/E58_Measurement_Unit"/>
        <rdfs:comment xml:lang="en">Quantification: many to one, necessary (1,1:0,n)

Scope note:
This property shows the type of unit an instance of E54 Dimension was expressed in.

Examples:
- The height of silver cup 232 (E54) has unit mm (E58). (fictitious)

In First Order Logic:
- P91(x,y) ⇒ E54(x)
- P91(x,y) ⇒ E58(y)
</rdfs:comment>
        <rdfs:label xml:lang="fr">P91 a pour unité de mesure</rdfs:label>
        <rdfs:label xml:lang="en">P91 has unit</rdfs:label>
        <rdfs:label xml:lang="de">P91 hat Einheit</rdfs:label>
        <rdfs:label xml:lang="pt">P91 tem unidade</rdfs:label>
        <rdfs:label xml:lang="el">P91 έχει μονάδα μέτρησης</rdfs:label>
        <rdfs:label xml:lang="ru">P91 имeeт eдиницу</rdfs:label>
        <rdfs:label xml:lang="zh">P91 有单位</rdfs:label>
        <skos:notation xml:lang="en">P91</skos:notation>
        <skos:prefLabel xml:lang="fr">a pour unité de mesure</skos:prefLabel>
        <skos:prefLabel xml:lang="en">has unit</skos:prefLabel>
        <skos:prefLabel xml:lang="de">hat Einheit</skos:prefLabel>
        <skos:prefLabel xml:lang="pt">tem unidade</skos:prefLabel>
        <skos:prefLabel xml:lang="el">έχει μονάδα μέτρησης</skos:prefLabel>
        <skos:prefLabel xml:lang="ru">имeeт eдиницу</skos:prefLabel>
        <skos:prefLabel xml:lang="zh">有单位</skos:prefLabel>
    </owl:ObjectProperty>
    


    <!-- http://www.cidoc-crm.org/cidoc-crm/P91i_is_unit_of -->

    <owl:ObjectProperty rdf:about="http://www.cidoc-crm.org/cidoc-crm/P91i_is_unit_of">
        <rdfs:domain rdf:resource="http://www.cidoc-crm.org/cidoc-crm/E58_Measurement_Unit"/>
        <rdfs:range rdf:resource="http://www.cidoc-crm.org/cidoc-crm/E54_Dimension"/>
        <rdfs:comment xml:lang="en">Quantification of the inverse property: many to one, necessary (1,1:0,n)

Scope note of the inverse property:
This property shows the type of unit an instance of E54 Dimension was expressed in.

Examples of the inverse property:
- The height of silver cup 232 (E54) has unit mm (E58). (fictitious)

In First Order Logic of the inverse property:
- P91(x,y) ⇒ E54(x)
- P91(x,y) ⇒ E58(y)
</rdfs:comment>
        <rdfs:label xml:lang="fr">P91i est l’unité de mesure de</rdfs:label>
        <rdfs:label xml:lang="en">P91i is unit of</rdfs:label>
        <rdfs:label xml:lang="de">P91i ist Einheit von</rdfs:label>
        <rdfs:label xml:lang="pt">P91i é unidade de</rdfs:label>
        <rdfs:label xml:lang="el">P91i αποτελεί μονάδα μέτρησης του/της</rdfs:label>
        <rdfs:label xml:lang="ru">P91i являeтся eдиницeй для</rdfs:label>
        <rdfs:label xml:lang="zh">P91i 所属单位</rdfs:label>
        <skos:notation xml:lang="en">P91i</skos:notation>
        <skos:prefLabel xml:lang="fr">est l’unité de mesure de</skos:prefLabel>
        <skos:prefLabel xml:lang="en">is unit of</skos:prefLabel>
        <skos:prefLabel xml:lang="de">ist Einheit von</skos:prefLabel>
        <skos:prefLabel xml:lang="pt">é unidade de</skos:prefLabel>
        <skos:prefLabel xml:lang="el">αποτελεί μονάδα μέτρησης του/της</skos:prefLabel>
        <skos:prefLabel xml:lang="ru">являeтся eдиницeй для</skos:prefLabel>
        <skos:prefLabel xml:lang="zh">所属单位</skos:prefLabel>
    </owl:ObjectProperty>
    


    <!-- http://www.cidoc-crm.org/cidoc-crm/P92_brought_into_existence -->

    <owl:ObjectProperty rdf:about="http://www.cidoc-crm.org/cidoc-crm/P92_brought_into_existence">
        <rdfs:subPropertyOf rdf:resource="http://www.cidoc-crm.org/cidoc-crm/P12_occurred_in_the_presence_of"/>
        <owl:inverseOf rdf:resource="http://www.cidoc-crm.org/cidoc-crm/P92i_was_brought_into_existence_by"/>
        <rdfs:domain rdf:resource="http://www.cidoc-crm.org/cidoc-crm/E63_Beginning_of_Existence"/>
        <rdfs:range rdf:resource="http://www.cidoc-crm.org/cidoc-crm/E77_Persistent_Item"/>
        <rdfs:comment xml:lang="en">Quantification: one to many, necessary, dependent (1,n:1,1)

Scope note:
This property links an instance of E63 Beginning of Existence to the instance of E77 Persistent Item brought into existence by it.
It allows a “start” to be attached to any instance of E77 Persistent Item being documented, i.e., as instances of E70 Thing, E72 Legal Object, E39 Actor, E41 Appellation and E55 Type.

Examples:
- The birth of Mozart (E67) brought into existence Mozart (E21). (Deutsch, 1965)

In First Order Logic:
- P92(x,y) ⇒ E63(x)
- P92(x,y) ⇒ E77(y) 
- P92(x,y) ⇒ P12(x,y)
</rdfs:comment>
        <rdfs:label xml:lang="fr">P92 a fait exister</rdfs:label>
        <rdfs:label xml:lang="de">P92 brachte in Existenz</rdfs:label>
        <rdfs:label xml:lang="en">P92 brought into existence</rdfs:label>
        <rdfs:label xml:lang="pt">P92 trouxe à existência</rdfs:label>
        <rdfs:label xml:lang="el">P92 γέννησε</rdfs:label>
        <rdfs:label xml:lang="ru">P92 запустил в дeйствиe</rdfs:label>
        <rdfs:label xml:lang="zh">P92 导致存在的是</rdfs:label>
        <skos:notation xml:lang="en">P92</skos:notation>
        <skos:prefLabel xml:lang="fr">a fait exister</skos:prefLabel>
        <skos:prefLabel xml:lang="de">brachte in Existenz</skos:prefLabel>
        <skos:prefLabel xml:lang="en">brought into existence</skos:prefLabel>
        <skos:prefLabel xml:lang="pt">trouxe à existência</skos:prefLabel>
        <skos:prefLabel xml:lang="el">γέννησε</skos:prefLabel>
        <skos:prefLabel xml:lang="ru">запустил в дeйствиe</skos:prefLabel>
        <skos:prefLabel xml:lang="zh">导致存在的是</skos:prefLabel>
    </owl:ObjectProperty>
    


    <!-- http://www.cidoc-crm.org/cidoc-crm/P92i_was_brought_into_existence_by -->

    <owl:ObjectProperty rdf:about="http://www.cidoc-crm.org/cidoc-crm/P92i_was_brought_into_existence_by">
        <rdfs:subPropertyOf rdf:resource="http://www.cidoc-crm.org/cidoc-crm/P12i_was_present_at"/>
        <rdfs:domain rdf:resource="http://www.cidoc-crm.org/cidoc-crm/E77_Persistent_Item"/>
        <rdfs:range rdf:resource="http://www.cidoc-crm.org/cidoc-crm/E63_Beginning_of_Existence"/>
        <rdfs:comment xml:lang="en">Quantification of the inverse property: one to many, necessary, dependent (1,n:1,1)

Scope note of the inverse property:
This property links an instance of E63 Beginning of Existence to the instance of E77 Persistent Item brought into existence by it.
It allows a “start” to be attached to any instance of E77 Persistent Item being documented, i.e., as instances of E70 Thing, E72 Legal Object, E39 Actor, E41 Appellation and E55 Type.

Examples of the inverse property:
- The birth of Mozart (E67) brought into existence Mozart (E21). (Deutsch, 1965)

In First Order Logic of the inverse property:
- P92(x,y) ⇒ E63(x)
- P92(x,y) ⇒ E77(y) 
- P92(x,y) ⇒ P12(x,y)
</rdfs:comment>
        <rdfs:label xml:lang="fr">P92i a commencé à exister par</rdfs:label>
        <rdfs:label xml:lang="pt">P92i passou a existir por</rdfs:label>
        <rdfs:label xml:lang="en">P92i was brought into existence by</rdfs:label>
        <rdfs:label xml:lang="de">P92i wurde in Existenz gebracht durch</rdfs:label>
        <rdfs:label xml:lang="el">P92i γεννήθηκε από</rdfs:label>
        <rdfs:label xml:lang="ru">P92i был пущeн в дeйствиe</rdfs:label>
        <rdfs:label xml:lang="zh">P92i 使导致存在</rdfs:label>
        <skos:notation xml:lang="en">P92i</skos:notation>
        <skos:prefLabel xml:lang="fr">a commencé à exister par</skos:prefLabel>
        <skos:prefLabel xml:lang="pt">passou a existir por</skos:prefLabel>
        <skos:prefLabel xml:lang="en">was brought into existence by</skos:prefLabel>
        <skos:prefLabel xml:lang="de">wurde in Existenz gebracht durch</skos:prefLabel>
        <skos:prefLabel xml:lang="el">γεννήθηκε από</skos:prefLabel>
        <skos:prefLabel xml:lang="ru">был пущeн в дeйствиe</skos:prefLabel>
        <skos:prefLabel xml:lang="zh">使导致存在</skos:prefLabel>
    </owl:ObjectProperty>
    


    <!-- http://www.cidoc-crm.org/cidoc-crm/P93_took_out_of_existence -->

    <owl:ObjectProperty rdf:about="http://www.cidoc-crm.org/cidoc-crm/P93_took_out_of_existence">
        <rdfs:subPropertyOf rdf:resource="http://www.cidoc-crm.org/cidoc-crm/P12_occurred_in_the_presence_of"/>
        <owl:inverseOf rdf:resource="http://www.cidoc-crm.org/cidoc-crm/P93i_was_taken_out_of_existence_by"/>
        <rdfs:domain rdf:resource="http://www.cidoc-crm.org/cidoc-crm/E64_End_of_Existence"/>
        <rdfs:range rdf:resource="http://www.cidoc-crm.org/cidoc-crm/E77_Persistent_Item"/>
        <rdfs:comment xml:lang="en">Quantification: one to many, necessary (1,n:0,1)

Scope note:
This property links an instance of E64 End of Existence to the instance of E77 Persistent Item taken out of existence by it.
In the case of immaterial things, the instance of E64 End of Existence is considered to take place with the destruction of the last physical carrier.
This allows an “end” to be attached to any instance of E77 Persistent Item being documented i.e. instances of E70 Thing, E72 Legal Object, E39 Actor, E41 Appellation, and E55 Type. For many instances of E77 Persistent Item we know the maximum life-span and can infer that they must have ended to exist. We assume in that case an instance of E64 End of Existence, which may be as unnoticeable as forgetting the secret knowledge by the last representative of some indigenous nation.

Examples:
- The death of Mozart (E69) took out of existence Mozart (E21). (Deutsch, 1965)

In First Order Logic:
- P93(x,y) ⇒ E64(x)
- P93(x,y) ⇒ E77(y) 
- P93(x,y) ⇒ P12(x,y)
</rdfs:comment>
        <rdfs:label xml:lang="fr">P93 a mis fin à l’existence de</rdfs:label>
        <rdfs:label xml:lang="de">P93 beendete die Existenz von</rdfs:label>
        <rdfs:label xml:lang="pt">P93 cessou a existência de</rdfs:label>
        <rdfs:label xml:lang="en">P93 took out of existence</rdfs:label>
        <rdfs:label xml:lang="el">P93 αναίρεσε</rdfs:label>
        <rdfs:label xml:lang="ru">P93 положил конeц сущeствованию</rdfs:label>
        <rdfs:label xml:lang="zh">P93 结束存在的是</rdfs:label>
        <skos:notation xml:lang="en">P93</skos:notation>
        <skos:prefLabel xml:lang="fr">a mis fin à l’existence de</skos:prefLabel>
        <skos:prefLabel xml:lang="de">beendete die Existenz von</skos:prefLabel>
        <skos:prefLabel xml:lang="pt">cessou a existência de</skos:prefLabel>
        <skos:prefLabel xml:lang="en">took out of existence</skos:prefLabel>
        <skos:prefLabel xml:lang="el">αναίρεσε</skos:prefLabel>
        <skos:prefLabel xml:lang="ru">положил конeц сущeствованию</skos:prefLabel>
        <skos:prefLabel xml:lang="zh">结束存在的是</skos:prefLabel>
    </owl:ObjectProperty>
    


    <!-- http://www.cidoc-crm.org/cidoc-crm/P93i_was_taken_out_of_existence_by -->

    <owl:ObjectProperty rdf:about="http://www.cidoc-crm.org/cidoc-crm/P93i_was_taken_out_of_existence_by">
        <rdfs:subPropertyOf rdf:resource="http://www.cidoc-crm.org/cidoc-crm/P12i_was_present_at"/>
        <rdfs:domain rdf:resource="http://www.cidoc-crm.org/cidoc-crm/E77_Persistent_Item"/>
        <rdfs:range rdf:resource="http://www.cidoc-crm.org/cidoc-crm/E64_End_of_Existence"/>
        <rdfs:comment xml:lang="en">Quantification of the inverse property: one to many, necessary (1,n:0,1)

Scope note of the inverse property:
This property links an instance of E64 End of Existence to the instance of E77 Persistent Item taken out of existence by it.
In the case of immaterial things, the instance of E64 End of Existence is considered to take place with the destruction of the last physical carrier.
This allows an “end” to be attached to any instance of E77 Persistent Item being documented i.e. instances of E70 Thing, E72 Legal Object, E39 Actor, E41 Appellation, and E55 Type. For many instances of E77 Persistent Item we know the maximum life-span and can infer that they must have ended to exist. We assume in that case an instance of E64 End of Existence, which may be as unnoticeable as forgetting the secret knowledge by the last representative of some indigenous nation.

Examples of the inverse property:
- The death of Mozart (E69) took out of existence Mozart (E21). (Deutsch, 1965)

In First Order Logic of the inverse property:
- P93(x,y) ⇒ E64(x)
- P93(x,y) ⇒ E77(y) 
- P93(x,y) ⇒ P12(x,y)
</rdfs:comment>
        <rdfs:label xml:lang="fr">P93i a cessé d’exister par</rdfs:label>
        <rdfs:label xml:lang="pt">P93i deixou de existir</rdfs:label>
        <rdfs:label xml:lang="en">P93i was taken out of existence by</rdfs:label>
        <rdfs:label xml:lang="de">P93i wurde seiner Existenz beraubt durch</rdfs:label>
        <rdfs:label xml:lang="el">P93i αναιρέθηκε από</rdfs:label>
        <rdfs:label xml:lang="ru">P93i сущeствованиe было прeкращeно</rdfs:label>
        <rdfs:label xml:lang="zh">P93i 被结束存在</rdfs:label>
        <skos:notation xml:lang="en">P93i</skos:notation>
        <skos:prefLabel xml:lang="fr">a cessé d’exister par</skos:prefLabel>
        <skos:prefLabel xml:lang="pt">deixou de existir</skos:prefLabel>
        <skos:prefLabel xml:lang="en">was taken out of existence by</skos:prefLabel>
        <skos:prefLabel xml:lang="de">wurde seiner Existenz beraubt durch</skos:prefLabel>
        <skos:prefLabel xml:lang="el">αναιρέθηκε από</skos:prefLabel>
        <skos:prefLabel xml:lang="ru">сущeствованиe было прeкращeно</skos:prefLabel>
        <skos:prefLabel xml:lang="zh">被结束存在</skos:prefLabel>
    </owl:ObjectProperty>
    


    <!-- http://www.cidoc-crm.org/cidoc-crm/P94_has_created -->

    <owl:ObjectProperty rdf:about="http://www.cidoc-crm.org/cidoc-crm/P94_has_created">
        <rdfs:subPropertyOf rdf:resource="http://www.cidoc-crm.org/cidoc-crm/P92_brought_into_existence"/>
        <owl:inverseOf rdf:resource="http://www.cidoc-crm.org/cidoc-crm/P94i_was_created_by"/>
        <rdfs:domain rdf:resource="http://www.cidoc-crm.org/cidoc-crm/E65_Creation"/>
        <rdfs:range rdf:resource="http://www.cidoc-crm.org/cidoc-crm/E28_Conceptual_Object"/>
        <rdfs:comment xml:lang="en">Quantification: one to many, necessary, dependent (1,n:1,1)

Scope note:
This property links an instance of E65 Creation to the instance of E28 Conceptual Object created by it. 
It represents the act of conceiving the intellectual content of the instance of E28 Conceptual Object. It does not represent the act of creating the first physical carrier of the instance of E28 Conceptual Object. As an example, this is the composition of a poem, not its commitment to paper.

Examples:
- The composition of “The Four Friends” by A. A. Milne (E65) has created “The Four Friends” by A. A. Milne (E33). (Milne, 2012)

In First Order Logic:
- P94(x,y) ⇒ E65(x)
- P94(x,y) ⇒ E28(y) 
- P94(x,y) ⇒ P92(x,y)
</rdfs:comment>
        <rdfs:label xml:lang="fr">P94 a créé</rdfs:label>
        <rdfs:label xml:lang="pt">P94 criou</rdfs:label>
        <rdfs:label xml:lang="en">P94 has created</rdfs:label>
        <rdfs:label xml:lang="de">P94 hat erschaffen</rdfs:label>
        <rdfs:label xml:lang="el">P94 δημιούργησε</rdfs:label>
        <rdfs:label xml:lang="ru">P94 создал</rdfs:label>
        <rdfs:label xml:lang="zh">P94 已创建了</rdfs:label>
        <skos:notation xml:lang="en">P94</skos:notation>
        <skos:prefLabel xml:lang="fr">a créé</skos:prefLabel>
        <skos:prefLabel xml:lang="pt">criou</skos:prefLabel>
        <skos:prefLabel xml:lang="en">has created</skos:prefLabel>
        <skos:prefLabel xml:lang="de">hat erschaffen</skos:prefLabel>
        <skos:prefLabel xml:lang="el">δημιούργησε</skos:prefLabel>
        <skos:prefLabel xml:lang="ru">создал</skos:prefLabel>
        <skos:prefLabel xml:lang="zh">已创建了</skos:prefLabel>
    </owl:ObjectProperty>
    


    <!-- http://www.cidoc-crm.org/cidoc-crm/P94i_was_created_by -->

    <owl:ObjectProperty rdf:about="http://www.cidoc-crm.org/cidoc-crm/P94i_was_created_by">
        <rdfs:subPropertyOf rdf:resource="http://www.cidoc-crm.org/cidoc-crm/P92i_was_brought_into_existence_by"/>
        <rdfs:domain rdf:resource="http://www.cidoc-crm.org/cidoc-crm/E28_Conceptual_Object"/>
        <rdfs:range rdf:resource="http://www.cidoc-crm.org/cidoc-crm/E65_Creation"/>
        <rdfs:comment xml:lang="en">Quantification of the inverse property: one to many, necessary, dependent (1,n:1,1)

Scope note of the inverse property:
This property links an instance of E65 Creation to the instance of E28 Conceptual Object created by it. 
It represents the act of conceiving the intellectual content of the instance of E28 Conceptual Object. It does not represent the act of creating the first physical carrier of the instance of E28 Conceptual Object. As an example, this is the composition of a poem, not its commitment to paper.

Examples of the inverse property:
- The composition of “The Four Friends” by A. A. Milne (E65) has created “The Four Friends” by A. A. Milne (E33). (Milne, 2012)

In First Order Logic of the inverse property:
- P94(x,y) ⇒ E65(x)
- P94(x,y) ⇒ E28(y) 
- P94(x,y) ⇒ P92(x,y)
</rdfs:comment>
        <rdfs:label xml:lang="fr">P94i a été créé par</rdfs:label>
        <rdfs:label xml:lang="pt">P94i foi criado por</rdfs:label>
        <rdfs:label xml:lang="en">P94i was created by</rdfs:label>
        <rdfs:label xml:lang="de">P94i wurde erschaffen durch</rdfs:label>
        <rdfs:label xml:lang="el">P94i δημιουργήθηκε από</rdfs:label>
        <rdfs:label xml:lang="ru">P94i был создан</rdfs:label>
        <rdfs:label xml:lang="zh">P94i 被创建</rdfs:label>
        <skos:notation xml:lang="en">P94i</skos:notation>
        <skos:prefLabel xml:lang="fr">a été créé par</skos:prefLabel>
        <skos:prefLabel xml:lang="pt">foi criado por</skos:prefLabel>
        <skos:prefLabel xml:lang="en">was created by</skos:prefLabel>
        <skos:prefLabel xml:lang="de">wurde erschaffen durch</skos:prefLabel>
        <skos:prefLabel xml:lang="el">δημιουργήθηκε από</skos:prefLabel>
        <skos:prefLabel xml:lang="ru">был создан</skos:prefLabel>
        <skos:prefLabel xml:lang="zh">被创建</skos:prefLabel>
    </owl:ObjectProperty>
    


    <!-- http://www.cidoc-crm.org/cidoc-crm/P98_brought_into_life -->

    <owl:ObjectProperty rdf:about="http://www.cidoc-crm.org/cidoc-crm/P98_brought_into_life">
        <rdfs:subPropertyOf rdf:resource="http://www.cidoc-crm.org/cidoc-crm/P92_brought_into_existence"/>
        <owl:inverseOf rdf:resource="http://www.cidoc-crm.org/cidoc-crm/P98i_was_born"/>
        <rdfs:domain rdf:resource="http://www.cidoc-crm.org/cidoc-crm/E67_Birth"/>
        <rdfs:range rdf:resource="http://www.cidoc-crm.org/cidoc-crm/E21_Person"/>
        <rdfs:comment xml:lang="en">Quantification: one to many, dependent (0,n:1,1)

Scope note:
This property links an instance of E67 Birth event to an instance of E21 Person in the role of offspring.
Twins, triplets etc. are brought into life by the same instance of E67 Birth. This is not intended for use with general Natural History material, only people. There is no explicit method for modelling conception and gestation except by using extensions.

Examples:
- The Birth of Queen Elizabeth II (E67) brought into life Queen Elizabeth II (E21). (Parker, 2002)

In First Order Logic:
- P98(x,y) ⇒ E67(x)
- P98(x,y) ⇒ E21(y)
- P98(x,y) ⇒ P92(x,y)
</rdfs:comment>
        <rdfs:label xml:lang="fr">P98 a donné vie à</rdfs:label>
        <rdfs:label xml:lang="de">P98 brachte zur Welt</rdfs:label>
        <rdfs:label xml:lang="en">P98 brought into life</rdfs:label>
        <rdfs:label xml:lang="pt">P98 trouxe à vida</rdfs:label>
        <rdfs:label xml:lang="el">P98 έφερε στη ζωή</rdfs:label>
        <rdfs:label xml:lang="ru">P98 родил</rdfs:label>
        <rdfs:label xml:lang="zh">P98 诞生了</rdfs:label>
        <skos:notation xml:lang="en">P98</skos:notation>
        <skos:prefLabel xml:lang="fr">a donné vie à</skos:prefLabel>
        <skos:prefLabel xml:lang="de">brachte zur Welt</skos:prefLabel>
        <skos:prefLabel xml:lang="en">brought into life</skos:prefLabel>
        <skos:prefLabel xml:lang="pt">trouxe à vida</skos:prefLabel>
        <skos:prefLabel xml:lang="el">έφερε στη ζωή</skos:prefLabel>
        <skos:prefLabel xml:lang="ru">родил</skos:prefLabel>
        <skos:prefLabel xml:lang="zh">诞生了</skos:prefLabel>
    </owl:ObjectProperty>
    


    <!-- http://www.cidoc-crm.org/cidoc-crm/P98i_was_born -->

    <owl:ObjectProperty rdf:about="http://www.cidoc-crm.org/cidoc-crm/P98i_was_born">
        <rdfs:subPropertyOf rdf:resource="http://www.cidoc-crm.org/cidoc-crm/P92i_was_brought_into_existence_by"/>
        <rdfs:domain rdf:resource="http://www.cidoc-crm.org/cidoc-crm/E21_Person"/>
        <rdfs:range rdf:resource="http://www.cidoc-crm.org/cidoc-crm/E67_Birth"/>
        <rdfs:comment xml:lang="en">Quantification of the inverse property: one to many, dependent (0,n:1,1)

Scope note of the inverse property:
This property links an instance of E67 Birth event to an instance of E21 Person in the role of offspring.
Twins, triplets etc. are brought into life by the same instance of E67 Birth. This is not intended for use with general Natural History material, only people. There is no explicit method for modelling conception and gestation except by using extensions.

Examples of the inverse property:
- The Birth of Queen Elizabeth II (E67) brought into life Queen Elizabeth II (E21). (Parker, 2002)

In First Order Logic of the inverse property:
- P98(x,y) ⇒ E67(x)
- P98(x,y) ⇒ E21(y)
- P98(x,y) ⇒ P92(x,y)
</rdfs:comment>
        <rdfs:label xml:lang="fr">P98i est né</rdfs:label>
        <rdfs:label xml:lang="pt">P98i veio à vida pelo</rdfs:label>
        <rdfs:label xml:lang="en">P98i was born</rdfs:label>
        <rdfs:label xml:lang="de">P98i wurde geboren durch</rdfs:label>
        <rdfs:label xml:lang="el">P98i γεννήθηκε</rdfs:label>
        <rdfs:label xml:lang="ru">P98i был рождeн</rdfs:label>
        <rdfs:label xml:lang="zh">P98i 被诞生</rdfs:label>
        <skos:notation xml:lang="en">P98i</skos:notation>
        <skos:prefLabel xml:lang="fr">est né</skos:prefLabel>
        <skos:prefLabel xml:lang="pt">veio à vida pelo</skos:prefLabel>
        <skos:prefLabel xml:lang="en">was born</skos:prefLabel>
        <skos:prefLabel xml:lang="de">wurde geboren durch</skos:prefLabel>
        <skos:prefLabel xml:lang="el">γεννήθηκε</skos:prefLabel>
        <skos:prefLabel xml:lang="ru">был рождeн</skos:prefLabel>
        <skos:prefLabel xml:lang="zh">被诞生</skos:prefLabel>
    </owl:ObjectProperty>
    


    <!-- http://www.w3.org/ns/odrl/2/action -->

    <owl:ObjectProperty rdf:about="http://www.w3.org/ns/odrl/2/action">
        <rdfs:domain>
            <owl:Class>
                <owl:unionOf rdf:parseType="Collection">
                    <rdf:Description rdf:about="http://www.w3.org/ns/odrl/2/Policy"/>
                    <rdf:Description rdf:about="http://www.w3.org/ns/odrl/2/Rule"/>
                </owl:unionOf>
            </owl:Class>
        </rdfs:domain>
        <rdfs:range rdf:resource="http://www.w3.org/ns/odrl/2/Action"/>
    </owl:ObjectProperty>
    


    <!-- http://www.w3.org/ns/odrl/2/and -->

    <owl:ObjectProperty rdf:about="http://www.w3.org/ns/odrl/2/and">
        <rdfs:subPropertyOf rdf:resource="http://www.w3.org/ns/odrl/2/operand"/>
    </owl:ObjectProperty>
    


    <!-- http://www.w3.org/ns/odrl/2/andSequence -->

    <owl:ObjectProperty rdf:about="http://www.w3.org/ns/odrl/2/andSequence">
        <rdfs:subPropertyOf rdf:resource="http://www.w3.org/ns/odrl/2/operand"/>
    </owl:ObjectProperty>
    


    <!-- http://www.w3.org/ns/odrl/2/assignee -->

    <owl:ObjectProperty rdf:about="http://www.w3.org/ns/odrl/2/assignee">
        <rdfs:subPropertyOf rdf:resource="http://www.w3.org/ns/odrl/2/function"/>
        <rdfs:domain>
            <owl:Class>
                <owl:unionOf rdf:parseType="Collection">
                    <rdf:Description rdf:about="http://www.w3.org/ns/odrl/2/Policy"/>
                    <rdf:Description rdf:about="http://www.w3.org/ns/odrl/2/Rule"/>
                </owl:unionOf>
            </owl:Class>
        </rdfs:domain>
        <rdfs:range rdf:resource="http://www.w3.org/ns/odrl/2/Party"/>
    </owl:ObjectProperty>
    


    <!-- http://www.w3.org/ns/odrl/2/assigneeOf -->

    <owl:ObjectProperty rdf:about="http://www.w3.org/ns/odrl/2/assigneeOf">
        <rdfs:domain rdf:resource="http://www.w3.org/ns/odrl/2/Party"/>
        <rdfs:range rdf:resource="http://www.w3.org/ns/odrl/2/Policy"/>
    </owl:ObjectProperty>
    


    <!-- http://www.w3.org/ns/odrl/2/assigner -->

    <owl:ObjectProperty rdf:about="http://www.w3.org/ns/odrl/2/assigner">
        <rdfs:subPropertyOf rdf:resource="http://www.w3.org/ns/odrl/2/function"/>
        <rdfs:domain>
            <owl:Class>
                <owl:unionOf rdf:parseType="Collection">
                    <rdf:Description rdf:about="http://www.w3.org/ns/odrl/2/Policy"/>
                    <rdf:Description rdf:about="http://www.w3.org/ns/odrl/2/Rule"/>
                </owl:unionOf>
            </owl:Class>
        </rdfs:domain>
        <rdfs:range rdf:resource="http://www.w3.org/ns/odrl/2/Party"/>
    </owl:ObjectProperty>
    


    <!-- http://www.w3.org/ns/odrl/2/assignerOf -->

    <owl:ObjectProperty rdf:about="http://www.w3.org/ns/odrl/2/assignerOf">
        <rdfs:domain rdf:resource="http://www.w3.org/ns/odrl/2/Party"/>
        <rdfs:range rdf:resource="http://www.w3.org/ns/odrl/2/Policy"/>
    </owl:ObjectProperty>
    


    <!-- http://www.w3.org/ns/odrl/2/attributedParty -->

    <owl:ObjectProperty rdf:about="http://www.w3.org/ns/odrl/2/attributedParty">
        <rdfs:subPropertyOf rdf:resource="http://www.w3.org/ns/odrl/2/function"/>
    </owl:ObjectProperty>
    


    <!-- http://www.w3.org/ns/odrl/2/attributingParty -->

    <owl:ObjectProperty rdf:about="http://www.w3.org/ns/odrl/2/attributingParty">
        <rdfs:subPropertyOf rdf:resource="http://www.w3.org/ns/odrl/2/function"/>
    </owl:ObjectProperty>
    


    <!-- http://www.w3.org/ns/odrl/2/compensatedParty -->

    <owl:ObjectProperty rdf:about="http://www.w3.org/ns/odrl/2/compensatedParty">
        <rdfs:subPropertyOf rdf:resource="http://www.w3.org/ns/odrl/2/function"/>
    </owl:ObjectProperty>
    


    <!-- http://www.w3.org/ns/odrl/2/compensatingParty -->

    <owl:ObjectProperty rdf:about="http://www.w3.org/ns/odrl/2/compensatingParty">
        <rdfs:subPropertyOf rdf:resource="http://www.w3.org/ns/odrl/2/function"/>
    </owl:ObjectProperty>
    


    <!-- http://www.w3.org/ns/odrl/2/conflict -->

    <owl:ObjectProperty rdf:about="http://www.w3.org/ns/odrl/2/conflict">
        <rdfs:domain rdf:resource="http://www.w3.org/ns/odrl/2/Policy"/>
        <rdfs:range rdf:resource="http://www.w3.org/ns/odrl/2/ConflictTerm"/>
    </owl:ObjectProperty>
    


    <!-- http://www.w3.org/ns/odrl/2/consentedParty -->

    <owl:ObjectProperty rdf:about="http://www.w3.org/ns/odrl/2/consentedParty">
        <rdfs:subPropertyOf rdf:resource="http://www.w3.org/ns/odrl/2/function"/>
    </owl:ObjectProperty>
    


    <!-- http://www.w3.org/ns/odrl/2/consentingParty -->

    <owl:ObjectProperty rdf:about="http://www.w3.org/ns/odrl/2/consentingParty">
        <rdfs:subPropertyOf rdf:resource="http://www.w3.org/ns/odrl/2/function"/>
    </owl:ObjectProperty>
    


    <!-- http://www.w3.org/ns/odrl/2/consequence -->

    <owl:ObjectProperty rdf:about="http://www.w3.org/ns/odrl/2/consequence">
        <rdfs:subPropertyOf rdf:resource="http://www.w3.org/ns/odrl/2/failure"/>
        <rdfs:domain rdf:resource="http://www.w3.org/ns/odrl/2/Duty"/>
        <rdfs:range rdf:resource="http://www.w3.org/ns/odrl/2/Duty"/>
    </owl:ObjectProperty>
    


    <!-- http://www.w3.org/ns/odrl/2/constraint -->

    <owl:ObjectProperty rdf:about="http://www.w3.org/ns/odrl/2/constraint">
        <rdfs:domain>
            <owl:Class>
                <owl:unionOf rdf:parseType="Collection">
                    <rdf:Description rdf:about="http://www.w3.org/ns/odrl/2/Policy"/>
                    <rdf:Description rdf:about="http://www.w3.org/ns/odrl/2/Rule"/>
                </owl:unionOf>
            </owl:Class>
        </rdfs:domain>
        <rdfs:range>
            <owl:Class>
                <owl:unionOf rdf:parseType="Collection">
                    <rdf:Description rdf:about="http://www.w3.org/ns/odrl/2/Constraint"/>
                    <rdf:Description rdf:about="http://www.w3.org/ns/odrl/2/LogicalConstraint"/>
                </owl:unionOf>
            </owl:Class>
        </rdfs:range>
    </owl:ObjectProperty>
    


    <!-- http://www.w3.org/ns/odrl/2/contractedParty -->

    <owl:ObjectProperty rdf:about="http://www.w3.org/ns/odrl/2/contractedParty">
        <rdfs:subPropertyOf rdf:resource="http://www.w3.org/ns/odrl/2/function"/>
    </owl:ObjectProperty>
    


    <!-- http://www.w3.org/ns/odrl/2/contractingParty -->

    <owl:ObjectProperty rdf:about="http://www.w3.org/ns/odrl/2/contractingParty">
        <rdfs:subPropertyOf rdf:resource="http://www.w3.org/ns/odrl/2/function"/>
    </owl:ObjectProperty>
    


    <!-- http://www.w3.org/ns/odrl/2/dataType -->

    <owl:ObjectProperty rdf:about="http://www.w3.org/ns/odrl/2/dataType">
        <rdfs:domain rdf:resource="http://www.w3.org/ns/odrl/2/Constraint"/>
        <rdfs:range rdf:resource="http://www.w3.org/2000/01/rdf-schema#Datatype"/>
    </owl:ObjectProperty>
    


    <!-- http://www.w3.org/ns/odrl/2/duty -->

    <owl:ObjectProperty rdf:about="http://www.w3.org/ns/odrl/2/duty">
        <rdfs:domain rdf:resource="http://www.w3.org/ns/odrl/2/Permission"/>
        <rdfs:range rdf:resource="http://www.w3.org/ns/odrl/2/Duty"/>
    </owl:ObjectProperty>
    


    <!-- http://www.w3.org/ns/odrl/2/failure -->

    <owl:ObjectProperty rdf:about="http://www.w3.org/ns/odrl/2/failure">
        <rdfs:domain rdf:resource="http://www.w3.org/ns/odrl/2/Rule"/>
        <rdfs:range rdf:resource="http://www.w3.org/ns/odrl/2/Rule"/>
    </owl:ObjectProperty>
    


    <!-- http://www.w3.org/ns/odrl/2/function -->

    <owl:ObjectProperty rdf:about="http://www.w3.org/ns/odrl/2/function">
        <rdfs:domain>
            <owl:Class>
                <owl:unionOf rdf:parseType="Collection">
                    <rdf:Description rdf:about="http://www.w3.org/ns/odrl/2/Policy"/>
                    <rdf:Description rdf:about="http://www.w3.org/ns/odrl/2/Rule"/>
                </owl:unionOf>
            </owl:Class>
        </rdfs:domain>
        <rdfs:range rdf:resource="http://www.w3.org/ns/odrl/2/Party"/>
    </owl:ObjectProperty>
    


    <!-- http://www.w3.org/ns/odrl/2/hasPolicy -->

    <owl:ObjectProperty rdf:about="http://www.w3.org/ns/odrl/2/hasPolicy">
        <rdfs:domain rdf:resource="http://www.w3.org/ns/odrl/2/Asset"/>
        <rdfs:range rdf:resource="http://www.w3.org/ns/odrl/2/Policy"/>
    </owl:ObjectProperty>
    


    <!-- http://www.w3.org/ns/odrl/2/implies -->

    <owl:ObjectProperty rdf:about="http://www.w3.org/ns/odrl/2/implies">
        <rdfs:domain rdf:resource="http://www.w3.org/ns/odrl/2/Action"/>
        <rdfs:range rdf:resource="http://www.w3.org/ns/odrl/2/Action"/>
    </owl:ObjectProperty>
    


    <!-- http://www.w3.org/ns/odrl/2/includedIn -->

    <owl:ObjectProperty rdf:about="http://www.w3.org/ns/odrl/2/includedIn">
        <rdf:type rdf:resource="http://www.w3.org/2002/07/owl#TransitiveProperty"/>
        <rdfs:domain rdf:resource="http://www.w3.org/ns/odrl/2/Action"/>
        <rdfs:range rdf:resource="http://www.w3.org/ns/odrl/2/Action"/>
    </owl:ObjectProperty>
    


    <!-- http://www.w3.org/ns/odrl/2/informedParty -->

    <owl:ObjectProperty rdf:about="http://www.w3.org/ns/odrl/2/informedParty">
        <rdfs:subPropertyOf rdf:resource="http://www.w3.org/ns/odrl/2/function"/>
    </owl:ObjectProperty>
    


    <!-- http://www.w3.org/ns/odrl/2/inheritFrom -->

    <owl:ObjectProperty rdf:about="http://www.w3.org/ns/odrl/2/inheritFrom">
        <rdfs:domain rdf:resource="http://www.w3.org/ns/odrl/2/Policy"/>
        <rdfs:range rdf:resource="http://www.w3.org/ns/odrl/2/Policy"/>
    </owl:ObjectProperty>
    


    <!-- http://www.w3.org/ns/odrl/2/leftOperand -->

    <owl:ObjectProperty rdf:about="http://www.w3.org/ns/odrl/2/leftOperand">
        <rdfs:domain rdf:resource="http://www.w3.org/ns/odrl/2/Constraint"/>
        <rdfs:range rdf:resource="http://www.w3.org/ns/odrl/2/LeftOperand"/>
    </owl:ObjectProperty>
    


    <!-- http://www.w3.org/ns/odrl/2/obligation -->

    <owl:ObjectProperty rdf:about="http://www.w3.org/ns/odrl/2/obligation">
        <rdfs:domain rdf:resource="http://www.w3.org/ns/odrl/2/Policy"/>
        <rdfs:range rdf:resource="http://www.w3.org/ns/odrl/2/Duty"/>
    </owl:ObjectProperty>
    


    <!-- http://www.w3.org/ns/odrl/2/operand -->

    <owl:ObjectProperty rdf:about="http://www.w3.org/ns/odrl/2/operand">
        <rdfs:domain rdf:resource="http://www.w3.org/ns/odrl/2/LogicalConstraint"/>
    </owl:ObjectProperty>
    


    <!-- http://www.w3.org/ns/odrl/2/operator -->

    <owl:ObjectProperty rdf:about="http://www.w3.org/ns/odrl/2/operator">
        <rdfs:domain rdf:resource="http://www.w3.org/ns/odrl/2/Constraint"/>
        <rdfs:range rdf:resource="http://www.w3.org/ns/odrl/2/Operator"/>
    </owl:ObjectProperty>
    


    <!-- http://www.w3.org/ns/odrl/2/or -->

    <owl:ObjectProperty rdf:about="http://www.w3.org/ns/odrl/2/or">
        <rdfs:subPropertyOf rdf:resource="http://www.w3.org/ns/odrl/2/operand"/>
    </owl:ObjectProperty>
    


    <!-- http://www.w3.org/ns/odrl/2/output -->

    <owl:ObjectProperty rdf:about="http://www.w3.org/ns/odrl/2/output">
        <rdfs:subPropertyOf rdf:resource="http://www.w3.org/ns/odrl/2/relation"/>
        <rdfs:domain rdf:resource="http://www.w3.org/ns/odrl/2/Rule"/>
        <rdfs:range rdf:resource="http://www.w3.org/ns/odrl/2/Asset"/>
    </owl:ObjectProperty>
    


    <!-- http://www.w3.org/ns/odrl/2/partOf -->

    <owl:ObjectProperty rdf:about="http://www.w3.org/ns/odrl/2/partOf">
        <rdfs:domain>
            <owl:Class>
                <owl:unionOf rdf:parseType="Collection">
                    <rdf:Description rdf:about="http://www.w3.org/ns/odrl/2/Asset"/>
                    <rdf:Description rdf:about="http://www.w3.org/ns/odrl/2/Party"/>
                </owl:unionOf>
            </owl:Class>
        </rdfs:domain>
        <rdfs:range>
            <owl:Class>
                <owl:unionOf rdf:parseType="Collection">
                    <rdf:Description rdf:about="http://www.w3.org/ns/odrl/2/AssetCollection"/>
                    <rdf:Description rdf:about="http://www.w3.org/ns/odrl/2/PartyCollection"/>
                </owl:unionOf>
            </owl:Class>
        </rdfs:range>
    </owl:ObjectProperty>
    


    <!-- http://www.w3.org/ns/odrl/2/permission -->

    <owl:ObjectProperty rdf:about="http://www.w3.org/ns/odrl/2/permission">
        <rdfs:domain rdf:resource="http://www.w3.org/ns/odrl/2/Policy"/>
        <rdfs:range rdf:resource="http://www.w3.org/ns/odrl/2/Permission"/>
    </owl:ObjectProperty>
    


    <!-- http://www.w3.org/ns/odrl/2/prohibition -->

    <owl:ObjectProperty rdf:about="http://www.w3.org/ns/odrl/2/prohibition">
        <rdfs:domain rdf:resource="http://www.w3.org/ns/odrl/2/Policy"/>
        <rdfs:range rdf:resource="http://www.w3.org/ns/odrl/2/Prohibition"/>
    </owl:ObjectProperty>
    


    <!-- http://www.w3.org/ns/odrl/2/refinement -->

    <owl:ObjectProperty rdf:about="http://www.w3.org/ns/odrl/2/refinement">
        <rdfs:domain>
            <owl:Class>
                <owl:unionOf rdf:parseType="Collection">
                    <rdf:Description rdf:about="http://www.w3.org/ns/odrl/2/Action"/>
                    <rdf:Description rdf:about="http://www.w3.org/ns/odrl/2/AssetCollection"/>
                    <rdf:Description rdf:about="http://www.w3.org/ns/odrl/2/PartyCollection"/>
                </owl:unionOf>
            </owl:Class>
        </rdfs:domain>
        <rdfs:range>
            <owl:Class>
                <owl:unionOf rdf:parseType="Collection">
                    <rdf:Description rdf:about="http://www.w3.org/ns/odrl/2/Constraint"/>
                    <rdf:Description rdf:about="http://www.w3.org/ns/odrl/2/LogicalConstraint"/>
                </owl:unionOf>
            </owl:Class>
        </rdfs:range>
    </owl:ObjectProperty>
    


    <!-- http://www.w3.org/ns/odrl/2/relation -->

    <owl:ObjectProperty rdf:about="http://www.w3.org/ns/odrl/2/relation">
        <rdfs:domain>
            <owl:Class>
                <owl:unionOf rdf:parseType="Collection">
                    <rdf:Description rdf:about="http://www.w3.org/ns/odrl/2/Policy"/>
                    <rdf:Description rdf:about="http://www.w3.org/ns/odrl/2/Rule"/>
                </owl:unionOf>
            </owl:Class>
        </rdfs:domain>
        <rdfs:range rdf:resource="http://www.w3.org/ns/odrl/2/Asset"/>
    </owl:ObjectProperty>
    


    <!-- http://www.w3.org/ns/odrl/2/remedy -->

    <owl:ObjectProperty rdf:about="http://www.w3.org/ns/odrl/2/remedy">
        <rdfs:subPropertyOf rdf:resource="http://www.w3.org/ns/odrl/2/failure"/>
        <rdfs:domain rdf:resource="http://www.w3.org/ns/odrl/2/Prohibition"/>
        <rdfs:range rdf:resource="http://www.w3.org/ns/odrl/2/Duty"/>
    </owl:ObjectProperty>
    


    <!-- http://www.w3.org/ns/odrl/2/rightOperand -->

    <owl:ObjectProperty rdf:about="http://www.w3.org/ns/odrl/2/rightOperand">
        <rdfs:domain rdf:resource="http://www.w3.org/ns/odrl/2/Constraint"/>
        <rdfs:range>
            <owl:Class>
                <owl:unionOf rdf:parseType="Collection">
                    <rdf:Description rdf:about="http://www.w3.org/2000/01/rdf-schema#Literal"/>
                    <rdf:Description rdf:about="http://www.w3.org/2001/XMLSchema#anyURI"/>
                    <rdf:Description rdf:about="http://www.w3.org/ns/odrl/2/RightOperand"/>
                </owl:unionOf>
            </owl:Class>
        </rdfs:range>
    </owl:ObjectProperty>
    


    <!-- http://www.w3.org/ns/odrl/2/target -->

    <owl:ObjectProperty rdf:about="http://www.w3.org/ns/odrl/2/target">
        <rdfs:subPropertyOf rdf:resource="http://www.w3.org/ns/odrl/2/relation"/>
        <rdfs:domain>
            <owl:Class>
                <owl:unionOf rdf:parseType="Collection">
                    <rdf:Description rdf:about="http://www.w3.org/ns/odrl/2/Policy"/>
                    <rdf:Description rdf:about="http://www.w3.org/ns/odrl/2/Rule"/>
                </owl:unionOf>
            </owl:Class>
        </rdfs:domain>
        <rdfs:range rdf:resource="http://www.w3.org/ns/odrl/2/Asset"/>
    </owl:ObjectProperty>
    


    <!-- http://www.w3.org/ns/odrl/2/trackedParty -->

    <owl:ObjectProperty rdf:about="http://www.w3.org/ns/odrl/2/trackedParty">
        <rdfs:subPropertyOf rdf:resource="http://www.w3.org/ns/odrl/2/function"/>
    </owl:ObjectProperty>
    


    <!-- http://www.w3.org/ns/odrl/2/trackingParty -->

    <owl:ObjectProperty rdf:about="http://www.w3.org/ns/odrl/2/trackingParty">
        <rdfs:subPropertyOf rdf:resource="http://www.w3.org/ns/odrl/2/function"/>
    </owl:ObjectProperty>
    


    <!-- http://www.w3.org/ns/odrl/2/xone -->

    <owl:ObjectProperty rdf:about="http://www.w3.org/ns/odrl/2/xone">
        <rdfs:subPropertyOf rdf:resource="http://www.w3.org/ns/odrl/2/operand"/>
    </owl:ObjectProperty>
    


    <!-- https://schema.org/description -->

    <owl:ObjectProperty rdf:about="https://schema.org/description">
        <rdfs:domain rdf:resource="https://schema.org/Thing"/>
        <rdfs:range>
            <owl:Class>
                <owl:unionOf rdf:parseType="Collection">
                    <rdf:Description rdf:about="https://schema.org/Role"/>
                    <rdf:Description rdf:about="https://schema.org/Text"/>
                    <rdf:Description rdf:about="https://schema.org/TextObject"/>
                    <rdf:Description rdf:about="https://schema.org/URL"/>
                </owl:unionOf>
            </owl:Class>
        </rdfs:range>
        <rdfs:comment xml:lang="en">A description of the item.</rdfs:comment>
        <rdfs:isDefinedBy rdf:resource="https://schema.org/description"/>
        <rdfs:label xml:lang="en">description</rdfs:label>
    </owl:ObjectProperty>
    


    <!-- https://schema.org/nationality -->

    <owl:ObjectProperty rdf:about="https://schema.org/nationality">
        <rdfs:domain rdf:resource="https://schema.org/Person"/>
        <rdfs:range>
            <owl:Class>
                <owl:unionOf rdf:parseType="Collection">
                    <rdf:Description rdf:about="https://schema.org/Country"/>
                    <rdf:Description rdf:about="https://schema.org/Role"/>
                    <rdf:Description rdf:about="https://schema.org/Text"/>
                    <rdf:Description rdf:about="https://schema.org/URL"/>
                </owl:unionOf>
            </owl:Class>
        </rdfs:range>
        <rdfs:comment xml:lang="en">Nationality of the person.</rdfs:comment>
        <rdfs:isDefinedBy rdf:resource="https://schema.org/nationality"/>
        <rdfs:label xml:lang="en">nationality</rdfs:label>
    </owl:ObjectProperty>
    


    <!-- https://schema.org/supersededBy -->

    <owl:ObjectProperty rdf:about="https://schema.org/supersededBy">
        <rdfs:domain>
            <owl:Class>
                <owl:unionOf rdf:parseType="Collection">
                    <rdf:Description rdf:about="https://schema.org/Class"/>
                    <rdf:Description rdf:about="https://schema.org/Enumeration"/>
                    <rdf:Description rdf:about="https://schema.org/Property"/>
                </owl:unionOf>
            </owl:Class>
        </rdfs:domain>
        <rdfs:range>
            <owl:Class>
                <owl:unionOf rdf:parseType="Collection">
                    <rdf:Description rdf:about="https://schema.org/Class"/>
                    <rdf:Description rdf:about="https://schema.org/Enumeration"/>
                    <rdf:Description rdf:about="https://schema.org/Property"/>
                    <rdf:Description rdf:about="https://schema.org/Role"/>
                    <rdf:Description rdf:about="https://schema.org/Text"/>
                    <rdf:Description rdf:about="https://schema.org/URL"/>
                </owl:unionOf>
            </owl:Class>
        </rdfs:range>
        <rdfs:comment xml:lang="en">Relates a term (i.e. a property, class or enumeration) to one that supersedes it.</rdfs:comment>
        <rdfs:isDefinedBy rdf:resource="https://meta.schema.org/supersededBy"/>
        <rdfs:label xml:lang="en">supersededBy</rdfs:label>
    </owl:ObjectProperty>
    


    <!-- 
    ///////////////////////////////////////////////////////////////////////////////////////
    //
    // Data properties
    //
    ///////////////////////////////////////////////////////////////////////////////////////
     -->

    


    <!-- http://www.cidoc-crm.org/cidoc-crm/P190_has_symbolic_content -->

    <owl:DatatypeProperty rdf:about="http://www.cidoc-crm.org/cidoc-crm/P190_has_symbolic_content">
        <rdfs:subPropertyOf rdf:resource="http://www.cidoc-crm.org/cidoc-crm/P3_has_note"/>
        <rdfs:domain rdf:resource="http://www.cidoc-crm.org/cidoc-crm/E90_Symbolic_Object"/>
        <rdfs:comment xml:lang="en">Quantification: many to many (0,n:0,n)

Scope note:
This property associates an instance of E90 Symbolic Object with a complete, identifying representation of its content in the form of an instance of E62 String. 
This property only applies to instances of E90 Symbolic Object that can be represented completely in this form. The representation may be more specific than the symbolic level defining the identity condition of the represented. This depends on the type of the symbolic object represented. For instance, if a name has type “Modern Greek character sequence”, it may be represented in a loss-free Latin transcription, meaning however the sequence of Greek letters. 
As another example, if the represented object has type “English words sequence”, American English or British English spelling variants may be chosen to represent the English word “colour” without defining a different symbolic object. If a name has type “European traditional name”, no particular string may define its content.

Examples:
- The materials description of the painting (E33) has symbolic content “Oil, French Watercolors on Paper, Graphite and Ink on Canvas, with an Oak frame.” (E62).
- The title of Einstein’s 1915 text (E35) has symbolic content “Relativity, the Special and the General Theory” (E62). (Einstein, 2001)
- The story of Little Red Riding Hood (E33) has symbolic content “Once upon a time there lived in a certain village.” (E62). (Lang, 1965)
- The inscription on Rijksmuseum object SK-A-1601 (E34) has symbolic content “B” (E62). [reference: https://www.rijksmuseum.nl/en/collection/SK-A-1601/catalogue-entry (accessed 10(th) April 2021)]

In First Order Logic:
- P190(x,y) ⇒ E90(x)
- P190(x,y) ⇒ E62(y)
</rdfs:comment>
        <rdfs:label xml:lang="fr">P190 a pour contenu symbolique</rdfs:label>
        <rdfs:label xml:lang="en">P190 has symbolic content</rdfs:label>
        <rdfs:label xml:lang="ru">P190 имeeт символичeскоe содeржаниe</rdfs:label>
        <skos:notation xml:lang="en">P190</skos:notation>
        <skos:prefLabel xml:lang="fr">a pour contenu symbolique</skos:prefLabel>
        <skos:prefLabel xml:lang="en">has symbolic content</skos:prefLabel>
        <skos:prefLabel xml:lang="ru">имeeт символичeскоe содeржаниe</skos:prefLabel>
    </owl:DatatypeProperty>
    


    <!-- http://www.cidoc-crm.org/cidoc-crm/P3_has_note -->

    <owl:DatatypeProperty rdf:about="http://www.cidoc-crm.org/cidoc-crm/P3_has_note">
        <rdfs:domain rdf:resource="http://www.cidoc-crm.org/cidoc-crm/E1_CRM_Entity"/>
        <rdfs:comment xml:lang="en">Quantification: one to many (0,n:0,1)

Scope note:
This property is a container for all informal descriptions about an object that have not been expressed in terms of CIDOC CRM constructs. 
In particular, it captures the characterisation of the item itself, its internal structures, appearance, etc.
Like property P2 has type (is type of), this property is a consequence of the restricted focus of the CIDOC CRM. The aim is not to capture, in a structured form, everything that can be said about an item; indeed, the CIDOC CRM formalism is not regarded as sufficient to express everything that can be said. Good practice requires use of distinct note fields for different aspects of a characterisation. The P3.1 has type property of P3 has note allows differentiation of specific notes, e.g. “construction”, “decoration”, etc. 
An item may have many notes, but a note is attached to a specific item.

Examples:
- Coffee mug – OXCMS:1983.1.1 (E19) has note “chipped at edge of handle” (E62) has type Condition (E55). (fictitious)

Properties:
- P3.1 has type: E55 Type

In First Order Logic:
- P3(x,y) ⇒ E1(x)
- P3(x,y) ⇒ E62(y) 
- P3(x,y,z) ⇒ [P3(x,y) ∧ E55(z)]
</rdfs:comment>
        <rdfs:label xml:lang="fr">P3 a pour note</rdfs:label>
        <rdfs:label xml:lang="en">P3 has note</rdfs:label>
        <rdfs:label xml:lang="de">P3 hat Anmerkung</rdfs:label>
        <rdfs:label xml:lang="pt">P3 tem nota</rdfs:label>
        <rdfs:label xml:lang="el">P3 έχει επεξήγηση</rdfs:label>
        <rdfs:label xml:lang="ru">P3 имeeт примeчаниe</rdfs:label>
        <rdfs:label xml:lang="zh">P3 有注释</rdfs:label>
        <skos:notation xml:lang="en">P3</skos:notation>
        <skos:prefLabel xml:lang="fr">a pour note</skos:prefLabel>
        <skos:prefLabel xml:lang="en">has note</skos:prefLabel>
        <skos:prefLabel xml:lang="de">hat Anmerkung</skos:prefLabel>
        <skos:prefLabel xml:lang="pt">tem nota</skos:prefLabel>
        <skos:prefLabel xml:lang="el">έχει επεξήγηση</skos:prefLabel>
        <skos:prefLabel xml:lang="ru">имeeт примeчаниe</skos:prefLabel>
        <skos:prefLabel xml:lang="zh">有注释</skos:prefLabel>
    </owl:DatatypeProperty>
    


    <!-- http://www.cidoc-crm.org/cidoc-crm/P79_beginning_is_qualified_by -->

    <owl:DatatypeProperty rdf:about="http://www.cidoc-crm.org/cidoc-crm/P79_beginning_is_qualified_by">
        <rdfs:subPropertyOf rdf:resource="http://www.cidoc-crm.org/cidoc-crm/P3_has_note"/>
        <rdfs:domain rdf:resource="http://www.cidoc-crm.org/cidoc-crm/E52_Time-Span"/>
        <rdfs:comment xml:lang="en">Quantification: many to one (0,1:0,n)

Scope note:
This property associates an instance of E52 Time-Span with a note detailing the scholarly or scientific opinions and justifications about the certainty, precision, sources etc. of its beginning. Such notes may also be used to elaborate arguments about constraints or to give explanations of alternatives.

Examples:
- The time-span of the Holocene (E52) beginning is qualified by “The formal definition and dating of the GSSP (GlobalStratotype Section and Point) for the base of the Holocene using the Greenland NGRIP ice core, and selected auxiliary records” (E62). (Walker et al., 2009)

In First Order Logic:
- P79(x,y) ⇒ E52(x)
- P79(x,y) ⇒ E62(y) 
- P79(x,y) ⇒ P3(x,y)
</rdfs:comment>
        <rdfs:label xml:lang="fr">P79 a son début qualifié par</rdfs:label>
        <rdfs:label xml:lang="en">P79 beginning is qualified by</rdfs:label>
        <rdfs:label xml:lang="de">P79 hat Anfangsbegründung</rdfs:label>
        <rdfs:label xml:lang="pt">P79 início é qualificado por</rdfs:label>
        <rdfs:label xml:lang="el">P79 αρχή προσδιορίζεται από</rdfs:label>
        <rdfs:label xml:lang="ru">P79 начало ограничeно</rdfs:label>
        <rdfs:label xml:lang="zh">P79 起始限定</rdfs:label>
        <skos:notation xml:lang="en">P79</skos:notation>
        <skos:prefLabel xml:lang="fr">a son début qualifié par</skos:prefLabel>
        <skos:prefLabel xml:lang="en">beginning is qualified by</skos:prefLabel>
        <skos:prefLabel xml:lang="de">hat Anfangsbegründung</skos:prefLabel>
        <skos:prefLabel xml:lang="pt">início é qualificado por</skos:prefLabel>
        <skos:prefLabel xml:lang="el">αρχή προσδιορίζεται από</skos:prefLabel>
        <skos:prefLabel xml:lang="ru">начало ограничeно</skos:prefLabel>
        <skos:prefLabel xml:lang="zh">起始限定</skos:prefLabel>
    </owl:DatatypeProperty>
    


    <!-- http://www.cidoc-crm.org/cidoc-crm/P80_end_is_qualified_by -->

    <owl:DatatypeProperty rdf:about="http://www.cidoc-crm.org/cidoc-crm/P80_end_is_qualified_by">
        <rdfs:subPropertyOf rdf:resource="http://www.cidoc-crm.org/cidoc-crm/P3_has_note"/>
        <rdfs:domain rdf:resource="http://www.cidoc-crm.org/cidoc-crm/E52_Time-Span"/>
        <rdfs:comment xml:lang="en">Quantification: many to one (0,1:0,n)

Scope note:
This property associates an instance of E52 Time-Span with a note detailing the scholarly or scientific opinions and justifications about the end of this time-span concerning certainty, precision, sources etc. This property may also be used to describe arguments constraining possible dates and to distinguish reasons for alternative dates.

Examples:
- The time-span of the Holocene (E52) end is qualified by “still ongoing” (E62). (Walker et al., 2009)

In First Order Logic:
- P80(x,y) ⇒ E52(x) 
- P80(x,y) ⇒ E62(y) 
- P80(x,y) ⇒ P3(x,y)
</rdfs:comment>
        <rdfs:label xml:lang="fr">P80 a sa fin qualifiée par</rdfs:label>
        <rdfs:label xml:lang="en">P80 end is qualified by</rdfs:label>
        <rdfs:label xml:lang="pt">P80 final é qualificado por</rdfs:label>
        <rdfs:label xml:lang="de">P80 hat Begründung des Endes</rdfs:label>
        <rdfs:label xml:lang="el">P80 τέλος προσδιορίζεται από</rdfs:label>
        <rdfs:label xml:lang="ru">P80 конeц ограничeн</rdfs:label>
        <rdfs:label xml:lang="zh">P80 结束限定</rdfs:label>
        <skos:notation xml:lang="en">P80</skos:notation>
        <skos:prefLabel xml:lang="fr">a sa fin qualifiée par</skos:prefLabel>
        <skos:prefLabel xml:lang="en">end is qualified by</skos:prefLabel>
        <skos:prefLabel xml:lang="pt">final é qualificado por</skos:prefLabel>
        <skos:prefLabel xml:lang="de">hat Begründung des Endes</skos:prefLabel>
        <skos:prefLabel xml:lang="el">τέλος προσδιορίζεται από</skos:prefLabel>
        <skos:prefLabel xml:lang="ru">конeц ограничeн</skos:prefLabel>
        <skos:prefLabel xml:lang="zh">结束限定</skos:prefLabel>
    </owl:DatatypeProperty>
    


    <!-- http://www.cidoc-crm.org/cidoc-crm/P90_has_value -->

    <owl:DatatypeProperty rdf:about="http://www.cidoc-crm.org/cidoc-crm/P90_has_value">
        <rdfs:domain rdf:resource="http://www.cidoc-crm.org/cidoc-crm/E54_Dimension"/>
        <rdfs:comment xml:lang="en">Quantification: many to one, necessary (1,1:0,n)

Scope note:
This property allows an instance of E54 Dimension to be approximated by an instance of E60 Number primitive.

Examples:
- The height of silver cup 232 (E54) has value 226 (E60). (fictitious)
- Christie’s hammer price for Vincent van Gogh’s “Still Life: Vase with Fifteen Sunflowers” in London on 30(th) March 1987 (E97) has value 24,750,000 (E60).

In First Order Logic:
- P90(x,y) ⇒ E54(x)
- P90(x,y) ⇒ E60(y)
</rdfs:comment>
        <rdfs:label xml:lang="fr">P90 a pour valeur</rdfs:label>
        <rdfs:label xml:lang="en">P90 has value</rdfs:label>
        <rdfs:label xml:lang="de">P90 hat Wert</rdfs:label>
        <rdfs:label xml:lang="pt">P90 tem valor</rdfs:label>
        <rdfs:label xml:lang="el">P90 έχει τιμή</rdfs:label>
        <rdfs:label xml:lang="ru">P90 имeeт значeниe</rdfs:label>
        <rdfs:label xml:lang="zh">P90 有数值</rdfs:label>
        <skos:notation xml:lang="en">P90</skos:notation>
        <skos:prefLabel xml:lang="fr">a pour valeur</skos:prefLabel>
        <skos:prefLabel xml:lang="en">has value</skos:prefLabel>
        <skos:prefLabel xml:lang="de">hat Wert</skos:prefLabel>
        <skos:prefLabel xml:lang="pt">tem valor</skos:prefLabel>
        <skos:prefLabel xml:lang="el">έχει τιμή</skos:prefLabel>
        <skos:prefLabel xml:lang="ru">имeeт значeниe</skos:prefLabel>
        <skos:prefLabel xml:lang="zh">有数值</skos:prefLabel>
    </owl:DatatypeProperty>
    


    <!-- http://www.w3.org/ns/odrl/2/rightOperand -->

    <owl:DatatypeProperty rdf:about="http://www.w3.org/ns/odrl/2/rightOperand"/>
    


    <!-- 
    ///////////////////////////////////////////////////////////////////////////////////////
    //
    // Classes
    //
    ///////////////////////////////////////////////////////////////////////////////////////
     -->

    


    <!-- http://schema.org/Action -->

    <owl:Class rdf:about="http://schema.org/Action"/>
    


    <!-- http://schema.org/Organization -->

    <owl:Class rdf:about="http://schema.org/Organization"/>
    


    <!-- http://schema.org/Person -->

    <owl:Class rdf:about="http://schema.org/Person"/>
    


    <!-- http://w3id.org/cacao/CACAO_0000002 -->

    <owl:Class rdf:about="http://w3id.org/cacao/CACAO_0000002">
        <rdfs:subClassOf rdf:resource="http://www.cidoc-crm.org/cidoc-crm/E39_Actor"/>
        <rdfs:subClassOf rdf:resource="http://www.w3.org/ns/odrl/2/Party"/>
        <dcterms:contributor rdf:resource="https://orcid.org/0000-0002-0905-7033"/>
        <dcterms:date rdf:datatype="http://www.w3.org/2001/XMLSchema#dateTime">2024-11-13T16:18:33Z</dcterms:date>
        <rdfs:comment xml:lang="en">Scope note:
This class comprises agents, whether human individuals, groups, or non-human entities such as software applications, algorithms, or automated processes, that interact with digital systems or services by initiating actions, consuming resources, or producing outputs. Users are characterized by their capacity to perform intentional actions within a digital environment, for which they can be held responsible.​

Unlike E21 Person, which is limited to real or assumed human individuals, the class User encompasses a broader range of agents, including non-human actors that operate autonomously or semi-autonomously within digital contexts. This includes, but is not limited to, artificial intelligence models, automated scripts, and other algorithmic entities that engage with web services or digital platforms.​

The classification of an entity as a User does not necessitate legal personhood or consciousness; rather, it is based on the entity&apos;s functional role in interacting with digital systems in a manner that can be documented and attributed.​

Examples:
- A registered individual accessing an online museum catalog.​
- An AI-driven recommendation engine suggesting artifacts to users.​
- A software bot performing automated data curation tasks.​</rdfs:comment>
        <rdfs:label xml:lang="en">User</rdfs:label>
    </owl:Class>
    


    <!-- http://w3id.org/cacao/CACAO_0000003 -->

    <owl:Class rdf:about="http://w3id.org/cacao/CACAO_0000003">
        <rdfs:subClassOf rdf:resource="http://www.cidoc-crm.org/cidoc-crm/E73_Information_Object"/>
        <dcterms:contributor rdf:resource="https://orcid.org/0000-0002-0905-7033"/>
        <dcterms:date rdf:datatype="http://www.w3.org/2001/XMLSchema#dateTime">2024-11-13T16:20:05Z</dcterms:date>
        <rdfs:comment xml:lang="en">Scope note:
This class comprises identifiable immaterial items, such as digital images, texts, multimedia objects, computer program code, algorithms, or mathematical formulae, that are created, modified, or stored in digital formats. Digital Artefacts have an objectively recognizable structure and are documented as single units. They exist independently of specific physical carriers and can reside on multiple digital mediums simultaneously. While E73 Information Objects encompass a broad range of immaterial items, including those stored in human memory or on physical media, Digital Artefacts are specifically associated with digital technologies. This subclassification aids in distinguishing between general information entities and those uniquely tied to digital environments.​

Examples:
- A digital photograph of an ancient manuscript.​
- A 3D model of an archaeological excavation site.​
- The source code of a software application developed to catalog museum collections.​
- A dataset containing measurements of physical artefacts.</rdfs:comment>
        <rdfs:label xml:lang="en">Digital Artefact</rdfs:label>
    </owl:Class>
    


    <!-- http://w3id.org/cacao/CACAO_0000005 -->

    <owl:Class rdf:about="http://w3id.org/cacao/CACAO_0000005">
        <rdfs:subClassOf rdf:resource="http://www.cidoc-crm.org/cidoc-crm/E5_Event"/>
        <dcterms:contributor rdf:resource="https://orcid.org/0000-0002-0905-7033"/>
        <dcterms:date rdf:datatype="http://www.w3.org/2001/XMLSchema#dateTime">2024-11-19T12:02:07Z</dcterms:date>
        <dcterms:description>A specialized version of E5_Event, where we only refer to events with historical value. Historical value reflects the role that the heritage item has played in a broader historical narrative, offering insights into cultural, political, social, or technological contexts of specific periods.</dcterms:description>
        <rdfs:label xml:lang="en">Historical Event</rdfs:label>
    </owl:Class>
    


    <!-- http://w3id.org/cacao/CACAO_0000010 -->

    <owl:Class rdf:about="http://w3id.org/cacao/CACAO_0000010">
        <rdfs:subClassOf rdf:resource="http://www.cidoc-crm.org/cidoc-crm/E55_Type"/>
        <dcterms:contributor rdf:resource="https://orcid.org/0000-0002-0905-7033"/>
        <dcterms:date rdf:datatype="http://www.w3.org/2001/XMLSchema#dateTime">2024-11-19T12:50:33Z</dcterms:date>
        <dcterms:description>From wikidata (Q49773): loosely organized effort by a large group of people to achieve a particular set of goals</dcterms:description>
        <rdfs:comment xml:lang="en">From wikidata (Q49773): loosely organized effort by a large group of people to achieve a particular set of goals

Scope note:
A Social Movement is a loosely organized effort by a large group of people to achieve a particular set of goals, typically aiming to promote or resist changes in society&apos;s structure or values. These movements are characterized by collective action, where individuals unite based on shared beliefs or objectives, often seeking social, political, economic, or cultural transformations. ​

Social movements differ from formal organizations in that they may lack a defined organizational structure or formal membership, relying instead on informal networks and shared commitments. They can vary widely in size and scope, ranging from localized grassroots initiatives to large-scale national or international campaigns. The methods employed can include protests, demonstrations, advocacy, and other forms of collective action aimed at influencing public opinion and policy. ​

Examples:
- The Civil Rights Movement in the United States,
- The Environmental Movement
- The Feminist Movement,
- The LGBTQ+ Rights Movement</rdfs:comment>
        <rdfs:label xml:lang="en">Social movement</rdfs:label>
    </owl:Class>
    


    <!-- http://w3id.org/cacao/CACAO_0000011 -->

    <owl:Class rdf:about="http://w3id.org/cacao/CACAO_0000011">
        <rdfs:subClassOf rdf:resource="http://w3id.org/cacao/CACAO_0000010"/>
        <dcterms:contributor rdf:resource="https://orcid.org/0000-0002-0905-7033"/>
        <dcterms:date rdf:datatype="http://www.w3.org/2001/XMLSchema#dateTime">2024-11-19T12:51:24Z</dcterms:date>
        <dcterms:description>Wikidata: Q1826286, social and ideological movement in the religious sphere</dcterms:description>
        <rdfs:comment xml:lang="en">Wikidata: Q1826286, social and ideological movement in the religious sphere

Scope note:
A Religious Movement is a collective effort by a group of people aiming to promote, reform, or resist changes within religious beliefs, practices, or institutions.

Examples:
- The Protestant Reformation in the 16th century, which led to significant changes in Christian practices and beliefs.​
- The Charismatic Movement, emphasizing direct personal experience of God through baptism with the Holy Spirit.​
- The New Age Movement, a broad range of spiritual or religious beliefs and practices that developed in the Western world during the 1970s.</rdfs:comment>
        <rdfs:label xml:lang="en">Religious movement</rdfs:label>
    </owl:Class>
    


    <!-- http://w3id.org/cacao/CACAO_0000012 -->

    <owl:Class rdf:about="http://w3id.org/cacao/CACAO_0000012">
        <rdfs:subClassOf rdf:resource="http://w3id.org/cacao/CACAO_0000010"/>
        <dcterms:contributor rdf:resource="https://orcid.org/0000-0002-0905-7033"/>
        <dcterms:date rdf:datatype="http://www.w3.org/2001/XMLSchema#dateTime">2024-11-19T12:51:32Z</dcterms:date>
        <dcterms:description>Wikidata: Q2198855, period and movement in cultural history</dcterms:description>
        <rdfs:comment xml:lang="en">Wikidata: Q2198855, period and movement in cultural history

Scope note:
A Cultural Movement is a collective effort by loosely affiliated individuals aiming to transform societal perspectives through the dissemination of ideas via various art forms and intentional lifestyle choices. These movements often overlap with social and political movements, making them integral to broader cultural transformations. ​

Examples:
- The Renaissance
- The Romanticism movement
- The Alté Movement in Nigeria</rdfs:comment>
        <rdfs:label xml:lang="en">Cultural movement</rdfs:label>
    </owl:Class>
    


    <!-- http://w3id.org/cacao/CACAO_0000013 -->

    <owl:Class rdf:about="http://w3id.org/cacao/CACAO_0000013">
        <rdfs:subClassOf rdf:resource="http://w3id.org/cacao/CACAO_0000010"/>
        <dcterms:contributor rdf:resource="https://orcid.org/0000-0002-0905-7033"/>
        <dcterms:date rdf:datatype="http://www.w3.org/2001/XMLSchema#dateTime">2024-11-19T12:51:42Z</dcterms:date>
        <dcterms:description>Wikidata: Q2738074, movement to obtain a political goal</dcterms:description>
        <rdfs:comment>Wikidata: Q2738074, movement to obtain a political goal

Scope note:
A Political Movement is a collective effort by a group of people aiming to influence government policy, social values, or achieve specific political objectives. These movements are typically organized around particular issues or ideologies and seek to bring about change within the political system. They differ from political parties, which aim to gain political office, by focusing on specific goals rather than seeking electoral power. ​

Examples:
- The Anti-Apartheid Movement, which campaigned against the system of racial segregation in South Africa.​
- The Tea Party Movement in the United States, advocating for reduced government spending and taxation.​
- The Brexit Movement, which sought the United Kingdom&apos;s withdrawal from the European Union.</rdfs:comment>
        <rdfs:label xml:lang="en">Political movement</rdfs:label>
    </owl:Class>
    


    <!-- http://w3id.org/cacao/CACAO_0000014 -->

    <owl:Class rdf:about="http://w3id.org/cacao/CACAO_0000014">
        <rdfs:subClassOf rdf:resource="http://www.cidoc-crm.org/cidoc-crm/E55_Type"/>
        <dcterms:contributor rdf:resource="https://orcid.org/0000-0002-0905-7033"/>
        <dcterms:date rdf:datatype="http://www.w3.org/2001/XMLSchema#dateTime">2024-12-06T13:27:25Z</dcterms:date>
        <rdfs:comment xml:lang="en">Scope note:
This class comprises categories or fields of specialized knowledge, disciplines, or areas of expertise that are used to classify and contextualize instances of CIDOC CRM classes. Instances of Domain represent specific spheres of human thought or activity, providing a framework for understanding the context, provenance, or thematic classification of cultural heritage information.​

The Domain class serves as a means to associate cultural heritage entities with particular areas of study or professional practice, facilitating interdisciplinary research and knowledge organization. For example, associating an artifact with the domain of &quot;archaeology&quot; or &quot;art history&quot; helps in understanding its scholarly context and the methodologies applied to its study.​

Examples:
- Archaeology​
- Art History​
- Ethnomusicology​
- Conservation Science</rdfs:comment>
        <rdfs:label xml:lang="en">Domain</rdfs:label>
    </owl:Class>
    


    <!-- http://w3id.org/cacao/CACAO_0000015 -->

    <owl:Class rdf:about="http://w3id.org/cacao/CACAO_0000015">
        <rdfs:subClassOf rdf:resource="http://www.cidoc-crm.org/cidoc-crm/E55_Type"/>
        <dcterms:contributor rdf:resource="https://orcid.org/0000-0002-0905-7033"/>
        <dcterms:date rdf:datatype="http://www.w3.org/2001/XMLSchema#dateTime">2024-12-06T13:30:25Z</dcterms:date>
        <rdfs:comment xml:lang="en">Scope note:
Economic Relevance pertains to concepts that define the economic significance or impact of entities, events, or activities. This class encompasses terms and categories used to classify and assess the economic aspects of cultural heritage items, historical events, or societal practices.

Examples:
- The economic impact of the Silk Road trade routes on participating civilizations.​
- The assessment of a museum&apos;s collection in terms of its monetary value and contribution to tourism revenue.​
- Analysis of the financial significance of a historical event, such as the Industrial Revolution, on global markets.</rdfs:comment>
        <rdfs:label xml:lang="en">Economic Relevance</rdfs:label>
    </owl:Class>
    


    <!-- http://w3id.org/cacao/CACAO_0000016 -->

    <owl:Class rdf:about="http://w3id.org/cacao/CACAO_0000016">
        <rdfs:subClassOf rdf:resource="http://www.cidoc-crm.org/cidoc-crm/E55_Type"/>
        <dcterms:contributor rdf:resource="https://orcid.org/0000-0002-0905-7033"/>
        <dcterms:date rdf:datatype="http://www.w3.org/2001/XMLSchema#dateTime">2024-12-06T13:43:53Z</dcterms:date>
        <rdfs:label xml:lang="en">Symbolism</rdfs:label>
    </owl:Class>
    


    <!-- http://w3id.org/cacao/CACAO_0000020 -->

    <owl:Class rdf:about="http://w3id.org/cacao/CACAO_0000020">
        <rdfs:subClassOf rdf:resource="http://www.cidoc-crm.org/cidoc-crm/E74_Group"/>
        <dcterms:contributor rdf:resource="https://orcid.org/0000-0002-0905-7033"/>
        <dcterms:date rdf:datatype="http://www.w3.org/2001/XMLSchema#dateTime">2025-04-11T08:31:05Z</dcterms:date>
        <rdfs:comment xml:lang="en">Scope note:
This class comprises organizations that are established to collect, preserve, research, interpret, and exhibit tangible and intangible cultural heritage for the purposes of education, study, and enjoyment. Museums operate as collective entities, often encompassing various departments and professionals, and may be public or private institutions.​

As instances of E74 Group, museums are characterized by their organizational structure and collective actions aimed at the stewardship of cultural artifacts and information. They may also engage in activities such as publishing, educational programming, and community outreach.​

Museums can vary widely in scope and specialization, including but not limited to art museums, history museums, science museums, and ethnographic museums. Their defining feature is the systematic curation and presentation of collections to the public or specific audiences.​

Examples:
- The British Museum​
- The Louvre​
- The Metropolitan Museum of Art​
- The National Museum of Denmark</rdfs:comment>
        <rdfs:label xml:lang="en">Museum</rdfs:label>
    </owl:Class>
    


    <!-- http://w3id.org/cacao/CACAO_0000022 -->

    <owl:Class rdf:about="http://w3id.org/cacao/CACAO_0000022">
        <rdfs:subClassOf rdf:resource="http://www.cidoc-crm.org/cidoc-crm/E21_Person"/>
        <rdfs:subClassOf rdf:resource="https://schema.org/Person"/>
        <dcterms:contributor rdf:resource="https://orcid.org/0000-0002-0905-7033"/>
        <dcterms:date rdf:datatype="http://www.w3.org/2001/XMLSchema#dateTime">2025-04-11T08:32:18Z</dcterms:date>
        <rdfs:comment xml:lang="en">Scope note:
This class comprises persons who are recognized for engaging in the creation or performance of works in the visual, performing, literary, or applied arts. This includes, but is not limited to, painters, sculptors, musicians, composers, writers, poets, actors, dancers, designers, and multimedia artists. An individual is regarded as an instance of Artist when there exists documented evidence of their engagement in artistic practices or when they are attributed with the authorship, performance, or conceptualization of artistic works, either by themselves or by third parties (such as curators, critics, or historical sources).

Artists may be associated with specific cultural movements, artistic periods, or creative practices. The classification of a Person as an Artist does not require professional status or formal recognition; amateur and self-taught individuals are also included when their artistic activity is documented and contextually significant.

In bibliographic or curatorial contexts, attribution of a creative work to an individual is sufficient to regard them as an Artist, even if the attribution is anonymous, pseudonymous, or contested.

Examples:
- Leonardo da Vinci
- Frida Kahlo
- William Shakespeare
- Maya Deren</rdfs:comment>
        <rdfs:label xml:lang="en">Artist</rdfs:label>
    </owl:Class>
    


    <!-- http://w3id.org/cacao/CACAO_0000023 -->

    <owl:Class rdf:about="http://w3id.org/cacao/CACAO_0000023">
        <rdfs:subClassOf rdf:resource="http://www.cidoc-crm.org/cidoc-crm/E22_Human-Made_Object"/>
        <dcterms:contributor rdf:resource="https://orcid.org/0000-0002-0905-7033"/>
        <dcterms:date rdf:datatype="http://www.w3.org/2001/XMLSchema#dateTime">2025-04-11T08:35:55Z</dcterms:date>
        <rdfs:comment xml:lang="en">Scope note:
This class comprises all persistent physical objects of any size that are purposely created by human activity and have physical boundaries that separate them completely in an objective way from other objects. The class also includes all aggregates of objects made for functional purposes of whatever kind, independent of physical coherence, such as a set of chessmen.​

Physical Artefacts are distinguished by their tangible nature and intentional creation, serving various purposes such as utility, artistic expression, or cultural significance. They may range from individual items like tools and artworks to assembled collections designed to function as a whole.​

Examples:
- The Rosetta Stone
- LNER Class A4 4468 Mallard [the World’s fastest steam locomotive, preserved at the National Railway Museum of York, UK]
- The Portland Vase</rdfs:comment>
        <rdfs:label xml:lang="en">Physical Artefact</rdfs:label>
    </owl:Class>
    


    <!-- http://w3id.org/cacao/CACAO_0000024 -->

    <owl:Class rdf:about="http://w3id.org/cacao/CACAO_0000024">
        <rdfs:subClassOf rdf:resource="http://w3id.org/cacao/CACAO_0000023"/>
        <dcterms:contributor rdf:resource="https://orcid.org/0000-0002-0905-7033"/>
        <dcterms:date rdf:datatype="http://www.w3.org/2001/XMLSchema#dateTime">2025-04-11T08:37:01Z</dcterms:date>
        <rdfs:comment xml:lang="en">Scope note:
This class comprises physical artefacts that are primarily created as expressions of aesthetic, conceptual, or symbolic intent. Artworks encompass a wide range of tangible objects produced through artistic practices, including but not limited to paintings, sculptures, installations, and mixed-media pieces.​

Artworks are distinguished by their purpose of conveying artistic expression, emotion, or commentary, rather than serving utilitarian functions. They are often characterized by their unique form, style, and the creative processes involved in their production.​

While all artworks are physical artefacts, not all physical artefacts qualify as artworks; the classification depends on the creator&apos;s intent and the cultural context attributing artistic value to the object.​
CIDOC CRM

Examples:
- The Mona Lisa by Leonardo da Vinci​
- The Thinker by Auguste Rodin​
- The Starry Night by Vincent van Gogh​
- Balloon Dog (Red) by Jeff Koons</rdfs:comment>
        <rdfs:label xml:lang="en">Artwork</rdfs:label>
    </owl:Class>
    


    <!-- http://w3id.org/cacao/CACAO_0000025 -->

    <owl:Class rdf:about="http://w3id.org/cacao/CACAO_0000025">
        <rdfs:subClassOf rdf:resource="http://w3id.org/cacao/CACAO_0000023"/>
        <dcterms:contributor rdf:resource="https://orcid.org/0000-0002-0905-7033"/>
        <dcterms:date rdf:datatype="http://www.w3.org/2001/XMLSchema#dateTime">2025-04-11T08:37:08Z</dcterms:date>
        <rdfs:comment xml:lang="en">Scope note:
This class comprises physical artefacts that are intentionally created and utilized by humans to produce, modify, or measure sound, music, or other forms of audio. Instruments are designed with specific acoustic properties or mechanisms to facilitate the creation or manipulation of auditory phenomena. This includes, but is not limited to, musical instruments such as string, wind, percussion, and electronic instruments.​

Instruments are characterized by their functional design aimed at generating or controlling sound, distinguishing them from other physical artefacts. They may vary in complexity from simple objects like drums and flutes to intricate devices like synthesizers and orchestral instruments.​

Examples:
- A Stradivarius violin​
- A Steinway grand piano​
- A traditional African djembe drum​
- A Moog synthesizer</rdfs:comment>
        <rdfs:label xml:lang="en">Instrument</rdfs:label>
    </owl:Class>
    


    <!-- http://w3id.org/cacao/CACAO_0000027 -->

    <owl:Class rdf:about="http://w3id.org/cacao/CACAO_0000027">
        <rdfs:subClassOf rdf:resource="http://www.cidoc-crm.org/cidoc-crm/E55_Type"/>
        <dcterms:contributor rdf:resource="https://orcid.org/0000-0002-0905-7033"/>
        <dcterms:date rdf:datatype="http://www.w3.org/2001/XMLSchema#dateTime">2025-04-11T11:18:31Z</dcterms:date>
        <rdfs:comment xml:lang="en">Scope note:
The Genre class encompasses concepts that denote specific categories or styles of creative works, including but not limited to:​

- Music Genres: Such as classical, jazz, rock, or electronic.​
- Film Genres: Including drama, comedy, thriller, or documentary.​
- Artistic Genres: Like impressionism, surrealism, or abstract expressionism.​
- Literary Genres: Such as fiction, non-fiction, poetry, or drama.​

Instances of the Genre class provide a means to classify and contextualize creative works within their respective domains, enhancing the discovery and analysis of cultural heritage materials based on their genre-specific characteristics.​

Examples:
- Jazz (music genre)​
- Film Noir (film genre)​
- Renaissance Art (artistic genre)​
- Science Fiction (literary genre)</rdfs:comment>
        <rdfs:label xml:lang="en">Genre</rdfs:label>
    </owl:Class>
    


    <!-- http://w3id.org/cacao/CACAO_0000028 -->

    <owl:Class rdf:about="http://w3id.org/cacao/CACAO_0000028">
        <rdfs:subClassOf rdf:resource="http://www.cidoc-crm.org/cidoc-crm/E55_Type"/>
        <dcterms:contributor rdf:resource="https://orcid.org/0000-0002-0905-7033"/>
        <dcterms:date rdf:datatype="http://www.w3.org/2001/XMLSchema#dateTime">2025-04-11T11:18:41Z</dcterms:date>
        <rdfs:comment xml:lang="en">Scope note:
This class comprises concepts that denote areas of professional, academic, or creative activity in which individuals, groups, or organizations engage. Instances of Field of Work represent specific domains of expertise or practice, such as &quot;architecture,&quot; &quot;literature,&quot; or &quot;engineering,&quot; and are used to classify and contextualize the roles, contributions, or affiliations of persons within the CIDOC CRM framework.​

By associating persons with a Field of Work, one can provide semantic context regarding the nature of their activities or specializations. 

Examples:
- Architecture​
- Literature​
- Engineering​
- Performing Arts​</rdfs:comment>
        <rdfs:label xml:lang="en">Field Of Work</rdfs:label>
    </owl:Class>
    


    <!-- http://w3id.org/cacao/CACAO_0000036 -->

    <owl:Class rdf:about="http://w3id.org/cacao/CACAO_0000036">
        <rdfs:subClassOf rdf:resource="http://www.cidoc-crm.org/cidoc-crm/E55_Type"/>
        <dcterms:contributor rdf:resource="https://orcid.org/0000-0002-0905-7033"/>
        <dcterms:date rdf:datatype="http://www.w3.org/2001/XMLSchema#dateTime">2025-04-12T09:17:34Z</dcterms:date>
        <rdfs:comment xml:lang="en">Scope note:
This class comprises concepts that denote distinct movements or scenes in the realms of literature, art, science, or philosophy. It is used to classify and contextualize creative and intellectual currents by grouping together works or individuals according to shared aesthetics, ideologies, methodologies, or historical trends. 

Examples:
- Impressionism
- Romanticism
- Modernism
- Existentialism</rdfs:comment>
        <rdfs:label xml:lang="en">Movement</rdfs:label>
    </owl:Class>
    


    <!-- http://www.cidoc-crm.org/cidoc-crm/E13_Attribute_Assignment -->

    <owl:Class rdf:about="http://www.cidoc-crm.org/cidoc-crm/E13_Attribute_Assignment">
        <rdfs:subClassOf rdf:resource="http://www.cidoc-crm.org/cidoc-crm/E7_Activity"/>
        <rdfs:comment xml:lang="en">Scope note:
This class comprises the actions of making assertions about one property of an object or any single relation between two items or concepts. The type of the property asserted to hold between two items or concepts can be described by the property P177 assigned property of type (is type of property assigned): E55 Type. 
For example, the class describes the actions of people making propositions and statements during certain scientific/scholarly procedures, e.g. the person and date when a condition statement was made, an identifier was assigned, the museum object was measured, etc. Which kinds of such assignments and statements need to be documented explicitly in structures of a schema rather than free text, depends on whether this information should be accessible by structured queries.
This class allows for the documentation of how the respective assignment came about, and whose opinion it was. Note that all instances of properties described in a knowledge base are the opinion of someone. Per default, they are the opinion of the team maintaining the knowledge base. This fact must not individually be registered for all instances of properties provided by the maintaining team, because it would result in an endless recursion of whose opinion was the description of an opinion. Therefore, the use of instances of E13 Attribute Assignment marks the fact that the maintaining team is in general neutral to the validity of the respective assertion, but registers someone else’s opinion and how it came about.
All properties assigned in such an action can also be seen as directly relating the respective pair of items or concepts. Multiple use of instances of E13 Attribute Assignment may possibly lead to a collection of contradictory values.

Examples:
- the examination of MS Sinai Greek 418 by Nicholas Pickwoad in November 2003 (Honey &amp; Pickwoad, 2010)
- the assessment of the current ownership of Martin Doerr’s silver cup in February 1997 (fictitious)

In First Order Logic:
- E13(x) ⇒ E7(x)
</rdfs:comment>
        <rdfs:label xml:lang="fr">E13 Assignation d’attribut</rdfs:label>
        <rdfs:label xml:lang="pt">E13 Atribuição de Característica</rdfs:label>
        <rdfs:label xml:lang="en">E13 Attribute Assignment</rdfs:label>
        <rdfs:label xml:lang="de">E13 Merkmalszuweisung</rdfs:label>
        <rdfs:label xml:lang="el">E13 Απόδοση Ιδιοτήτων</rdfs:label>
        <rdfs:label xml:lang="ru">E13 Назначeниe Атрибута</rdfs:label>
        <rdfs:label xml:lang="zh">E13 属性赋值</rdfs:label>
        <skos:notation xml:lang="en">E13</skos:notation>
        <skos:prefLabel xml:lang="fr">Assignation d’attribut</skos:prefLabel>
        <skos:prefLabel xml:lang="pt">Atribuição de Característica</skos:prefLabel>
        <skos:prefLabel xml:lang="en">Attribute Assignment</skos:prefLabel>
        <skos:prefLabel xml:lang="de">Merkmalszuweisung</skos:prefLabel>
        <skos:prefLabel xml:lang="el">Απόδοση Ιδιοτήτων</skos:prefLabel>
        <skos:prefLabel xml:lang="ru">Назначeниe Атрибута</skos:prefLabel>
        <skos:prefLabel xml:lang="zh">属性赋值</skos:prefLabel>
    </owl:Class>
    


    <!-- http://www.cidoc-crm.org/cidoc-crm/E16_Measurement -->

    <owl:Class rdf:about="http://www.cidoc-crm.org/cidoc-crm/E16_Measurement">
        <rdfs:subClassOf rdf:resource="http://www.cidoc-crm.org/cidoc-crm/E13_Attribute_Assignment"/>
        <rdfs:comment xml:lang="en">Scope note:
This class comprises actions measuring physical properties and other values that can be determined by a systematic, objective procedure of direct observation of particular states of physical reality. 
An instance of E16 Measurement may use simple counting or tools, such as yardsticks or radiation detection devices. The interest is in the method and care applied, so that the reliability of the result may be judged at a later stage, or research continued on the associated documents. The date of the event is important for dimensions, which may change value over time, such as the length of an object subject to shrinkage. Methods and devices employed should be associated with instances of E16 Measurement by properties such as P33 used specific technique: E29 Design or Procedure, P125 used object of type: E55 Type, P16 used specific object (was used for): E70 Thing, whereas basic techniques such as &quot;carbon-14 dating&quot; should be encoded using P2 has type (is type of): E55 Type. Details of methods and devices reused or reusable in other instances of E16 Measurement should be documented for these entities rather than the measurements themselves, whereas details of particular execution may be documented by free text or by instantiating adequate sub-activities, if the detail may be of interest for an overarching query.
Regardless whether a measurement is made by an instrument or by human senses, it represents the initial transition from physical reality to information without any other documented information object in between within the reasoning chain that would represent the result of the interaction of the observer or device with reality. Therefore, determining properties of an instance of E90 Symbolic Object is regarded as an instance of E13 Attribute Assignment, which may be inferred from observing and measuring representative carriers. In the case that the carrier can be named, the property P16 used specific object (was used for) should be used to indicate the instance(s) of E18 Physical Thing that was used as the empirical basis for the attribute assignment. For instance, inferring properties of depicted items using image material, such as satellite images, is not regarded as an instance of E16 Measurement, but as a subsequent instance of E13 Attribute Assignment. Rather, only the production of the images, understood as arrays of radiation intensities, is regarded as an instance of E16 Measurement. The same reasoning holds for other sensor data.

Examples:
- measurement of the height of silver cup 232 on 31(st) August 1997 (fictitious)
- the carbon 14 dating of the “Schoeninger Speer II” in 1996 [The carbon 14 dating of an approximately 400.000 year old complete Old Palaeolithic wooden spear found in Schoeningen, Niedersachsen, Germany, in 1995.] (Kouwenhoven, 1997)

In First Order Logic:
- E16(x) ⇒ E13(x)
</rdfs:comment>
        <rdfs:label xml:lang="en">E16 Measurement</rdfs:label>
        <rdfs:label xml:lang="pt">E16 Medição</rdfs:label>
        <rdfs:label xml:lang="de">E16 Messung</rdfs:label>
        <rdfs:label xml:lang="fr">E16 Mesurage</rdfs:label>
        <rdfs:label xml:lang="el">E16 Μέτρηση</rdfs:label>
        <rdfs:label xml:lang="ru">E16 Измeрeниe</rdfs:label>
        <rdfs:label xml:lang="zh">E16 测量</rdfs:label>
        <skos:notation xml:lang="en">E16</skos:notation>
        <skos:prefLabel xml:lang="en">Measurement</skos:prefLabel>
        <skos:prefLabel xml:lang="pt">Medição</skos:prefLabel>
        <skos:prefLabel xml:lang="de">Messung</skos:prefLabel>
        <skos:prefLabel xml:lang="fr">Mesurage</skos:prefLabel>
        <skos:prefLabel xml:lang="el">Μέτρηση</skos:prefLabel>
        <skos:prefLabel xml:lang="ru">Измeрeниe</skos:prefLabel>
        <skos:prefLabel xml:lang="zh">测量</skos:prefLabel>
    </owl:Class>
    


    <!-- http://www.cidoc-crm.org/cidoc-crm/E18_Physical_Thing -->

    <owl:Class rdf:about="http://www.cidoc-crm.org/cidoc-crm/E18_Physical_Thing">
        <rdfs:subClassOf rdf:resource="http://www.cidoc-crm.org/cidoc-crm/E72_Legal_Object"/>
        <rdfs:subClassOf rdf:resource="http://www.w3.org/ns/odrl/2/Asset"/>
        <rdfs:comment xml:lang="en">Scope note:
This class comprises all persistent physical items with a relatively stable form, human-made or natural.
Depending on the existence of natural boundaries of such things, the CIDOC CRM distinguishes the instances of E19 Physical Object from instances of E26 Physical Feature, such as holes, rivers, pieces of land, etc. Most instances of E19 Physical Object can be moved (if not too heavy), whereas features are integral to the surrounding matter.
An instance of E18 Physical Thing occupies not only a particular geometric space at any instant of its existence, but in the course of its existence it also forms a trajectory through spacetime, which occupies a real, that is phenomenal, volume in spacetime. We include in the occupied space the space filled by the matter of the physical thing and all its inner spaces, such as the interior of a box. For the purpose of more detailed descriptions of the presence of an instance of E18 Physical Thing in space and time it can be associated with its specific instance of E92 Spacetime Volume by the property P196 defines (is defined by). 
The CIDOC CRM is generally not concerned with amounts of matter in fluid or gaseous states, as long as they are not confined in an identifiable way for an identifiable minimal time-span.

Examples:
- the Cullinan Diamond (E19) (Scarratt and Shor, 2006)
- the cave “Ideon Andron” in Crete (E26) (Smith, 1844-49)
- the Mona Lisa (E22) (Mohen, 2006)

In First Order Logic:
- E18(x) ⇒ E72(x)
</rdfs:comment>
        <rdfs:label xml:lang="fr">E18 Chose matérielle</rdfs:label>
        <rdfs:label xml:lang="pt">E18 Coisa Material</rdfs:label>
        <rdfs:label xml:lang="de">E18 Materielles</rdfs:label>
        <rdfs:label xml:lang="en">E18 Physical Thing</rdfs:label>
        <rdfs:label xml:lang="el">E18 Υλικό Πράγμα</rdfs:label>
        <rdfs:label xml:lang="ru">E18 Матeриальный Прeдмeт</rdfs:label>
        <rdfs:label xml:lang="zh">E18 实物</rdfs:label>
        <skos:notation xml:lang="en">E18</skos:notation>
        <skos:prefLabel xml:lang="fr">Chose matérielle</skos:prefLabel>
        <skos:prefLabel xml:lang="pt">Coisa Material</skos:prefLabel>
        <skos:prefLabel xml:lang="de">Materielles</skos:prefLabel>
        <skos:prefLabel xml:lang="en">Physical Thing</skos:prefLabel>
        <skos:prefLabel xml:lang="el">Υλικό Πράγμα</skos:prefLabel>
        <skos:prefLabel xml:lang="ru">Матeриальный Прeдмeт</skos:prefLabel>
        <skos:prefLabel xml:lang="zh">实物</skos:prefLabel>
    </owl:Class>
    


    <!-- http://www.cidoc-crm.org/cidoc-crm/E19_Physical_Object -->

    <owl:Class rdf:about="http://www.cidoc-crm.org/cidoc-crm/E19_Physical_Object">
        <rdfs:subClassOf rdf:resource="http://www.cidoc-crm.org/cidoc-crm/E18_Physical_Thing"/>
        <rdfs:comment xml:lang="en">Scope note:
This class comprises items of a material nature that are units for documentation and have physical boundaries that separate them completely in an objective way from other objects. 
The class also includes all aggregates of objects made for functional purposes of whatever kind, independent of physical coherence, such as a set of chessmen. Typically, instances of E19 Physical Object can be moved (if not too heavy).
In some contexts, such objects, except for aggregates, are also called “bona fide objects”, i.e. naturally defined objects (Smith &amp; Varzi, 2000). 
The decision as to what is documented as a complete item, rather than by its parts or components, may be purely administrative or may be a result of the order in which the item was acquired.

Examples:
- Aphrodite of Milos (E22) (Kousser, 2005)
- the Cullinan Diamond (Scarratt and Shor, 2006)
- Apollo 13 at the time of launch (E22) (Lovell and Kluger, 1994)

In First Order Logic:
- E19(x) ⇒ E18(x)
</rdfs:comment>
        <rdfs:label xml:lang="de">E19 Materieller Gegenstand</rdfs:label>
        <rdfs:label xml:lang="fr">E19 Objet matériel</rdfs:label>
        <rdfs:label xml:lang="pt">E19 Objeto Material</rdfs:label>
        <rdfs:label xml:lang="en">E19 Physical Object</rdfs:label>
        <rdfs:label xml:lang="el">E19 Υλικό Αντικείμενο</rdfs:label>
        <rdfs:label xml:lang="ru">E19 Матeриальный Объeкт</rdfs:label>
        <rdfs:label xml:lang="zh">E19 物质对象</rdfs:label>
        <skos:notation xml:lang="en">E19</skos:notation>
        <skos:prefLabel xml:lang="de">Materieller Gegenstand</skos:prefLabel>
        <skos:prefLabel xml:lang="fr">Objet matériel</skos:prefLabel>
        <skos:prefLabel xml:lang="pt">Objeto Material</skos:prefLabel>
        <skos:prefLabel xml:lang="en">Physical Object</skos:prefLabel>
        <skos:prefLabel xml:lang="el">Υλικό Αντικείμενο</skos:prefLabel>
        <skos:prefLabel xml:lang="ru">Матeриальный Объeкт</skos:prefLabel>
        <skos:prefLabel xml:lang="zh">物质对象</skos:prefLabel>
    </owl:Class>
    


    <!-- http://www.cidoc-crm.org/cidoc-crm/E1_CRM_Entity -->

    <owl:Class rdf:about="http://www.cidoc-crm.org/cidoc-crm/E1_CRM_Entity">
        <rdfs:comment xml:lang="en">Scope note:
This class comprises all things in the universe of discourse of the CIDOC Conceptual Reference Model. 
It is an abstract concept providing for three general properties:
- Identification by name or appellation, and in particular by a preferred identifier
- Classification by type, allowing further refinement of the specific subclass to which an instance belongs 
- Attachment of free text and other unstructured data for the expression of anything not captured by formal properties
All other classes within the CIDOC CRM are directly or indirectly specialisations of E1 CRM Entity.

Examples:
- the earthquake in Lisbon 1755 (E5) (Chester, 2001)

In First Order Logic:
- E1(x)
</rdfs:comment>
        <rdfs:label xml:lang="en">E1 CRM Entity</rdfs:label>
        <rdfs:label xml:lang="de">E1 CRM Entität</rdfs:label>
        <rdfs:label xml:lang="ru">E1 CRM Сущность</rdfs:label>
        <rdfs:label xml:lang="zh">E1 CRM实体</rdfs:label>
        <rdfs:label xml:lang="pt">E1 Entidade CRM</rdfs:label>
        <rdfs:label xml:lang="fr">E1 Entité CRM</rdfs:label>
        <rdfs:label xml:lang="el">E1 Οντότητα CIDOC CRM</rdfs:label>
        <skos:notation xml:lang="en">E1</skos:notation>
        <skos:prefLabel xml:lang="en">CRM Entity</skos:prefLabel>
        <skos:prefLabel xml:lang="de">CRM Entität</skos:prefLabel>
        <skos:prefLabel xml:lang="ru">CRM Сущность</skos:prefLabel>
        <skos:prefLabel xml:lang="zh">CRM实体</skos:prefLabel>
        <skos:prefLabel xml:lang="pt">Entidade CRM</skos:prefLabel>
        <skos:prefLabel xml:lang="fr">Entité CRM</skos:prefLabel>
        <skos:prefLabel xml:lang="el">Οντότητα CIDOC CRM</skos:prefLabel>
    </owl:Class>
    


    <!-- http://www.cidoc-crm.org/cidoc-crm/E20_Biological_Object -->

    <owl:Class rdf:about="http://www.cidoc-crm.org/cidoc-crm/E20_Biological_Object">
        <rdfs:subClassOf rdf:resource="http://www.cidoc-crm.org/cidoc-crm/E19_Physical_Object"/>
        <rdfs:comment xml:lang="en">Scope note:
This class comprises individual items of a material nature, which live, have lived, or are natural products of or from living organisms. 
Artificial objects that incorporate biological elements, such as Victorian butterfly frames, can be documented as both instances of E20 Biological Object and E22 Human-Made Object.

Examples:
- me (fictitious)
- Tut-Ankh-Amun (Edwards and Boltin, 1979)
- Boukephalus [Horse of Alexander the Great] (Lamb, 2005)
- petrified dinosaur excrement PA1906-344

In First Order Logic:
- E20(x) ⇒ E19(x)
</rdfs:comment>
        <rdfs:label xml:lang="en">E20 Biological Object</rdfs:label>
        <rdfs:label xml:lang="de">E20 Biologischer Gegenstand</rdfs:label>
        <rdfs:label xml:lang="fr">E20 Objet biologique</rdfs:label>
        <rdfs:label xml:lang="pt">E20 Objeto Biológico</rdfs:label>
        <rdfs:label xml:lang="el">E20 Βιολογικό Ακτικείμενο</rdfs:label>
        <rdfs:label xml:lang="ru">E20 Биологичeский Объeкт</rdfs:label>
        <rdfs:label xml:lang="zh">E20 生物对象</rdfs:label>
        <skos:notation xml:lang="en">E20</skos:notation>
        <skos:prefLabel xml:lang="en">Biological Object</skos:prefLabel>
        <skos:prefLabel xml:lang="de">Biologischer Gegenstand</skos:prefLabel>
        <skos:prefLabel xml:lang="fr">Objet biologique</skos:prefLabel>
        <skos:prefLabel xml:lang="pt">Objeto Biológico</skos:prefLabel>
        <skos:prefLabel xml:lang="el">Βιολογικό Ακτικείμενο</skos:prefLabel>
        <skos:prefLabel xml:lang="ru">Биологичeский Объeкт</skos:prefLabel>
        <skos:prefLabel xml:lang="zh">生物对象</skos:prefLabel>
    </owl:Class>
    


    <!-- http://www.cidoc-crm.org/cidoc-crm/E21_Person -->

    <owl:Class rdf:about="http://www.cidoc-crm.org/cidoc-crm/E21_Person">
        <owl:equivalentClass rdf:resource="https://schema.org/Person"/>
        <rdfs:subClassOf rdf:resource="http://www.cidoc-crm.org/cidoc-crm/E20_Biological_Object"/>
        <rdfs:subClassOf rdf:resource="http://www.cidoc-crm.org/cidoc-crm/E39_Actor"/>
        <rdfs:subClassOf rdf:resource="http://www.w3.org/ns/odrl/2/Party"/>
        <rdfs:subClassOf rdf:resource="https://schema.org/Thing"/>
        <rdfs:comment xml:lang="en">Scope note:
This class comprises real persons who live or are assumed to have lived. 
Legendary figures that may have existed, such as Ulysses and King Arthur, fall into this class if the documentation refers to them as historical figures. In cases where doubt exists as to whether several persons are in fact identical, multiple instances can be created and linked to indicate their relationship. The CIDOC CRM does not propose a specific form to support reasoning about possible identity.
In a bibliographic context, a name presented following the conventions usually employed for personal names will be assumed to correspond to an actual real person (an instance of E21 Person), unless evidence is available to indicate that this is not the case. The fact that a persona may erroneously be classified as an instance of E21 Person does not imply that the concept comprises personae.

Examples:
- Tut-Ankh-Amun (Edwards and Boltin, 1979)
- Nelson Mandela (Brown and Hort, 2006)

In First Order Logic:
- E21(x) ⇒ E20(x)
- E21(x) ⇒ E39(x)
</rdfs:comment>
        <rdfs:label xml:lang="de">E21 Person</rdfs:label>
        <rdfs:label xml:lang="en">E21 Person</rdfs:label>
        <rdfs:label xml:lang="fr">E21 Personne</rdfs:label>
        <rdfs:label xml:lang="pt">E21 Pessoa</rdfs:label>
        <rdfs:label xml:lang="el">E21 Πρόσωπο</rdfs:label>
        <rdfs:label xml:lang="ru">E21 Личность</rdfs:label>
        <rdfs:label xml:lang="zh">E21 人物</rdfs:label>
        <skos:notation xml:lang="en">E21</skos:notation>
        <skos:prefLabel xml:lang="de">Person</skos:prefLabel>
        <skos:prefLabel xml:lang="en">Person</skos:prefLabel>
        <skos:prefLabel xml:lang="fr">Personne</skos:prefLabel>
        <skos:prefLabel xml:lang="pt">Pessoa</skos:prefLabel>
        <skos:prefLabel xml:lang="el">Πρόσωπο</skos:prefLabel>
        <skos:prefLabel xml:lang="ru">Личность</skos:prefLabel>
        <skos:prefLabel xml:lang="zh">人物</skos:prefLabel>
    </owl:Class>
    


    <!-- http://www.cidoc-crm.org/cidoc-crm/E22_Human-Made_Object -->

    <owl:Class rdf:about="http://www.cidoc-crm.org/cidoc-crm/E22_Human-Made_Object">
        <rdfs:subClassOf rdf:resource="http://www.cidoc-crm.org/cidoc-crm/E19_Physical_Object"/>
        <rdfs:subClassOf rdf:resource="http://www.cidoc-crm.org/cidoc-crm/E24_Physical_Human-Made_Thing"/>
        <rdfs:comment xml:lang="en">Scope note:
This class comprises all persistent physical objects of any size that are purposely created by human activity and have physical boundaries that separate them completely in an objective way from other objects. 
The class also includes all aggregates of objects made for functional purposes of whatever kind, independent of physical coherence, such as a set of chessmen.

Examples:
- the Rosetta Stone (E22)
- LNER Class A4 4468 Mallard [the World’s fastest steam locomotive, preserved at the National Railway Museum of York, UK] (Solomon, 2003)
- the Portland Vase (Walker, 2004)

In First Order Logic:
- E22(x) ⇒ E19(x)
- E22(x) ⇒ E24(x)
</rdfs:comment>
        <rdfs:label xml:lang="en">E22 Human-Made Object</rdfs:label>
        <rdfs:label xml:lang="fr">E22 Objet élaboré par l’humain</rdfs:label>
        <rdfs:label xml:lang="ru">E22 Рукотворный Объeкт</rdfs:label>
        <skos:notation xml:lang="en">E22</skos:notation>
        <skos:prefLabel xml:lang="en">Human-Made Object</skos:prefLabel>
        <skos:prefLabel xml:lang="fr">Objet élaboré par l’humain</skos:prefLabel>
        <skos:prefLabel xml:lang="ru">Рукотворный Объeкт</skos:prefLabel>
    </owl:Class>
    


    <!-- http://www.cidoc-crm.org/cidoc-crm/E24_Physical_Human-Made_Thing -->

    <owl:Class rdf:about="http://www.cidoc-crm.org/cidoc-crm/E24_Physical_Human-Made_Thing">
        <rdfs:subClassOf rdf:resource="http://www.cidoc-crm.org/cidoc-crm/E18_Physical_Thing"/>
        <rdfs:subClassOf rdf:resource="http://www.cidoc-crm.org/cidoc-crm/E71_Human-Made_Thing"/>
        <rdfs:comment xml:lang="en">Scope note:
This class comprises all persistent physical items of any size that are purposely created by human activity. This class comprises, besides others, human-made objects, such as a sword, and human-made features, such as rock art. For example, a “cup and ring” carving on bedrock is regarded as instance of E24 Physical Human-Made Thing.
Instances of E24 Physical Human-Made Thing may be the result of modifying pre-existing physical things, preserving larger parts or most of the original matter and structure, which poses the question if they are new or even human-made, the respective interventions of production made on such original material should be obvious and sufficient to regard that the product has a new, distinct identity and intended function and is human-made. Substantial continuity of the previous matter and structure in the new product can be documented by describing the production process also as an instance of E81 Transformation.
Whereas interventions of conservation and repair are not regarded to produce a new instance of E24 Physical Human-Made Thing, the results of preparation of natural history specimens that substantially change their natural or original state should be regarded as instances of E24 Physical Human-Made Things, including the uncovering of petrified biological features from a solid piece of stone. On the other side, scribbling a museum number on a natural object should not be regarded to make it human-made. This notwithstanding, parts, sections, segments, or features of an instance of E24 Physical Human-Made Thing may continue to be non-human-made and preserved during the production process, for example natural pearls used as a part of an eardrop.

Examples:
- the Forth Railway Bridge (Shipway, Bouch, Baker and Fowler, 1990).
- the Channel Tunnel (E25) (Holliday, Marcou and Vickerman, 1991)
- the Palace of Knossos (Evans, 1921)
- the Colosseum in Rome, Italy (Hopkins and Beard, 2011)
- the Historical Collection of the Museum Benaki in Athens (E78) (Georgoula, 2005)
- the Rosetta Stone (E22)
- my paperback copy of Crime &amp; Punishment (E22) (fictitious)
- the computer disk at ICS-FORTH that stores the canonical Definition of the CIDOC CRM v.3.2 (E22)
- my empty DVD disk (E22) (fictitious)

In First Order Logic:
- E24(x) ⇒ E18(x)
- E24(x) ⇒ E71(x)
</rdfs:comment>
        <rdfs:label xml:lang="fr">E24 Chose matérielle élaborée par l’humain</rdfs:label>
        <rdfs:label xml:lang="en">E24 Physical Human-Made Thing</rdfs:label>
        <rdfs:label xml:lang="ru">E24 Матeриальный Рукотворный Объeкт</rdfs:label>
        <skos:notation xml:lang="en">E24</skos:notation>
        <skos:prefLabel xml:lang="fr">Chose matérielle élaborée par l’humain</skos:prefLabel>
        <skos:prefLabel xml:lang="en">Physical Human-Made Thing</skos:prefLabel>
        <skos:prefLabel xml:lang="ru">Матeриальный Рукотворный Объeкт</skos:prefLabel>
    </owl:Class>
    


    <!-- http://www.cidoc-crm.org/cidoc-crm/E28_Conceptual_Object -->

    <owl:Class rdf:about="http://www.cidoc-crm.org/cidoc-crm/E28_Conceptual_Object">
        <rdfs:subClassOf rdf:resource="http://www.cidoc-crm.org/cidoc-crm/E71_Human-Made_Thing"/>
        <rdfs:comment xml:lang="en">Scope note:
This class comprises non-material products of our minds and other human produced data that have become objects of a discourse about their identity, circumstances of creation, or historical implication. The production of such information might have been supported by the use of technical devices such as cameras or computers.
Characteristically, instances of this class are created, invented or thought by someone, and then may be documented or communicated between persons. Instances of E28 Conceptual Object have the ability to exist on more than one particular carrier at the same time, such as paper, electronic signals, marks, audio media, paintings, photos, human memories, etc.
They cannot be destroyed. They exist as long as they can be found on at least one carrier or in at least one human memory. Their existence ends when the last carrier and the last memory are lost.

Examples:
- Beethoven’s “Ode an die Freude” (Ode to Joy) (E73) (Kershaw, 1999)
- the definition of “ontology” in the Oxford English Dictionary (E73) (Oxford University Press, 1989)
- the knowledge about the victory at Marathon carried by the famous runner (E89) (Lagos &amp; Karyanos, 2020)
- [Explanation note: The following examples illustrate the distinction between a propositional object, its names and its encoded forms. The Maxwell equations (Ball, 1962) are a good example, because they belong to the fundamental laws of physics and their mathematical content yields identical, unambiguous results regardless formulation and encoding.] 
- “Maxwell equations” (E41) [preferred subject access point from LCSH, http://lccn.loc.gov/sh85082387, accessed 18(th) April 2021. This is only the name for the Maxwell equations as standardized by the Library of Congress and not the equations themselves.]
- “Equations, Maxwell” (E41) [variant subject access point from LCSH, http://lccn.loc.gov/sh85082387, accessed 18(th) April 2021. This is another name for the equation standardized by the Library of Congress and not the equations themselves.]
- Maxwell&apos;s equations (E89) [This is the propositional content of the equations proper, independent of any particular notation or mathematical formalism.] (Ball, 1962)
- The encoding of Maxwells equations as in https://upload.wikimedia.org/wikipedia/commons/c/c4/Maxwell%27sEquations.svg (E73) [accessed 18(th) April 2021. This is one possible symbolic encoding of the propositional content of the equations.]

In First Order Logic:
- E28(x) ⇒ E71(x)
</rdfs:comment>
        <rdfs:label xml:lang="de">E28 Begrifflicher Gegenstand</rdfs:label>
        <rdfs:label xml:lang="en">E28 Conceptual Object</rdfs:label>
        <rdfs:label xml:lang="fr">E28 Objet conceptuel</rdfs:label>
        <rdfs:label xml:lang="pt">E28 Objeto Conceitual</rdfs:label>
        <rdfs:label xml:lang="el">E28 Νοητικό Αντικείμενο</rdfs:label>
        <rdfs:label xml:lang="ru">E28 Концeптуальный Объeкт</rdfs:label>
        <rdfs:label xml:lang="zh">E28 概念对象</rdfs:label>
        <skos:notation xml:lang="en">E28</skos:notation>
        <skos:prefLabel xml:lang="de">Begrifflicher Gegenstand</skos:prefLabel>
        <skos:prefLabel xml:lang="en">Conceptual Object</skos:prefLabel>
        <skos:prefLabel xml:lang="fr">Objet conceptuel</skos:prefLabel>
        <skos:prefLabel xml:lang="pt">Objeto Conceitual</skos:prefLabel>
        <skos:prefLabel xml:lang="el">Νοητικό Αντικείμενο</skos:prefLabel>
        <skos:prefLabel xml:lang="ru">Концeптуальный Объeкт</skos:prefLabel>
        <skos:prefLabel xml:lang="zh">概念对象</skos:prefLabel>
    </owl:Class>
    


    <!-- http://www.cidoc-crm.org/cidoc-crm/E2_Temporal_Entity -->

    <owl:Class rdf:about="http://www.cidoc-crm.org/cidoc-crm/E2_Temporal_Entity">
        <rdfs:subClassOf rdf:resource="http://www.cidoc-crm.org/cidoc-crm/E1_CRM_Entity"/>
        <rdfs:comment xml:lang="en">Scope note:
This class comprises all phenomena, such as the instances of E4 Periods and E5 Events, which happen over a limited extent in time. This extent in time must be contiguous, i.e., without gaps. In case the defining kinds of phenomena for an instance of E2 Temporal Entity cease to happen, and occur later again at another time, we regard that the former instance of E2 Temporal Entity has ended and a new instance has come into existence. In more intuitive terms, the same event cannot happen twice.
In some contexts, such phenomena are also called perdurants. This class is disjoint from E77 Persistent Item and is an abstract class that typically has no direct instances. E2 Temporal Entity is specialized into E4 Period, which applies to a particular geographic area (defined with a greater or lesser degree of precision), and E3 Condition State, which applies to instances of E18 Physical Thing.

Examples:
- Bronze Age (E4) (Childe, 1963)
- the earthquake in Lisbon 1755 (E5) (Chester, 2001)
- the Peterhof Palace near Saint Petersburg being in ruins from 1944 to 1946 (E3) (Maddox, 2015)

In First Order Logic:
- E2(x) ⇒ E1(x)
</rdfs:comment>
        <rdfs:label xml:lang="pt">E2 Entidade Temporal</rdfs:label>
        <rdfs:label xml:lang="fr">E2 Entité temporelle</rdfs:label>
        <rdfs:label xml:lang="de">E2 Geschehendes</rdfs:label>
        <rdfs:label xml:lang="en">E2 Temporal Entity</rdfs:label>
        <rdfs:label xml:lang="el">E2 Έγχρονη Οντότητα</rdfs:label>
        <rdfs:label xml:lang="ru">E2 Врeмeнная Сущность</rdfs:label>
        <rdfs:label xml:lang="zh">E2 时序实体</rdfs:label>
        <skos:notation xml:lang="en">E2</skos:notation>
        <skos:prefLabel xml:lang="pt">Entidade Temporal</skos:prefLabel>
        <skos:prefLabel xml:lang="fr">Entité temporelle</skos:prefLabel>
        <skos:prefLabel xml:lang="de">Geschehendes</skos:prefLabel>
        <skos:prefLabel xml:lang="en">Temporal Entity</skos:prefLabel>
        <skos:prefLabel xml:lang="el">Έγχρονη Οντότητα</skos:prefLabel>
        <skos:prefLabel xml:lang="ru">Врeмeнная Сущность</skos:prefLabel>
        <skos:prefLabel xml:lang="zh">时序实体</skos:prefLabel>
    </owl:Class>
    


    <!-- http://www.cidoc-crm.org/cidoc-crm/E30_Right -->

    <owl:Class rdf:about="http://www.cidoc-crm.org/cidoc-crm/E30_Right">
        <owl:equivalentClass rdf:resource="http://www.w3.org/ns/odrl/2/Policy"/>
        <rdfs:subClassOf rdf:resource="http://www.cidoc-crm.org/cidoc-crm/E89_Propositional_Object"/>
        <rdfs:comment xml:lang="en">Scope note:
This class comprises legal privileges concerning material and immaterial things or their derivatives. 
These include reproduction and property rights.

Examples:
- copyright held by ISO on ISO/CD 21127
- ownership of the “Mona Lisa” by the museum of the Louvre, Paris, France

In First Order Logic:
- E30(x) ⇒ E89(x)
</rdfs:comment>
        <rdfs:label xml:lang="pt">E30 Direitos</rdfs:label>
        <rdfs:label xml:lang="fr">E30 Droit</rdfs:label>
        <rdfs:label xml:lang="de">E30 Recht</rdfs:label>
        <rdfs:label xml:lang="en">E30 Right</rdfs:label>
        <rdfs:label xml:lang="el">E30 Δικαίωμα</rdfs:label>
        <rdfs:label xml:lang="ru">E30 Право</rdfs:label>
        <rdfs:label xml:lang="zh">E30 权限</rdfs:label>
        <skos:notation xml:lang="en">E30</skos:notation>
        <skos:prefLabel xml:lang="pt">Direitos</skos:prefLabel>
        <skos:prefLabel xml:lang="fr">Droit</skos:prefLabel>
        <skos:prefLabel xml:lang="de">Recht</skos:prefLabel>
        <skos:prefLabel xml:lang="en">Right</skos:prefLabel>
        <skos:prefLabel xml:lang="el">Δικαίωμα</skos:prefLabel>
        <skos:prefLabel xml:lang="ru">Право</skos:prefLabel>
        <skos:prefLabel xml:lang="zh">权限</skos:prefLabel>
    </owl:Class>
    


    <!-- http://www.cidoc-crm.org/cidoc-crm/E33_Linguistic_Object -->

    <owl:Class rdf:about="http://www.cidoc-crm.org/cidoc-crm/E33_Linguistic_Object">
        <rdfs:subClassOf rdf:resource="http://www.cidoc-crm.org/cidoc-crm/E73_Information_Object"/>
        <rdfs:comment xml:lang="en">Scope note:
This class comprises identifiable expressions in natural language or languages. 
Instances of E33 Linguistic Object can be expressed in many ways: e.g. as written texts, recorded speech, or sign language. However, the CIDOC CRM treats instances of E33 Linguistic Object independently from the medium or method by which they are expressed. Expressions in formal languages, such as computer code or mathematical formulae, are not treated as instances of E33 Linguistic Object by the CIDOC CRM. These should be modelled as instances of E73 Information Object.
In general, an instance of E33 Linguistic Object may also contain non-linguistic information, often of artistic or aesthetic value. Only in cases in which the content of an instance of E33 Linguistic Object can completely be expressed by a series of binary-encoded symbols, its content may be documented within a respective knowledge base by the property P190 has symbolic content: E62 String. Otherwise, it should be understood as an identifiable digital resource only available independently from the respective knowledge base. 
In other cases, such as pages of an illuminated manuscript or recordings containing speech in a language supported by a writing system, the linguistic part of the content of an instance of E33 Linguistic Object may be documented within a respective knowledge base in a note by P3 has note: E62 String. Otherwise, it may be described using the property P165 incorporates (is incorporated in): E73 Information Object as a different object with its own identity.

Examples:
- the text of the Ellesmere Chaucer manuscript (Hilmo, 2019)
- the lyrics of the song “Blue Suede Shoes” (Cooper, 2008)
- the text of the “Jabberwocky” by Lewis Carroll (Carroll, 1981)
- the text of “Doktoro Jekyll kaj Sinjoro Hyde” [an Esperanto translation of Dr. Jekyll and Mr. Hyde]. (Stevenson, Morrison and Mann, 1909)
- the free dialog in the local dialect recorded in 1958, Telemark, Norway stored on tape or.7-89.s1 (00.15:46-00:34), The Language Collection at the University Library in Bergen, Norway (verified on 2020)

In First Order Logic:
- E33(x) ⇒ E73(x)
</rdfs:comment>
        <rdfs:label xml:lang="en">E33 Linguistic Object</rdfs:label>
        <rdfs:label xml:lang="fr">E33 Objet linguistique</rdfs:label>
        <rdfs:label xml:lang="pt">E33 Objeto Lingüístico</rdfs:label>
        <rdfs:label xml:lang="de">E33 Sprachlicher Gegenstand</rdfs:label>
        <rdfs:label xml:lang="el">E33 Γλωσσικό Αντικείμενο</rdfs:label>
        <rdfs:label xml:lang="ru">E33 Лингвистичeский Объeкт</rdfs:label>
        <rdfs:label xml:lang="zh">E33 语言对象</rdfs:label>
        <skos:notation xml:lang="en">E33</skos:notation>
        <skos:prefLabel xml:lang="en">Linguistic Object</skos:prefLabel>
        <skos:prefLabel xml:lang="fr">Objet linguistique</skos:prefLabel>
        <skos:prefLabel xml:lang="pt">Objeto Lingüístico</skos:prefLabel>
        <skos:prefLabel xml:lang="de">Sprachlicher Gegenstand</skos:prefLabel>
        <skos:prefLabel xml:lang="el">Γλωσσικό Αντικείμενο</skos:prefLabel>
        <skos:prefLabel xml:lang="ru">Лингвистичeский Объeкт</skos:prefLabel>
        <skos:prefLabel xml:lang="zh">语言对象</skos:prefLabel>
    </owl:Class>
    


    <!-- http://www.cidoc-crm.org/cidoc-crm/E35_Title -->

    <owl:Class rdf:about="http://www.cidoc-crm.org/cidoc-crm/E35_Title">
        <rdfs:subClassOf rdf:resource="http://www.cidoc-crm.org/cidoc-crm/E33_Linguistic_Object"/>
        <rdfs:subClassOf rdf:resource="http://www.cidoc-crm.org/cidoc-crm/E41_Appellation"/>
        <rdfs:comment xml:lang="en">Scope note:
This class comprises the textual strings that within a cultural context can be clearly identified as titles due to their form. Being a subclass of E41 Appellation, E35 Title can only be used when such a string is actually used as a title of a work, such as a text, an artwork, or a piece of music.
Titles are proper noun phrases or verbal phrases, and should not be confused with generic object names such as “chair”, “painting”, or “book” (the latter are common nouns that stand for instances of E55 Type). Titles may be assigned by the creator of the work itself, or by a social group.
This class also comprises the translations of titles that are used as surrogates for the original titles in different social contexts.

Examples:
- “The Merchant of Venice” (McCullough, 2005)
- “Mona Lisa” (Mohen, Menu and Mottin, 2006)
- “La Pie” (Bortolatto, 1981)
- “Lucy in the Sky with Diamonds” (Lennon, 1967)

In First Order Logic:
- E35(x) ⇒ E33(x)
- E35(x) ⇒ E41(x)
</rdfs:comment>
        <rdfs:label xml:lang="de">E35 Titel</rdfs:label>
        <rdfs:label xml:lang="en">E35 Title</rdfs:label>
        <rdfs:label xml:lang="fr">E35 Titre</rdfs:label>
        <rdfs:label xml:lang="pt">E35 Título</rdfs:label>
        <rdfs:label xml:lang="el">E35 Τίτλος</rdfs:label>
        <rdfs:label xml:lang="ru">E35 Названиe</rdfs:label>
        <rdfs:label xml:lang="zh">E35 题名</rdfs:label>
        <skos:notation xml:lang="en">E35</skos:notation>
        <skos:prefLabel xml:lang="de">Titel</skos:prefLabel>
        <skos:prefLabel xml:lang="en">Title</skos:prefLabel>
        <skos:prefLabel xml:lang="fr">Titre</skos:prefLabel>
        <skos:prefLabel xml:lang="pt">Título</skos:prefLabel>
        <skos:prefLabel xml:lang="el">Τίτλος</skos:prefLabel>
        <skos:prefLabel xml:lang="ru">Названиe</skos:prefLabel>
        <skos:prefLabel xml:lang="zh">题名</skos:prefLabel>
    </owl:Class>
    


    <!-- http://www.cidoc-crm.org/cidoc-crm/E36_Visual_Item -->

    <owl:Class rdf:about="http://www.cidoc-crm.org/cidoc-crm/E36_Visual_Item">
        <rdfs:subClassOf rdf:resource="http://www.cidoc-crm.org/cidoc-crm/E73_Information_Object"/>
        <rdfs:comment xml:lang="en">Scope note:
This class comprises the intellectual or conceptual aspects of recognisable marks and images.
This class does not intend to describe the idiosyncratic characteristics of an individual physical embodiment of a visual item, but the underlying prototype. For example, a mark such as the ICOM logo is generally considered to be the same logo when used on any number of publications. The size, orientation, and colour may change, but the logo remains uniquely identifiable. The same is true of images that are reproduced many times. This means that visual items are independent of their physical support.
The E36 Visual Item class provides a means of identifying and linking together instances of E24 Physical Human-Made Thing that carry the same visual symbols, marks, or images, etc. The property P62 depicts (is depicted by) between E24 Physical Human-Made Thing and the depicted subjects (E1 CRM Entity) can be regarded as a shortcut of the more fully developed path from E24 Physical Human-Made Thing through P65 shows visual item (is shown by), E36 Visual Item, P138 represents (has representation) to E1 CRM Entity, which in addition captures the optical features of the depiction.

Examples:
- the visual appearance of Monet’s “La Pie” (Bortolatto, 1981)
- the Coca-Cola logo (E34)
- the Chi-Rho (E37)
- the communist red star (E37)
- the surface shape of Auguste Rodin&apos;s statue &quot;Le Penseur&quot; [There exist more than 20 copies, even of different size. Therefore, this is a good example that it is only the common surface shape, an immaterial visual item, which justifies displaying these copies as works of Auguste Rodin. As usual practice, Rodin himself did not produce the bronze statue, but only the prototype model.]

In First Order Logic:
- E36(x) ⇒ E73(x)
</rdfs:comment>
        <rdfs:label xml:lang="de">E36 Bildliches</rdfs:label>
        <rdfs:label xml:lang="fr">E36 Entité visuelle</rdfs:label>
        <rdfs:label xml:lang="pt">E36 Item Visual</rdfs:label>
        <rdfs:label xml:lang="en">E36 Visual Item</rdfs:label>
        <rdfs:label xml:lang="el">E36 Οπτικό Στοιχείο</rdfs:label>
        <rdfs:label xml:lang="ru">E36 Визуальный Прeдмeт</rdfs:label>
        <rdfs:label xml:lang="zh">E36 可视项</rdfs:label>
        <skos:notation xml:lang="en">E36</skos:notation>
        <skos:prefLabel xml:lang="de">Bildliches</skos:prefLabel>
        <skos:prefLabel xml:lang="fr">Entité visuelle</skos:prefLabel>
        <skos:prefLabel xml:lang="pt">Item Visual</skos:prefLabel>
        <skos:prefLabel xml:lang="en">Visual Item</skos:prefLabel>
        <skos:prefLabel xml:lang="el">Οπτικό Στοιχείο</skos:prefLabel>
        <skos:prefLabel xml:lang="ru">Визуальный Прeдмeт</skos:prefLabel>
        <skos:prefLabel xml:lang="zh">可视项</skos:prefLabel>
    </owl:Class>
    


    <!-- http://www.cidoc-crm.org/cidoc-crm/E39_Actor -->

    <owl:Class rdf:about="http://www.cidoc-crm.org/cidoc-crm/E39_Actor">
        <owl:equivalentClass rdf:resource="http://www.w3.org/ns/odrl/2/Party"/>
        <rdfs:subClassOf rdf:resource="http://www.cidoc-crm.org/cidoc-crm/E77_Persistent_Item"/>
        <rdfs:comment xml:lang="en">Scope note:
This class comprises people, either individually or in groups, who have the potential to perform intentional actions of kinds for which they can be held responsible.

Examples:
- London and Continental Railways (E74)
- the Governor of the Bank of England in 1975 (E21)
- Sir Ian McKellen (E21) (Gibson, 1986)

In First Order Logic:
- E39(x) ⇒ E77(x)
</rdfs:comment>
        <rdfs:label xml:lang="fr">E39 Actant</rdfs:label>
        <rdfs:label xml:lang="en">E39 Actor</rdfs:label>
        <rdfs:label xml:lang="pt">E39 Agente</rdfs:label>
        <rdfs:label xml:lang="de">E39 Akteur</rdfs:label>
        <rdfs:label xml:lang="el">E39 Δράστης</rdfs:label>
        <rdfs:label xml:lang="ru">E39 Дeйствующий Субъeкт</rdfs:label>
        <rdfs:label xml:lang="zh">E39 参与者</rdfs:label>
        <skos:notation xml:lang="en">E39</skos:notation>
        <skos:prefLabel xml:lang="fr">Actant</skos:prefLabel>
        <skos:prefLabel xml:lang="en">Actor</skos:prefLabel>
        <skos:prefLabel xml:lang="pt">Agente</skos:prefLabel>
        <skos:prefLabel xml:lang="de">Akteur</skos:prefLabel>
        <skos:prefLabel xml:lang="el">Δράστης</skos:prefLabel>
        <skos:prefLabel xml:lang="ru">Дeйствующий Субъeкт</skos:prefLabel>
        <skos:prefLabel xml:lang="zh">参与者</skos:prefLabel>
    </owl:Class>
    


    <!-- http://www.cidoc-crm.org/cidoc-crm/E3_Condition_State -->

    <owl:Class rdf:about="http://www.cidoc-crm.org/cidoc-crm/E3_Condition_State">
        <rdfs:subClassOf rdf:resource="http://www.cidoc-crm.org/cidoc-crm/E2_Temporal_Entity"/>
        <rdfs:comment xml:lang="en">Scope note:
This class comprises the states of objects characterised by a certain condition over a time-span. 
An instance of this class describes the prevailing physical condition of any material object or feature during a specific instance of E52 Time-Span. In general, the time-span for which a certain condition can be asserted may be shorter than the real time-span, for which this condition held.
The nature of that condition can be described using P2 has type. For example, the instance of E3 Condition State “condition of the SS Great Britain between 22(nd) September 1846 and 27(th) August 1847” can be characterized as an instance “wrecked” of E55 Type.

Examples:
- the &quot;reconstructed&quot; state of the “Amber Room” in Tsarskoje Selo from summer 2003 until now (Owen, 2009)
- the &quot;ruined&quot; state of Peterhof Palace near Saint Petersburg from 1944 to 1946 (Maddox, 2015)
- the state of my turkey in the oven at 14:30 on 25(th) December 2002 [P2 has type: E55 Type “still not cooked”] (fictitious)
- the topography of the leaves of Sinai Printed Book 3234.2361 on the 10(th) July 2007 [described as: of type &quot;cockled&quot;] (fictitious)

In First Order Logic:
- E3(x) ⇒ E2(x)
</rdfs:comment>
        <rdfs:label xml:lang="en">E3 Condition State</rdfs:label>
        <rdfs:label xml:lang="pt">E3 Estado Material</rdfs:label>
        <rdfs:label xml:lang="de">E3 Zustandsphase</rdfs:label>
        <rdfs:label xml:lang="fr">E3 État matériel</rdfs:label>
        <rdfs:label xml:lang="el">E3 Κατάσταση</rdfs:label>
        <rdfs:label xml:lang="ru">E3 Состояниe</rdfs:label>
        <rdfs:label xml:lang="zh">E3 条件状态</rdfs:label>
        <skos:notation xml:lang="en">E3</skos:notation>
        <skos:prefLabel xml:lang="en">Condition State</skos:prefLabel>
        <skos:prefLabel xml:lang="pt">Estado Material</skos:prefLabel>
        <skos:prefLabel xml:lang="de">Zustandsphase</skos:prefLabel>
        <skos:prefLabel xml:lang="fr">État matériel</skos:prefLabel>
        <skos:prefLabel xml:lang="el">Κατάσταση</skos:prefLabel>
        <skos:prefLabel xml:lang="ru">Состояниe</skos:prefLabel>
        <skos:prefLabel xml:lang="zh">条件状态</skos:prefLabel>
    </owl:Class>
    


    <!-- http://www.cidoc-crm.org/cidoc-crm/E41_Appellation -->

    <owl:Class rdf:about="http://www.cidoc-crm.org/cidoc-crm/E41_Appellation">
        <rdfs:subClassOf rdf:resource="http://www.cidoc-crm.org/cidoc-crm/E90_Symbolic_Object"/>
        <rdfs:comment xml:lang="en">Scope note:
This class comprises all signs, either meaningful or not, or arrangements of signs following a specific syntax, that are used or can be used to refer to and identify a specific instance of some class within a certain context.
Instances of E41 Appellation do not identify things by their meaning, even if they happen to have one, but by convention, tradition, or agreement. Instances of E41 Appellation are cultural constructs; as such, they have a context, a history, and a use in time and space by some group of users. A given instance of E41 Appellation can have alternative forms, i.e. other instances of E41 Appellation that are regarded as equivalent, regardless of the thing it denotes.
Different languages may use different appellations for the same thing, such as the names of major cities. Some appellations may be formulated using a valid noun phrase of a particular language. In these cases, the respective instances of E41 Appellation should also be declared as instances of E33 Linguistic Object. Then the language using the appellation can be declared with the property P72 has language: E56 Language.
Instances of E41 Appellation may be used to identify any instance of E1 CRM Entity and sometimes are characteristic for instances of more specific subclasses of E1 CRM Entity, such as for instances of E52 Time-Span (for instance “dates”), E39 Actor, E53 Place or E28 Conceptual Object. Postal addresses and E-mail addresses are characteristic examples of identifiers used by services transporting things between clients.
Even numerically expressed identifiers for extents in space or time are also regarded as instances of E41 Appellation, such as Gregorian dates or spatial coordinates, even though they allow for determining some time or location by a known procedure starting from a reference point and by virtue of that fact play a double role as instances of E59 Primitive Value.
E41 Appellation should not be confused with the act of naming something. Cf. E15 Identifier Assignment.

Examples:
- “Martin”
- “Aquae Sulis Minerva”
- “the Merchant of Venice” (E35) (McCullough, 2005)
- “Spigelia marilandica (L.) L.” [not the species, just the name] (Hershberger, Robacker and Jenkins, 2015)
- “information science” [not the science itself, but the name used to refer to the subject matter in an English-speaking context]
- “安” [Chinese “an”, meaning “peace”]
- “6°5’29”N 45°12’13”W” [example of a spatial coordinate]
- “Black queen’s bishop 4” [chess coordinate, example of an identifier in a conceptual space (E89)]
- “19-MAR-1922” [example of date]
- “+41 22 418 5571” [example of contact point]
- “weasel@paveprime.com” [example of contact point]
- “CH-1211, Genève” [example of place appellation]
- “1-29-3 Otsuka, Bunkyo-ku, Tokyo, 121, Japan” [example of a postal address]
- “the poop deck of H.M.S Victory” [example of a section definition on a human-made object (E22)]
- “the Venus de Milo’s left buttock” [example of a section definition on a human-made object (E22)]

In First Order Logic:
- E41(x) ⇒ E90(x)
</rdfs:comment>
        <rdfs:label xml:lang="en">E41 Appellation</rdfs:label>
        <rdfs:label xml:lang="fr">E41 Appellation</rdfs:label>
        <rdfs:label xml:lang="de">E41 Benennung</rdfs:label>
        <rdfs:label xml:lang="pt">E41 Designação</rdfs:label>
        <rdfs:label xml:lang="el">E41 Ονομασία</rdfs:label>
        <rdfs:label xml:lang="ru">E41 Обозначeниe</rdfs:label>
        <rdfs:label xml:lang="zh">E41 称谓</rdfs:label>
        <skos:notation xml:lang="en">E41</skos:notation>
        <skos:prefLabel xml:lang="en">Appellation</skos:prefLabel>
        <skos:prefLabel xml:lang="fr">Appellation</skos:prefLabel>
        <skos:prefLabel xml:lang="de">Benennung</skos:prefLabel>
        <skos:prefLabel xml:lang="pt">Designação</skos:prefLabel>
        <skos:prefLabel xml:lang="el">Ονομασία</skos:prefLabel>
        <skos:prefLabel xml:lang="ru">Обозначeниe</skos:prefLabel>
        <skos:prefLabel xml:lang="zh">称谓</skos:prefLabel>
    </owl:Class>
    


    <!-- http://www.cidoc-crm.org/cidoc-crm/E42_Identifier -->

    <owl:Class rdf:about="http://www.cidoc-crm.org/cidoc-crm/E42_Identifier">
        <rdfs:subClassOf rdf:resource="http://www.cidoc-crm.org/cidoc-crm/E41_Appellation"/>
        <rdfs:comment xml:lang="en">Scope note:
This class comprises strings or codes assigned to instances of E1 CRM Entity in order to identify them uniquely and permanently within the context of one or more organisations. Such codes are often known as inventory numbers, registration codes, etc. and are typically composed of alphanumeric sequences. Postal addresses, telephone numbers, URLs and e-mail addresses are characteristic examples of identifiers used by services transporting things between clients.
The class E42 Identifier is not normally used for machine-generated identifiers used for automated processing unless these are also used by human agents.

Examples:
- “MM.GE.195”
- “13.45.1976”
- “OXCMS: 1997.4.1” (fictitious)
- “ISSN 0041-5278” [Identifier for “The UNESCO Courier (Print)”]
- ISRC “FIFIN8900186” [Identifier for : Kraft (29 min 14 s) / Magnus Lindberg, comp. ; Toimii Ensemble ; Swedish Radio symphony orchestra ; Esa-Pekka Salonen, dir.]
- Shelf mark “Res 8 P 10” 
- “Guillaume de Machaut (1300?-1377)” [a controlled personal name heading that follows the French rules] (Reaney, 1974)
- “+41 22 418 5571”
- “ weasel@paveprime.com”
- “Rue David Dufour 5, CH-1211, Genève”
- “1-29-3 Otsuka, Bunkyo-ku, Tokyo, 121, Japan”

In First Order Logic:
- E42(x) ⇒ E41(x)
</rdfs:comment>
        <rdfs:label xml:lang="fr">E42 Identifiant</rdfs:label>
        <rdfs:label xml:lang="pt">E42 Identificador de Objeto</rdfs:label>
        <rdfs:label xml:lang="en">E42 Identifier</rdfs:label>
        <rdfs:label xml:lang="de">E42 Kennung</rdfs:label>
        <rdfs:label xml:lang="el">E42 Κωδικός Αναγνώρισης</rdfs:label>
        <rdfs:label xml:lang="ru">E42 Идeнтификатор</rdfs:label>
        <rdfs:label xml:lang="zh">E42 标识符</rdfs:label>
        <skos:notation xml:lang="en">E42</skos:notation>
        <skos:prefLabel xml:lang="fr">Identifiant</skos:prefLabel>
        <skos:prefLabel xml:lang="pt">Identificador de Objeto</skos:prefLabel>
        <skos:prefLabel xml:lang="en">Identifier</skos:prefLabel>
        <skos:prefLabel xml:lang="de">Kennung</skos:prefLabel>
        <skos:prefLabel xml:lang="el">Κωδικός Αναγνώρισης</skos:prefLabel>
        <skos:prefLabel xml:lang="ru">Идeнтификатор</skos:prefLabel>
        <skos:prefLabel xml:lang="zh">标识符</skos:prefLabel>
    </owl:Class>
    


    <!-- http://www.cidoc-crm.org/cidoc-crm/E4_Period -->

    <owl:Class rdf:about="http://www.cidoc-crm.org/cidoc-crm/E4_Period">
        <rdfs:subClassOf rdf:resource="http://www.cidoc-crm.org/cidoc-crm/E2_Temporal_Entity"/>
        <rdfs:subClassOf rdf:resource="http://www.cidoc-crm.org/cidoc-crm/E92_Spacetime_Volume"/>
        <rdfs:comment xml:lang="en">Scope note:
This class comprises sets of coherent phenomena or cultural manifestations occurring in time and space.
It is the social or physical coherence of these phenomena that identify an instance of E4 Period and not the associated spatiotemporal extent. This extent is only the “ground” or space in an abstract physical sense that the actual process of growth, spread and retreat has covered. Consequently, different periods can overlap and coexist in time and space, such as when a nomadic culture exists in the same area and time as a sedentary culture. This also means that overlapping land use rights, common among first nations, amounts to overlapping periods.
Often, this class is used to describe prehistoric or historic periods such as the “Neolithic Period”, the “Ming Dynasty” or the “McCarthy Era”, but also geopolitical units and activities of settlements are regarded as special cases of E4 Period. However, there are no assumptions about the scale of the associated phenomena. In particular all events are seen as synthetic processes consisting of coherent phenomena. Therefore, E4 Period is a superclass of E5 Event. For example, a modern clinical birth, an instance of E67 Birth, can be seen as both a single event, i.e. an instance of E5 Event, and as an extended period, i.e. an instance of E4 Period, that consists of multiple physical processes and complementary activities performed by multiple instances of E39 Actor.
E4 Period is a subclass of E2 Temporal Entity and of E92 Spacetime Volume. The latter is intended as a phenomenal spacetime volume as defined in CIDOC CRMgeo (Doerr &amp; Hiebel, 2013). By virtue of this multiple inheritance, it is possible to discuss the physical extent of an instance of E4 Period without representing each instance of it together with an instance of its associated spacetime volume. This model combines two quite different kinds of substance: an instance of E4 Period is a phenomenon while an instance of E92 Spacetime Volume is an aggregation of points in spacetime. However, the real spatiotemporal extent of an instance of E4 Period is regarded to be unique to it due to all its details and fuzziness; its identity and existence depends uniquely on the identity of the instance of E4 Period. Therefore, this multiple inheritance is unambiguous and effective and furthermore corresponds to the intuitions of natural language.
Typical use of this class in cultural heritage documentation is for documenting cultural and artistic periods. There are two different conceptualisations of ‘artistic style’, defined either by physical features or by historical context. For example, “Impressionism” can be viewed as a period in the European sphere of influence lasting from approximately 1870 to 1905 during which paintings with particular characteristics were produced by a group of artists that included (among others) Monet, Renoir, Pissarro, Sisley and Degas. Alternatively, it can be regarded as a style applicable to all paintings sharing the characteristics of the works produced by the Impressionist painters, regardless of historical context. The first interpretation is an instance of E4 Period, and the second defines morphological object types that fall under E55 Type.
A geopolitical unit as a specific case of an instance of E4 Period is the set of activities and phenomena related to the claim of power, the consequences of belonging to a jurisdictional area and an administrative system that establishes a geopolitical unit. Examples from the modern period are countries or administrative areas of countries such as districts whose actions and structures define activities and phenomena in the area that they intend to govern. The borders of geopolitical units are often defined in contracts or treaties although they may deviate from the actual practice. The spatiotemporal properties of Geopolitical units can be modelled through the properties inherited from E92 Spacetime Volume.
Another specific case of an instance of E4 Period is the actual extent of the set of activities and phenomena as evidenced by their physical traces that define a settlement, such as the populated period of Nineveh.

Examples:
- Jurassic (Hallam, 1975)
- Populated Period of Nineveh
- Imperial Rome under Marcus Aurelius
- European Bronze Age (Harrison, 2004) 
- Italian Renaissance (Macdonald, 1992)
- Thirty Years War (Lee, 1991)
- Sturm und Drang (Berkoff, 2013)
- Cubism (Cox, 2000)
- The Capital of Russia (E4) [the capital of Russia in the sense of an administrative unit moved in historical times from Moscow to St Petersburg and then back to Moscow. This exemplifies an administrative unit changing place over time without temporal discontinuity]
- The settling activity of the community of Helsinki (a.k.a. Helsingfors) (E7) [the original settlement called Helsinki was located in the area of the modern airport. The community moved later to settle on the coast. This exemplifies a continued activity changing place over time without temporal discontinuity]
- Bronze Age (E4) [Bronze Age, in the sense of technological adoption, spread over disjoint areas including islands such as the British Isles without temporal discontinuity]
- Japan, the state (E4) [In 2021, the Japanese state as a political unit comprised in 6852 islands extending along the Pacific coast of Asia]

In First Order Logic:
- E4(x) ⇒ E2(x)
- E4(x) ⇒ E92(x)
</rdfs:comment>
        <rdfs:label xml:lang="en">E4 Period</rdfs:label>
        <rdfs:label xml:lang="pt">E4 Período</rdfs:label>
        <rdfs:label xml:lang="de">E4 Phase</rdfs:label>
        <rdfs:label xml:lang="fr">E4 Période</rdfs:label>
        <rdfs:label xml:lang="el">E4 Περίοδος</rdfs:label>
        <rdfs:label xml:lang="ru">E4 Пeриод</rdfs:label>
        <rdfs:label xml:lang="zh">E4 时期</rdfs:label>
        <skos:notation xml:lang="en">E4</skos:notation>
        <skos:prefLabel xml:lang="en">Period</skos:prefLabel>
        <skos:prefLabel xml:lang="pt">Período</skos:prefLabel>
        <skos:prefLabel xml:lang="de">Phase</skos:prefLabel>
        <skos:prefLabel xml:lang="fr">Période</skos:prefLabel>
        <skos:prefLabel xml:lang="el">Περίοδος</skos:prefLabel>
        <skos:prefLabel xml:lang="ru">Пeриод</skos:prefLabel>
        <skos:prefLabel xml:lang="zh">时期</skos:prefLabel>
    </owl:Class>
    


    <!-- http://www.cidoc-crm.org/cidoc-crm/E52_Time-Span -->

    <owl:Class rdf:about="http://www.cidoc-crm.org/cidoc-crm/E52_Time-Span">
        <rdfs:subClassOf rdf:resource="http://www.cidoc-crm.org/cidoc-crm/E1_CRM_Entity"/>
        <rdfs:comment xml:lang="en">Scope note:
This class comprises abstract temporal extents, in the sense of Galilean physics, having a beginning, an end, and a duration. 
Instances of E52 Time-Span have no semantic connotations about phenomena happening within the temporal extent they represent. They do not convey any meaning other than a positioning on the “time-line” of chronology. The actual extent of an instance of E52 Time-Span can be approximated by properties of E52 Time-Span giving inner and outer bounds in the form of dates (instances of E61 Time Primitive). Comparing knowledge about time-spans is fundamental for chronological reasoning.
Some instances of E52 Time-Span may be defined as the actual, in principle observable, temporal extent of instances of E2 Temporal Entity via the property P4 has time-span (is time-span of): E52 Time-Span. They constitute phenomenal time-spans as defined in CRMgeo (Doerr &amp; Hiebel 2013). Since our knowledge of history is imperfect and physical phenomena are fuzzy in nature, the extent of phenomenal time-spans can only be described in approximation. An extreme case of approximation, might, for example, define an instance of E52 Time-Span having unknown beginning, end and duration. It may, nevertheless, be associated with other descriptions by which people can infer knowledge about it, such as in relative chronologies.
Some instances of E52 may be defined precisely as representing a declaration of a temporal extent, as, for instance, done in a business contract. They constitute declarative time-spans as defined in CRMgeo (Doerr &amp; Hiebel 2013) and can be described via the property E61 Time Primitive P170 defines time (time is defined by): E52 Time-Span. 
When used as a common E52 Time-Span for two events, it will nevertheless describe them as being simultaneous, even if nothing else is known.

Examples:
- 1961
- From 12-17-1993 to 12-8-1996
- 14h30 to 16h22 4(th) July 1945
- 9.30 am 1.1.1999 to 2.00 pm 1.1.1999
- the time-span of the Ming Dynasty (Chan, 2011)

In First Order Logic:
- E52(x) ⇒ E1(x)
</rdfs:comment>
        <rdfs:label xml:lang="fr">E52 Intervalle temporel</rdfs:label>
        <rdfs:label xml:lang="pt">E52 Período de Tempo</rdfs:label>
        <rdfs:label xml:lang="en">E52 Time-Span</rdfs:label>
        <rdfs:label xml:lang="de">E52 Zeitspanne</rdfs:label>
        <rdfs:label xml:lang="el">E52 Χρονικό Διάστημα</rdfs:label>
        <rdfs:label xml:lang="ru">E52 Интeрвал Врeмeни</rdfs:label>
        <rdfs:label xml:lang="zh">E52 时段</rdfs:label>
        <skos:notation xml:lang="en">E52</skos:notation>
        <skos:prefLabel xml:lang="fr">Intervalle temporel</skos:prefLabel>
        <skos:prefLabel xml:lang="pt">Período de Tempo</skos:prefLabel>
        <skos:prefLabel xml:lang="en">Time-Span</skos:prefLabel>
        <skos:prefLabel xml:lang="de">Zeitspanne</skos:prefLabel>
        <skos:prefLabel xml:lang="el">Χρονικό Διάστημα</skos:prefLabel>
        <skos:prefLabel xml:lang="ru">Интeрвал Врeмeни</skos:prefLabel>
        <skos:prefLabel xml:lang="zh">时段</skos:prefLabel>
    </owl:Class>
    


    <!-- http://www.cidoc-crm.org/cidoc-crm/E53_Place -->

    <owl:Class rdf:about="http://www.cidoc-crm.org/cidoc-crm/E53_Place">
        <rdfs:subClassOf rdf:resource="http://www.cidoc-crm.org/cidoc-crm/E1_CRM_Entity"/>
        <rdfs:comment xml:lang="en">Scope note:
This class comprises extents in the natural space where people live, in particular on the surface of the Earth, in the pure sense of physics: independent from temporal phenomena and matter. They may serve describing the physical location of things or phenomena or other areas of interest. Geometrically, instances of E53 Place constitute single contiguous areas or a finite aggregation of disjoint areas in space which are each individually contiguous. They may have fuzzy boundaries.
The instances of E53 Place are usually determined by reference to the position of “immobile” objects such as buildings, cities, mountains, rivers, or dedicated geodetic marks, but may also be determined by reference to mobile objects. A Place can be determined by combining a frame of reference and a location with respect to this frame.
It is sometimes argued that instances of E53 Place are best identified by global coordinates or absolute reference systems. However, relative references are often more relevant in the context of cultural documentation and tend to be more precise. In particular, people are often interested in position in relation to large, mobile objects, such as ships. For example, the Place at which Nelson died is known with reference to a large mobile object, i.e. H.M.S Victory. A resolution of this Place in terms of absolute coordinates would require knowledge of the movements of the vessel and the precise time of death, either of which may be revised, and the result would lack historical and cultural relevance.
Any instance of E18 Physical Thing can serve as a frame of reference for an instance of E53 Place. This may be documented using the property P157 is at rest relative to (provides reference space for).

Examples:
- the extent of the UK in the year 2003
- the position of the hallmark on the inside of my wedding ring (fictitious)
- the place referred to in the phrase: “Fish collected at three miles north of the confluence of the Arve and the Rhone”
- here -&gt; &lt;- [the place between these two arrows in one of the reader&apos;s paper copy of this document. Each copy constitutes a different place of this spot.]

In First Order Logic:
- E53(x) ⇒ E1(x)
</rdfs:comment>
        <rdfs:label xml:lang="fr">E53 Lieu</rdfs:label>
        <rdfs:label xml:lang="pt">E53 Local</rdfs:label>
        <rdfs:label xml:lang="de">E53 Ort</rdfs:label>
        <rdfs:label xml:lang="en">E53 Place</rdfs:label>
        <rdfs:label xml:lang="el">E53 Τόπος</rdfs:label>
        <rdfs:label xml:lang="ru">E53 Мeсто</rdfs:label>
        <rdfs:label xml:lang="zh">E53 地点</rdfs:label>
        <skos:notation xml:lang="en">E53</skos:notation>
        <skos:prefLabel xml:lang="fr">Lieu</skos:prefLabel>
        <skos:prefLabel xml:lang="pt">Local</skos:prefLabel>
        <skos:prefLabel xml:lang="de">Ort</skos:prefLabel>
        <skos:prefLabel xml:lang="en">Place</skos:prefLabel>
        <skos:prefLabel xml:lang="el">Τόπος</skos:prefLabel>
        <skos:prefLabel xml:lang="ru">Мeсто</skos:prefLabel>
        <skos:prefLabel xml:lang="zh">地点</skos:prefLabel>
    </owl:Class>
    


    <!-- http://www.cidoc-crm.org/cidoc-crm/E54_Dimension -->

    <owl:Class rdf:about="http://www.cidoc-crm.org/cidoc-crm/E54_Dimension">
        <rdfs:subClassOf rdf:resource="http://www.cidoc-crm.org/cidoc-crm/E1_CRM_Entity"/>
        <rdfs:comment xml:lang="en">Scope note:
This class comprises quantifiable properties that can be measured by some calibrated means and can be approximated by values, i.e. points or regions in a mathematical or conceptual space, such as natural or real numbers, RGB values, etc.
An instance of E54 Dimension represents the empirical or theoretically derived quantity, including the precision tolerances resulting from the particular method or calculation. The identity of an instance of E54 Dimension depends on the method of its determination because each method may produce different values even when determining comparable qualities. For instance, the wingspan of a bird alive or dead is a different dimension. Thermoluminescence dating and Rehydroxylation [RHX] dating are different dimensions of temporal distance from now, even if they aim at dating the same object. The method of determination should be expressed using the property P2 has type (is type of). Note that simple terms such as “diameter” or “length” are normally insufficient to unambiguously describe a respective dimension. In contrast, “maximum linear extent” may be sufficient.
The properties of the class E54 Dimension allow for expressing the numerical approximation of the values of instances of E54 Dimension adequate to the precision of the applied method of determination. If the respective quantity belongs to a non-discrete space according to the laws of physics, such as spatial distances, it is recommended to record them as approximations by intervals or regions of indeterminacy enclosing the assumed true values. For instance, a length of 5 cm may be recorded as 4.5-5.5 cm, according to the precision of the respective observation. Note, that comparability of values described in different units depends critically on the representation as value regions.
Numerical approximations in archaic instances of E58 Measurement Unit used in historical records should be preserved. Equivalents corresponding to current knowledge should be recorded as additional instances of E54 Dimension, as appropriate.

Examples:
- the weight of the Luxor Obelisk [250 metric tons]
- the vertical height of the statue of David by Michelangelo [5.17 metres]
- the weight of the Great Star of Africa diamond [530.2 carats]
- the calibrated C14 date for the Shroud of Turin [AD1262-1312, 1303-1384]
- the horizontal diameter of the Stonehenge Sarsen Circle [33 metres] (Pryor, 2016)
- the length of the sides of the Great Pyramid at Giza [230.34 metres] (Lehner and Hawass, 2017)
- the duration of the time-span of the Battle of Issos/Issus on 15(th) November 333 B.C.E. [less than 12 hours] (Howard, 2012)
- Christie’s hammer price, in British Pounds, for Vincent van Gogh&apos;s &quot;Still Life: Vase with Fifteen Sunflowers&quot; in London on 30(th) March 1987 (E97) [24.75 million GBP (British Pounds)]

In First Order Logic:
- E54(x) ⇒ E1(x)
</rdfs:comment>
        <rdfs:label xml:lang="en">E54 Dimension</rdfs:label>
        <rdfs:label xml:lang="fr">E54 Dimension</rdfs:label>
        <rdfs:label xml:lang="pt">E54 Dimensão</rdfs:label>
        <rdfs:label xml:lang="de">E54 Maß</rdfs:label>
        <rdfs:label xml:lang="el">E54 Μέγεθος</rdfs:label>
        <rdfs:label xml:lang="ru">E54 Размeр</rdfs:label>
        <rdfs:label xml:lang="zh">E54 度量规格</rdfs:label>
        <skos:notation xml:lang="en">E54</skos:notation>
        <skos:prefLabel xml:lang="en">Dimension</skos:prefLabel>
        <skos:prefLabel xml:lang="fr">Dimension</skos:prefLabel>
        <skos:prefLabel xml:lang="pt">Dimensão</skos:prefLabel>
        <skos:prefLabel xml:lang="de">Maß</skos:prefLabel>
        <skos:prefLabel xml:lang="el">Μέγεθος</skos:prefLabel>
        <skos:prefLabel xml:lang="ru">Размeр</skos:prefLabel>
        <skos:prefLabel xml:lang="zh">度量规格</skos:prefLabel>
    </owl:Class>
    


    <!-- http://www.cidoc-crm.org/cidoc-crm/E55_Type -->

    <owl:Class rdf:about="http://www.cidoc-crm.org/cidoc-crm/E55_Type">
        <rdfs:subClassOf rdf:resource="http://www.cidoc-crm.org/cidoc-crm/E28_Conceptual_Object"/>
        <rdfs:comment xml:lang="en">Scope note:
This class comprises concepts denoted by terms from thesauri and controlled vocabularies used to characterize and classify instances of CIDOC CRM classes. Instances of E55 Type represent concepts, in contrast to instances of E41 Appellation which are used to name instances of CIDOC CRM classes. 
E55 Type provides an interface to domain specific ontologies and thesauri. These can be represented in the CIDOC CRM as subclasses of E55 Type, forming hierarchies of terms, i.e. instances of E55 Type linked via P127 has broader term (has narrower term): E55 Type. Such hierarchies may be extended with additional properties.

Examples:
- weight, length, depth [types for instances of E54 Dimension]
- portrait, sketch, animation [types for instances of E36 Visual Item]
- French, English, German [types for instances of E56 Language]
- excellent, good, poor [types for instances of E3 Condition State]
- Ford Model T, chop stick [types for instances of E22 Human-Made Object]
- cave, doline, scratch [types for instances of E26 Physical Feature]
- poem, short story [types for instances of E33 Linguistic Object]
- wedding, earthquake, skirmish [types for instances of E5 Event]

In First Order Logic:
- E55(x) ⇒ E28(x)
</rdfs:comment>
        <rdfs:label xml:lang="pt">E55 Tipo</rdfs:label>
        <rdfs:label xml:lang="en">E55 Type</rdfs:label>
        <rdfs:label xml:lang="fr">E55 Type</rdfs:label>
        <rdfs:label xml:lang="de">E55 Typus</rdfs:label>
        <rdfs:label xml:lang="ru">E55 Tип</rdfs:label>
        <rdfs:label xml:lang="el">E55 Τύπος</rdfs:label>
        <rdfs:label xml:lang="zh">E55 类型</rdfs:label>
        <skos:notation xml:lang="en">E55</skos:notation>
        <skos:prefLabel xml:lang="pt">Tipo</skos:prefLabel>
        <skos:prefLabel xml:lang="en">Type</skos:prefLabel>
        <skos:prefLabel xml:lang="fr">Type</skos:prefLabel>
        <skos:prefLabel xml:lang="de">Typus</skos:prefLabel>
        <skos:prefLabel xml:lang="ru">Tип</skos:prefLabel>
        <skos:prefLabel xml:lang="el">Τύπος</skos:prefLabel>
        <skos:prefLabel xml:lang="zh">类型</skos:prefLabel>
    </owl:Class>
    


    <!-- http://www.cidoc-crm.org/cidoc-crm/E57_Material -->

    <owl:Class rdf:about="http://www.cidoc-crm.org/cidoc-crm/E57_Material">
        <rdfs:subClassOf rdf:resource="http://www.cidoc-crm.org/cidoc-crm/E55_Type"/>
        <rdfs:comment xml:lang="en">Scope note:
This class is a specialization of E55 Type and comprises the concepts of materials. 
Instances of E57 Material may denote properties of matter before its use, during its use, and as incorporated in an object, such as ultramarine powder, tempera paste, reinforced concrete. Discrete pieces of raw-materials kept in museums, such as bricks, sheets of fabric, pieces of metal, should be modelled individually in the same way as other objects. Discrete used or processed pieces, such as the stones from Nefer Titi&apos;s temple, should be modelled as parts (cf. P46 is composed of (forms part of): E18 Physical Thing).
This type is used categorically in the model without reference to instances of it, i.e. the Model does not foresee the description of instances of instances of E57 Material, e.g. “instances of gold”.
It is recommended that internationally or nationally agreed codes and terminology should be used.

Examples:
- brick (Gurcke, 1987)
- gold (Watson, 1990)
- aluminium (Norman, 1986)
- polycarbonate (Mhaske, 2011)
- resin (Barton, 1992)

In First Order Logic:
- E57(x) ⇒ E55(x)
</rdfs:comment>
        <rdfs:label xml:lang="de">E57 Material</rdfs:label>
        <rdfs:label xml:lang="en">E57 Material</rdfs:label>
        <rdfs:label xml:lang="pt">E57 Material</rdfs:label>
        <rdfs:label xml:lang="fr">E57 Matériau</rdfs:label>
        <rdfs:label xml:lang="el">E57 Υλικό</rdfs:label>
        <rdfs:label xml:lang="ru">E57 Матeриал</rdfs:label>
        <rdfs:label xml:lang="zh">E57 材质</rdfs:label>
        <skos:notation xml:lang="en">E57</skos:notation>
        <skos:prefLabel xml:lang="de">Material</skos:prefLabel>
        <skos:prefLabel xml:lang="en">Material</skos:prefLabel>
        <skos:prefLabel xml:lang="pt">Material</skos:prefLabel>
        <skos:prefLabel xml:lang="fr">Matériau</skos:prefLabel>
        <skos:prefLabel xml:lang="el">Υλικό</skos:prefLabel>
        <skos:prefLabel xml:lang="ru">Матeриал</skos:prefLabel>
        <skos:prefLabel xml:lang="zh">材质</skos:prefLabel>
    </owl:Class>
    


    <!-- http://www.cidoc-crm.org/cidoc-crm/E58_Measurement_Unit -->

    <owl:Class rdf:about="http://www.cidoc-crm.org/cidoc-crm/E58_Measurement_Unit">
        <rdfs:subClassOf rdf:resource="http://www.cidoc-crm.org/cidoc-crm/E55_Type"/>
        <rdfs:comment xml:lang="en">Scope note:
This class is a specialization of E55 Type and comprises the types of measurement units: feet, inches, centimetres, litres, lumens, etc. 
This type is used categorically in the model without reference to instances of it, i.e. the model does not foresee the description of instances of instances of E58 Measurement Unit, e.g. “instances of cm”.
Système International (SI) units or internationally recognized non-SI terms should be used whenever possible, such as those defined by ISO80000:2009. Archaic Measurement Units used in historical records should be preserved.

Examples:
- cm [centimetre]
- km [kilometre]
- m [metre]
- m/s [metres per second] (Hau et al., 1999)
- A [ampere]
- GRD [Greek Drachma] (E98) (Daniel, 2014)
- C [degrees centigrade] (Beckman, 1998)

In First Order Logic:
- E58(x) ⇒ E55(x)
</rdfs:comment>
        <rdfs:label xml:lang="ru">E58 Eдиница Измeрeния</rdfs:label>
        <rdfs:label xml:lang="de">E58 Maßeinheit</rdfs:label>
        <rdfs:label xml:lang="en">E58 Measurement Unit</rdfs:label>
        <rdfs:label xml:lang="pt">E58 Unidade de Medida</rdfs:label>
        <rdfs:label xml:lang="fr">E58 Unité de mesure</rdfs:label>
        <rdfs:label xml:lang="el">E58 Μονάδα Μέτρησης</rdfs:label>
        <rdfs:label xml:lang="zh">E58 测量单位</rdfs:label>
        <skos:notation xml:lang="en">E58</skos:notation>
        <skos:prefLabel xml:lang="ru">Eдиница Измeрeния</skos:prefLabel>
        <skos:prefLabel xml:lang="de">Maßeinheit</skos:prefLabel>
        <skos:prefLabel xml:lang="en">Measurement Unit</skos:prefLabel>
        <skos:prefLabel xml:lang="pt">Unidade de Medida</skos:prefLabel>
        <skos:prefLabel xml:lang="fr">Unité de mesure</skos:prefLabel>
        <skos:prefLabel xml:lang="el">Μονάδα Μέτρησης</skos:prefLabel>
        <skos:prefLabel xml:lang="zh">测量单位</skos:prefLabel>
    </owl:Class>
    


    <!-- http://www.cidoc-crm.org/cidoc-crm/E5_Event -->

    <owl:Class rdf:about="http://www.cidoc-crm.org/cidoc-crm/E5_Event">
        <rdfs:subClassOf rdf:resource="http://www.cidoc-crm.org/cidoc-crm/E4_Period"/>
        <rdfs:comment xml:lang="en">Scope note:
This class comprises distinct, delimited and coherent processes and interactions of a material nature, in cultural, social or physical systems, involving and affecting instances of E77 Persistent Item in a way characteristic of the kind of process. Typical examples are meetings, births, deaths, actions of decision taking, making or inventing things, but also more complex and extended ones such as conferences, elections, building of a castle, or battles.
While the continuous growth of a tree lacks the limits characteristic of an event, its germination from a seed does qualify as an event. Similarly, the blowing of the wind lacks the distinctness and limits of an event, but a hurricane, flood or earthquake would qualify as an event. Mental processes are considered as events, in cases where they are connected with the material externalization of their results; for example, the creation of a poem, a performance or a change of intention that becomes obvious from subsequent actions or declarations.
The effects of an instance of E5 Event may not lead to relevant permanent changes of properties or relations of the items involved in it, for example an unrecorded performance. Of course, in order to be documented, some kind of evidence for an event must exist, be it witnesses, traces or products of the event.
While instances of E4 Period always require some form of coherence between its constituent phenomena, in addition, the essential constituents of instances of E5 Event should contribute to an overall effect; for example, the statements made during a meeting and the listening of the audience.
Viewed at a coarse level of detail, an instance of E5 Event may appear as if it had an ‘instantaneous’ overall effect, but any process or interaction of material nature in reality have an extent in time and space. At a fine level, instances of E5 Event may be analysed into component phenomena and phases within a space and timeframe, and as such can be seen as a period, regardless of the size of the phenomena. The reverse is not necessarily the case: not all instances of E4 Period give rise to a noteworthy overall effect and are thus not instances of E5 Event.

Examples:
- the birth of Cleopatra (E67) (Pomeroy, 1984)
- the destruction of Herculaneum by volcanic eruption in 79 AD (E6) (Camardo, 2013)
- World War II (E7) (Barber, 1994)
- the Battle of Stalingrad (E7) (Hoyt, 1993)
- the Yalta Conference (E7) (Harbutt, 2010)
- my birthday celebration 28-6-1995 (E7)
- the falling of a tile from my roof last Sunday (fictitious)
- the CIDOC conference 2003 (E7)

In First Order Logic:
- E5(x) ⇒ E4(x)
</rdfs:comment>
        <rdfs:label xml:lang="de">E5 Ereignis</rdfs:label>
        <rdfs:label xml:lang="en">E5 Event</rdfs:label>
        <rdfs:label xml:lang="pt">E5 Evento</rdfs:label>
        <rdfs:label xml:lang="fr">E5 Évènement</rdfs:label>
        <rdfs:label xml:lang="el">E5 Συμβάν</rdfs:label>
        <rdfs:label xml:lang="ru">E5 Событиe</rdfs:label>
        <rdfs:label xml:lang="zh">E5 事件</rdfs:label>
        <skos:notation xml:lang="en">E5</skos:notation>
        <skos:prefLabel xml:lang="de">Ereignis</skos:prefLabel>
        <skos:prefLabel xml:lang="en">Event</skos:prefLabel>
        <skos:prefLabel xml:lang="pt">Evento</skos:prefLabel>
        <skos:prefLabel xml:lang="fr">Évènement</skos:prefLabel>
        <skos:prefLabel xml:lang="el">Συμβάν</skos:prefLabel>
        <skos:prefLabel xml:lang="ru">Событиe</skos:prefLabel>
        <skos:prefLabel xml:lang="zh">事件</skos:prefLabel>
    </owl:Class>
    


    <!-- http://www.cidoc-crm.org/cidoc-crm/E63_Beginning_of_Existence -->

    <owl:Class rdf:about="http://www.cidoc-crm.org/cidoc-crm/E63_Beginning_of_Existence">
        <rdfs:subClassOf rdf:resource="http://www.cidoc-crm.org/cidoc-crm/E5_Event"/>
        <rdfs:comment xml:lang="en">Scope note:
This class comprises events that bring into existence any instance of E77 Persistent Item. 
It may be used for temporal reasoning about things (intellectual products, physical items, groups of people, living beings) beginning to exist; it serves as a hook for both a terminus post quem and a terminus ante quem.

Examples:
- the birth of my child (E67) (fictitious)
- the birth of Snoopy, my dog (fictitious)
- the calving of the iceberg that sank the Titanic
- the construction of the Eiffel Tower (E12) (Tissandier, 1889)

In First Order Logic:
- E63(x) ⇒ E5(x)
</rdfs:comment>
        <rdfs:label xml:lang="en">E63 Beginning of Existence</rdfs:label>
        <rdfs:label xml:lang="de">E63 Daseinsbeginn</rdfs:label>
        <rdfs:label xml:lang="fr">E63 Début d’existence</rdfs:label>
        <rdfs:label xml:lang="pt">E63 Início da Existência</rdfs:label>
        <rdfs:label xml:lang="el">E63 Αρχή Ύπαρξης</rdfs:label>
        <rdfs:label xml:lang="ru">E63 Начало Сущeствования</rdfs:label>
        <rdfs:label xml:lang="zh">E63 初始</rdfs:label>
        <skos:notation xml:lang="en">E63</skos:notation>
        <skos:prefLabel xml:lang="en">Beginning of Existence</skos:prefLabel>
        <skos:prefLabel xml:lang="de">Daseinsbeginn</skos:prefLabel>
        <skos:prefLabel xml:lang="fr">Début d’existence</skos:prefLabel>
        <skos:prefLabel xml:lang="pt">Início da Existência</skos:prefLabel>
        <skos:prefLabel xml:lang="el">Αρχή Ύπαρξης</skos:prefLabel>
        <skos:prefLabel xml:lang="ru">Начало Сущeствования</skos:prefLabel>
        <skos:prefLabel xml:lang="zh">初始</skos:prefLabel>
    </owl:Class>
    


    <!-- http://www.cidoc-crm.org/cidoc-crm/E64_End_of_Existence -->

    <owl:Class rdf:about="http://www.cidoc-crm.org/cidoc-crm/E64_End_of_Existence">
        <rdfs:subClassOf rdf:resource="http://www.cidoc-crm.org/cidoc-crm/E5_Event"/>
        <rdfs:comment xml:lang="en">Scope note:
This class comprises events that end the existence of any instance of E77 Persistent Item. 
It may be used for temporal reasoning about things (physical items, groups of people, living beings) ceasing to exist; it serves as a hook both a terminus post quem and a terminus ante quem. In cases where substance from an instance of E77 Persistent Item continues to exist in a new form, the process would be documented as instances of E81 Transformation.

Examples:
- the death of Snoopy, my dog (fictitious)
- the melting of the snowman (E6)
- the burning of the Temple of Artemis in Ephesos by Herostratos in 356 BC (E7, E6) (Trell, 1945)

In First Order Logic:
- E64(x) ⇒ E5(x)
</rdfs:comment>
        <rdfs:label xml:lang="de">E64 Daseinsende</rdfs:label>
        <rdfs:label xml:lang="en">E64 End of Existence</rdfs:label>
        <rdfs:label xml:lang="pt">E64 Fim da Existência</rdfs:label>
        <rdfs:label xml:lang="fr">E64 Fin d’existence</rdfs:label>
        <rdfs:label xml:lang="el">E64 Τέλος Ύπαρξης</rdfs:label>
        <rdfs:label xml:lang="ru">E64 Конeц Сущeствования</rdfs:label>
        <rdfs:label xml:lang="zh">E64 结束</rdfs:label>
        <skos:notation xml:lang="en">E64</skos:notation>
        <skos:prefLabel xml:lang="de">Daseinsende</skos:prefLabel>
        <skos:prefLabel xml:lang="en">End of Existence</skos:prefLabel>
        <skos:prefLabel xml:lang="pt">Fim da Existência</skos:prefLabel>
        <skos:prefLabel xml:lang="fr">Fin d’existence</skos:prefLabel>
        <skos:prefLabel xml:lang="el">Τέλος Ύπαρξης</skos:prefLabel>
        <skos:prefLabel xml:lang="ru">Конeц Сущeствования</skos:prefLabel>
        <skos:prefLabel xml:lang="zh">结束</skos:prefLabel>
    </owl:Class>
    


    <!-- http://www.cidoc-crm.org/cidoc-crm/E65_Creation -->

    <owl:Class rdf:about="http://www.cidoc-crm.org/cidoc-crm/E65_Creation">
        <rdfs:subClassOf rdf:resource="http://www.cidoc-crm.org/cidoc-crm/E63_Beginning_of_Existence"/>
        <rdfs:subClassOf rdf:resource="http://www.cidoc-crm.org/cidoc-crm/E7_Activity"/>
        <rdfs:comment xml:lang="en">Scope note:
This class comprises events that result in the creation of conceptual items or immaterial products, such as legends, poems, texts, music, images, movies, laws, types, etc.

Examples:
- the framing of the U.S. Constitution (Farrand, 1913)
- the drafting of U.N. Resolution 1441 (United Nations Security Council, 2002)

In First Order Logic:
- E65(x) ⇒ E7(x)
- E65(x) ⇒ E63(x)
</rdfs:comment>
        <rdfs:label xml:lang="de">E65 Begriffliche Schöpfung</rdfs:label>
        <rdfs:label xml:lang="en">E65 Creation</rdfs:label>
        <rdfs:label xml:lang="pt">E65 Criação</rdfs:label>
        <rdfs:label xml:lang="fr">E65 Création</rdfs:label>
        <rdfs:label xml:lang="el">E65 Δημιουργία</rdfs:label>
        <rdfs:label xml:lang="ru">E65 Созданиe</rdfs:label>
        <rdfs:label xml:lang="zh">E65 创建</rdfs:label>
        <skos:notation xml:lang="en">E65</skos:notation>
        <skos:prefLabel xml:lang="de">Begriffliche Schöpfung</skos:prefLabel>
        <skos:prefLabel xml:lang="en">Creation</skos:prefLabel>
        <skos:prefLabel xml:lang="pt">Criação</skos:prefLabel>
        <skos:prefLabel xml:lang="fr">Création</skos:prefLabel>
        <skos:prefLabel xml:lang="el">Δημιουργία</skos:prefLabel>
        <skos:prefLabel xml:lang="ru">Созданиe</skos:prefLabel>
        <skos:prefLabel xml:lang="zh">创建</skos:prefLabel>
    </owl:Class>
    


    <!-- http://www.cidoc-crm.org/cidoc-crm/E67_Birth -->

    <owl:Class rdf:about="http://www.cidoc-crm.org/cidoc-crm/E67_Birth">
        <rdfs:subClassOf rdf:resource="http://www.cidoc-crm.org/cidoc-crm/E63_Beginning_of_Existence"/>
        <rdfs:comment xml:lang="en">Scope note:
This class comprises the births of human beings. E67 Birth is a biological event focussing on the context of people coming into life. (E63 Beginning of Existence comprises the coming into life of any living being.) 
Twins, triplets, etc. are brought into life by the same instance of E67 Birth. The introduction of the E67 Birth event as a documentation element allows the description of a range of family relationships in a simple model. Suitable extensions may describe more details and the complexity of motherhood since the advent of modern medicine. In this model, the biological father is not seen as a necessary participant in the E67 Birth.

Examples:
- the birth of Alexander the Great (Stoneman, 2004)

In First Order Logic:
- E67(x) ⇒ E63(x)
</rdfs:comment>
        <rdfs:label xml:lang="en">E67 Birth</rdfs:label>
        <rdfs:label xml:lang="de">E67 Geburt</rdfs:label>
        <rdfs:label xml:lang="fr">E67 Naissance</rdfs:label>
        <rdfs:label xml:lang="pt">E67 Nascimento</rdfs:label>
        <rdfs:label xml:lang="el">E67 Γέννηση</rdfs:label>
        <rdfs:label xml:lang="ru">E67 Рождeниe</rdfs:label>
        <rdfs:label xml:lang="zh">E67 出生</rdfs:label>
        <skos:notation xml:lang="en">E67</skos:notation>
        <skos:prefLabel xml:lang="en">Birth</skos:prefLabel>
        <skos:prefLabel xml:lang="de">Geburt</skos:prefLabel>
        <skos:prefLabel xml:lang="fr">Naissance</skos:prefLabel>
        <skos:prefLabel xml:lang="pt">Nascimento</skos:prefLabel>
        <skos:prefLabel xml:lang="el">Γέννηση</skos:prefLabel>
        <skos:prefLabel xml:lang="ru">Рождeниe</skos:prefLabel>
        <skos:prefLabel xml:lang="zh">出生</skos:prefLabel>
    </owl:Class>
    


    <!-- http://www.cidoc-crm.org/cidoc-crm/E69_Death -->

    <owl:Class rdf:about="http://www.cidoc-crm.org/cidoc-crm/E69_Death">
        <rdfs:subClassOf rdf:resource="http://www.cidoc-crm.org/cidoc-crm/E64_End_of_Existence"/>
        <rdfs:comment xml:lang="en">Scope note:
This class comprises the deaths of human beings. 
If a person is killed, their death should be instantiated as E69 Death and as E7 Activity. The death or perishing of other living beings should be documented as instances of E64 End of Existence.

Examples:
- the murder of Julius Caesar (E69, E7) (Irwin, 1935)
- the death of Senator Paul Wellstone (Monast and Tao, 2002)

In First Order Logic:
- E69(x) ⇒ E64(x)
</rdfs:comment>
        <rdfs:label xml:lang="en">E69 Death</rdfs:label>
        <rdfs:label xml:lang="fr">E69 Mort</rdfs:label>
        <rdfs:label xml:lang="pt">E69 Morte</rdfs:label>
        <rdfs:label xml:lang="de">E69 Tod</rdfs:label>
        <rdfs:label xml:lang="el">E69 Θάνατος</rdfs:label>
        <rdfs:label xml:lang="ru">E69 Смeрть</rdfs:label>
        <rdfs:label xml:lang="zh">E69 死亡</rdfs:label>
        <skos:notation xml:lang="en">E69</skos:notation>
        <skos:prefLabel xml:lang="en">Death</skos:prefLabel>
        <skos:prefLabel xml:lang="fr">Mort</skos:prefLabel>
        <skos:prefLabel xml:lang="pt">Morte</skos:prefLabel>
        <skos:prefLabel xml:lang="de">Tod</skos:prefLabel>
        <skos:prefLabel xml:lang="el">Θάνατος</skos:prefLabel>
        <skos:prefLabel xml:lang="ru">Смeрть</skos:prefLabel>
        <skos:prefLabel xml:lang="zh">死亡</skos:prefLabel>
    </owl:Class>
    


    <!-- http://www.cidoc-crm.org/cidoc-crm/E70_Thing -->

    <owl:Class rdf:about="http://www.cidoc-crm.org/cidoc-crm/E70_Thing">
        <rdfs:subClassOf rdf:resource="http://www.cidoc-crm.org/cidoc-crm/E77_Persistent_Item"/>
        <rdfs:comment xml:lang="en">Scope note:
This general class comprises discrete, identifiable, instances of E77 Persistent Item that are documented as single units, that either consist of matter or depend on being carried by matter and are characterized by relative stability. 
They may be intellectual products or physical things. They may, for instance, have a solid physical form, an electronic encoding, or they may be a logical concept or structure.

Examples:
- my photograph collection (E78) (fictitious)
- the bottle of milk in my refrigerator (E22) (fictitious)
- the Riss A1 plan of the Straßburger Münster (French: Cathédrale Notre-Dame de Strasbourg) (E29) (Liess, R., 1985)
- the thing on the top of Otto Hahn’s desk (E19)
- the form of the no-smoking sign (E36)
- the cave of Dirou, Mani, Greece (E26) (Psimenos, 2005)

In First Order Logic:
- E70(x) ⇒ E77(x)
</rdfs:comment>
        <rdfs:label xml:lang="fr">E70 Chose</rdfs:label>
        <rdfs:label xml:lang="pt">E70 Coisa</rdfs:label>
        <rdfs:label xml:lang="de">E70 Sache</rdfs:label>
        <rdfs:label xml:lang="en">E70 Thing</rdfs:label>
        <rdfs:label xml:lang="el">E70 Πράγμα</rdfs:label>
        <rdfs:label xml:lang="ru">E70 Вeщь</rdfs:label>
        <rdfs:label xml:lang="zh">E70 事物</rdfs:label>
        <skos:notation xml:lang="en">E70</skos:notation>
        <skos:prefLabel xml:lang="fr">Chose</skos:prefLabel>
        <skos:prefLabel xml:lang="pt">Coisa</skos:prefLabel>
        <skos:prefLabel xml:lang="de">Sache</skos:prefLabel>
        <skos:prefLabel xml:lang="en">Thing</skos:prefLabel>
        <skos:prefLabel xml:lang="el">Πράγμα</skos:prefLabel>
        <skos:prefLabel xml:lang="ru">Вeщь</skos:prefLabel>
        <skos:prefLabel xml:lang="zh">事物</skos:prefLabel>
    </owl:Class>
    


    <!-- http://www.cidoc-crm.org/cidoc-crm/E71_Human-Made_Thing -->

    <owl:Class rdf:about="http://www.cidoc-crm.org/cidoc-crm/E71_Human-Made_Thing">
        <rdfs:subClassOf rdf:resource="http://www.cidoc-crm.org/cidoc-crm/E70_Thing"/>
        <rdfs:comment xml:lang="en">Scope note:
This class comprises discrete, identifiable human-made items that are documented as single units. 
These items are either intellectual products or human-made physical things, and are characterized by relative stability. They may, for instance, have a solid physical form, an electronic encoding, or they may be logical concepts or structures.

Examples:
- Beethoven’s 5(th) Symphony (E73) (Lockwood, 2015)
- Michelangelo’s David (E22) (Paoletti and Bagemihl, 2015)
- Einstein’s Theory of General Relativity (E89) (Hartle, 2003)
- the taxon ‘Fringilla coelebs Linnaeus,1758’ (E55) (Sinkevicius and Narusevicius, 2002)

In First Order Logic:
- E71(x) ⇒ E70(x)
</rdfs:comment>
        <rdfs:label xml:lang="fr">E71 Chose élaborée par l’humain</rdfs:label>
        <rdfs:label xml:lang="en">E71 Human-Made Thing</rdfs:label>
        <rdfs:label xml:lang="ru">E71 Рукотворный Прeдмeт</rdfs:label>
        <skos:notation xml:lang="en">E71</skos:notation>
        <skos:prefLabel xml:lang="fr">Chose élaborée par l’humain</skos:prefLabel>
        <skos:prefLabel xml:lang="en">Human-Made Thing</skos:prefLabel>
        <skos:prefLabel xml:lang="ru">Рукотворный Прeдмeт</skos:prefLabel>
    </owl:Class>
    


    <!-- http://www.cidoc-crm.org/cidoc-crm/E72_Legal_Object -->

    <owl:Class rdf:about="http://www.cidoc-crm.org/cidoc-crm/E72_Legal_Object">
        <owl:equivalentClass rdf:resource="http://www.w3.org/ns/odrl/2/Asset"/>
        <rdfs:subClassOf rdf:resource="http://www.cidoc-crm.org/cidoc-crm/E70_Thing"/>
        <rdfs:comment xml:lang="en">Scope note:
This class comprises those material or immaterial items to which instances of E30 Right, such as the right of ownership or use, can be applied. 
This is generally true for all instances of E18 Physical Thing. In the case of instances of E28 Conceptual Object, however, the identity of an instance of E28 Conceptual Object or the method of its use may be too ambiguous to reliably establish instances of E30 Right, as in the case of taxa and inspirations. Ownership of corporations is currently regarded as out of scope of the CIDOC CRM.

Examples:
- the Cullinan diamond (E19) (Scarratt and Shor, 2006)
- definition of the CIDOC Conceptual Reference Model Version 5.0.4 (E73) (ISO 21127: 2014)

In First Order Logic:
- E72(x) ⇒ E70(x)
</rdfs:comment>
        <rdfs:label xml:lang="en">E72 Legal Object</rdfs:label>
        <rdfs:label xml:lang="fr">E72 Objet juridique</rdfs:label>
        <rdfs:label xml:lang="pt">E72 Objeto Jurídico</rdfs:label>
        <rdfs:label xml:lang="de">E72 Rechtsobjekt</rdfs:label>
        <rdfs:label xml:lang="el">E72 Νομικό Αντικείμενο</rdfs:label>
        <rdfs:label xml:lang="ru">E72 Объeкт Права</rdfs:label>
        <rdfs:label xml:lang="zh">E72 法律对象</rdfs:label>
        <skos:notation xml:lang="en">E72</skos:notation>
        <skos:prefLabel xml:lang="en">Legal Object</skos:prefLabel>
        <skos:prefLabel xml:lang="fr">Objet juridique</skos:prefLabel>
        <skos:prefLabel xml:lang="pt">Objeto Jurídico</skos:prefLabel>
        <skos:prefLabel xml:lang="de">Rechtsobjekt</skos:prefLabel>
        <skos:prefLabel xml:lang="el">Νομικό Αντικείμενο</skos:prefLabel>
        <skos:prefLabel xml:lang="ru">Объeкт Права</skos:prefLabel>
        <skos:prefLabel xml:lang="zh">法律对象</skos:prefLabel>
    </owl:Class>
    


    <!-- http://www.cidoc-crm.org/cidoc-crm/E73_Information_Object -->

    <owl:Class rdf:about="http://www.cidoc-crm.org/cidoc-crm/E73_Information_Object">
        <rdfs:subClassOf rdf:resource="http://www.cidoc-crm.org/cidoc-crm/E89_Propositional_Object"/>
        <rdfs:subClassOf rdf:resource="http://www.cidoc-crm.org/cidoc-crm/E90_Symbolic_Object"/>
        <rdfs:comment xml:lang="en">Scope note:
This class comprises identifiable immaterial items, such as poems, jokes, data sets, images, texts, multimedia objects, procedural prescriptions, computer program code, algorithm or mathematical formulae, that have an objectively recognizable structure and are documented as single units. The encoding structure known as a “named graph” also falls under this class, so that each “named graph” is an instance of E73 Information Object.
An instance of E73 Information Object does not depend on a specific physical carrier, which can include human memory, and it can exist on one or more carriers simultaneously.
Instances of E73 Information Object of a linguistic nature should be declared as instances of the E33 Linguistic Object subclass. Instances of E73 Information Object of a documentary nature should be declared as instances of the E31 Document subclass. Conceptual items such as types and classes are not instances of E73 Information Object, nor are ideas without a reproducible expression.

Examples:
- image BM000038850.JPG from the Clayton Herbarium in London (E31) (Natural History Museum, 2021)
- E. A. Poe&apos;s “The Raven” (Poe, 1869)
- the movie “The Seven Samurai” by Akira Kurosawa (Mellen, 2002)
- the text of Huray describing the Maxwell Equations (Huray, 2010)
- the Getty AAT as published as Linked Open Data, accessed 1/10/2014

In First Order Logic:
- E73(x) ⇒ E89(x)
- E73(x) ⇒ E90(x)
</rdfs:comment>
        <rdfs:label xml:lang="en">E73 Information Object</rdfs:label>
        <rdfs:label xml:lang="de">E73 Informationsgegenstand</rdfs:label>
        <rdfs:label xml:lang="fr">E73 Objet informationnel</rdfs:label>
        <rdfs:label xml:lang="pt">E73 Objeto de Informação</rdfs:label>
        <rdfs:label xml:lang="el">E73 Πληροφοριακό Αντικείμενο</rdfs:label>
        <rdfs:label xml:lang="ru">E73 Информационный Объeкт</rdfs:label>
        <rdfs:label xml:lang="zh">E73 信息对象</rdfs:label>
        <skos:notation xml:lang="en">E73</skos:notation>
        <skos:prefLabel xml:lang="en">Information Object</skos:prefLabel>
        <skos:prefLabel xml:lang="de">Informationsgegenstand</skos:prefLabel>
        <skos:prefLabel xml:lang="fr">Objet informationnel</skos:prefLabel>
        <skos:prefLabel xml:lang="pt">Objeto de Informação</skos:prefLabel>
        <skos:prefLabel xml:lang="el">Πληροφοριακό Αντικείμενο</skos:prefLabel>
        <skos:prefLabel xml:lang="ru">Информационный Объeкт</skos:prefLabel>
        <skos:prefLabel xml:lang="zh">信息对象</skos:prefLabel>
    </owl:Class>
    


    <!-- http://www.cidoc-crm.org/cidoc-crm/E74_Group -->

    <owl:Class rdf:about="http://www.cidoc-crm.org/cidoc-crm/E74_Group">
        <rdfs:subClassOf rdf:resource="http://www.cidoc-crm.org/cidoc-crm/E39_Actor"/>
        <rdfs:subClassOf rdf:resource="http://www.w3.org/ns/odrl/2/Party"/>
        <rdfs:comment xml:lang="en">Scope note:
This class comprises any gatherings or organizations of human individuals or groups that act collectively or in a similar way due to any form of unifying relationship. In the wider sense this class also comprises official positions which used to be regarded in certain contexts as one actor, independent of the current holder of the office, such as the president of a country. In such cases, it may happen that the group never had more than one member. A joint pseudonym (i.e. a name that seems indicative of an individual but that is actually used as a persona by two or more people) is a particular case of E74 Group.
A gathering of people becomes an instance of E74 Group when it exhibits organizational characteristics usually typified by a set of ideas or beliefs held in common, or actions performed together. These might be communication, creating some common artifact, a common purpose such as study, worship, business, sports, etc. Nationality can be modelled as membership in an instance of E74 Group. Married couples and other concepts of family are regarded as particular examples of E74 Group.

Examples:
- the Impressionists (Wilson, 1994)
- the Navajo (Correll, 1972)
- the Greeks (Williams, 1993)
- the peace protestors in New York City on 15(th) February 2003
- Exxon-Mobil (Raymond, 2006)
- King Solomon and his wives (Thieberger, 1947)
- the President of the Swiss Confederation
- Nicolas Bourbaki [the collective pseudonym of a group of mathematicians, predominantly French alumni of the École normale supérieure] (Aczel, 2007)
- Betty Crocker (Crocker, 2012)
- Ellery Queen [Ellery Queen is a pseudonym created in 1929 by American crime fiction writers Frederic Dannay and Manfred Bennington Lee.] (Wheat, 2005)
- Greenpeace
- Paveprime Ltd
- the National Museum of Denmark

In First Order Logic:
- E74(x) ⇒ E39(x)
</rdfs:comment>
        <rdfs:label xml:lang="en">E74 Group</rdfs:label>
        <rdfs:label xml:lang="fr">E74 Groupe</rdfs:label>
        <rdfs:label xml:lang="pt">E74 Grupo</rdfs:label>
        <rdfs:label xml:lang="de">E74 Menschliche Gruppe</rdfs:label>
        <rdfs:label xml:lang="el">E74 Ομάδα</rdfs:label>
        <rdfs:label xml:lang="ru">E74 Группа</rdfs:label>
        <rdfs:label xml:lang="zh">E74 团体</rdfs:label>
        <skos:notation xml:lang="en">E74</skos:notation>
        <skos:prefLabel xml:lang="en">Group</skos:prefLabel>
        <skos:prefLabel xml:lang="fr">Groupe</skos:prefLabel>
        <skos:prefLabel xml:lang="pt">Grupo</skos:prefLabel>
        <skos:prefLabel xml:lang="de">Menschliche Gruppe</skos:prefLabel>
        <skos:prefLabel xml:lang="el">Ομάδα</skos:prefLabel>
        <skos:prefLabel xml:lang="ru">Группа</skos:prefLabel>
        <skos:prefLabel xml:lang="zh">团体</skos:prefLabel>
    </owl:Class>
    


    <!-- http://www.cidoc-crm.org/cidoc-crm/E77_Persistent_Item -->

    <owl:Class rdf:about="http://www.cidoc-crm.org/cidoc-crm/E77_Persistent_Item">
        <rdfs:subClassOf rdf:resource="http://www.cidoc-crm.org/cidoc-crm/E1_CRM_Entity"/>
        <rdfs:comment xml:lang="en">Scope note:
This class comprises items that have persistent characteristics of structural nature substantially related to their identity and their integrity, sometimes known as “endurants” in philosophy. Persistent Items may be physical entities, such as people, animals or things, conceptual entities such as ideas, concepts, products of the imagination or even names. 
Instances of E77 Persistent Item may be present or be part of interactions in different periods or events. They can repeatedly be recognized at disparate occasions during their existence by characteristics of structural nature. The respective characteristics need not be exactly the same during all the existence of an instance of E77 Persistent Item. Often, they undergo gradual change, still bearing some similarities with that of previous times, or disappear completely and new emerge. For instance, a person, from the time of being born on, will gradually change all its features and acquire new ones, such as a scar. Even the DNA in different body cells will develop defects and mutations. Nevertheless, relevant characteristics used should be sufficiently similar to recognize the instance for some substantial period of time. 
The more specific criteria that determine the identity of instances of subclasses of E77 Persistent Item may vary considerably and are described or referred to in the respective scope notes. The decision about which exact criteria to use depends on whether the observable behaviour of the respective part of reality such confined conforms to the reasoning the user is interested in. For example, a building can be regarded as no longer existing if it is dismantled and the materials reused in a different configuration. On the other hand, human beings go through radical and profound changes during their life-span, affecting both material composition and form, yet preserve their identity by other criteria, such as being bodily separated from other persons. Similarly, inanimate objects may be subject to exchange of parts and matter. On the opposite, the identity of a (version of a) text of a scientific publication is given by the exact arrangement of its relevant symbols. 
The main classes of objects that fall outside the scope of the E77 Persistent Item class are temporal objects such as periods, events and acts, and descriptive properties. 
An instance of E77 Persistent Item does not require actual knowledge of the identifying features of the instance being currently known. There may be cases, where the actual identifying features of an instance of E77 Persistent Item are not decidable at a particular state of knowledge.

Examples:
- Leonardo da Vinci (E21) (Strano, 1953)
- Stonehenge (E24) (Pryor, 2016)
- the hole in the ozone layer (E4) (Hufford and Horwitz, 2005)
- the First Law of Thermodynamics (E89) (Craig and Gislason, 2002)
- the Bermuda Triangle (E53) (Dolan, 2005)

In First Order Logic:
- E77(x) ⇒ E1(x)
</rdfs:comment>
        <rdfs:label xml:lang="pt">E77 Entidade Persistente</rdfs:label>
        <rdfs:label xml:lang="fr">E77 Entité persistante</rdfs:label>
        <rdfs:label xml:lang="en">E77 Persistent Item</rdfs:label>
        <rdfs:label xml:lang="de">E77 Seiendes</rdfs:label>
        <rdfs:label xml:lang="el">E77 Ον</rdfs:label>
        <rdfs:label xml:lang="ru">E77 Постоянная Сущность</rdfs:label>
        <rdfs:label xml:lang="zh">E77 持久项</rdfs:label>
        <skos:notation xml:lang="en">E77</skos:notation>
        <skos:prefLabel xml:lang="pt">Entidade Persistente</skos:prefLabel>
        <skos:prefLabel xml:lang="fr">Entité persistante</skos:prefLabel>
        <skos:prefLabel xml:lang="en">Persistent Item</skos:prefLabel>
        <skos:prefLabel xml:lang="de">Seiendes</skos:prefLabel>
        <skos:prefLabel xml:lang="el">Ον</skos:prefLabel>
        <skos:prefLabel xml:lang="ru">Постоянная Сущность</skos:prefLabel>
        <skos:prefLabel xml:lang="zh">持久项</skos:prefLabel>
    </owl:Class>
    


    <!-- http://www.cidoc-crm.org/cidoc-crm/E78_Curated_Holding -->

    <owl:Class rdf:about="http://www.cidoc-crm.org/cidoc-crm/E78_Curated_Holding">
        <rdfs:subClassOf rdf:resource="http://www.cidoc-crm.org/cidoc-crm/E24_Physical_Human-Made_Thing"/>
        <rdfs:comment xml:lang="en">Scope note:
This class comprises aggregations of instances of E18 Physical Thing that are assembled and maintained (“curated” and “preserved,” in museological terminology) by one or more instances of E39 Actor over time for a specific purpose and audience, and according to a particular collection development plan. Typical instances of curated holdings are museum collections, archives, library holdings and digital libraries. A digital library is regarded as an instance of E18 Physical Thing because it requires keeping physical carriers of the electronic content.
Items may be added or removed from an E78 Curated Holding in pursuit of this plan. This class should not be confused with the E39 Actor maintaining the E78 Curated Holding who is often referred to using the name of the E78 Curated Holding (e.g. “The Wallace Collection decided…”). 
Collective objects in the general sense, like a tomb full of gifts, a folder with stamps, or a set of chessmen, should be documented as instances of E19 Physical Object, and not as instances of E78 Curated Holding. This is because they form wholes, either because they are physically bound together or because they are kept together for their functionality.

Examples:
- the John Clayton Herbarium (Blake, 1918), (Natural History Museum, 2021)
- the Wallace Collection (Ingamells, 1990)
- Mikael Heggelund Foslie’s coralline red algae Herbarium at the Museum of Natural History and Archaeology, Trondheim, Norway (Woelkerling et al., 2005)
- the Digital Collections of the Munich DigitiZation Center (MDZ) accessible via https://www.digitale-sammlungen.de/ at least in January 2018.

In First Order Logic:
- E78(x) ⇒ E24(x)
</rdfs:comment>
        <rdfs:label xml:lang="fr">E78 Collection</rdfs:label>
        <rdfs:label xml:lang="en">E78 Curated Holding</rdfs:label>
        <rdfs:label xml:lang="ru">E78 Отвeтствeнноe Хранeниe</rdfs:label>
        <skos:notation xml:lang="en">E78</skos:notation>
        <skos:prefLabel xml:lang="fr">Collection</skos:prefLabel>
        <skos:prefLabel xml:lang="en">Curated Holding</skos:prefLabel>
        <skos:prefLabel xml:lang="ru">Отвeтствeнноe Хранeниe</skos:prefLabel>
    </owl:Class>
    


    <!-- http://www.cidoc-crm.org/cidoc-crm/E7_Activity -->

    <owl:Class rdf:about="http://www.cidoc-crm.org/cidoc-crm/E7_Activity">
        <rdfs:subClassOf rdf:resource="http://www.cidoc-crm.org/cidoc-crm/E5_Event"/>
        <rdfs:comment xml:lang="en">Scope note:
This class comprises actions intentionally carried out by instances of E39 Actor that result in changes of state in the cultural, social, or physical systems documented. 
This notion includes complex, composite, and long-lasting actions such as the building of a settlement or a war, as well as simple, short-lived actions such as the opening of a door.

Examples:
- the Battle of Stalingrad (Hoyt, 1993)
- the Yalta Conference (Harbutt, 2010)
- my birthday celebration 28-6-1995
- the writing of “Faust” by Goethe (E65) (Williams, 2020)
- the formation of the Bauhaus 1919 (E66) (Droste, 2006)
- the people of Iraq giving the name ‘Quyunjig’ to the place identified by the TGN as ‘7017998’
- Kira Weber working in glass art from 1984 to 1993
- Kira Weber working in oil and pastel painting from 1993

In First Order Logic:
- E7(x) ⇒ E5(x)
</rdfs:comment>
        <rdfs:label xml:lang="en">E7 Activity</rdfs:label>
        <rdfs:label xml:lang="fr">E7 Activité</rdfs:label>
        <rdfs:label xml:lang="pt">E7 Atividade</rdfs:label>
        <rdfs:label xml:lang="de">E7 Handlung</rdfs:label>
        <rdfs:label xml:lang="el">E7 Δράση</rdfs:label>
        <rdfs:label xml:lang="ru">E7 Дeятeльность</rdfs:label>
        <rdfs:label xml:lang="zh">E7 活动</rdfs:label>
        <skos:notation xml:lang="en">E7</skos:notation>
        <skos:prefLabel xml:lang="en">Activity</skos:prefLabel>
        <skos:prefLabel xml:lang="fr">Activité</skos:prefLabel>
        <skos:prefLabel xml:lang="pt">Atividade</skos:prefLabel>
        <skos:prefLabel xml:lang="de">Handlung</skos:prefLabel>
        <skos:prefLabel xml:lang="el">Δράση</skos:prefLabel>
        <skos:prefLabel xml:lang="ru">Дeятeльность</skos:prefLabel>
        <skos:prefLabel xml:lang="zh">活动</skos:prefLabel>
    </owl:Class>
    


    <!-- http://www.cidoc-crm.org/cidoc-crm/E89_Propositional_Object -->

    <owl:Class rdf:about="http://www.cidoc-crm.org/cidoc-crm/E89_Propositional_Object">
        <rdfs:subClassOf rdf:resource="http://www.cidoc-crm.org/cidoc-crm/E28_Conceptual_Object"/>
        <rdfs:comment xml:lang="en">Scope note:
This class comprises immaterial items, including but not limited to stories, plots, procedural prescriptions, algorithms, laws of physics or images that are, or represent in some sense, sets of propositions about real or imaginary things and that are documented as single units or serve as topic of discourse. 
This class also comprises items that are “about” something in the sense of a subject. In the wider sense, this class includes expressions of psychological value such as non-figural art and musical themes. However, conceptual items such as types and classes are not instances of E89 Propositional Object. This should not be confused with the definition of a type, which is indeed an instance of E89 Propositional Object.

Examples:
- Maxwell’s Equations (Ball, 1962)
- the ideational contents of Aristotle’s book entitled ‘Metaphysics’ as rendered in the Greek texts translated in Oxford edition
- the underlying prototype of any “no-smoking” sign (E36)
- the common ideas of the plots of the movie “The Seven Samurai” by Akira Kurosawa and the movie “The Magnificent Seven” by John Sturges (Mellen, 2002)
- the image content of the photo of the Allied Leaders at Yalta published by UPI, 1945 (E36)
- the character “Little Red Riding Hood”, variants of which appear amongst others in Grimm brothers’ “Rotkäppchen”, other oral fairy tales and the film “Hoodwinked”
- the place “Havnor” as invented by Ursula K. Le Guin for her “Earthsea” book series, the related maps and appearing in derivative works based on these novels

In First Order Logic:
- E89(x) ⇒ E28(x)
</rdfs:comment>
        <rdfs:label xml:lang="de">E89 Aussagenobjekt</rdfs:label>
        <rdfs:label xml:lang="fr">E89 Objet propositionnel</rdfs:label>
        <rdfs:label xml:lang="en">E89 Propositional Object</rdfs:label>
        <rdfs:label xml:lang="ru">E89 Пропозициональный Объeкт</rdfs:label>
        <rdfs:label xml:lang="zh">E89 命题对象</rdfs:label>
        <skos:notation xml:lang="en">E89</skos:notation>
        <skos:prefLabel xml:lang="de">Aussagenobjekt</skos:prefLabel>
        <skos:prefLabel xml:lang="fr">Objet propositionnel</skos:prefLabel>
        <skos:prefLabel xml:lang="en">Propositional Object</skos:prefLabel>
        <skos:prefLabel xml:lang="ru">Пропозициональный Объeкт</skos:prefLabel>
        <skos:prefLabel xml:lang="zh">命题对象</skos:prefLabel>
    </owl:Class>
    


    <!-- http://www.cidoc-crm.org/cidoc-crm/E90_Symbolic_Object -->

    <owl:Class rdf:about="http://www.cidoc-crm.org/cidoc-crm/E90_Symbolic_Object">
        <rdfs:subClassOf rdf:resource="http://www.cidoc-crm.org/cidoc-crm/E28_Conceptual_Object"/>
        <rdfs:subClassOf rdf:resource="http://www.cidoc-crm.org/cidoc-crm/E72_Legal_Object"/>
        <rdfs:subClassOf rdf:resource="http://www.w3.org/ns/odrl/2/Asset"/>
        <rdfs:comment xml:lang="en">Scope note:
This class comprises identifiable symbols and any aggregation of symbols, such as characters, identifiers, traffic signs, emblems, texts, data sets, images, musical scores, multimedia objects, computer program code, or mathematical formulae that have an objectively recognizable structure and that are documented as single units.
It includes sets of signs of any nature, which may serve to designate something, or to communicate some propositional content. An instance of E90 Symbolic Object may or may not have a specific meaning, for example an arbitrary character string.
In some cases, the content of an instance of E90 Symbolic Object may completely be represented by a serialized digital content model, such as a sequence of ASCII-encoded characters, an XML or HTML document, or a TIFF image. The property P3 has note and its subproperty P190 has symbolic content allow for the description of this content model. In order to disambiguate which symbolic level is the carrier of the meaning, the property P3.1 has type can be used to specify the encoding (e.g. “bit”, “Latin character”, RGB pixel).

Examples:
- ‘ecognizabl’
- the “no-smoking” sign (E36)
- “BM000038850.JPG” (E41) [identifies a digital image] (Natural History Museum, 2021)
- image BM000038850.JPG from the Clayton Herbarium in London (E36) [depicts specimen of Verbesina virginica] (Natural History Museum, 2021)
- the distribution of form, tone and colour found on Leonardo da Vinci’s painting named “Mona Lisa” in daylight (E36)
- the Italian text of Dante’s “Divina Commedia” as found in the authoritative critical edition “La Commedia secondo l’antica vulgata a cura di Giorgio Petrocchi” (E33) (Petrocchi, 1967)

In First Order Logic:
- E90(x) ⇒ E28(x)
- E90(x) ⇒ E72(x)
</rdfs:comment>
        <rdfs:label xml:lang="fr">E90 Objet symbolique</rdfs:label>
        <rdfs:label xml:lang="en">E90 Symbolic Object</rdfs:label>
        <rdfs:label xml:lang="de">E90 Symbolisches Objekt</rdfs:label>
        <rdfs:label xml:lang="ru">E90 Символичeский Объeкт</rdfs:label>
        <rdfs:label xml:lang="zh">E90 符号对象</rdfs:label>
        <skos:notation xml:lang="en">E90</skos:notation>
        <skos:prefLabel xml:lang="fr">Objet symbolique</skos:prefLabel>
        <skos:prefLabel xml:lang="en">Symbolic Object</skos:prefLabel>
        <skos:prefLabel xml:lang="de">Symbolisches Objekt</skos:prefLabel>
        <skos:prefLabel xml:lang="ru">Символичeский Объeкт</skos:prefLabel>
        <skos:prefLabel xml:lang="zh">符号对象</skos:prefLabel>
    </owl:Class>
    


    <!-- http://www.cidoc-crm.org/cidoc-crm/E92_Spacetime_Volume -->

    <owl:Class rdf:about="http://www.cidoc-crm.org/cidoc-crm/E92_Spacetime_Volume">
        <rdfs:subClassOf rdf:resource="http://www.cidoc-crm.org/cidoc-crm/E1_CRM_Entity"/>
        <rdfs:comment xml:lang="en">Scope note:
This class comprises 4-dimensional point sets (volumes) in physical spacetime (in contrast to mathematical models of it) regardless of their true geometric forms. They may derive their identity from being the extent of a material phenomenon or from being the interpretation of an expression defining an extent in spacetime. Intersections of instances of E92 Spacetime Volume, E53 Place, and E52 Time-Span are also regarded as instances of E92 Spacetime Volume. An instance of E92 Spacetime Volume is either contiguous or composed of a finite number of contiguous subsets. Its boundaries may be fuzzy due to the properties of the phenomena it derives from or due to the limited precision up to which defining expression can be identified with a real extent in spacetime. The duration of existence of an instance of E92 Spacetime Volume is its projection on time.

Examples:
- the extent in space and time of the Event of Caesar’s murder (Irwin, 1935)
- where and when the carbon 14 dating of the “Schoeninger Speer II” in 1996 took place (Kouwenhoven, 1997)
- the spatio-temporal trajectory of the H.M.S. Victory from its building to its actual location (Goodwin, 2015)
- the extent in space and time defined by a polygon approximating the Danube river flood in Austria between 6(th) and 9(th) August 2002

In First Order Logic:
- E92(x) ⇒ E1(x)
</rdfs:comment>
        <rdfs:label xml:lang="en">E92 Spacetime Volume</rdfs:label>
        <rdfs:label xml:lang="fr">E92 Volume spatio-temporel</rdfs:label>
        <rdfs:label xml:lang="ru">E92 Область Пространства-Врeмeни</rdfs:label>
        <skos:notation xml:lang="en">E92</skos:notation>
        <skos:prefLabel xml:lang="en">Spacetime Volume</skos:prefLabel>
        <skos:prefLabel xml:lang="fr">Volume spatio-temporel</skos:prefLabel>
        <skos:prefLabel xml:lang="ru">Область Пространства-Врeмeни</skos:prefLabel>
    </owl:Class>
    


    <!-- http://www.w3.org/2000/01/rdf-schema#Class -->

    <owl:Class rdf:about="http://www.w3.org/2000/01/rdf-schema#Class"/>
    


    <!-- http://www.w3.org/2000/01/rdf-schema#Datatype -->

    <owl:Class rdf:about="http://www.w3.org/2000/01/rdf-schema#Datatype"/>
    


    <!-- http://www.w3.org/2000/01/rdf-schema#Literal -->

    <owl:Class rdf:about="http://www.w3.org/2000/01/rdf-schema#Literal"/>
    


    <!-- http://www.w3.org/2001/XMLSchema#anyURI -->

    <owl:Class rdf:about="http://www.w3.org/2001/XMLSchema#anyURI"/>
    


    <!-- http://www.w3.org/2004/02/skos/core#Collection -->

    <owl:Class rdf:about="http://www.w3.org/2004/02/skos/core#Collection"/>
    


    <!-- http://www.w3.org/2004/02/skos/core#Concept -->

    <owl:Class rdf:about="http://www.w3.org/2004/02/skos/core#Concept"/>
    


    <!-- http://www.w3.org/2006/vcard/ns#Agent -->

    <owl:Class rdf:about="http://www.w3.org/2006/vcard/ns#Agent"/>
    


    <!-- http://www.w3.org/2006/vcard/ns#Individual -->

    <owl:Class rdf:about="http://www.w3.org/2006/vcard/ns#Individual"/>
    


    <!-- http://www.w3.org/2006/vcard/ns#Organization -->

    <owl:Class rdf:about="http://www.w3.org/2006/vcard/ns#Organization"/>
    


    <!-- http://www.w3.org/ns/odrl/2/Action -->

    <owl:Class rdf:about="http://www.w3.org/ns/odrl/2/Action">
        <rdfs:subClassOf rdf:resource="http://schema.org/Action"/>
    </owl:Class>
    


    <!-- http://www.w3.org/ns/odrl/2/Agreement -->

    <owl:Class rdf:about="http://www.w3.org/ns/odrl/2/Agreement">
        <rdfs:subClassOf rdf:resource="http://www.cidoc-crm.org/cidoc-crm/E30_Right"/>
        <rdfs:subClassOf rdf:resource="http://www.w3.org/ns/odrl/2/Policy"/>
        <owl:disjointWith rdf:resource="http://www.w3.org/ns/odrl/2/Assertion"/>
        <owl:disjointWith rdf:resource="http://www.w3.org/ns/odrl/2/Offer"/>
        <owl:disjointWith rdf:resource="http://www.w3.org/ns/odrl/2/Privacy"/>
        <owl:disjointWith rdf:resource="http://www.w3.org/ns/odrl/2/Request"/>
        <owl:disjointWith rdf:resource="http://www.w3.org/ns/odrl/2/Set"/>
        <owl:disjointWith rdf:resource="http://www.w3.org/ns/odrl/2/Ticket"/>
    </owl:Class>
    


    <!-- http://www.w3.org/ns/odrl/2/Assertion -->

    <owl:Class rdf:about="http://www.w3.org/ns/odrl/2/Assertion">
        <rdfs:subClassOf rdf:resource="http://www.cidoc-crm.org/cidoc-crm/E30_Right"/>
        <rdfs:subClassOf rdf:resource="http://www.w3.org/ns/odrl/2/Policy"/>
        <owl:disjointWith rdf:resource="http://www.w3.org/ns/odrl/2/Offer"/>
        <owl:disjointWith rdf:resource="http://www.w3.org/ns/odrl/2/Privacy"/>
        <owl:disjointWith rdf:resource="http://www.w3.org/ns/odrl/2/Request"/>
        <owl:disjointWith rdf:resource="http://www.w3.org/ns/odrl/2/Set"/>
        <owl:disjointWith rdf:resource="http://www.w3.org/ns/odrl/2/Ticket"/>
    </owl:Class>
    


    <!-- http://www.w3.org/ns/odrl/2/Asset -->

    <owl:Class rdf:about="http://www.w3.org/ns/odrl/2/Asset">
        <rdfs:subClassOf rdf:resource="http://www.cidoc-crm.org/cidoc-crm/E70_Thing"/>
    </owl:Class>
    


    <!-- http://www.w3.org/ns/odrl/2/AssetCollection -->

    <owl:Class rdf:about="http://www.w3.org/ns/odrl/2/AssetCollection">
        <rdfs:subClassOf rdf:resource="http://www.cidoc-crm.org/cidoc-crm/E72_Legal_Object"/>
        <rdfs:subClassOf rdf:resource="http://www.w3.org/ns/odrl/2/Asset"/>
    </owl:Class>
    


    <!-- http://www.w3.org/ns/odrl/2/ConflictTerm -->

    <owl:Class rdf:about="http://www.w3.org/ns/odrl/2/ConflictTerm"/>
    


    <!-- http://www.w3.org/ns/odrl/2/Constraint -->

    <owl:Class rdf:about="http://www.w3.org/ns/odrl/2/Constraint"/>
    


    <!-- http://www.w3.org/ns/odrl/2/Duty -->

    <owl:Class rdf:about="http://www.w3.org/ns/odrl/2/Duty">
        <rdfs:subClassOf rdf:resource="http://www.w3.org/ns/odrl/2/Rule"/>
        <owl:disjointWith rdf:resource="http://www.w3.org/ns/odrl/2/Permission"/>
        <owl:disjointWith rdf:resource="http://www.w3.org/ns/odrl/2/Prohibition"/>
    </owl:Class>
    


    <!-- http://www.w3.org/ns/odrl/2/LeftOperand -->

    <owl:Class rdf:about="http://www.w3.org/ns/odrl/2/LeftOperand"/>
    


    <!-- http://www.w3.org/ns/odrl/2/LogicalConstraint -->

    <owl:Class rdf:about="http://www.w3.org/ns/odrl/2/LogicalConstraint"/>
    


    <!-- http://www.w3.org/ns/odrl/2/Offer -->

    <owl:Class rdf:about="http://www.w3.org/ns/odrl/2/Offer">
        <rdfs:subClassOf rdf:resource="http://www.cidoc-crm.org/cidoc-crm/E30_Right"/>
        <rdfs:subClassOf rdf:resource="http://www.w3.org/ns/odrl/2/Policy"/>
        <owl:disjointWith rdf:resource="http://www.w3.org/ns/odrl/2/Privacy"/>
        <owl:disjointWith rdf:resource="http://www.w3.org/ns/odrl/2/Request"/>
        <owl:disjointWith rdf:resource="http://www.w3.org/ns/odrl/2/Set"/>
        <owl:disjointWith rdf:resource="http://www.w3.org/ns/odrl/2/Ticket"/>
    </owl:Class>
    


    <!-- http://www.w3.org/ns/odrl/2/Operator -->

    <owl:Class rdf:about="http://www.w3.org/ns/odrl/2/Operator"/>
    


    <!-- http://www.w3.org/ns/odrl/2/Party -->

    <owl:Class rdf:about="http://www.w3.org/ns/odrl/2/Party">
        <rdfs:subClassOf rdf:resource="http://www.cidoc-crm.org/cidoc-crm/E77_Persistent_Item"/>
        <rdfs:subClassOf>
            <owl:Class>
                <owl:unionOf rdf:parseType="Collection">
                    <rdf:Description rdf:about="http://schema.org/Organization"/>
                    <rdf:Description rdf:about="http://schema.org/Person"/>
                    <rdf:Description rdf:about="http://www.w3.org/2006/vcard/ns#Agent"/>
                    <rdf:Description rdf:about="http://www.w3.org/2006/vcard/ns#Individual"/>
                    <rdf:Description rdf:about="http://www.w3.org/2006/vcard/ns#Organization"/>
                    <rdf:Description rdf:about="http://xmlns.com/foaf/0.1/Agent"/>
                    <rdf:Description rdf:about="http://xmlns.com/foaf/0.1/Organization"/>
                    <rdf:Description rdf:about="http://xmlns.com/foaf/0.1/Person"/>
                </owl:unionOf>
            </owl:Class>
        </rdfs:subClassOf>
    </owl:Class>
    


    <!-- http://www.w3.org/ns/odrl/2/PartyCollection -->

    <owl:Class rdf:about="http://www.w3.org/ns/odrl/2/PartyCollection">
        <rdfs:subClassOf rdf:resource="http://www.cidoc-crm.org/cidoc-crm/E39_Actor"/>
        <rdfs:subClassOf rdf:resource="http://www.w3.org/ns/odrl/2/Party"/>
    </owl:Class>
    


    <!-- http://www.w3.org/ns/odrl/2/PartyScope -->

    <owl:Class rdf:about="http://www.w3.org/ns/odrl/2/PartyScope"/>
    


    <!-- http://www.w3.org/ns/odrl/2/Permission -->

    <owl:Class rdf:about="http://www.w3.org/ns/odrl/2/Permission">
        <rdfs:subClassOf rdf:resource="http://www.w3.org/ns/odrl/2/Rule"/>
        <owl:disjointWith rdf:resource="http://www.w3.org/ns/odrl/2/Prohibition"/>
    </owl:Class>
    


    <!-- http://www.w3.org/ns/odrl/2/Policy -->

    <owl:Class rdf:about="http://www.w3.org/ns/odrl/2/Policy">
        <rdfs:subClassOf rdf:resource="http://www.cidoc-crm.org/cidoc-crm/E89_Propositional_Object"/>
    </owl:Class>
    


    <!-- http://www.w3.org/ns/odrl/2/Privacy -->

    <owl:Class rdf:about="http://www.w3.org/ns/odrl/2/Privacy">
        <rdfs:subClassOf rdf:resource="http://www.cidoc-crm.org/cidoc-crm/E30_Right"/>
        <rdfs:subClassOf rdf:resource="http://www.w3.org/ns/odrl/2/Policy"/>
        <owl:disjointWith rdf:resource="http://www.w3.org/ns/odrl/2/Request"/>
        <owl:disjointWith rdf:resource="http://www.w3.org/ns/odrl/2/Set"/>
        <owl:disjointWith rdf:resource="http://www.w3.org/ns/odrl/2/Ticket"/>
    </owl:Class>
    


    <!-- http://www.w3.org/ns/odrl/2/Prohibition -->

    <owl:Class rdf:about="http://www.w3.org/ns/odrl/2/Prohibition">
        <rdfs:subClassOf rdf:resource="http://www.w3.org/ns/odrl/2/Rule"/>
    </owl:Class>
    


    <!-- http://www.w3.org/ns/odrl/2/Request -->

    <owl:Class rdf:about="http://www.w3.org/ns/odrl/2/Request">
        <rdfs:subClassOf rdf:resource="http://www.cidoc-crm.org/cidoc-crm/E30_Right"/>
        <rdfs:subClassOf rdf:resource="http://www.w3.org/ns/odrl/2/Policy"/>
        <owl:disjointWith rdf:resource="http://www.w3.org/ns/odrl/2/Set"/>
        <owl:disjointWith rdf:resource="http://www.w3.org/ns/odrl/2/Ticket"/>
    </owl:Class>
    


    <!-- http://www.w3.org/ns/odrl/2/RightOperand -->

    <owl:Class rdf:about="http://www.w3.org/ns/odrl/2/RightOperand"/>
    


    <!-- http://www.w3.org/ns/odrl/2/Rule -->

    <owl:Class rdf:about="http://www.w3.org/ns/odrl/2/Rule"/>
    


    <!-- http://www.w3.org/ns/odrl/2/Set -->

    <owl:Class rdf:about="http://www.w3.org/ns/odrl/2/Set">
        <rdfs:subClassOf rdf:resource="http://www.cidoc-crm.org/cidoc-crm/E30_Right"/>
        <rdfs:subClassOf rdf:resource="http://www.w3.org/ns/odrl/2/Policy"/>
        <owl:disjointWith rdf:resource="http://www.w3.org/ns/odrl/2/Ticket"/>
    </owl:Class>
    


    <!-- http://www.w3.org/ns/odrl/2/Ticket -->

    <owl:Class rdf:about="http://www.w3.org/ns/odrl/2/Ticket">
        <rdfs:subClassOf rdf:resource="http://www.cidoc-crm.org/cidoc-crm/E30_Right"/>
        <rdfs:subClassOf rdf:resource="http://www.w3.org/ns/odrl/2/Policy"/>
    </owl:Class>
    


    <!-- http://www.w3.org/ns/odrl/2/UndefinedTerm -->

    <owl:Class rdf:about="http://www.w3.org/ns/odrl/2/UndefinedTerm"/>
    


    <!-- http://xmlns.com/foaf/0.1/Agent -->

    <owl:Class rdf:about="http://xmlns.com/foaf/0.1/Agent"/>
    


    <!-- http://xmlns.com/foaf/0.1/Organization -->

    <owl:Class rdf:about="http://xmlns.com/foaf/0.1/Organization"/>
    


    <!-- http://xmlns.com/foaf/0.1/Person -->

    <owl:Class rdf:about="http://xmlns.com/foaf/0.1/Person"/>
    


    <!-- https://schema.org/AdministrativeArea -->

    <owl:Class rdf:about="https://schema.org/AdministrativeArea">
        <rdfs:subClassOf rdf:resource="https://schema.org/Place"/>
        <rdfs:comment xml:lang="en">A geographical region, typically under the jurisdiction of a particular government.</rdfs:comment>
        <rdfs:isDefinedBy rdf:resource="https://schema.org/AdministrativeArea"/>
        <rdfs:label xml:lang="en">AdministrativeArea</rdfs:label>
    </owl:Class>
    


    <!-- https://schema.org/Class -->

    <owl:Class rdf:about="https://schema.org/Class">
        <rdfs:subClassOf rdf:resource="https://schema.org/Intangible"/>
        <rdfs:comment xml:lang="en">A class, also often called a &apos;Type&apos;; equivalent to rdfs:Class.</rdfs:comment>
        <rdfs:isDefinedBy rdf:resource="https://meta.schema.org/Class"/>
        <rdfs:label xml:lang="en">Class</rdfs:label>
    </owl:Class>
    


    <!-- https://schema.org/Country -->

    <owl:Class rdf:about="https://schema.org/Country">
        <rdfs:subClassOf rdf:resource="https://schema.org/AdministrativeArea"/>
        <rdfs:comment xml:lang="en">A country.</rdfs:comment>
        <rdfs:isDefinedBy rdf:resource="https://schema.org/Country"/>
        <rdfs:label xml:lang="en">Country</rdfs:label>
    </owl:Class>
    


    <!-- https://schema.org/CreativeWork -->

    <owl:Class rdf:about="https://schema.org/CreativeWork">
        <rdfs:subClassOf rdf:resource="https://schema.org/Thing"/>
        <rdfs:comment xml:lang="en">The most generic kind of creative work, including books, movies, photographs, software programs, etc.</rdfs:comment>
        <rdfs:isDefinedBy rdf:resource="https://schema.org/CreativeWork"/>
        <rdfs:label xml:lang="en">CreativeWork</rdfs:label>
    </owl:Class>
    


    <!-- https://schema.org/DataType -->

    <owl:Class rdf:about="https://schema.org/DataType">
        <rdfs:subClassOf rdf:resource="http://www.w3.org/2000/01/rdf-schema#Class"/>
        <rdfs:comment xml:lang="en">The basic data types such as Integers, Strings, etc.</rdfs:comment>
        <rdfs:isDefinedBy rdf:resource="https://schema.org/DataType"/>
        <rdfs:label xml:lang="en">DataType</rdfs:label>
    </owl:Class>
    


    <!-- https://schema.org/Enumeration -->

    <owl:Class rdf:about="https://schema.org/Enumeration">
        <rdfs:subClassOf rdf:resource="https://schema.org/Intangible"/>
        <rdfs:comment xml:lang="en">Lists or enumerations—for example, a list of cuisines or music genres, etc.</rdfs:comment>
        <rdfs:isDefinedBy rdf:resource="https://schema.org/Enumeration"/>
        <rdfs:label xml:lang="en">Enumeration</rdfs:label>
    </owl:Class>
    


    <!-- https://schema.org/Intangible -->

    <owl:Class rdf:about="https://schema.org/Intangible">
        <rdfs:subClassOf rdf:resource="https://schema.org/Thing"/>
        <rdfs:comment xml:lang="en">A utility class that serves as the umbrella for a number of &apos;intangible&apos; things such as quantities, structured values, etc.</rdfs:comment>
        <rdfs:isDefinedBy rdf:resource="https://schema.org/Intangible"/>
        <rdfs:label xml:lang="en">Intangible</rdfs:label>
    </owl:Class>
    


    <!-- https://schema.org/MediaObject -->

    <owl:Class rdf:about="https://schema.org/MediaObject">
        <rdfs:subClassOf rdf:resource="https://schema.org/CreativeWork"/>
        <rdfs:comment xml:lang="en">A media object, such as an image, video, audio, or text object embedded in a web page or a downloadable dataset i.e. DataDownload. Note that a creative work may have many media objects associated with it on the same web page. For example, a page about a single song (MusicRecording) may have a music video (VideoObject), and a high and low bandwidth audio stream (2 AudioObject&apos;s).</rdfs:comment>
        <rdfs:isDefinedBy rdf:resource="https://schema.org/MediaObject"/>
        <rdfs:label xml:lang="en">MediaObject</rdfs:label>
    </owl:Class>
    


    <!-- https://schema.org/Person -->

    <owl:Class rdf:about="https://schema.org/Person">
        <rdfs:subClassOf rdf:resource="http://www.cidoc-crm.org/cidoc-crm/E20_Biological_Object"/>
        <rdfs:subClassOf rdf:resource="http://www.cidoc-crm.org/cidoc-crm/E39_Actor"/>
        <rdfs:subClassOf rdf:resource="http://www.w3.org/ns/odrl/2/Party"/>
        <rdfs:subClassOf rdf:resource="https://schema.org/Thing"/>
        <rdfs:comment xml:lang="en">A person (alive, dead, undead, or fictional).</rdfs:comment>
        <rdfs:isDefinedBy rdf:resource="https://schema.org/Person"/>
        <rdfs:label xml:lang="en">Person</rdfs:label>
    </owl:Class>
    


    <!-- https://schema.org/Place -->

    <owl:Class rdf:about="https://schema.org/Place">
        <rdfs:subClassOf rdf:resource="https://schema.org/Thing"/>
        <rdfs:comment xml:lang="en">Entities that have a somewhat fixed, physical extension.</rdfs:comment>
        <rdfs:isDefinedBy rdf:resource="https://schema.org/Place"/>
        <rdfs:label xml:lang="en">Place</rdfs:label>
    </owl:Class>
    


    <!-- https://schema.org/Property -->

    <owl:Class rdf:about="https://schema.org/Property">
        <rdfs:subClassOf rdf:resource="https://schema.org/Intangible"/>
        <rdfs:comment xml:lang="en">A property, used to indicate attributes and relationships of some Thing; equivalent to rdf:Property.</rdfs:comment>
        <rdfs:isDefinedBy rdf:resource="https://meta.schema.org/Property"/>
        <rdfs:label xml:lang="en">Property</rdfs:label>
    </owl:Class>
    


    <!-- https://schema.org/Role -->

    <owl:Class rdf:about="https://schema.org/Role">
        <rdfs:subClassOf rdf:resource="https://schema.org/Intangible"/>
        <rdfs:comment xml:lang="en">Represents additional information about a relationship or property. For example a Role can be used to say that a &apos;member&apos; role linking some SportsTeam to a player occurred during a particular time period. Or that a Person&apos;s &apos;actor&apos; role in a Movie was for some particular characterName. Such properties can be attached to a Role entity, which is then associated with the main entities using ordinary properties like &apos;member&apos; or &apos;actor&apos;.&lt;br/&gt;&lt;br/&gt;

See also &lt;a href=&quot;http://blog.schema.org/2014/06/introducing-role.html&quot;&gt;blog post&lt;/a&gt;.</rdfs:comment>
        <rdfs:isDefinedBy rdf:resource="https://schema.org/Role"/>
        <rdfs:label xml:lang="en">Role</rdfs:label>
    </owl:Class>
    


    <!-- https://schema.org/Specialty -->

    <owl:Class rdf:about="https://schema.org/Specialty">
        <rdfs:subClassOf rdf:resource="https://schema.org/Enumeration"/>
        <rdfs:comment xml:lang="en">Any branch of a field in which people typically develop specific expertise, usually after significant study, time, and effort.</rdfs:comment>
        <rdfs:isDefinedBy rdf:resource="https://schema.org/Specialty"/>
        <rdfs:label xml:lang="en">Specialty</rdfs:label>
    </owl:Class>
    


    <!-- https://schema.org/Text -->

    <owl:Class rdf:about="https://schema.org/Text">
        <rdfs:subClassOf rdf:resource="https://schema.org/DataType"/>
        <rdfs:comment xml:lang="en">Data type: Text.</rdfs:comment>
        <rdfs:isDefinedBy rdf:resource="https://schema.org/Text"/>
        <rdfs:label xml:lang="en">Text</rdfs:label>
    </owl:Class>
    


    <!-- https://schema.org/TextObject -->

    <owl:Class rdf:about="https://schema.org/TextObject">
        <rdfs:subClassOf rdf:resource="https://schema.org/MediaObject"/>
        <rdfs:comment xml:lang="en">A text file. The text can be unformatted or contain markup, html, etc.</rdfs:comment>
        <rdfs:isDefinedBy rdf:resource="https://schema.org/TextObject"/>
        <rdfs:label xml:lang="en">TextObject</rdfs:label>
    </owl:Class>
    


    <!-- https://schema.org/Thing -->

    <owl:Class rdf:about="https://schema.org/Thing">
        <rdfs:comment xml:lang="en">The most generic type of item.</rdfs:comment>
        <rdfs:isDefinedBy rdf:resource="https://schema.org/Thing"/>
        <rdfs:label xml:lang="en">Thing</rdfs:label>
    </owl:Class>
    


    <!-- https://schema.org/URL -->

    <owl:Class rdf:about="https://schema.org/URL">
        <rdfs:subClassOf rdf:resource="https://schema.org/Text"/>
        <rdfs:comment xml:lang="en">Data type: URL.</rdfs:comment>
        <rdfs:isDefinedBy rdf:resource="https://schema.org/URL"/>
        <rdfs:label xml:lang="en">URL</rdfs:label>
    </owl:Class>
    


    <!-- 
    ///////////////////////////////////////////////////////////////////////////////////////
    //
    // Individuals
    //
    ///////////////////////////////////////////////////////////////////////////////////////
     -->

    


    <!-- http://creativecommons.org/ns#Attribution -->

    <owl:NamedIndividual rdf:about="http://creativecommons.org/ns#Attribution">
        <rdf:type rdf:resource="http://www.w3.org/2004/02/skos/core#Concept"/>
        <rdf:type rdf:resource="http://www.w3.org/ns/odrl/2/Action"/>
        <odrl:includedIn rdf:resource="http://www.w3.org/ns/odrl/2/use"/>
        <rdfs:isDefinedBy rdf:resource="http://www.w3.org/ns/odrl/2/"/>
        <rdfs:label xml:lang="en">Attribution</rdfs:label>
        <skos:definition xml:lang="en">Credit be given to copyright holder and/or author.</skos:definition>
        <skos:note xml:lang="en">This term is defined by Creative Commons.</skos:note>
        <skos:scopeNote xml:lang="en">Non-Normative</skos:scopeNote>
    </owl:NamedIndividual>
    


    <!-- http://creativecommons.org/ns#CommercialUse -->

    <owl:NamedIndividual rdf:about="http://creativecommons.org/ns#CommercialUse">
        <rdf:type rdf:resource="http://www.w3.org/2004/02/skos/core#Concept"/>
        <rdf:type rdf:resource="http://www.w3.org/ns/odrl/2/Action"/>
        <odrl:includedIn rdf:resource="http://www.w3.org/ns/odrl/2/use"/>
        <rdfs:isDefinedBy rdf:resource="http://www.w3.org/ns/odrl/2/"/>
        <rdfs:label xml:lang="en">Commercial Use</rdfs:label>
        <skos:definition xml:lang="en">Exercising rights for commercial purposes.</skos:definition>
        <skos:note xml:lang="en">This term is defined by Creative Commons.</skos:note>
        <skos:scopeNote xml:lang="en">Non-Normative</skos:scopeNote>
    </owl:NamedIndividual>
    


    <!-- http://creativecommons.org/ns#DerivativeWorks -->

    <owl:NamedIndividual rdf:about="http://creativecommons.org/ns#DerivativeWorks">
        <rdf:type rdf:resource="http://www.w3.org/2004/02/skos/core#Concept"/>
        <rdf:type rdf:resource="http://www.w3.org/ns/odrl/2/Action"/>
        <odrl:includedIn rdf:resource="http://www.w3.org/ns/odrl/2/use"/>
        <rdfs:isDefinedBy rdf:resource="http://www.w3.org/ns/odrl/2/"/>
        <rdfs:label xml:lang="en">Derivative Works</rdfs:label>
        <skos:definition xml:lang="en">Distribution of derivative works.</skos:definition>
        <skos:note xml:lang="en">This term is defined by Creative Commons.</skos:note>
        <skos:scopeNote xml:lang="en">Non-Normative</skos:scopeNote>
    </owl:NamedIndividual>
    


    <!-- http://creativecommons.org/ns#Distribution -->

    <owl:NamedIndividual rdf:about="http://creativecommons.org/ns#Distribution">
        <rdf:type rdf:resource="http://www.w3.org/2004/02/skos/core#Concept"/>
        <rdf:type rdf:resource="http://www.w3.org/ns/odrl/2/Action"/>
        <odrl:includedIn rdf:resource="http://www.w3.org/ns/odrl/2/use"/>
        <rdfs:isDefinedBy rdf:resource="http://www.w3.org/ns/odrl/2/"/>
        <rdfs:label xml:lang="en">Distribution</rdfs:label>
        <skos:definition xml:lang="en">Distribution, public display, and publicly performance.</skos:definition>
        <skos:note xml:lang="en">This term is defined by Creative Commons.</skos:note>
        <skos:scopeNote xml:lang="en">Non-Normative</skos:scopeNote>
    </owl:NamedIndividual>
    


    <!-- http://creativecommons.org/ns#Notice -->

    <owl:NamedIndividual rdf:about="http://creativecommons.org/ns#Notice">
        <rdf:type rdf:resource="http://www.w3.org/2004/02/skos/core#Concept"/>
        <rdf:type rdf:resource="http://www.w3.org/ns/odrl/2/Action"/>
        <odrl:includedIn rdf:resource="http://www.w3.org/ns/odrl/2/use"/>
        <rdfs:isDefinedBy rdf:resource="http://www.w3.org/ns/odrl/2/"/>
        <rdfs:label xml:lang="en">Notice</rdfs:label>
        <skos:definition xml:lang="en">Copyright and license notices be kept intact.</skos:definition>
        <skos:note xml:lang="en">This term is defined by Creative Commons.</skos:note>
        <skos:scopeNote xml:lang="en">Non-Normative</skos:scopeNote>
    </owl:NamedIndividual>
    


    <!-- http://creativecommons.org/ns#Reproduction -->

    <owl:NamedIndividual rdf:about="http://creativecommons.org/ns#Reproduction">
        <rdf:type rdf:resource="http://www.w3.org/2004/02/skos/core#Concept"/>
        <rdf:type rdf:resource="http://www.w3.org/ns/odrl/2/Action"/>
        <odrl:includedIn rdf:resource="http://www.w3.org/ns/odrl/2/use"/>
        <rdfs:isDefinedBy rdf:resource="http://www.w3.org/ns/odrl/2/"/>
        <rdfs:label xml:lang="en">Reproduction</rdfs:label>
        <skos:definition xml:lang="en">Making multiple copies.</skos:definition>
        <skos:note xml:lang="en">This term is defined by Creative Commons.</skos:note>
        <skos:scopeNote xml:lang="en">Non-Normative</skos:scopeNote>
    </owl:NamedIndividual>
    


    <!-- http://creativecommons.org/ns#ShareAlike -->

    <owl:NamedIndividual rdf:about="http://creativecommons.org/ns#ShareAlike">
        <rdf:type rdf:resource="http://www.w3.org/2004/02/skos/core#Concept"/>
        <rdf:type rdf:resource="http://www.w3.org/ns/odrl/2/Action"/>
        <odrl:includedIn rdf:resource="http://www.w3.org/ns/odrl/2/use"/>
        <rdfs:isDefinedBy rdf:resource="http://www.w3.org/ns/odrl/2/"/>
        <rdfs:label xml:lang="en">Share Alike</rdfs:label>
        <skos:definition xml:lang="en">Derivative works be licensed under the same terms or compatible terms as the original work.</skos:definition>
        <skos:note xml:lang="en">This term is defined by Creative Commons.</skos:note>
        <skos:scopeNote xml:lang="en">Non-Normative</skos:scopeNote>
    </owl:NamedIndividual>
    


    <!-- http://creativecommons.org/ns#Sharing -->

    <owl:NamedIndividual rdf:about="http://creativecommons.org/ns#Sharing">
        <rdf:type rdf:resource="http://www.w3.org/2004/02/skos/core#Concept"/>
        <rdf:type rdf:resource="http://www.w3.org/ns/odrl/2/Action"/>
        <odrl:includedIn rdf:resource="http://www.w3.org/ns/odrl/2/use"/>
        <rdfs:isDefinedBy rdf:resource="http://www.w3.org/ns/odrl/2/"/>
        <rdfs:label xml:lang="en">Sharing</rdfs:label>
        <skos:definition xml:lang="en">Permits commercial derivatives, but only non-commercial distribution.</skos:definition>
        <skos:note xml:lang="en">This term is defined by Creative Commons.</skos:note>
        <skos:scopeNote xml:lang="en">Non-Normative</skos:scopeNote>
    </owl:NamedIndividual>
    


    <!-- http://creativecommons.org/ns#SourceCode -->

    <owl:NamedIndividual rdf:about="http://creativecommons.org/ns#SourceCode">
        <rdf:type rdf:resource="http://www.w3.org/2004/02/skos/core#Concept"/>
        <rdf:type rdf:resource="http://www.w3.org/ns/odrl/2/Action"/>
        <odrl:includedIn rdf:resource="http://www.w3.org/ns/odrl/2/use"/>
        <rdfs:isDefinedBy rdf:resource="http://www.w3.org/ns/odrl/2/"/>
        <rdfs:label xml:lang="en">Source Code</rdfs:label>
        <skos:definition xml:lang="en">Source code (the preferred form for making modifications) must be provided when exercising some rights granted by the license.</skos:definition>
        <skos:note xml:lang="en">This term is defined by Creative Commons.</skos:note>
        <skos:scopeNote xml:lang="en">Non-Normative</skos:scopeNote>
    </owl:NamedIndividual>
    


    <!-- http://www.w3.org/ns/odrl/2/Action -->

    <owl:NamedIndividual rdf:about="http://www.w3.org/ns/odrl/2/Action">
        <rdf:type rdf:resource="http://www.w3.org/2004/02/skos/core#Concept"/>
    </owl:NamedIndividual>
    


    <!-- http://www.w3.org/ns/odrl/2/Agreement -->

    <owl:NamedIndividual rdf:about="http://www.w3.org/ns/odrl/2/Agreement">
        <rdf:type rdf:resource="http://www.w3.org/2004/02/skos/core#Concept"/>
    </owl:NamedIndividual>
    


    <!-- http://www.w3.org/ns/odrl/2/All -->

    <owl:NamedIndividual rdf:about="http://www.w3.org/ns/odrl/2/All">
        <rdf:type rdf:resource="http://www.w3.org/2004/02/skos/core#Concept"/>
        <rdf:type rdf:resource="http://www.w3.org/ns/odrl/2/PartyScope"/>
        <rdfs:isDefinedBy rdf:resource="http://www.w3.org/ns/odrl/2/"/>
        <rdfs:label xml:lang="en">All</rdfs:label>
        <owl:deprecated rdf:datatype="http://www.w3.org/2001/XMLSchema#boolean">true</owl:deprecated>
        <skos:definition xml:lang="en">Specifies that the scope of the relationship is all of the collective individuals within a context.</skos:definition>
        <skos:note xml:lang="en">For example, may be used to indicate all the users of a specific social network the party is a member of. Note that “group” scope is also assumed.</skos:note>
        <skos:scopeNote xml:lang="en">Non-Normative</skos:scopeNote>
    </owl:NamedIndividual>
    


    <!-- http://www.w3.org/ns/odrl/2/All2ndConnections -->

    <owl:NamedIndividual rdf:about="http://www.w3.org/ns/odrl/2/All2ndConnections">
        <rdf:type rdf:resource="http://www.w3.org/2004/02/skos/core#Concept"/>
        <rdf:type rdf:resource="http://www.w3.org/ns/odrl/2/PartyScope"/>
        <rdfs:isDefinedBy rdf:resource="http://www.w3.org/ns/odrl/2/"/>
        <rdfs:label xml:lang="en">All Second-level Connections</rdfs:label>
        <owl:deprecated rdf:datatype="http://www.w3.org/2001/XMLSchema#boolean">true</owl:deprecated>
        <skos:definition xml:lang="en">Specifies that the scope of the relationship is all of the second-level connections to the Party.</skos:definition>
        <skos:note xml:lang="en">For example, may be used to indicate all “friends of friends” of the Party. Note that “group” scope is also assumed.</skos:note>
        <skos:scopeNote xml:lang="en">Non-Normative</skos:scopeNote>
    </owl:NamedIndividual>
    


    <!-- http://www.w3.org/ns/odrl/2/AllConnections -->

    <owl:NamedIndividual rdf:about="http://www.w3.org/ns/odrl/2/AllConnections">
        <rdf:type rdf:resource="http://www.w3.org/2004/02/skos/core#Concept"/>
        <rdf:type rdf:resource="http://www.w3.org/ns/odrl/2/PartyScope"/>
        <rdfs:isDefinedBy rdf:resource="http://www.w3.org/ns/odrl/2/"/>
        <rdfs:label xml:lang="en">All First-Level Connections</rdfs:label>
        <owl:deprecated rdf:datatype="http://www.w3.org/2001/XMLSchema#boolean">true</owl:deprecated>
        <skos:definition xml:lang="en">Specifies that the scope of the relationship is all of the first-level connections of the Party.</skos:definition>
        <skos:note xml:lang="en">For example, may be used to indicate all “friends” of the Party. Note that “group” scope is also assumed.</skos:note>
        <skos:scopeNote xml:lang="en">Non-Normative</skos:scopeNote>
    </owl:NamedIndividual>
    


    <!-- http://www.w3.org/ns/odrl/2/AllGroups -->

    <owl:NamedIndividual rdf:about="http://www.w3.org/ns/odrl/2/AllGroups">
        <rdf:type rdf:resource="http://www.w3.org/2004/02/skos/core#Concept"/>
        <rdf:type rdf:resource="http://www.w3.org/ns/odrl/2/PartyScope"/>
        <rdfs:isDefinedBy rdf:resource="http://www.w3.org/ns/odrl/2/"/>
        <rdfs:label xml:lang="en">All Group Connections</rdfs:label>
        <owl:deprecated rdf:datatype="http://www.w3.org/2001/XMLSchema#boolean">true</owl:deprecated>
        <skos:definition xml:lang="en">Specifies that the scope of the relationship is all of the group connections of the Party.</skos:definition>
        <skos:note xml:lang="en">For example, may be used to indicate all groups that the Party is a member of. Note that “group” scope is also assumed.</skos:note>
        <skos:scopeNote xml:lang="en">Non-Normative</skos:scopeNote>
    </owl:NamedIndividual>
    


    <!-- http://www.w3.org/ns/odrl/2/Assertion -->

    <owl:NamedIndividual rdf:about="http://www.w3.org/ns/odrl/2/Assertion">
        <rdf:type rdf:resource="http://www.w3.org/2004/02/skos/core#Concept"/>
    </owl:NamedIndividual>
    


    <!-- http://www.w3.org/ns/odrl/2/Asset -->

    <owl:NamedIndividual rdf:about="http://www.w3.org/ns/odrl/2/Asset">
        <rdf:type rdf:resource="http://www.w3.org/2004/02/skos/core#Concept"/>
    </owl:NamedIndividual>
    


    <!-- http://www.w3.org/ns/odrl/2/AssetCollection -->

    <owl:NamedIndividual rdf:about="http://www.w3.org/ns/odrl/2/AssetCollection">
        <rdf:type rdf:resource="http://www.w3.org/2004/02/skos/core#Concept"/>
    </owl:NamedIndividual>
    


    <!-- http://www.w3.org/ns/odrl/2/AssetScope -->

    <owl:NamedIndividual rdf:about="http://www.w3.org/ns/odrl/2/AssetScope">
        <rdf:type rdf:resource="http://www.w3.org/2004/02/skos/core#Concept"/>
        <rdfs:isDefinedBy rdf:resource="http://www.w3.org/ns/odrl/2/"/>
        <rdfs:label xml:lang="en">Asset Scope</rdfs:label>
        <owl:deprecated rdf:datatype="http://www.w3.org/2001/XMLSchema#boolean">true</owl:deprecated>
        <skos:definition xml:lang="en">Scopes for Asset Scope expressions.</skos:definition>
        <skos:note xml:lang="en">Instances of the AssetScope class represent the terms for the scope property of Assets.</skos:note>
    </owl:NamedIndividual>
    


    <!-- http://www.w3.org/ns/odrl/2/ConflictTerm -->

    <owl:NamedIndividual rdf:about="http://www.w3.org/ns/odrl/2/ConflictTerm">
        <rdf:type rdf:resource="http://www.w3.org/2004/02/skos/core#Concept"/>
    </owl:NamedIndividual>
    


    <!-- http://www.w3.org/ns/odrl/2/Constraint -->

    <owl:NamedIndividual rdf:about="http://www.w3.org/ns/odrl/2/Constraint">
        <rdf:type rdf:resource="http://www.w3.org/2004/02/skos/core#Concept"/>
    </owl:NamedIndividual>
    


    <!-- http://www.w3.org/ns/odrl/2/Duty -->

    <owl:NamedIndividual rdf:about="http://www.w3.org/ns/odrl/2/Duty">
        <rdf:type rdf:resource="http://www.w3.org/2004/02/skos/core#Concept"/>
    </owl:NamedIndividual>
    


    <!-- http://www.w3.org/ns/odrl/2/Group -->

    <owl:NamedIndividual rdf:about="http://www.w3.org/ns/odrl/2/Group">
        <rdf:type rdf:resource="http://www.w3.org/2004/02/skos/core#Concept"/>
        <rdf:type rdf:resource="http://www.w3.org/ns/odrl/2/PartyScope"/>
        <rdfs:isDefinedBy rdf:resource="http://www.w3.org/ns/odrl/2/"/>
        <rdfs:label xml:lang="en">Group</rdfs:label>
        <owl:deprecated rdf:datatype="http://www.w3.org/2001/XMLSchema#boolean">true</owl:deprecated>
        <skos:definition xml:lang="en">Specifies that the scope of the relationship is the defined group with multiple individual members.</skos:definition>
        <skos:scopeNote xml:lang="en">Non-Normative</skos:scopeNote>
    </owl:NamedIndividual>
    


    <!-- http://www.w3.org/ns/odrl/2/Individual -->

    <owl:NamedIndividual rdf:about="http://www.w3.org/ns/odrl/2/Individual">
        <rdf:type rdf:resource="http://www.w3.org/2004/02/skos/core#Concept"/>
        <rdf:type rdf:resource="http://www.w3.org/ns/odrl/2/PartyScope"/>
        <rdfs:isDefinedBy rdf:resource="http://www.w3.org/ns/odrl/2/"/>
        <rdfs:label xml:lang="en">Individual</rdfs:label>
        <owl:deprecated rdf:datatype="http://www.w3.org/2001/XMLSchema#boolean">true</owl:deprecated>
        <skos:definition xml:lang="en">Specifies that the scope of the relationship is the single Party individual.</skos:definition>
    </owl:NamedIndividual>
    


    <!-- http://www.w3.org/ns/odrl/2/LeftOperand -->

    <owl:NamedIndividual rdf:about="http://www.w3.org/ns/odrl/2/LeftOperand">
        <rdf:type rdf:resource="http://www.w3.org/2004/02/skos/core#Concept"/>
    </owl:NamedIndividual>
    


    <!-- http://www.w3.org/ns/odrl/2/LogicalConstraint -->

    <owl:NamedIndividual rdf:about="http://www.w3.org/ns/odrl/2/LogicalConstraint">
        <rdf:type rdf:resource="http://www.w3.org/2004/02/skos/core#Concept"/>
    </owl:NamedIndividual>
    


    <!-- http://www.w3.org/ns/odrl/2/Offer -->

    <owl:NamedIndividual rdf:about="http://www.w3.org/ns/odrl/2/Offer">
        <rdf:type rdf:resource="http://www.w3.org/2004/02/skos/core#Concept"/>
    </owl:NamedIndividual>
    


    <!-- http://www.w3.org/ns/odrl/2/Operator -->

    <owl:NamedIndividual rdf:about="http://www.w3.org/ns/odrl/2/Operator">
        <rdf:type rdf:resource="http://www.w3.org/2004/02/skos/core#Concept"/>
    </owl:NamedIndividual>
    


    <!-- http://www.w3.org/ns/odrl/2/Party -->

    <owl:NamedIndividual rdf:about="http://www.w3.org/ns/odrl/2/Party">
        <rdf:type rdf:resource="http://www.w3.org/2004/02/skos/core#Concept"/>
    </owl:NamedIndividual>
    


    <!-- http://www.w3.org/ns/odrl/2/PartyCollection -->

    <owl:NamedIndividual rdf:about="http://www.w3.org/ns/odrl/2/PartyCollection">
        <rdf:type rdf:resource="http://www.w3.org/2004/02/skos/core#Concept"/>
    </owl:NamedIndividual>
    


    <!-- http://www.w3.org/ns/odrl/2/PartyScope -->

    <owl:NamedIndividual rdf:about="http://www.w3.org/ns/odrl/2/PartyScope">
        <rdf:type rdf:resource="http://www.w3.org/2004/02/skos/core#Concept"/>
    </owl:NamedIndividual>
    


    <!-- http://www.w3.org/ns/odrl/2/Permission -->

    <owl:NamedIndividual rdf:about="http://www.w3.org/ns/odrl/2/Permission">
        <rdf:type rdf:resource="http://www.w3.org/2004/02/skos/core#Concept"/>
    </owl:NamedIndividual>
    


    <!-- http://www.w3.org/ns/odrl/2/Policy -->

    <owl:NamedIndividual rdf:about="http://www.w3.org/ns/odrl/2/Policy">
        <rdf:type rdf:resource="http://www.w3.org/2004/02/skos/core#Concept"/>
    </owl:NamedIndividual>
    


    <!-- http://www.w3.org/ns/odrl/2/Privacy -->

    <owl:NamedIndividual rdf:about="http://www.w3.org/ns/odrl/2/Privacy">
        <rdf:type rdf:resource="http://www.w3.org/2004/02/skos/core#Concept"/>
    </owl:NamedIndividual>
    


    <!-- http://www.w3.org/ns/odrl/2/Prohibition -->

    <owl:NamedIndividual rdf:about="http://www.w3.org/ns/odrl/2/Prohibition">
        <rdf:type rdf:resource="http://www.w3.org/2004/02/skos/core#Concept"/>
    </owl:NamedIndividual>
    


    <!-- http://www.w3.org/ns/odrl/2/Request -->

    <owl:NamedIndividual rdf:about="http://www.w3.org/ns/odrl/2/Request">
        <rdf:type rdf:resource="http://www.w3.org/2004/02/skos/core#Concept"/>
    </owl:NamedIndividual>
    


    <!-- http://www.w3.org/ns/odrl/2/RightOperand -->

    <owl:NamedIndividual rdf:about="http://www.w3.org/ns/odrl/2/RightOperand">
        <rdf:type rdf:resource="http://www.w3.org/2004/02/skos/core#Concept"/>
    </owl:NamedIndividual>
    


    <!-- http://www.w3.org/ns/odrl/2/Rule -->

    <owl:NamedIndividual rdf:about="http://www.w3.org/ns/odrl/2/Rule">
        <rdf:type rdf:resource="http://www.w3.org/2004/02/skos/core#Concept"/>
    </owl:NamedIndividual>
    


    <!-- http://www.w3.org/ns/odrl/2/Set -->

    <owl:NamedIndividual rdf:about="http://www.w3.org/ns/odrl/2/Set">
        <rdf:type rdf:resource="http://www.w3.org/2004/02/skos/core#Concept"/>
    </owl:NamedIndividual>
    


    <!-- http://www.w3.org/ns/odrl/2/Ticket -->

    <owl:NamedIndividual rdf:about="http://www.w3.org/ns/odrl/2/Ticket">
        <rdf:type rdf:resource="http://www.w3.org/2004/02/skos/core#Concept"/>
    </owl:NamedIndividual>
    


    <!-- http://www.w3.org/ns/odrl/2/UndefinedTerm -->

    <owl:NamedIndividual rdf:about="http://www.w3.org/ns/odrl/2/UndefinedTerm">
        <rdf:type rdf:resource="http://www.w3.org/2004/02/skos/core#Concept"/>
    </owl:NamedIndividual>
    


    <!-- http://www.w3.org/ns/odrl/2/absolutePosition -->

    <owl:NamedIndividual rdf:about="http://www.w3.org/ns/odrl/2/absolutePosition">
        <rdf:type rdf:resource="http://www.w3.org/2004/02/skos/core#Concept"/>
        <rdf:type rdf:resource="http://www.w3.org/ns/odrl/2/LeftOperand"/>
        <rdfs:isDefinedBy rdf:resource="http://www.w3.org/ns/odrl/2/"/>
        <rdfs:label xml:lang="en">Absolute Asset Position</rdfs:label>
        <skos:definition xml:lang="en">A point in space or time defined with absolute coordinates for the positioning of the target Asset.</skos:definition>
        <skos:note xml:lang="en">Example: The upper left corner of a picture may be constrained to a specific position of the canvas rendering it.</skos:note>
        <skos:scopeNote xml:lang="en">Non-Normative</skos:scopeNote>
    </owl:NamedIndividual>
    


    <!-- http://www.w3.org/ns/odrl/2/absoluteSize -->

    <owl:NamedIndividual rdf:about="http://www.w3.org/ns/odrl/2/absoluteSize">
        <rdf:type rdf:resource="http://www.w3.org/2004/02/skos/core#Concept"/>
        <rdf:type rdf:resource="http://www.w3.org/ns/odrl/2/LeftOperand"/>
        <rdfs:isDefinedBy rdf:resource="http://www.w3.org/ns/odrl/2/"/>
        <rdfs:label xml:lang="en">Absolute Asset Size</rdfs:label>
        <skos:definition xml:lang="en">Measure(s) of one or two axes for 2D-objects or measure(s) of one to tree axes for 3D-objects of the target Asset.</skos:definition>
        <skos:note xml:lang="en">Example: The image can be resized in width to a maximum of 1000px.</skos:note>
        <skos:scopeNote xml:lang="en">Non-Normative</skos:scopeNote>
    </owl:NamedIndividual>
    


    <!-- http://www.w3.org/ns/odrl/2/absoluteSpatialPosition -->

    <owl:NamedIndividual rdf:about="http://www.w3.org/ns/odrl/2/absoluteSpatialPosition">
        <rdf:type rdf:resource="http://www.w3.org/2004/02/skos/core#Concept"/>
        <rdf:type rdf:resource="http://www.w3.org/ns/odrl/2/LeftOperand"/>
        <rdfs:isDefinedBy rdf:resource="http://www.w3.org/ns/odrl/2/"/>
        <rdfs:label xml:lang="en">Absolute Spatial Asset Position</rdfs:label>
        <skos:broader rdf:resource="http://www.w3.org/ns/odrl/2/absolutePosition"/>
        <skos:definition xml:lang="en">The absolute spatial positions of four corners of a rectangle on a 2D-canvas or the eight corners of a cuboid in a 3D-space for the target Asset to fit.</skos:definition>
        <skos:note xml:lang="en">Example: The upper left corner of a picture may be constrained to a specific position of the canvas rendering it. Note: see also the Left Operand Relative Spatial Asset Position. </skos:note>
        <skos:scopeNote xml:lang="en">Non-Normative</skos:scopeNote>
    </owl:NamedIndividual>
    


    <!-- http://www.w3.org/ns/odrl/2/absoluteTemporalPosition -->

    <owl:NamedIndividual rdf:about="http://www.w3.org/ns/odrl/2/absoluteTemporalPosition">
        <rdf:type rdf:resource="http://www.w3.org/2004/02/skos/core#Concept"/>
        <rdf:type rdf:resource="http://www.w3.org/ns/odrl/2/LeftOperand"/>
        <rdfs:isDefinedBy rdf:resource="http://www.w3.org/ns/odrl/2/"/>
        <rdfs:label xml:lang="en">Absolute Temporal Asset Position</rdfs:label>
        <skos:broader rdf:resource="http://www.w3.org/ns/odrl/2/absolutePosition"/>
        <skos:definition xml:lang="en">The absolute temporal positions in a media stream the target Asset has to fit.</skos:definition>
        <skos:note xml:lang="en">Use with Actions including the target Asset in a larger media stream. The fragment part of a Media Fragment URI (https://www.w3.org/TR/media-frags/) may be used for the right operand. See the Left Operand realativeTemporalPosition. &lt;br /&gt;Example: The MP3 music file must be positioned between second 192 and 250 of the temporal length of a stream.</skos:note>
        <skos:scopeNote xml:lang="en">Non-Normative</skos:scopeNote>
    </owl:NamedIndividual>
    


    <!-- http://www.w3.org/ns/odrl/2/acceptTracking -->

    <owl:NamedIndividual rdf:about="http://www.w3.org/ns/odrl/2/acceptTracking">
        <rdf:type rdf:resource="http://www.w3.org/2004/02/skos/core#Concept"/>
        <rdf:type rdf:resource="http://www.w3.org/ns/odrl/2/Action"/>
        <odrl:includedIn rdf:resource="http://www.w3.org/ns/odrl/2/use"/>
        <rdfs:isDefinedBy rdf:resource="http://www.w3.org/ns/odrl/2/"/>
        <rdfs:label xml:lang="en">Accept Tracking</rdfs:label>
        <skos:definition xml:lang="en">To accept that the use of the Asset may be tracked.</skos:definition>
        <skos:note xml:lang="en">The collected information may be tracked by the Assigner, or may link to a Party with the role &apos;trackingParty&apos; function.</skos:note>
        <skos:scopeNote xml:lang="en">Non-Normative</skos:scopeNote>
    </owl:NamedIndividual>
    


    <!-- http://www.w3.org/ns/odrl/2/action -->

    <owl:NamedIndividual rdf:about="http://www.w3.org/ns/odrl/2/action">
        <rdf:type rdf:resource="http://www.w3.org/2004/02/skos/core#Concept"/>
    </owl:NamedIndividual>
    


    <!-- http://www.w3.org/ns/odrl/2/adHocShare -->

    <owl:NamedIndividual rdf:about="http://www.w3.org/ns/odrl/2/adHocShare">
        <rdf:type rdf:resource="http://www.w3.org/2004/02/skos/core#Concept"/>
        <rdf:type rdf:resource="http://www.w3.org/ns/odrl/2/Action"/>
        <rdfs:isDefinedBy rdf:resource="http://www.w3.org/ns/odrl/2/"/>
        <rdfs:label xml:lang="en">Ad-hoc sharing</rdfs:label>
        <owl:deprecated rdf:datatype="http://www.w3.org/2001/XMLSchema#boolean">true</owl:deprecated>
        <skos:definition xml:lang="en">The act of sharing the asset to parties in close proximity to the owner.</skos:definition>
        <skos:note xml:lang="en">This original term and URI from the OMA specification should be used: http://www.openmobilealliance.com/oma-dd/adhoc-share .</skos:note>
    </owl:NamedIndividual>
    


    <!-- http://www.w3.org/ns/odrl/2/aggregate -->

    <owl:NamedIndividual rdf:about="http://www.w3.org/ns/odrl/2/aggregate">
        <rdf:type rdf:resource="http://www.w3.org/2004/02/skos/core#Concept"/>
        <rdf:type rdf:resource="http://www.w3.org/ns/odrl/2/Action"/>
        <odrl:includedIn rdf:resource="http://www.w3.org/ns/odrl/2/use"/>
        <rdfs:isDefinedBy rdf:resource="http://www.w3.org/ns/odrl/2/"/>
        <rdfs:label xml:lang="en">Aggregate</rdfs:label>
        <skos:definition xml:lang="en">To use the Asset or parts of it as part of a composite collection.</skos:definition>
        <skos:scopeNote xml:lang="en">Non-Normative</skos:scopeNote>
    </owl:NamedIndividual>
    


    <!-- http://www.w3.org/ns/odrl/2/and -->

    <owl:NamedIndividual rdf:about="http://www.w3.org/ns/odrl/2/and">
        <rdf:type rdf:resource="http://www.w3.org/2004/02/skos/core#Concept"/>
    </owl:NamedIndividual>
    


    <!-- http://www.w3.org/ns/odrl/2/andSequence -->

    <owl:NamedIndividual rdf:about="http://www.w3.org/ns/odrl/2/andSequence">
        <rdf:type rdf:resource="http://www.w3.org/2004/02/skos/core#Concept"/>
    </owl:NamedIndividual>
    


    <!-- http://www.w3.org/ns/odrl/2/annotate -->

    <owl:NamedIndividual rdf:about="http://www.w3.org/ns/odrl/2/annotate">
        <rdf:type rdf:resource="http://www.w3.org/2004/02/skos/core#Concept"/>
        <rdf:type rdf:resource="http://www.w3.org/ns/odrl/2/Action"/>
        <odrl:includedIn rdf:resource="http://www.w3.org/ns/odrl/2/use"/>
        <rdfs:isDefinedBy rdf:resource="http://www.w3.org/ns/odrl/2/"/>
        <rdfs:label xml:lang="en">Annotate</rdfs:label>
        <skos:definition xml:lang="en">To add explanatory notations/commentaries to the Asset without modifying the Asset in any other way.</skos:definition>
        <skos:scopeNote xml:lang="en">Non-Normative</skos:scopeNote>
    </owl:NamedIndividual>
    


    <!-- http://www.w3.org/ns/odrl/2/anonymize -->

    <owl:NamedIndividual rdf:about="http://www.w3.org/ns/odrl/2/anonymize">
        <rdf:type rdf:resource="http://www.w3.org/2004/02/skos/core#Concept"/>
        <rdf:type rdf:resource="http://www.w3.org/ns/odrl/2/Action"/>
        <odrl:includedIn rdf:resource="http://www.w3.org/ns/odrl/2/use"/>
        <rdfs:isDefinedBy rdf:resource="http://www.w3.org/ns/odrl/2/"/>
        <rdfs:label xml:lang="en">Anonymize</rdfs:label>
        <skos:definition xml:lang="en">To anonymize all or parts of the Asset.</skos:definition>
        <skos:note xml:lang="en">For example, to remove identifying particulars for statistical or for other comparable purposes, or to use the Asset without stating the author/source.</skos:note>
        <skos:scopeNote xml:lang="en">Non-Normative</skos:scopeNote>
    </owl:NamedIndividual>
    


    <!-- http://www.w3.org/ns/odrl/2/append -->

    <owl:NamedIndividual rdf:about="http://www.w3.org/ns/odrl/2/append">
        <rdf:type rdf:resource="http://www.w3.org/2004/02/skos/core#Concept"/>
        <rdf:type rdf:resource="http://www.w3.org/ns/odrl/2/Action"/>
        <rdfs:isDefinedBy rdf:resource="http://www.w3.org/ns/odrl/2/"/>
        <rdfs:label xml:lang="en">Append</rdfs:label>
        <owl:deprecated rdf:datatype="http://www.w3.org/2001/XMLSchema#boolean">true</owl:deprecated>
        <skos:definition xml:lang="en">The act of adding to the end of an asset.</skos:definition>
        <skos:exactMatch rdf:resource="http://www.w3.org/ns/odrl/2/modify"/>
    </owl:NamedIndividual>
    


    <!-- http://www.w3.org/ns/odrl/2/appendTo -->

    <owl:NamedIndividual rdf:about="http://www.w3.org/ns/odrl/2/appendTo">
        <rdf:type rdf:resource="http://www.w3.org/2004/02/skos/core#Concept"/>
        <rdf:type rdf:resource="http://www.w3.org/ns/odrl/2/Action"/>
        <rdfs:isDefinedBy rdf:resource="http://www.w3.org/ns/odrl/2/"/>
        <rdfs:label xml:lang="en">Append To</rdfs:label>
        <owl:deprecated rdf:datatype="http://www.w3.org/2001/XMLSchema#boolean">true</owl:deprecated>
        <skos:definition xml:lang="en">The act of appending data to the Asset without modifying the Asset in any other way.</skos:definition>
        <skos:exactMatch rdf:resource="http://www.w3.org/ns/odrl/2/modify"/>
    </owl:NamedIndividual>
    


    <!-- http://www.w3.org/ns/odrl/2/archive -->

    <owl:NamedIndividual rdf:about="http://www.w3.org/ns/odrl/2/archive">
        <rdf:type rdf:resource="http://www.w3.org/2004/02/skos/core#Concept"/>
        <rdf:type rdf:resource="http://www.w3.org/ns/odrl/2/Action"/>
        <odrl:includedIn rdf:resource="http://www.w3.org/ns/odrl/2/use"/>
        <rdfs:isDefinedBy rdf:resource="http://www.w3.org/ns/odrl/2/"/>
        <rdfs:label xml:lang="en">Archive</rdfs:label>
        <skos:definition xml:lang="en">To store the Asset (in a non-transient form).</skos:definition>
        <skos:note xml:lang="en">Temporal constraints may be used for temporal conditions.</skos:note>
        <skos:scopeNote xml:lang="en">Non-Normative</skos:scopeNote>
    </owl:NamedIndividual>
    


    <!-- http://www.w3.org/ns/odrl/2/assignee -->

    <owl:NamedIndividual rdf:about="http://www.w3.org/ns/odrl/2/assignee">
        <rdf:type rdf:resource="http://www.w3.org/2004/02/skos/core#Concept"/>
    </owl:NamedIndividual>
    


    <!-- http://www.w3.org/ns/odrl/2/assigneeOf -->

    <owl:NamedIndividual rdf:about="http://www.w3.org/ns/odrl/2/assigneeOf">
        <rdf:type rdf:resource="http://www.w3.org/2004/02/skos/core#Concept"/>
    </owl:NamedIndividual>
    


    <!-- http://www.w3.org/ns/odrl/2/assigner -->

    <owl:NamedIndividual rdf:about="http://www.w3.org/ns/odrl/2/assigner">
        <rdf:type rdf:resource="http://www.w3.org/2004/02/skos/core#Concept"/>
    </owl:NamedIndividual>
    


    <!-- http://www.w3.org/ns/odrl/2/assignerOf -->

    <owl:NamedIndividual rdf:about="http://www.w3.org/ns/odrl/2/assignerOf">
        <rdf:type rdf:resource="http://www.w3.org/2004/02/skos/core#Concept"/>
    </owl:NamedIndividual>
    


    <!-- http://www.w3.org/ns/odrl/2/attachPolicy -->

    <owl:NamedIndividual rdf:about="http://www.w3.org/ns/odrl/2/attachPolicy">
        <rdf:type rdf:resource="http://www.w3.org/2004/02/skos/core#Concept"/>
        <rdf:type rdf:resource="http://www.w3.org/ns/odrl/2/Action"/>
        <rdfs:isDefinedBy rdf:resource="http://www.w3.org/ns/odrl/2/"/>
        <rdfs:label xml:lang="en">Attach policy</rdfs:label>
        <owl:deprecated rdf:datatype="http://www.w3.org/2001/XMLSchema#boolean">true</owl:deprecated>
        <skos:definition xml:lang="en">The act of keeping the policy notice with the asset.</skos:definition>
        <skos:exactMatch rdf:resource="http://creativecommons.org/ns#Notice"/>
    </owl:NamedIndividual>
    


    <!-- http://www.w3.org/ns/odrl/2/attachSource -->

    <owl:NamedIndividual rdf:about="http://www.w3.org/ns/odrl/2/attachSource">
        <rdf:type rdf:resource="http://www.w3.org/2004/02/skos/core#Concept"/>
        <rdf:type rdf:resource="http://www.w3.org/ns/odrl/2/Action"/>
        <rdfs:isDefinedBy rdf:resource="http://www.w3.org/ns/odrl/2/"/>
        <rdfs:label xml:lang="en">Attach source</rdfs:label>
        <owl:deprecated rdf:datatype="http://www.w3.org/2001/XMLSchema#boolean">true</owl:deprecated>
        <skos:definition xml:lang="en">The act of attaching the source of the asset and its derivatives.</skos:definition>
        <skos:exactMatch rdf:resource="http://creativecommons.org/ns#SourceCode"/>
    </owl:NamedIndividual>
    


    <!-- http://www.w3.org/ns/odrl/2/attribute -->

    <owl:NamedIndividual rdf:about="http://www.w3.org/ns/odrl/2/attribute">
        <rdf:type rdf:resource="http://www.w3.org/2004/02/skos/core#Concept"/>
        <rdf:type rdf:resource="http://www.w3.org/ns/odrl/2/Action"/>
        <odrl:includedIn rdf:resource="http://www.w3.org/ns/odrl/2/use"/>
        <rdfs:isDefinedBy rdf:resource="http://www.w3.org/ns/odrl/2/"/>
        <rdfs:label xml:lang="en">Attribute</rdfs:label>
        <skos:definition xml:lang="en">To attribute the use of the Asset.</skos:definition>
        <skos:note xml:lang="en">May link to an Asset with the attribution information. May link to a Party with the  role “attributedParty” function.</skos:note>
        <skos:scopeNote xml:lang="en">Non-Normative</skos:scopeNote>
    </owl:NamedIndividual>
    


    <!-- http://www.w3.org/ns/odrl/2/attributedParty -->

    <owl:NamedIndividual rdf:about="http://www.w3.org/ns/odrl/2/attributedParty">
        <rdf:type rdf:resource="http://www.w3.org/2004/02/skos/core#Concept"/>
    </owl:NamedIndividual>
    


    <!-- http://www.w3.org/ns/odrl/2/attributingParty -->

    <owl:NamedIndividual rdf:about="http://www.w3.org/ns/odrl/2/attributingParty">
        <rdf:type rdf:resource="http://www.w3.org/2004/02/skos/core#Concept"/>
    </owl:NamedIndividual>
    


    <!-- http://www.w3.org/ns/odrl/2/commercialize -->

    <owl:NamedIndividual rdf:about="http://www.w3.org/ns/odrl/2/commercialize">
        <rdf:type rdf:resource="http://www.w3.org/2004/02/skos/core#Concept"/>
        <rdf:type rdf:resource="http://www.w3.org/ns/odrl/2/Action"/>
        <rdfs:isDefinedBy rdf:resource="http://www.w3.org/ns/odrl/2/"/>
        <rdfs:label xml:lang="en">Commercialize</rdfs:label>
        <owl:deprecated rdf:datatype="http://www.w3.org/2001/XMLSchema#boolean">true</owl:deprecated>
        <skos:definition xml:lang="en">The act of using the asset in a business environment.</skos:definition>
        <skos:exactMatch rdf:resource="http://creativecommons.org/ns#CommercialUse"/>
    </owl:NamedIndividual>
    


    <!-- http://www.w3.org/ns/odrl/2/compensate -->

    <owl:NamedIndividual rdf:about="http://www.w3.org/ns/odrl/2/compensate">
        <rdf:type rdf:resource="http://www.w3.org/2004/02/skos/core#Concept"/>
        <rdf:type rdf:resource="http://www.w3.org/ns/odrl/2/Action"/>
        <odrl:includedIn rdf:resource="http://www.w3.org/ns/odrl/2/use"/>
        <rdfs:isDefinedBy rdf:resource="http://www.w3.org/ns/odrl/2/"/>
        <rdfs:label xml:lang="en">Compensate</rdfs:label>
        <skos:definition xml:lang="en">To compensate by transfer of some amount of value, if defined, for using or selling the Asset.</skos:definition>
        <skos:note xml:lang="en">The compensation may use different types of things with a value: (i) the thing is expressed by the value (term) of the Constraint name; (b) the value is expressed by operator, rightOperand, dataType and unit. Typically the assignee will compensate the assigner, but other compensation party roles may be used.</skos:note>
        <skos:scopeNote xml:lang="en">Non-Normative</skos:scopeNote>
    </owl:NamedIndividual>
    


    <!-- http://www.w3.org/ns/odrl/2/compensatedParty -->

    <owl:NamedIndividual rdf:about="http://www.w3.org/ns/odrl/2/compensatedParty">
        <rdf:type rdf:resource="http://www.w3.org/2004/02/skos/core#Concept"/>
    </owl:NamedIndividual>
    


    <!-- http://www.w3.org/ns/odrl/2/compensatingParty -->

    <owl:NamedIndividual rdf:about="http://www.w3.org/ns/odrl/2/compensatingParty">
        <rdf:type rdf:resource="http://www.w3.org/2004/02/skos/core#Concept"/>
    </owl:NamedIndividual>
    


    <!-- http://www.w3.org/ns/odrl/2/concurrentUse -->

    <owl:NamedIndividual rdf:about="http://www.w3.org/ns/odrl/2/concurrentUse">
        <rdf:type rdf:resource="http://www.w3.org/2004/02/skos/core#Concept"/>
        <rdf:type rdf:resource="http://www.w3.org/ns/odrl/2/Action"/>
        <odrl:includedIn rdf:resource="http://www.w3.org/ns/odrl/2/use"/>
        <rdfs:isDefinedBy rdf:resource="http://www.w3.org/ns/odrl/2/"/>
        <rdfs:label xml:lang="en">Concurrent Use</rdfs:label>
        <skos:definition xml:lang="en">To create multiple copies of the Asset that are being concurrently used.</skos:definition>
        <skos:scopeNote xml:lang="en">Non-Normative</skos:scopeNote>
    </owl:NamedIndividual>
    


    <!-- http://www.w3.org/ns/odrl/2/conflict -->

    <owl:NamedIndividual rdf:about="http://www.w3.org/ns/odrl/2/conflict">
        <rdf:type rdf:resource="http://www.w3.org/2004/02/skos/core#Concept"/>
    </owl:NamedIndividual>
    


    <!-- http://www.w3.org/ns/odrl/2/consentedParty -->

    <owl:NamedIndividual rdf:about="http://www.w3.org/ns/odrl/2/consentedParty">
        <rdf:type rdf:resource="http://www.w3.org/2004/02/skos/core#Concept"/>
    </owl:NamedIndividual>
    


    <!-- http://www.w3.org/ns/odrl/2/consentingParty -->

    <owl:NamedIndividual rdf:about="http://www.w3.org/ns/odrl/2/consentingParty">
        <rdf:type rdf:resource="http://www.w3.org/2004/02/skos/core#Concept"/>
    </owl:NamedIndividual>
    


    <!-- http://www.w3.org/ns/odrl/2/consequence -->

    <owl:NamedIndividual rdf:about="http://www.w3.org/ns/odrl/2/consequence">
        <rdf:type rdf:resource="http://www.w3.org/2004/02/skos/core#Concept"/>
    </owl:NamedIndividual>
    


    <!-- http://www.w3.org/ns/odrl/2/constraint -->

    <owl:NamedIndividual rdf:about="http://www.w3.org/ns/odrl/2/constraint">
        <rdf:type rdf:resource="http://www.w3.org/2004/02/skos/core#Concept"/>
    </owl:NamedIndividual>
    


    <!-- http://www.w3.org/ns/odrl/2/contractedParty -->

    <owl:NamedIndividual rdf:about="http://www.w3.org/ns/odrl/2/contractedParty">
        <rdf:type rdf:resource="http://www.w3.org/2004/02/skos/core#Concept"/>
    </owl:NamedIndividual>
    


    <!-- http://www.w3.org/ns/odrl/2/contractingParty -->

    <owl:NamedIndividual rdf:about="http://www.w3.org/ns/odrl/2/contractingParty">
        <rdf:type rdf:resource="http://www.w3.org/2004/02/skos/core#Concept"/>
    </owl:NamedIndividual>
    


    <!-- http://www.w3.org/ns/odrl/2/copy -->

    <owl:NamedIndividual rdf:about="http://www.w3.org/ns/odrl/2/copy">
        <rdf:type rdf:resource="http://www.w3.org/2004/02/skos/core#Concept"/>
        <rdf:type rdf:resource="http://www.w3.org/ns/odrl/2/Action"/>
        <owl:sameAs rdf:resource="http://www.w3.org/ns/odrl/2/reproduce"/>
        <rdfs:isDefinedBy rdf:resource="http://www.w3.org/ns/odrl/2/"/>
        <rdfs:label xml:lang="en">Copy</rdfs:label>
        <owl:deprecated rdf:datatype="http://www.w3.org/2001/XMLSchema#boolean">true</owl:deprecated>
        <skos:definition xml:lang="en">The act of making an exact reproduction of the asset.</skos:definition>
        <skos:exactMatch rdf:resource="http://www.w3.org/ns/odrl/2/reproduce"/>
    </owl:NamedIndividual>
    


    <!-- http://www.w3.org/ns/odrl/2/reproduce -->

    <rdf:Description rdf:about="http://www.w3.org/ns/odrl/2/reproduce"/>
    


    <!-- http://www.w3.org/ns/odrl/2/core -->

    <owl:NamedIndividual rdf:about="http://www.w3.org/ns/odrl/2/core">
        <rdf:type rdf:resource="http://www.w3.org/2004/02/skos/core#Concept"/>
        <rdfs:isDefinedBy rdf:resource="http://www.w3.org/ns/odrl/2/"/>
        <rdfs:label xml:lang="en">ODRL Core Profile</rdfs:label>
        <skos:definition xml:lang="en">Identifier for the ODRL Core Profile</skos:definition>
    </owl:NamedIndividual>
    


    <!-- http://www.w3.org/ns/odrl/2/count -->

    <owl:NamedIndividual rdf:about="http://www.w3.org/ns/odrl/2/count">
        <rdf:type rdf:resource="http://www.w3.org/2004/02/skos/core#Concept"/>
        <rdf:type rdf:resource="http://www.w3.org/ns/odrl/2/LeftOperand"/>
        <rdfs:isDefinedBy rdf:resource="http://www.w3.org/ns/odrl/2/"/>
        <rdfs:label xml:lang="en">Count</rdfs:label>
        <skos:definition xml:lang="en">Numeric count of executions of the action of the Rule.</skos:definition>
        <skos:scopeNote xml:lang="en">Non-Normative</skos:scopeNote>
    </owl:NamedIndividual>
    


    <!-- http://www.w3.org/ns/odrl/2/dataType -->

    <owl:NamedIndividual rdf:about="http://www.w3.org/ns/odrl/2/dataType">
        <rdf:type rdf:resource="http://www.w3.org/2004/02/skos/core#Concept"/>
    </owl:NamedIndividual>
    


    <!-- http://www.w3.org/ns/odrl/2/dateTime -->

    <owl:NamedIndividual rdf:about="http://www.w3.org/ns/odrl/2/dateTime">
        <rdf:type rdf:resource="http://www.w3.org/2004/02/skos/core#Concept"/>
        <rdf:type rdf:resource="http://www.w3.org/ns/odrl/2/LeftOperand"/>
        <rdfs:isDefinedBy rdf:resource="http://www.w3.org/ns/odrl/2/"/>
        <rdfs:label xml:lang="en">Datetime</rdfs:label>
        <skos:definition xml:lang="en">The date (and optional time and timezone) of exercising the action of the Rule. Right operand value MUST be an xsd:date or xsd:dateTime as defined by [[xmlschema11-2]].</skos:definition>
        <skos:note xml:lang="en">The use of Timezone information is strongly recommended. The Rule may be exercised before (with operator lt/lteq) or after (with operator gt/gteq) the date(time) defined by the Right operand. &lt;br /&gt;Example: &lt;code&gt;dateTime gteq 2017-12-31T06:00Z&lt;/code&gt; means the Rule can only be exercised after (and including) 6:00AM on the 31st Decemeber 2017 UTC time.</skos:note>
        <skos:scopeNote xml:lang="en">Non-Normative</skos:scopeNote>
    </owl:NamedIndividual>
    


    <!-- http://www.w3.org/ns/odrl/2/delayPeriod -->

    <owl:NamedIndividual rdf:about="http://www.w3.org/ns/odrl/2/delayPeriod">
        <rdf:type rdf:resource="http://www.w3.org/2004/02/skos/core#Concept"/>
        <rdf:type rdf:resource="http://www.w3.org/ns/odrl/2/LeftOperand"/>
        <rdfs:isDefinedBy rdf:resource="http://www.w3.org/ns/odrl/2/"/>
        <rdfs:label xml:lang="en">Delay Period</rdfs:label>
        <skos:definition xml:lang="en">A time delay period prior to exercising the action of the Rule. The point in time triggering this period MAY be defined by another temporal Constraint combined by a Logical Constraint (utilising the odrl:andSequence operand). Right operand value MUST be an xsd:duration as defined by [[xmlschema11-2]].</skos:definition>
        <skos:note xml:lang="en">Only the eq, gt, gteq operators SHOULD be used. &lt;br /&gt;Example: &lt;code&gt;delayPeriod eq P60M&lt;/code&gt; indicates a delay of 60 Minutes before exercising the action.</skos:note>
        <skos:scopeNote xml:lang="en">Non-Normative</skos:scopeNote>
    </owl:NamedIndividual>
    


    <!-- http://www.w3.org/ns/odrl/2/delete -->

    <owl:NamedIndividual rdf:about="http://www.w3.org/ns/odrl/2/delete">
        <rdf:type rdf:resource="http://www.w3.org/2004/02/skos/core#Concept"/>
        <rdf:type rdf:resource="http://www.w3.org/ns/odrl/2/Action"/>
        <odrl:includedIn rdf:resource="http://www.w3.org/ns/odrl/2/use"/>
        <rdfs:isDefinedBy rdf:resource="http://www.w3.org/ns/odrl/2/"/>
        <rdfs:label xml:lang="en">Delete</rdfs:label>
        <skos:definition xml:lang="en">To permanently remove all copies of the Asset after it has been used.</skos:definition>
        <skos:note xml:lang="en">Use a constraint to define under which conditions the Asset must be deleted.</skos:note>
        <skos:scopeNote xml:lang="en">Non-Normative</skos:scopeNote>
    </owl:NamedIndividual>
    


    <!-- http://www.w3.org/ns/odrl/2/deliveryChannel -->

    <owl:NamedIndividual rdf:about="http://www.w3.org/ns/odrl/2/deliveryChannel">
        <rdf:type rdf:resource="http://www.w3.org/2004/02/skos/core#Concept"/>
        <rdf:type rdf:resource="http://www.w3.org/ns/odrl/2/LeftOperand"/>
        <rdfs:isDefinedBy rdf:resource="http://www.w3.org/ns/odrl/2/"/>
        <rdfs:label xml:lang="en">Delivery Channel</rdfs:label>
        <skos:definition xml:lang="en">The delivery channel used for exercising the action of the Rule.</skos:definition>
        <skos:note xml:lang="en">Example: the asset may be distributed only on mobile networks.</skos:note>
        <skos:scopeNote xml:lang="en">Non-Normative</skos:scopeNote>
    </owl:NamedIndividual>
    


    <!-- http://www.w3.org/ns/odrl/2/derive -->

    <owl:NamedIndividual rdf:about="http://www.w3.org/ns/odrl/2/derive">
        <rdf:type rdf:resource="http://www.w3.org/2004/02/skos/core#Concept"/>
        <rdf:type rdf:resource="http://www.w3.org/ns/odrl/2/Action"/>
        <odrl:includedIn rdf:resource="http://www.w3.org/ns/odrl/2/use"/>
        <rdfs:isDefinedBy rdf:resource="http://www.w3.org/ns/odrl/2/"/>
        <rdfs:label xml:lang="en">Derive</rdfs:label>
        <skos:definition xml:lang="en">To create a new derivative Asset from this Asset and to edit or modify the derivative.</skos:definition>
        <skos:note xml:lang="en">A new asset is created and may have significant overlaps with the original Asset. (Note that the notion of whether or not the change is significant enough to qualify as a new asset is subjective). To the derived Asset a next policy may be applied.</skos:note>
        <skos:scopeNote xml:lang="en">Non-Normative</skos:scopeNote>
    </owl:NamedIndividual>
    


    <!-- http://www.w3.org/ns/odrl/2/device -->

    <owl:NamedIndividual rdf:about="http://www.w3.org/ns/odrl/2/device">
        <rdf:type rdf:resource="http://www.w3.org/2004/02/skos/core#Concept"/>
        <rdf:type rdf:resource="http://www.w3.org/ns/odrl/2/LeftOperand"/>
        <rdfs:isDefinedBy rdf:resource="http://www.w3.org/ns/odrl/2/"/>
        <rdfs:label xml:lang="en">Device</rdfs:label>
        <owl:deprecated rdf:datatype="http://www.w3.org/2001/XMLSchema#boolean">true</owl:deprecated>
        <skos:definition xml:lang="en">An identified device used for exercising the action of the Rule.</skos:definition>
        <skos:exactMatch rdf:resource="http://www.w3.org/ns/odrl/2/systemDevice"/>
        <skos:note>See System Device.</skos:note>
    </owl:NamedIndividual>
    


    <!-- http://www.w3.org/ns/odrl/2/digitize -->

    <owl:NamedIndividual rdf:about="http://www.w3.org/ns/odrl/2/digitize">
        <rdf:type rdf:resource="http://www.w3.org/2004/02/skos/core#Concept"/>
        <rdf:type rdf:resource="http://www.w3.org/ns/odrl/2/Action"/>
        <odrl:includedIn rdf:resource="http://www.w3.org/ns/odrl/2/use"/>
        <rdfs:isDefinedBy rdf:resource="http://www.w3.org/ns/odrl/2/"/>
        <rdfs:label xml:lang="en">Digitize</rdfs:label>
        <skos:definition xml:lang="en">To produce a digital copy of (or otherwise digitize) the Asset from its analogue form.</skos:definition>
        <skos:scopeNote xml:lang="en">Non-Normative</skos:scopeNote>
    </owl:NamedIndividual>
    


    <!-- http://www.w3.org/ns/odrl/2/display -->

    <owl:NamedIndividual rdf:about="http://www.w3.org/ns/odrl/2/display">
        <rdf:type rdf:resource="http://www.w3.org/2004/02/skos/core#Concept"/>
        <rdf:type rdf:resource="http://www.w3.org/ns/odrl/2/Action"/>
        <odrl:includedIn rdf:resource="http://www.w3.org/ns/odrl/2/play"/>
        <rdfs:isDefinedBy rdf:resource="http://www.w3.org/ns/odrl/2/"/>
        <rdfs:label xml:lang="en">Display</rdfs:label>
        <skos:definition xml:lang="en">To create a static and transient rendition of an Asset.</skos:definition>
        <skos:note xml:lang="en">For example, displaying an image on a screen. If the action is to be performed to a wider audience than just the Assignees, then the Recipient constraint is recommended to be used.</skos:note>
        <skos:scopeNote xml:lang="en">Non-Normative</skos:scopeNote>
    </owl:NamedIndividual>
    


    <!-- http://www.w3.org/ns/odrl/2/distribute -->

    <owl:NamedIndividual rdf:about="http://www.w3.org/ns/odrl/2/distribute">
        <rdf:type rdf:resource="http://www.w3.org/2004/02/skos/core#Concept"/>
        <rdf:type rdf:resource="http://www.w3.org/ns/odrl/2/Action"/>
        <odrl:includedIn rdf:resource="http://www.w3.org/ns/odrl/2/use"/>
        <rdfs:isDefinedBy rdf:resource="http://www.w3.org/ns/odrl/2/"/>
        <rdfs:label xml:lang="en">Distribute</rdfs:label>
        <skos:definition xml:lang="en">To supply the Asset to third-parties.</skos:definition>
        <skos:note xml:lang="en">It is recommended to use nextPolicy to express the allowable usages by third-parties.</skos:note>
        <skos:scopeNote xml:lang="en">Non-Normative</skos:scopeNote>
    </owl:NamedIndividual>
    


    <!-- http://www.w3.org/ns/odrl/2/duty -->

    <owl:NamedIndividual rdf:about="http://www.w3.org/ns/odrl/2/duty">
        <rdf:type rdf:resource="http://www.w3.org/2004/02/skos/core#Concept"/>
    </owl:NamedIndividual>
    


    <!-- http://www.w3.org/ns/odrl/2/elapsedTime -->

    <owl:NamedIndividual rdf:about="http://www.w3.org/ns/odrl/2/elapsedTime">
        <rdf:type rdf:resource="http://www.w3.org/2004/02/skos/core#Concept"/>
        <rdf:type rdf:resource="http://www.w3.org/ns/odrl/2/LeftOperand"/>
        <rdfs:isDefinedBy rdf:resource="http://www.w3.org/ns/odrl/2/"/>
        <rdfs:label xml:lang="en">Elapsed Time</rdfs:label>
        <skos:definition xml:lang="en">A continuous elapsed time period which may be used for exercising of the action of the Rule. Right operand value MUST be an xsd:duration as defined by [[xmlschema11-2]].</skos:definition>
        <skos:note>Only the eq, lt, lteq operators SHOULD be used. See also Metered Time. &lt;br /&gt;Example: &lt;code&gt;elpasedTime eq P60M&lt;/code&gt; indicates a total elapsed time of 60 Minutes.</skos:note>
        <skos:scopeNote xml:lang="en">Non-Normative</skos:scopeNote>
    </owl:NamedIndividual>
    


    <!-- http://www.w3.org/ns/odrl/2/ensureExclusivity -->

    <owl:NamedIndividual rdf:about="http://www.w3.org/ns/odrl/2/ensureExclusivity">
        <rdf:type rdf:resource="http://www.w3.org/2004/02/skos/core#Concept"/>
        <rdf:type rdf:resource="http://www.w3.org/ns/odrl/2/Action"/>
        <odrl:includedIn rdf:resource="http://www.w3.org/ns/odrl/2/use"/>
        <rdfs:isDefinedBy rdf:resource="http://www.w3.org/ns/odrl/2/"/>
        <rdfs:label xml:lang="en">Ensure Exclusivity</rdfs:label>
        <skos:definition xml:lang="en">To ensure that the Rule on the Asset is exclusive.</skos:definition>
        <skos:note xml:lang="en">If used as a Duty, the assignee should be explicitly indicated as the party that is ensuring the exclusivity of the Rule.</skos:note>
        <skos:scopeNote xml:lang="en">Non-Normative</skos:scopeNote>
    </owl:NamedIndividual>
    


    <!-- http://www.w3.org/ns/odrl/2/eq -->

    <owl:NamedIndividual rdf:about="http://www.w3.org/ns/odrl/2/eq">
        <rdf:type rdf:resource="http://www.w3.org/2004/02/skos/core#Concept"/>
        <rdf:type rdf:resource="http://www.w3.org/ns/odrl/2/Operator"/>
        <rdfs:isDefinedBy rdf:resource="http://www.w3.org/ns/odrl/2/"/>
        <rdfs:label xml:lang="en">Equal to</rdfs:label>
        <skos:definition xml:lang="en">Indicating that a given value equals the right operand of the Constraint.</skos:definition>
    </owl:NamedIndividual>
    


    <!-- http://www.w3.org/ns/odrl/2/event -->

    <owl:NamedIndividual rdf:about="http://www.w3.org/ns/odrl/2/event">
        <rdf:type rdf:resource="http://www.w3.org/2004/02/skos/core#Concept"/>
        <rdf:type rdf:resource="http://www.w3.org/ns/odrl/2/LeftOperand"/>
        <rdfs:isDefinedBy rdf:resource="http://www.w3.org/ns/odrl/2/"/>
        <rdfs:label xml:lang="en">Event</rdfs:label>
        <skos:definition xml:lang="en">An identified event setting a context for exercising the action of the Rule.</skos:definition>
        <skos:note xml:lang="en">Events are temporal periods of time, and operators can be used to signal before (lt), during (eq) or after (gt) the event. &lt;br /&gt;Example: May be taken during the “FIFA World Cup 2020” only.</skos:note>
        <skos:scopeNote xml:lang="en">Non-Normative</skos:scopeNote>
    </owl:NamedIndividual>
    


    <!-- http://www.w3.org/ns/odrl/2/execute -->

    <owl:NamedIndividual rdf:about="http://www.w3.org/ns/odrl/2/execute">
        <rdf:type rdf:resource="http://www.w3.org/2004/02/skos/core#Concept"/>
        <rdf:type rdf:resource="http://www.w3.org/ns/odrl/2/Action"/>
        <odrl:includedIn rdf:resource="http://www.w3.org/ns/odrl/2/use"/>
        <rdfs:isDefinedBy rdf:resource="http://www.w3.org/ns/odrl/2/"/>
        <rdfs:label xml:lang="en">Execute</rdfs:label>
        <skos:definition xml:lang="en">To run the computer program Asset.</skos:definition>
        <skos:note xml:lang="en">For example, machine executable code or Java such as a game or application.</skos:note>
        <skos:scopeNote xml:lang="en">Non-Normative</skos:scopeNote>
    </owl:NamedIndividual>
    


    <!-- http://www.w3.org/ns/odrl/2/export -->

    <owl:NamedIndividual rdf:about="http://www.w3.org/ns/odrl/2/export">
        <rdf:type rdf:resource="http://www.w3.org/2004/02/skos/core#Concept"/>
        <rdf:type rdf:resource="http://www.w3.org/ns/odrl/2/Action"/>
        <rdfs:isDefinedBy rdf:resource="http://www.w3.org/ns/odrl/2/"/>
        <rdfs:label xml:lang="en">Export</rdfs:label>
        <owl:deprecated rdf:datatype="http://www.w3.org/2001/XMLSchema#boolean">true</owl:deprecated>
        <skos:definition xml:lang="en">The act of transforming the asset into a new form.</skos:definition>
        <skos:exactMatch rdf:resource="http://www.w3.org/ns/odrl/2/transform"/>
    </owl:NamedIndividual>
    


    <!-- http://www.w3.org/ns/odrl/2/extract -->

    <owl:NamedIndividual rdf:about="http://www.w3.org/ns/odrl/2/extract">
        <rdf:type rdf:resource="http://www.w3.org/2004/02/skos/core#Concept"/>
        <rdf:type rdf:resource="http://www.w3.org/ns/odrl/2/Action"/>
        <odrl:includedIn rdf:resource="http://www.w3.org/ns/odrl/2/reproduce"/>
        <rdfs:isDefinedBy rdf:resource="http://www.w3.org/ns/odrl/2/"/>
        <rdfs:label xml:lang="en">Extract</rdfs:label>
        <skos:definition xml:lang="en">To extract parts of the Asset and to use it as a new Asset.</skos:definition>
        <skos:note xml:lang="en">A new asset is created and may have very little in common with the original Asset. (Note that the notion of whether or not the change is significant enough to qualify as a new asset is subjective). To the extracted Asset a next policy may be applied.</skos:note>
        <skos:scopeNote xml:lang="en">Non-Normative</skos:scopeNote>
    </owl:NamedIndividual>
    


    <!-- http://www.w3.org/ns/odrl/2/extractChar -->

    <owl:NamedIndividual rdf:about="http://www.w3.org/ns/odrl/2/extractChar">
        <rdf:type rdf:resource="http://www.w3.org/2004/02/skos/core#Concept"/>
        <rdf:type rdf:resource="http://www.w3.org/ns/odrl/2/Action"/>
        <rdfs:isDefinedBy rdf:resource="http://www.w3.org/ns/odrl/2/"/>
        <rdfs:label xml:lang="en">Extract character</rdfs:label>
        <owl:deprecated rdf:datatype="http://www.w3.org/2001/XMLSchema#boolean">true</owl:deprecated>
        <skos:definition xml:lang="en">The act of extracting (replicating) unchanged characters from the asset.</skos:definition>
        <skos:note xml:lang="en">This original term and URI from the ONIX specification should be used: http://www.editeur.org/onix-pl/extract-char .</skos:note>
    </owl:NamedIndividual>
    


    <!-- http://www.w3.org/ns/odrl/2/extractPage -->

    <owl:NamedIndividual rdf:about="http://www.w3.org/ns/odrl/2/extractPage">
        <rdf:type rdf:resource="http://www.w3.org/2004/02/skos/core#Concept"/>
        <rdf:type rdf:resource="http://www.w3.org/ns/odrl/2/Action"/>
        <rdfs:isDefinedBy rdf:resource="http://www.w3.org/ns/odrl/2/"/>
        <rdfs:label xml:lang="en">Extract page</rdfs:label>
        <owl:deprecated rdf:datatype="http://www.w3.org/2001/XMLSchema#boolean">true</owl:deprecated>
        <skos:definition xml:lang="en">The act of extracting (replicating) unchanged pages from the asset.</skos:definition>
        <skos:note xml:lang="en">This original term and URI from the ONIX specification should be used: http://www.editeur.org/onix-pl/extract-page .</skos:note>
    </owl:NamedIndividual>
    


    <!-- http://www.w3.org/ns/odrl/2/extractWord -->

    <owl:NamedIndividual rdf:about="http://www.w3.org/ns/odrl/2/extractWord">
        <rdf:type rdf:resource="http://www.w3.org/2004/02/skos/core#Concept"/>
        <rdf:type rdf:resource="http://www.w3.org/ns/odrl/2/Action"/>
        <rdfs:isDefinedBy rdf:resource="http://www.w3.org/ns/odrl/2/"/>
        <rdfs:label xml:lang="en">Extract word</rdfs:label>
        <owl:deprecated rdf:datatype="http://www.w3.org/2001/XMLSchema#boolean">true</owl:deprecated>
        <skos:definition xml:lang="en">The act of extracting (replicating) unchanged words from the asset.</skos:definition>
        <skos:note xml:lang="en">This original term and URI from the ONIX specification should be used: http://www.editeur.org/onix-pl/extract-word .</skos:note>
    </owl:NamedIndividual>
    


    <!-- http://www.w3.org/ns/odrl/2/failure -->

    <owl:NamedIndividual rdf:about="http://www.w3.org/ns/odrl/2/failure">
        <rdf:type rdf:resource="http://www.w3.org/2004/02/skos/core#Concept"/>
    </owl:NamedIndividual>
    


    <!-- http://www.w3.org/ns/odrl/2/fileFormat -->

    <owl:NamedIndividual rdf:about="http://www.w3.org/ns/odrl/2/fileFormat">
        <rdf:type rdf:resource="http://www.w3.org/2004/02/skos/core#Concept"/>
        <rdf:type rdf:resource="http://www.w3.org/ns/odrl/2/LeftOperand"/>
        <rdfs:isDefinedBy rdf:resource="http://www.w3.org/ns/odrl/2/"/>
        <rdfs:label xml:lang="en">File Format</rdfs:label>
        <skos:definition xml:lang="en">A transformed file format of the target Asset.</skos:definition>
        <skos:note xml:lang="en">Example: An asset may be transformed into JPEG format.</skos:note>
        <skos:scopeNote xml:lang="en">Non-Normative</skos:scopeNote>
    </owl:NamedIndividual>
    


    <!-- http://www.w3.org/ns/odrl/2/function -->

    <owl:NamedIndividual rdf:about="http://www.w3.org/ns/odrl/2/function">
        <rdf:type rdf:resource="http://www.w3.org/2004/02/skos/core#Concept"/>
    </owl:NamedIndividual>
    


    <!-- http://www.w3.org/ns/odrl/2/give -->

    <owl:NamedIndividual rdf:about="http://www.w3.org/ns/odrl/2/give">
        <rdf:type rdf:resource="http://www.w3.org/2004/02/skos/core#Concept"/>
        <rdf:type rdf:resource="http://www.w3.org/ns/odrl/2/Action"/>
        <odrl:includedIn rdf:resource="http://www.w3.org/ns/odrl/2/transfer"/>
        <rdfs:isDefinedBy rdf:resource="http://www.w3.org/ns/odrl/2/"/>
        <rdfs:label xml:lang="en">Give</rdfs:label>
        <skos:definition xml:lang="en">To transfer the ownership of the Asset to a third party without compensation and while deleting the original asset.</skos:definition>
        <skos:scopeNote xml:lang="en">Non-Normative</skos:scopeNote>
    </owl:NamedIndividual>
    


    <!-- http://www.w3.org/ns/odrl/2/grantUse -->

    <owl:NamedIndividual rdf:about="http://www.w3.org/ns/odrl/2/grantUse">
        <rdf:type rdf:resource="http://www.w3.org/2004/02/skos/core#Concept"/>
        <rdf:type rdf:resource="http://www.w3.org/ns/odrl/2/Action"/>
        <odrl:includedIn rdf:resource="http://www.w3.org/ns/odrl/2/use"/>
        <rdfs:isDefinedBy rdf:resource="http://www.w3.org/ns/odrl/2/"/>
        <rdfs:label xml:lang="en">Grant Use</rdfs:label>
        <skos:definition xml:lang="en">To grant the use of the Asset to third parties.</skos:definition>
        <skos:note xml:lang="en">This action enables the assignee to create policies for the use of the Asset for third parties. The nextPolicy is recommended to be agreed with the third party. Use of temporal constraints is recommended.</skos:note>
        <skos:scopeNote xml:lang="en">Non-Normative</skos:scopeNote>
    </owl:NamedIndividual>
    


    <!-- http://www.w3.org/ns/odrl/2/gt -->

    <owl:NamedIndividual rdf:about="http://www.w3.org/ns/odrl/2/gt">
        <rdf:type rdf:resource="http://www.w3.org/2004/02/skos/core#Concept"/>
        <rdf:type rdf:resource="http://www.w3.org/ns/odrl/2/Operator"/>
        <rdfs:isDefinedBy rdf:resource="http://www.w3.org/ns/odrl/2/"/>
        <rdfs:label xml:lang="en">Greater than</rdfs:label>
        <skos:definition xml:lang="en">Indicating that a given value is greater than the right operand of the Constraint.</skos:definition>
    </owl:NamedIndividual>
    


    <!-- http://www.w3.org/ns/odrl/2/gteq -->

    <owl:NamedIndividual rdf:about="http://www.w3.org/ns/odrl/2/gteq">
        <rdf:type rdf:resource="http://www.w3.org/2004/02/skos/core#Concept"/>
        <rdf:type rdf:resource="http://www.w3.org/ns/odrl/2/Operator"/>
        <rdfs:isDefinedBy rdf:resource="http://www.w3.org/ns/odrl/2/"/>
        <rdfs:label xml:lang="en">Greater than or equal to</rdfs:label>
        <skos:definition xml:lang="en">Indicating that a given value is greater than or equal to the right operand of the Constraint.</skos:definition>
    </owl:NamedIndividual>
    


    <!-- http://www.w3.org/ns/odrl/2/hasPart -->

    <owl:NamedIndividual rdf:about="http://www.w3.org/ns/odrl/2/hasPart">
        <rdf:type rdf:resource="http://www.w3.org/2004/02/skos/core#Concept"/>
        <rdf:type rdf:resource="http://www.w3.org/ns/odrl/2/Operator"/>
        <rdfs:isDefinedBy rdf:resource="http://www.w3.org/ns/odrl/2/"/>
        <rdfs:label xml:lang="en">Has part</rdfs:label>
        <skos:definition xml:lang="en">A set-based operator indicating that a given value contains the right operand of the Constraint.</skos:definition>
    </owl:NamedIndividual>
    


    <!-- http://www.w3.org/ns/odrl/2/hasPolicy -->

    <owl:NamedIndividual rdf:about="http://www.w3.org/ns/odrl/2/hasPolicy">
        <rdf:type rdf:resource="http://www.w3.org/2004/02/skos/core#Concept"/>
    </owl:NamedIndividual>
    


    <!-- http://www.w3.org/ns/odrl/2/ignore -->

    <owl:NamedIndividual rdf:about="http://www.w3.org/ns/odrl/2/ignore">
        <rdf:type rdf:resource="http://www.w3.org/2004/02/skos/core#Concept"/>
        <rdf:type rdf:resource="http://www.w3.org/ns/odrl/2/UndefinedTerm"/>
        <rdfs:isDefinedBy rdf:resource="http://www.w3.org/ns/odrl/2/"/>
        <rdfs:label xml:lang="en">Ignore Undefined Actions</rdfs:label>
        <owl:deprecated rdf:datatype="http://www.w3.org/2001/XMLSchema#boolean">true</owl:deprecated>
        <skos:definition xml:lang="en">The Action is to be ignored and is not part of the policy – and the policy remains valid.</skos:definition>
        <skos:note xml:lang="en">Used to support actions not known to the policy system.</skos:note>
    </owl:NamedIndividual>
    


    <!-- http://www.w3.org/ns/odrl/2/implies -->

    <owl:NamedIndividual rdf:about="http://www.w3.org/ns/odrl/2/implies">
        <rdf:type rdf:resource="http://www.w3.org/2004/02/skos/core#Concept"/>
    </owl:NamedIndividual>
    


    <!-- http://www.w3.org/ns/odrl/2/include -->

    <owl:NamedIndividual rdf:about="http://www.w3.org/ns/odrl/2/include">
        <rdf:type rdf:resource="http://www.w3.org/2004/02/skos/core#Concept"/>
        <rdf:type rdf:resource="http://www.w3.org/ns/odrl/2/Action"/>
        <odrl:includedIn rdf:resource="http://www.w3.org/ns/odrl/2/use"/>
        <rdfs:isDefinedBy rdf:resource="http://www.w3.org/ns/odrl/2/"/>
        <rdfs:label xml:lang="en">Include</rdfs:label>
        <skos:definition xml:lang="en">To include other related assets in the Asset.</skos:definition>
        <skos:note xml:lang="en">For example: bio picture must be included in the attribution. Use of a relation sub-property is required for the related assets.</skos:note>
        <skos:scopeNote xml:lang="en">Non-Normative</skos:scopeNote>
    </owl:NamedIndividual>
    


    <!-- http://www.w3.org/ns/odrl/2/includedIn -->

    <owl:NamedIndividual rdf:about="http://www.w3.org/ns/odrl/2/includedIn">
        <rdf:type rdf:resource="http://www.w3.org/2004/02/skos/core#Concept"/>
    </owl:NamedIndividual>
    


    <!-- http://www.w3.org/ns/odrl/2/index -->

    <owl:NamedIndividual rdf:about="http://www.w3.org/ns/odrl/2/index">
        <rdf:type rdf:resource="http://www.w3.org/2004/02/skos/core#Concept"/>
        <rdf:type rdf:resource="http://www.w3.org/ns/odrl/2/Action"/>
        <odrl:includedIn rdf:resource="http://www.w3.org/ns/odrl/2/use"/>
        <rdfs:isDefinedBy rdf:resource="http://www.w3.org/ns/odrl/2/"/>
        <rdfs:label xml:lang="en">Index</rdfs:label>
        <skos:definition xml:lang="en">To record the Asset in an index.</skos:definition>
        <skos:note xml:lang="en">For example, to include a link to the Asset in a search engine database.</skos:note>
        <skos:scopeNote xml:lang="en">Non-Normative</skos:scopeNote>
    </owl:NamedIndividual>
    


    <!-- http://www.w3.org/ns/odrl/2/industry -->

    <owl:NamedIndividual rdf:about="http://www.w3.org/ns/odrl/2/industry">
        <rdf:type rdf:resource="http://www.w3.org/2004/02/skos/core#Concept"/>
        <rdf:type rdf:resource="http://www.w3.org/ns/odrl/2/LeftOperand"/>
        <rdfs:isDefinedBy rdf:resource="http://www.w3.org/ns/odrl/2/"/>
        <rdfs:label xml:lang="en">Industry Context</rdfs:label>
        <skos:definition xml:lang="en">A defined industry sector setting a context for exercising the action of the Rule.</skos:definition>
        <skos:note xml:lang="en">Example: publishing or financial industry.</skos:note>
        <skos:scopeNote xml:lang="en">Non-Normative</skos:scopeNote>
    </owl:NamedIndividual>
    


    <!-- http://www.w3.org/ns/odrl/2/inform -->

    <owl:NamedIndividual rdf:about="http://www.w3.org/ns/odrl/2/inform">
        <rdf:type rdf:resource="http://www.w3.org/2004/02/skos/core#Concept"/>
        <rdf:type rdf:resource="http://www.w3.org/ns/odrl/2/Action"/>
        <odrl:includedIn rdf:resource="http://www.w3.org/ns/odrl/2/use"/>
        <rdfs:isDefinedBy rdf:resource="http://www.w3.org/ns/odrl/2/"/>
        <rdfs:label xml:lang="en">Inform</rdfs:label>
        <skos:definition xml:lang="en">To inform that an action has been performed on or in relation to the Asset.</skos:definition>
        <skos:note xml:lang="en">May link to a Party with the role &apos;informedParty&apos; function.</skos:note>
        <skos:scopeNote xml:lang="en">Non-Normative</skos:scopeNote>
    </owl:NamedIndividual>
    


    <!-- http://www.w3.org/ns/odrl/2/informedParty -->

    <owl:NamedIndividual rdf:about="http://www.w3.org/ns/odrl/2/informedParty">
        <rdf:type rdf:resource="http://www.w3.org/2004/02/skos/core#Concept"/>
    </owl:NamedIndividual>
    


    <!-- http://www.w3.org/ns/odrl/2/informingParty -->

    <owl:NamedIndividual rdf:about="http://www.w3.org/ns/odrl/2/informingParty">
        <rdf:type rdf:resource="http://www.w3.org/2004/02/skos/core#Concept"/>
        <rdfs:isDefinedBy rdf:resource="http://www.w3.org/ns/odrl/2/"/>
        <rdfs:label xml:lang="en">Informing Party</rdfs:label>
        <skos:definition xml:lang="en">The Party who provides the inform use data.</skos:definition>
        <skos:note xml:lang="en">Maybe specified as part of the inform action.</skos:note>
        <skos:scopeNote xml:lang="en">Non-Normative</skos:scopeNote>
    </owl:NamedIndividual>
    


    <!-- http://www.w3.org/ns/odrl/2/inheritAllowed -->

    <owl:NamedIndividual rdf:about="http://www.w3.org/ns/odrl/2/inheritAllowed">
        <rdf:type rdf:resource="http://www.w3.org/2004/02/skos/core#Concept"/>
        <rdfs:isDefinedBy rdf:resource="http://www.w3.org/ns/odrl/2/"/>
        <rdfs:label xml:lang="en">Inheritance Allowed</rdfs:label>
        <owl:deprecated rdf:datatype="http://www.w3.org/2001/XMLSchema#boolean">true</owl:deprecated>
        <skos:definition xml:lang="en">Indicates if the Policy entity can be inherited.</skos:definition>
        <skos:note xml:lang="en">A boolean value.</skos:note>
    </owl:NamedIndividual>
    


    <!-- http://www.w3.org/ns/odrl/2/inheritFrom -->

    <owl:NamedIndividual rdf:about="http://www.w3.org/ns/odrl/2/inheritFrom">
        <rdf:type rdf:resource="http://www.w3.org/2004/02/skos/core#Concept"/>
    </owl:NamedIndividual>
    


    <!-- http://www.w3.org/ns/odrl/2/inheritRelation -->

    <owl:NamedIndividual rdf:about="http://www.w3.org/ns/odrl/2/inheritRelation">
        <rdf:type rdf:resource="http://www.w3.org/2004/02/skos/core#Concept"/>
        <rdfs:isDefinedBy rdf:resource="http://www.w3.org/ns/odrl/2/"/>
        <rdfs:label xml:lang="en">Inherit Relation</rdfs:label>
        <owl:deprecated rdf:datatype="http://www.w3.org/2001/XMLSchema#boolean">true</owl:deprecated>
        <skos:definition xml:lang="en">Indentifies the type of inheritance.</skos:definition>
        <skos:note xml:lang="en">For example, this may indicate the business scenario, such as subscription, or prior arrangements between the parties (that are not machine representable).</skos:note>
    </owl:NamedIndividual>
    


    <!-- http://www.w3.org/ns/odrl/2/install -->

    <owl:NamedIndividual rdf:about="http://www.w3.org/ns/odrl/2/install">
        <rdf:type rdf:resource="http://www.w3.org/2004/02/skos/core#Concept"/>
        <rdf:type rdf:resource="http://www.w3.org/ns/odrl/2/Action"/>
        <odrl:includedIn rdf:resource="http://www.w3.org/ns/odrl/2/use"/>
        <rdfs:isDefinedBy rdf:resource="http://www.w3.org/ns/odrl/2/"/>
        <rdfs:label xml:lang="en">Install</rdfs:label>
        <skos:definition xml:lang="en">To load the computer program Asset onto a storage device which allows operating or running the Asset.</skos:definition>
        <skos:scopeNote xml:lang="en">Non-Normative</skos:scopeNote>
    </owl:NamedIndividual>
    


    <!-- http://www.w3.org/ns/odrl/2/invalid -->

    <owl:NamedIndividual rdf:about="http://www.w3.org/ns/odrl/2/invalid">
        <rdf:type rdf:resource="http://www.w3.org/2004/02/skos/core#Concept"/>
        <rdf:type rdf:resource="http://www.w3.org/ns/odrl/2/ConflictTerm"/>
        <rdfs:isDefinedBy rdf:resource="http://www.w3.org/ns/odrl/2/"/>
        <rdfs:label xml:lang="en">Void Policy</rdfs:label>
        <skos:definition xml:lang="en">The policy is void.</skos:definition>
        <skos:note xml:lang="en">Used to indicate the policy is void for Conflict Strategy.</skos:note>
        <skos:scopeNote xml:lang="en">Non-Normative</skos:scopeNote>
    </owl:NamedIndividual>
    


    <!-- http://www.w3.org/ns/odrl/2/isA -->

    <owl:NamedIndividual rdf:about="http://www.w3.org/ns/odrl/2/isA">
        <rdf:type rdf:resource="http://www.w3.org/2004/02/skos/core#Concept"/>
        <rdf:type rdf:resource="http://www.w3.org/ns/odrl/2/Operator"/>
        <rdfs:isDefinedBy rdf:resource="http://www.w3.org/ns/odrl/2/"/>
        <rdfs:label xml:lang="en">Is a</rdfs:label>
        <skos:definition xml:lang="en">A set-based operator indicating that a given value is an instance of the right operand of the Constraint.</skos:definition>
    </owl:NamedIndividual>
    


    <!-- http://www.w3.org/ns/odrl/2/isAllOf -->

    <owl:NamedIndividual rdf:about="http://www.w3.org/ns/odrl/2/isAllOf">
        <rdf:type rdf:resource="http://www.w3.org/2004/02/skos/core#Concept"/>
        <rdf:type rdf:resource="http://www.w3.org/ns/odrl/2/Operator"/>
        <rdfs:isDefinedBy rdf:resource="http://www.w3.org/ns/odrl/2/"/>
        <rdfs:label xml:lang="en">Is all of</rdfs:label>
        <skos:definition xml:lang="en">A set-based operator indicating that a given value is all of the right operand of the Constraint.</skos:definition>
    </owl:NamedIndividual>
    


    <!-- http://www.w3.org/ns/odrl/2/isAnyOf -->

    <owl:NamedIndividual rdf:about="http://www.w3.org/ns/odrl/2/isAnyOf">
        <rdf:type rdf:resource="http://www.w3.org/2004/02/skos/core#Concept"/>
        <rdf:type rdf:resource="http://www.w3.org/ns/odrl/2/Operator"/>
        <rdfs:isDefinedBy rdf:resource="http://www.w3.org/ns/odrl/2/"/>
        <rdfs:label xml:lang="en">Is any of</rdfs:label>
        <skos:definition xml:lang="en">A set-based operator indicating that a given value is any of the right operand of the Constraint.</skos:definition>
    </owl:NamedIndividual>
    


    <!-- http://www.w3.org/ns/odrl/2/isNoneOf -->

    <owl:NamedIndividual rdf:about="http://www.w3.org/ns/odrl/2/isNoneOf">
        <rdf:type rdf:resource="http://www.w3.org/2004/02/skos/core#Concept"/>
        <rdf:type rdf:resource="http://www.w3.org/ns/odrl/2/Operator"/>
        <rdfs:isDefinedBy rdf:resource="http://www.w3.org/ns/odrl/2/"/>
        <rdfs:label xml:lang="en">Is none of</rdfs:label>
        <skos:definition xml:lang="en">A set-based operator indicating that a given value is none of the right operand of the Constraint.</skos:definition>
    </owl:NamedIndividual>
    


    <!-- http://www.w3.org/ns/odrl/2/isPartOf -->

    <owl:NamedIndividual rdf:about="http://www.w3.org/ns/odrl/2/isPartOf">
        <rdf:type rdf:resource="http://www.w3.org/2004/02/skos/core#Concept"/>
        <rdf:type rdf:resource="http://www.w3.org/ns/odrl/2/Operator"/>
        <rdfs:isDefinedBy rdf:resource="http://www.w3.org/ns/odrl/2/"/>
        <rdfs:label xml:lang="en">Is part of</rdfs:label>
        <skos:definition xml:lang="en">A set-based operator indicating that a given value is contained by the right operand of the Constraint.</skos:definition>
    </owl:NamedIndividual>
    


    <!-- http://www.w3.org/ns/odrl/2/language -->

    <owl:NamedIndividual rdf:about="http://www.w3.org/ns/odrl/2/language">
        <rdf:type rdf:resource="http://www.w3.org/2004/02/skos/core#Concept"/>
        <rdf:type rdf:resource="http://www.w3.org/ns/odrl/2/LeftOperand"/>
        <rdfs:isDefinedBy rdf:resource="http://www.w3.org/ns/odrl/2/"/>
        <rdfs:label xml:lang="en">Language</rdfs:label>
        <skos:definition xml:lang="en">A natural language used by the target Asset.</skos:definition>
        <skos:note xml:lang="en">Example: the asset can only be translated into Greek. Must use [[bcp47]] codes for language values.</skos:note>
        <skos:scopeNote xml:lang="en">Non-Normative</skos:scopeNote>
    </owl:NamedIndividual>
    


    <!-- http://www.w3.org/ns/odrl/2/lease -->

    <owl:NamedIndividual rdf:about="http://www.w3.org/ns/odrl/2/lease">
        <rdf:type rdf:resource="http://www.w3.org/2004/02/skos/core#Concept"/>
        <rdf:type rdf:resource="http://www.w3.org/ns/odrl/2/Action"/>
        <rdfs:isDefinedBy rdf:resource="http://www.w3.org/ns/odrl/2/"/>
        <rdfs:label xml:lang="en">Lease</rdfs:label>
        <owl:deprecated rdf:datatype="http://www.w3.org/2001/XMLSchema#boolean">true</owl:deprecated>
        <skos:definition xml:lang="en">The act of making available the asset to a third-party for a fixed period of time with exchange of value.</skos:definition>
    </owl:NamedIndividual>
    


    <!-- http://www.w3.org/ns/odrl/2/leftOperand -->

    <owl:NamedIndividual rdf:about="http://www.w3.org/ns/odrl/2/leftOperand">
        <rdf:type rdf:resource="http://www.w3.org/2004/02/skos/core#Concept"/>
    </owl:NamedIndividual>
    


    <!-- http://www.w3.org/ns/odrl/2/lend -->

    <owl:NamedIndividual rdf:about="http://www.w3.org/ns/odrl/2/lend">
        <rdf:type rdf:resource="http://www.w3.org/2004/02/skos/core#Concept"/>
        <rdf:type rdf:resource="http://www.w3.org/ns/odrl/2/Action"/>
        <rdfs:isDefinedBy rdf:resource="http://www.w3.org/ns/odrl/2/"/>
        <rdfs:label xml:lang="en">Lend</rdfs:label>
        <owl:deprecated rdf:datatype="http://www.w3.org/2001/XMLSchema#boolean">true</owl:deprecated>
        <skos:definition xml:lang="en">The act of making available the asset to a third-party for a fixed period of time without exchange of value.</skos:definition>
    </owl:NamedIndividual>
    


    <!-- http://www.w3.org/ns/odrl/2/license -->

    <owl:NamedIndividual rdf:about="http://www.w3.org/ns/odrl/2/license">
        <rdf:type rdf:resource="http://www.w3.org/2004/02/skos/core#Concept"/>
        <rdf:type rdf:resource="http://www.w3.org/ns/odrl/2/Action"/>
        <rdfs:isDefinedBy rdf:resource="http://www.w3.org/ns/odrl/2/"/>
        <rdfs:label xml:lang="en">License</rdfs:label>
        <owl:deprecated rdf:datatype="http://www.w3.org/2001/XMLSchema#boolean">true</owl:deprecated>
        <skos:definition xml:lang="en">The act of granting the right to use the asset to a third-party.</skos:definition>
        <skos:exactMatch rdf:resource="http://www.w3.org/ns/odrl/2/grantUse"/>
    </owl:NamedIndividual>
    


    <!-- http://www.w3.org/ns/odrl/2/lt -->

    <owl:NamedIndividual rdf:about="http://www.w3.org/ns/odrl/2/lt">
        <rdf:type rdf:resource="http://www.w3.org/2004/02/skos/core#Concept"/>
        <rdf:type rdf:resource="http://www.w3.org/ns/odrl/2/Operator"/>
        <rdfs:isDefinedBy rdf:resource="http://www.w3.org/ns/odrl/2/"/>
        <rdfs:label xml:lang="en">Less than</rdfs:label>
        <skos:definition xml:lang="en">Indicating that a given value is less than the right operand of the Constraint.</skos:definition>
    </owl:NamedIndividual>
    


    <!-- http://www.w3.org/ns/odrl/2/lteq -->

    <owl:NamedIndividual rdf:about="http://www.w3.org/ns/odrl/2/lteq">
        <rdf:type rdf:resource="http://www.w3.org/2004/02/skos/core#Concept"/>
        <rdf:type rdf:resource="http://www.w3.org/ns/odrl/2/Operator"/>
        <rdfs:isDefinedBy rdf:resource="http://www.w3.org/ns/odrl/2/"/>
        <rdfs:label xml:lang="en">Less than or equal to</rdfs:label>
        <skos:definition xml:lang="en">Indicating that a given value is less than or equal to the right operand of the Constraint.</skos:definition>
    </owl:NamedIndividual>
    


    <!-- http://www.w3.org/ns/odrl/2/media -->

    <owl:NamedIndividual rdf:about="http://www.w3.org/ns/odrl/2/media">
        <rdf:type rdf:resource="http://www.w3.org/2004/02/skos/core#Concept"/>
        <rdf:type rdf:resource="http://www.w3.org/ns/odrl/2/LeftOperand"/>
        <rdfs:isDefinedBy rdf:resource="http://www.w3.org/ns/odrl/2/"/>
        <rdfs:label xml:lang="en">Media Context</rdfs:label>
        <skos:definition xml:lang="en">Category of a media asset setting a context for exercising the action of the Rule.</skos:definition>
        <skos:note xml:lang="en">Example media types: electronic, print, advertising, marketing. Note: The used type should not be an IANA MediaType as they are focused on technical characteristics. </skos:note>
        <skos:scopeNote xml:lang="en">Non-Normative</skos:scopeNote>
    </owl:NamedIndividual>
    


    <!-- http://www.w3.org/ns/odrl/2/meteredTime -->

    <owl:NamedIndividual rdf:about="http://www.w3.org/ns/odrl/2/meteredTime">
        <rdf:type rdf:resource="http://www.w3.org/2004/02/skos/core#Concept"/>
        <rdf:type rdf:resource="http://www.w3.org/ns/odrl/2/LeftOperand"/>
        <rdfs:isDefinedBy rdf:resource="http://www.w3.org/ns/odrl/2/"/>
        <rdfs:label xml:lang="en">Metered Time</rdfs:label>
        <skos:definition xml:lang="en">An accumulated amount of one to many metered time periods which were used for exercising the action of the Rule. Right operand value MUST be an xsd:duration as defined by [[xmlschema11-2]].</skos:definition>
        <skos:note>Only the eq, lt, lteq operators SHOULD be used. See also Elapsed Time. &lt;br /&gt;Example: &lt;code&gt;meteredTime lteq P60M&lt;/code&gt; indicates an accumulated period of 60 Minutes or less.</skos:note>
        <skos:scopeNote xml:lang="en">Non-Normative</skos:scopeNote>
    </owl:NamedIndividual>
    


    <!-- http://www.w3.org/ns/odrl/2/modify -->

    <owl:NamedIndividual rdf:about="http://www.w3.org/ns/odrl/2/modify">
        <rdf:type rdf:resource="http://www.w3.org/2004/02/skos/core#Concept"/>
        <rdf:type rdf:resource="http://www.w3.org/ns/odrl/2/Action"/>
        <odrl:includedIn rdf:resource="http://www.w3.org/ns/odrl/2/use"/>
        <rdfs:isDefinedBy rdf:resource="http://www.w3.org/ns/odrl/2/"/>
        <rdfs:label xml:lang="en">Modify</rdfs:label>
        <skos:definition xml:lang="en">To change existing content of the Asset. A new asset is not created by this action.</skos:definition>
        <skos:note xml:lang="en">This action will modify an asset which is typically updated from time to time without creating a new asset. If the result from modifying the asset should be a new asset the actions derive or extract should be used. (Note that the notion of whether or not the change is significant enough to qualify as a new asset is subjective).</skos:note>
        <skos:scopeNote xml:lang="en">Non-Normative</skos:scopeNote>
    </owl:NamedIndividual>
    


    <!-- http://www.w3.org/ns/odrl/2/move -->

    <owl:NamedIndividual rdf:about="http://www.w3.org/ns/odrl/2/move">
        <rdf:type rdf:resource="http://www.w3.org/2004/02/skos/core#Concept"/>
        <rdf:type rdf:resource="http://www.w3.org/ns/odrl/2/Action"/>
        <odrl:includedIn rdf:resource="http://www.w3.org/ns/odrl/2/use"/>
        <rdfs:isDefinedBy rdf:resource="http://www.w3.org/ns/odrl/2/"/>
        <rdfs:label xml:lang="en">Move</rdfs:label>
        <skos:definition xml:lang="en">To move the Asset from one digital location to another including deleting the original copy.</skos:definition>
        <skos:note xml:lang="en">After the Asset has been moved, the original copy must be deleted.</skos:note>
        <skos:scopeNote xml:lang="en">Non-Normative</skos:scopeNote>
    </owl:NamedIndividual>
    


    <!-- http://www.w3.org/ns/odrl/2/neq -->

    <owl:NamedIndividual rdf:about="http://www.w3.org/ns/odrl/2/neq">
        <rdf:type rdf:resource="http://www.w3.org/2004/02/skos/core#Concept"/>
        <rdf:type rdf:resource="http://www.w3.org/ns/odrl/2/Operator"/>
        <rdfs:isDefinedBy rdf:resource="http://www.w3.org/ns/odrl/2/"/>
        <rdfs:label xml:lang="en">Not equal to</rdfs:label>
        <skos:definition xml:lang="en">Indicating that a given value is not equal to the right operand of the Constraint.</skos:definition>
    </owl:NamedIndividual>
    


    <!-- http://www.w3.org/ns/odrl/2/nextPolicy -->

    <owl:NamedIndividual rdf:about="http://www.w3.org/ns/odrl/2/nextPolicy">
        <rdf:type rdf:resource="http://www.w3.org/2004/02/skos/core#Concept"/>
        <rdf:type rdf:resource="http://www.w3.org/ns/odrl/2/Action"/>
        <odrl:includedIn rdf:resource="http://www.w3.org/ns/odrl/2/use"/>
        <rdfs:isDefinedBy rdf:resource="http://www.w3.org/ns/odrl/2/"/>
        <rdfs:label xml:lang="en">Next Policy</rdfs:label>
        <skos:definition xml:lang="en">To grant the specified Policy to a third party for their use of the Asset.</skos:definition>
        <skos:note xml:lang="en">Useful for downstream policies.</skos:note>
        <skos:scopeNote xml:lang="en">Non-Normative</skos:scopeNote>
    </owl:NamedIndividual>
    


    <!-- http://www.w3.org/ns/odrl/2/obligation -->

    <owl:NamedIndividual rdf:about="http://www.w3.org/ns/odrl/2/obligation">
        <rdf:type rdf:resource="http://www.w3.org/2004/02/skos/core#Concept"/>
    </owl:NamedIndividual>
    


    <!-- http://www.w3.org/ns/odrl/2/obtainConsent -->

    <owl:NamedIndividual rdf:about="http://www.w3.org/ns/odrl/2/obtainConsent">
        <rdf:type rdf:resource="http://www.w3.org/2004/02/skos/core#Concept"/>
        <rdf:type rdf:resource="http://www.w3.org/ns/odrl/2/Action"/>
        <odrl:includedIn rdf:resource="http://www.w3.org/ns/odrl/2/use"/>
        <rdfs:isDefinedBy rdf:resource="http://www.w3.org/ns/odrl/2/"/>
        <rdfs:label xml:lang="en">Obtain Consent</rdfs:label>
        <skos:definition xml:lang="en">To obtain verifiable consent to perform the requested action in relation to the Asset.</skos:definition>
        <skos:note xml:lang="en">May be used as a Duty to ensure that the Assigner or a Party is authorized to approve such actions on a case-by-case basis. May link to a Party with the role “consentingParty” function.</skos:note>
        <skos:scopeNote xml:lang="en">Non-Normative</skos:scopeNote>
    </owl:NamedIndividual>
    


    <!-- http://www.w3.org/ns/odrl/2/operand -->

    <owl:NamedIndividual rdf:about="http://www.w3.org/ns/odrl/2/operand">
        <rdf:type rdf:resource="http://www.w3.org/2004/02/skos/core#Concept"/>
    </owl:NamedIndividual>
    


    <!-- http://www.w3.org/ns/odrl/2/operator -->

    <owl:NamedIndividual rdf:about="http://www.w3.org/ns/odrl/2/operator">
        <rdf:type rdf:resource="http://www.w3.org/2004/02/skos/core#Concept"/>
    </owl:NamedIndividual>
    


    <!-- http://www.w3.org/ns/odrl/2/or -->

    <owl:NamedIndividual rdf:about="http://www.w3.org/ns/odrl/2/or">
        <rdf:type rdf:resource="http://www.w3.org/2004/02/skos/core#Concept"/>
    </owl:NamedIndividual>
    


    <!-- http://www.w3.org/ns/odrl/2/output -->

    <owl:NamedIndividual rdf:about="http://www.w3.org/ns/odrl/2/output">
        <rdf:type rdf:resource="http://www.w3.org/2004/02/skos/core#Concept"/>
    </owl:NamedIndividual>
    


    <!-- http://www.w3.org/ns/odrl/2/partOf -->

    <owl:NamedIndividual rdf:about="http://www.w3.org/ns/odrl/2/partOf">
        <rdf:type rdf:resource="http://www.w3.org/2004/02/skos/core#Concept"/>
    </owl:NamedIndividual>
    


    <!-- http://www.w3.org/ns/odrl/2/pay -->

    <owl:NamedIndividual rdf:about="http://www.w3.org/ns/odrl/2/pay">
        <rdf:type rdf:resource="http://www.w3.org/2004/02/skos/core#Concept"/>
        <rdf:type rdf:resource="http://www.w3.org/ns/odrl/2/Action"/>
        <rdfs:isDefinedBy rdf:resource="http://www.w3.org/ns/odrl/2/"/>
        <rdfs:label xml:lang="en">Pay</rdfs:label>
        <owl:deprecated rdf:datatype="http://www.w3.org/2001/XMLSchema#boolean">true</owl:deprecated>
        <skos:definition xml:lang="en">The act of paying a financial amount to a party for use of the asset.</skos:definition>
        <skos:exactMatch rdf:resource="http://www.w3.org/ns/odrl/2/compensate"/>
    </owl:NamedIndividual>
    


    <!-- http://www.w3.org/ns/odrl/2/payAmount -->

    <owl:NamedIndividual rdf:about="http://www.w3.org/ns/odrl/2/payAmount">
        <rdf:type rdf:resource="http://www.w3.org/2004/02/skos/core#Concept"/>
        <rdf:type rdf:resource="http://www.w3.org/ns/odrl/2/LeftOperand"/>
        <rdfs:isDefinedBy rdf:resource="http://www.w3.org/ns/odrl/2/"/>
        <rdfs:label xml:lang="en">Payment Amount</rdfs:label>
        <skos:definition xml:lang="en">The amount of a financial payment. Right operand value MUST be an xsd:decimal. </skos:definition>
        <skos:note xml:lang="en">Can be used for compensation duties with the unit property indicating the currency of the payment.</skos:note>
        <skos:scopeNote xml:lang="en">Non-Normative</skos:scopeNote>
    </owl:NamedIndividual>
    


    <!-- http://www.w3.org/ns/odrl/2/payeeParty -->

    <owl:NamedIndividual rdf:about="http://www.w3.org/ns/odrl/2/payeeParty">
        <rdf:type rdf:resource="http://www.w3.org/2004/02/skos/core#Concept"/>
        <rdfs:isDefinedBy rdf:resource="http://www.w3.org/ns/odrl/2/"/>
        <rdfs:label xml:lang="en">Payee Party</rdfs:label>
        <owl:deprecated rdf:datatype="http://www.w3.org/2001/XMLSchema#boolean">true</owl:deprecated>
        <skos:definition xml:lang="en">The Party is the recipient of the payment.</skos:definition>
        <skos:exactMatch rdf:resource="http://www.w3.org/ns/odrl/2/compensatedParty"/>
        <skos:scopeNote xml:lang="en">Non-Normative</skos:scopeNote>
    </owl:NamedIndividual>
    


    <!-- http://www.w3.org/ns/odrl/2/percentage -->

    <owl:NamedIndividual rdf:about="http://www.w3.org/ns/odrl/2/percentage">
        <rdf:type rdf:resource="http://www.w3.org/2004/02/skos/core#Concept"/>
        <rdf:type rdf:resource="http://www.w3.org/ns/odrl/2/LeftOperand"/>
        <rdfs:isDefinedBy rdf:resource="http://www.w3.org/ns/odrl/2/"/>
        <rdfs:label xml:lang="en">Asset Percentage</rdfs:label>
        <skos:definition xml:lang="en">A percentage amount of the target Asset relevant for exercising the action of the Rule. Right operand value MUST be an xsd:decimal from 0 to 100.</skos:definition>
        <skos:note xml:lang="en">Example: Extract less than or equal to 50%.</skos:note>
        <skos:scopeNote xml:lang="en">Non-Normative</skos:scopeNote>
    </owl:NamedIndividual>
    


    <!-- http://www.w3.org/ns/odrl/2/perm -->

    <owl:NamedIndividual rdf:about="http://www.w3.org/ns/odrl/2/perm">
        <rdf:type rdf:resource="http://www.w3.org/2004/02/skos/core#Concept"/>
        <rdf:type rdf:resource="http://www.w3.org/ns/odrl/2/ConflictTerm"/>
        <rdfs:isDefinedBy rdf:resource="http://www.w3.org/ns/odrl/2/"/>
        <rdfs:label xml:lang="en">Prefer Permissions</rdfs:label>
        <skos:definition xml:lang="en">Permissions take preference over prohibitions.</skos:definition>
        <skos:note xml:lang="en">Used to determine policy conflict outcomes.</skos:note>
    </owl:NamedIndividual>
    


    <!-- http://www.w3.org/ns/odrl/2/permission -->

    <owl:NamedIndividual rdf:about="http://www.w3.org/ns/odrl/2/permission">
        <rdf:type rdf:resource="http://www.w3.org/2004/02/skos/core#Concept"/>
    </owl:NamedIndividual>
    


    <!-- http://www.w3.org/ns/odrl/2/play -->

    <owl:NamedIndividual rdf:about="http://www.w3.org/ns/odrl/2/play">
        <rdf:type rdf:resource="http://www.w3.org/2004/02/skos/core#Concept"/>
        <rdf:type rdf:resource="http://www.w3.org/ns/odrl/2/Action"/>
        <odrl:includedIn rdf:resource="http://www.w3.org/ns/odrl/2/use"/>
        <rdfs:isDefinedBy rdf:resource="http://www.w3.org/ns/odrl/2/"/>
        <rdfs:label xml:lang="en">Play</rdfs:label>
        <skos:definition xml:lang="en">To create a sequential and transient rendition of an Asset.</skos:definition>
        <skos:note>For example, to play a video or audio track. If the action is to be performed to a wider audience than just the Assignees, then the Recipient constraint is recommended to be used.</skos:note>
        <skos:scopeNote xml:lang="en">Non-Normative</skos:scopeNote>
    </owl:NamedIndividual>
    


    <!-- http://www.w3.org/ns/odrl/2/policyUsage -->

    <owl:NamedIndividual rdf:about="http://www.w3.org/ns/odrl/2/policyUsage">
        <rdf:type rdf:resource="http://www.w3.org/2004/02/skos/core#Concept"/>
        <rdf:type rdf:resource="http://www.w3.org/ns/odrl/2/RightOperand"/>
        <rdfs:isDefinedBy rdf:resource="http://www.w3.org/ns/odrl/2/"/>
        <rdfs:label xml:lang="en">Policy Rule Usage</rdfs:label>
        <skos:definition xml:lang="en">Indicates the actual datetime the action of the Rule was exercised.</skos:definition>
        <skos:note xml:lang="en">This can be used to express constraints with a LeftOperand relative to the time the rule is exercised. Operators indicate before (lt, lteq), during (eq) or after (gt, gteq) the usage of the rule. &lt;br /&gt;Example: &lt;code&gt;event lt policyUsage&lt;/code&gt; expresses that the identified event must have happened before the action of the rule is exercised.</skos:note>
        <skos:scopeNote xml:lang="en">Non-Normative</skos:scopeNote>
    </owl:NamedIndividual>
    


    <!-- http://www.w3.org/ns/odrl/2/present -->

    <owl:NamedIndividual rdf:about="http://www.w3.org/ns/odrl/2/present">
        <rdf:type rdf:resource="http://www.w3.org/2004/02/skos/core#Concept"/>
        <rdf:type rdf:resource="http://www.w3.org/ns/odrl/2/Action"/>
        <odrl:includedIn rdf:resource="http://www.w3.org/ns/odrl/2/use"/>
        <rdfs:isDefinedBy rdf:resource="http://www.w3.org/ns/odrl/2/"/>
        <rdfs:label xml:lang="en">Present</rdfs:label>
        <skos:definition xml:lang="en">To publicly perform the Asset.</skos:definition>
        <skos:note>The asset can be performed (or communicated) in public.</skos:note>
        <skos:scopeNote xml:lang="en">Non-Normative</skos:scopeNote>
    </owl:NamedIndividual>
    


    <!-- http://www.w3.org/ns/odrl/2/preview -->

    <owl:NamedIndividual rdf:about="http://www.w3.org/ns/odrl/2/preview">
        <rdf:type rdf:resource="http://www.w3.org/2004/02/skos/core#Concept"/>
        <rdf:type rdf:resource="http://www.w3.org/ns/odrl/2/Action"/>
        <rdfs:isDefinedBy rdf:resource="http://www.w3.org/ns/odrl/2/"/>
        <rdfs:label xml:lang="en">Preview</rdfs:label>
        <owl:deprecated rdf:datatype="http://www.w3.org/2001/XMLSchema#boolean">true</owl:deprecated>
        <skos:definition xml:lang="en">The act of providing a short preview of the asset.</skos:definition>
        <skos:note xml:lang="en">Use a time constraint with the appropriate action.</skos:note>
    </owl:NamedIndividual>
    


    <!-- http://www.w3.org/ns/odrl/2/print -->

    <owl:NamedIndividual rdf:about="http://www.w3.org/ns/odrl/2/print">
        <rdf:type rdf:resource="http://www.w3.org/2004/02/skos/core#Concept"/>
        <rdf:type rdf:resource="http://www.w3.org/ns/odrl/2/Action"/>
        <odrl:includedIn rdf:resource="http://www.w3.org/ns/odrl/2/use"/>
        <rdfs:isDefinedBy rdf:resource="http://www.w3.org/ns/odrl/2/"/>
        <rdfs:label xml:lang="en">Print</rdfs:label>
        <skos:definition xml:lang="en">To create a tangible and permanent rendition of an Asset.</skos:definition>
        <skos:note xml:lang="en">For example, creating a permanent, fixed (static), and directly perceivable representation of the Asset, such as printing onto paper.</skos:note>
        <skos:scopeNote xml:lang="en">Non-Normative</skos:scopeNote>
    </owl:NamedIndividual>
    


    <!-- http://www.w3.org/ns/odrl/2/product -->

    <owl:NamedIndividual rdf:about="http://www.w3.org/ns/odrl/2/product">
        <rdf:type rdf:resource="http://www.w3.org/2004/02/skos/core#Concept"/>
        <rdf:type rdf:resource="http://www.w3.org/ns/odrl/2/LeftOperand"/>
        <rdfs:isDefinedBy rdf:resource="http://www.w3.org/ns/odrl/2/"/>
        <rdfs:label xml:lang="en">Product Context</rdfs:label>
        <skos:definition xml:lang="en">Category of product or service setting a context for exercising the action of the Rule.</skos:definition>
        <skos:note xml:lang="en">Example: May only be used in the XYZ Magazine.</skos:note>
        <skos:scopeNote xml:lang="en">Non-Normative</skos:scopeNote>
    </owl:NamedIndividual>
    


    <!-- http://www.w3.org/ns/odrl/2/profile -->

    <owl:NamedIndividual rdf:about="http://www.w3.org/ns/odrl/2/profile">
        <rdf:type rdf:resource="http://www.w3.org/2004/02/skos/core#Concept"/>
        <rdfs:isDefinedBy rdf:resource="http://www.w3.org/ns/odrl/2/"/>
        <rdfs:label xml:lang="en">Profile</rdfs:label>
        <skos:definition xml:lang="en">The identifier(s) of an ODRL Profile that the Policy conforms to.</skos:definition>
        <skos:note xml:lang="en">The profile property is mandatory if the Policy is using an ODRL Profile.</skos:note>
    </owl:NamedIndividual>
    


    <!-- http://www.w3.org/ns/odrl/2/prohibit -->

    <owl:NamedIndividual rdf:about="http://www.w3.org/ns/odrl/2/prohibit">
        <rdf:type rdf:resource="http://www.w3.org/2004/02/skos/core#Concept"/>
        <rdf:type rdf:resource="http://www.w3.org/ns/odrl/2/ConflictTerm"/>
        <rdfs:isDefinedBy rdf:resource="http://www.w3.org/ns/odrl/2/"/>
        <rdfs:label xml:lang="en">Prefer Prohibitions</rdfs:label>
        <skos:definition xml:lang="en">Prohibitions take preference over permissions.</skos:definition>
        <skos:note xml:lang="en">Used to determine policy conflict outcomes.</skos:note>
    </owl:NamedIndividual>
    


    <!-- http://www.w3.org/ns/odrl/2/prohibition -->

    <owl:NamedIndividual rdf:about="http://www.w3.org/ns/odrl/2/prohibition">
        <rdf:type rdf:resource="http://www.w3.org/2004/02/skos/core#Concept"/>
    </owl:NamedIndividual>
    


    <!-- http://www.w3.org/ns/odrl/2/proximity -->

    <owl:NamedIndividual rdf:about="http://www.w3.org/ns/odrl/2/proximity">
        <rdf:type rdf:resource="http://www.w3.org/2004/02/skos/core#Concept"/>
        <rdfs:isDefinedBy rdf:resource="http://www.w3.org/ns/odrl/2/"/>
        <rdfs:label xml:lang="en">proximity</rdfs:label>
        <owl:deprecated rdf:datatype="http://www.w3.org/2001/XMLSchema#boolean">true</owl:deprecated>
        <skos:definition xml:lang="en">An value indicating the closeness or nearness.</skos:definition>
        <skos:note xml:lang="en">This original term and URI from the OMA specification should be used: http://www.openmobilealliance.com/oma-dd/proximity .</skos:note>
    </owl:NamedIndividual>
    


    <!-- http://www.w3.org/ns/odrl/2/purpose -->

    <owl:NamedIndividual rdf:about="http://www.w3.org/ns/odrl/2/purpose">
        <rdf:type rdf:resource="http://www.w3.org/2004/02/skos/core#Concept"/>
        <rdf:type rdf:resource="http://www.w3.org/ns/odrl/2/LeftOperand"/>
        <rdfs:isDefinedBy rdf:resource="http://www.w3.org/ns/odrl/2/"/>
        <rdfs:label xml:lang="en">Purpose</rdfs:label>
        <skos:definition xml:lang="en">A defined purpose for exercising the action of the Rule.</skos:definition>
        <skos:note xml:lang="en">Example: Educational use.</skos:note>
        <skos:scopeNote xml:lang="en">Non-Normative</skos:scopeNote>
    </owl:NamedIndividual>
    


    <!-- http://www.w3.org/ns/odrl/2/read -->

    <owl:NamedIndividual rdf:about="http://www.w3.org/ns/odrl/2/read">
        <rdf:type rdf:resource="http://www.w3.org/2004/02/skos/core#Concept"/>
        <rdf:type rdf:resource="http://www.w3.org/ns/odrl/2/Action"/>
        <odrl:includedIn rdf:resource="http://www.w3.org/ns/odrl/2/use"/>
        <rdfs:isDefinedBy rdf:resource="http://www.w3.org/ns/odrl/2/"/>
        <rdfs:label xml:lang="en">Read</rdfs:label>
        <skos:definition xml:lang="en">To obtain data from the Asset.</skos:definition>
        <skos:note xml:lang="en">For example, the ability to read a record from a database (the Asset).</skos:note>
        <skos:scopeNote xml:lang="en">Non-Normative</skos:scopeNote>
    </owl:NamedIndividual>
    


    <!-- http://www.w3.org/ns/odrl/2/recipient -->

    <owl:NamedIndividual rdf:about="http://www.w3.org/ns/odrl/2/recipient">
        <rdf:type rdf:resource="http://www.w3.org/2004/02/skos/core#Concept"/>
        <rdf:type rdf:resource="http://www.w3.org/ns/odrl/2/LeftOperand"/>
        <rdfs:isDefinedBy rdf:resource="http://www.w3.org/ns/odrl/2/"/>
        <rdfs:label xml:lang="en">Recipient</rdfs:label>
        <skos:definition xml:lang="en">The party receiving the result/outcome of exercising the action of the Rule.</skos:definition>
        <skos:note xml:lang="en">The Right Operand must identify one or more specific Parties or category/ies of the Party.</skos:note>
        <skos:scopeNote xml:lang="en">Non-Normative</skos:scopeNote>
    </owl:NamedIndividual>
    


    <!-- http://www.w3.org/ns/odrl/2/refinement -->

    <owl:NamedIndividual rdf:about="http://www.w3.org/ns/odrl/2/refinement">
        <rdf:type rdf:resource="http://www.w3.org/2004/02/skos/core#Concept"/>
    </owl:NamedIndividual>
    


    <!-- http://www.w3.org/ns/odrl/2/relation -->

    <owl:NamedIndividual rdf:about="http://www.w3.org/ns/odrl/2/relation">
        <rdf:type rdf:resource="http://www.w3.org/2004/02/skos/core#Concept"/>
    </owl:NamedIndividual>
    


    <!-- http://www.w3.org/ns/odrl/2/relativePosition -->

    <owl:NamedIndividual rdf:about="http://www.w3.org/ns/odrl/2/relativePosition">
        <rdf:type rdf:resource="http://www.w3.org/2004/02/skos/core#Concept"/>
        <rdf:type rdf:resource="http://www.w3.org/ns/odrl/2/LeftOperand"/>
        <rdfs:isDefinedBy rdf:resource="http://www.w3.org/ns/odrl/2/"/>
        <rdfs:label xml:lang="en">Relative Asset Position</rdfs:label>
        <skos:definition xml:lang="en">A point in space or time defined with coordinates relative to full measures the positioning of the target Asset.</skos:definition>
        <skos:note xml:lang="en">Example: The upper left corner of a picture may be constrained to a specific position of the canvas rendering it.</skos:note>
        <skos:scopeNote xml:lang="en">Non-Normative</skos:scopeNote>
    </owl:NamedIndividual>
    


    <!-- http://www.w3.org/ns/odrl/2/relativeSize -->

    <owl:NamedIndividual rdf:about="http://www.w3.org/ns/odrl/2/relativeSize">
        <rdf:type rdf:resource="http://www.w3.org/2004/02/skos/core#Concept"/>
        <rdf:type rdf:resource="http://www.w3.org/ns/odrl/2/LeftOperand"/>
        <rdfs:isDefinedBy rdf:resource="http://www.w3.org/ns/odrl/2/"/>
        <rdfs:label xml:lang="en">Relative Asset Size</rdfs:label>
        <skos:definition xml:lang="en">Measure(s) of one or two axes for 2D-objects or measure(s) of one to tree axes for 3D-objects - expressed as percentages of full values - of the target Asset.</skos:definition>
        <skos:note xml:lang="en">Example: The image can be resized in width to a maximum of 200%. Note: See the Left Operand absoluteSize. </skos:note>
        <skos:scopeNote xml:lang="en">Non-Normative</skos:scopeNote>
    </owl:NamedIndividual>
    


    <!-- http://www.w3.org/ns/odrl/2/relativeSpatialPosition -->

    <owl:NamedIndividual rdf:about="http://www.w3.org/ns/odrl/2/relativeSpatialPosition">
        <rdf:type rdf:resource="http://www.w3.org/2004/02/skos/core#Concept"/>
        <rdf:type rdf:resource="http://www.w3.org/ns/odrl/2/LeftOperand"/>
        <rdfs:isDefinedBy rdf:resource="http://www.w3.org/ns/odrl/2/"/>
        <rdfs:label xml:lang="en">Relative Spatial Asset Position</rdfs:label>
        <skos:broader rdf:resource="http://www.w3.org/ns/odrl/2/relativePosition"/>
        <skos:definition xml:lang="en">The relative spatial positions - expressed as percentages of full values - of four corners of a rectangle on a 2D-canvas or the eight corners of a cuboid in a 3D-space of the target Asset.</skos:definition>
        <skos:note xml:lang="en">See also Absolute Spatial Asset Position.</skos:note>
        <skos:scopeNote xml:lang="en">Non-Normative</skos:scopeNote>
    </owl:NamedIndividual>
    


    <!-- http://www.w3.org/ns/odrl/2/relativeTemporalPosition -->

    <owl:NamedIndividual rdf:about="http://www.w3.org/ns/odrl/2/relativeTemporalPosition">
        <rdf:type rdf:resource="http://www.w3.org/2004/02/skos/core#Concept"/>
        <rdf:type rdf:resource="http://www.w3.org/ns/odrl/2/LeftOperand"/>
        <rdfs:isDefinedBy rdf:resource="http://www.w3.org/ns/odrl/2/"/>
        <rdfs:label xml:lang="en">Relative Temporal Asset Position</rdfs:label>
        <skos:broader rdf:resource="http://www.w3.org/ns/odrl/2/relativePosition"/>
        <skos:definition xml:lang="en">A point in space or time defined with coordinates relative to full measures the positioning of the target Asset.</skos:definition>
        <skos:note xml:lang="en">See also Absolute Temporal Asset Position. &lt;br /&gt;Example: The MP3 music file must be positioned between the positions at 33% and 48% of the temporal length of a stream. </skos:note>
        <skos:scopeNote xml:lang="en">Non-Normative</skos:scopeNote>
    </owl:NamedIndividual>
    


    <!-- http://www.w3.org/ns/odrl/2/remedy -->

    <owl:NamedIndividual rdf:about="http://www.w3.org/ns/odrl/2/remedy">
        <rdf:type rdf:resource="http://www.w3.org/2004/02/skos/core#Concept"/>
    </owl:NamedIndividual>
    


    <!-- http://www.w3.org/ns/odrl/2/reproduce -->

    <owl:NamedIndividual rdf:about="http://www.w3.org/ns/odrl/2/reproduce">
        <rdf:type rdf:resource="http://www.w3.org/2004/02/skos/core#Concept"/>
        <rdf:type rdf:resource="http://www.w3.org/ns/odrl/2/Action"/>
        <odrl:includedIn rdf:resource="http://www.w3.org/ns/odrl/2/use"/>
        <rdfs:isDefinedBy rdf:resource="http://www.w3.org/ns/odrl/2/"/>
        <rdfs:label xml:lang="en">Reproduce</rdfs:label>
        <skos:definition xml:lang="en">To make duplicate copies the Asset in any material form.</skos:definition>
        <skos:scopeNote xml:lang="en">Non-Normative</skos:scopeNote>
    </owl:NamedIndividual>
    


    <!-- http://www.w3.org/ns/odrl/2/resolution -->

    <owl:NamedIndividual rdf:about="http://www.w3.org/ns/odrl/2/resolution">
        <rdf:type rdf:resource="http://www.w3.org/2004/02/skos/core#Concept"/>
        <rdf:type rdf:resource="http://www.w3.org/ns/odrl/2/LeftOperand"/>
        <rdfs:isDefinedBy rdf:resource="http://www.w3.org/ns/odrl/2/"/>
        <rdfs:label xml:lang="en">Rendition Resolution</rdfs:label>
        <skos:definition xml:lang="en">Resolution of the rendition of the target Asset.</skos:definition>
        <skos:note xml:lang="en">Example: the image may be printed at 1200dpi.</skos:note>
        <skos:scopeNote xml:lang="en">Non-Normative</skos:scopeNote>
    </owl:NamedIndividual>
    


    <!-- http://www.w3.org/ns/odrl/2/reviewPolicy -->

    <owl:NamedIndividual rdf:about="http://www.w3.org/ns/odrl/2/reviewPolicy">
        <rdf:type rdf:resource="http://www.w3.org/2004/02/skos/core#Concept"/>
        <rdf:type rdf:resource="http://www.w3.org/ns/odrl/2/Action"/>
        <odrl:includedIn rdf:resource="http://www.w3.org/ns/odrl/2/use"/>
        <rdfs:isDefinedBy rdf:resource="http://www.w3.org/ns/odrl/2/"/>
        <rdfs:label xml:lang="en">Review Policy</rdfs:label>
        <skos:definition xml:lang="en">To review the Policy applicable to the Asset.</skos:definition>
        <skos:note xml:lang="en">Used when human intervention is required to review the Policy. May link to an Asset which represents the full Policy information.</skos:note>
        <skos:scopeNote xml:lang="en">Non-Normative</skos:scopeNote>
    </owl:NamedIndividual>
    


    <!-- http://www.w3.org/ns/odrl/2/rightOperand -->

    <owl:NamedIndividual rdf:about="http://www.w3.org/ns/odrl/2/rightOperand">
        <rdf:type rdf:resource="http://www.w3.org/2004/02/skos/core#Concept"/>
    </owl:NamedIndividual>
    


    <!-- http://www.w3.org/ns/odrl/2/rightOperandReference -->

    <owl:NamedIndividual rdf:about="http://www.w3.org/ns/odrl/2/rightOperandReference">
        <rdf:type rdf:resource="http://www.w3.org/2004/02/skos/core#Concept"/>
        <rdfs:isDefinedBy rdf:resource="http://www.w3.org/ns/odrl/2/"/>
        <rdfs:label xml:lang="en">Has Right Operand Reference</rdfs:label>
        <skos:definition xml:lang="en">A reference to a web resource providing the value for the right operand of a Constraint.</skos:definition>
        <skos:note xml:lang="en">An IRI that MUST be dereferenced to obtain the actual right operand value. When used with set-based operators, a list of IRIs may be used</skos:note>
    </owl:NamedIndividual>
    


    <!-- http://www.w3.org/ns/odrl/2/scope -->

    <owl:NamedIndividual rdf:about="http://www.w3.org/ns/odrl/2/scope">
        <rdf:type rdf:resource="http://www.w3.org/2004/02/skos/core#Concept"/>
        <rdfs:isDefinedBy rdf:resource="http://www.w3.org/ns/odrl/2/"/>
        <rdfs:label xml:lang="en">Scope</rdfs:label>
        <owl:deprecated rdf:datatype="http://www.w3.org/2001/XMLSchema#boolean">true</owl:deprecated>
        <skos:definition xml:lang="en">The identifier of a scope that provides context to the extent of the entity.</skos:definition>
        <skos:note xml:lang="en">Used to define scopes for Assets and Parties.</skos:note>
    </owl:NamedIndividual>
    


    <!-- http://www.w3.org/ns/odrl/2/secondaryUse -->

    <owl:NamedIndividual rdf:about="http://www.w3.org/ns/odrl/2/secondaryUse">
        <rdf:type rdf:resource="http://www.w3.org/2004/02/skos/core#Concept"/>
        <rdf:type rdf:resource="http://www.w3.org/ns/odrl/2/Action"/>
        <rdfs:isDefinedBy rdf:resource="http://www.w3.org/ns/odrl/2/"/>
        <rdfs:label xml:lang="en">Secondary Use</rdfs:label>
        <owl:deprecated rdf:datatype="http://www.w3.org/2001/XMLSchema#boolean">true</owl:deprecated>
        <skos:definition xml:lang="en">The act of using the asset for a purpose other than the purpose it was intended for.</skos:definition>
    </owl:NamedIndividual>
    


    <!-- http://www.w3.org/ns/odrl/2/sell -->

    <owl:NamedIndividual rdf:about="http://www.w3.org/ns/odrl/2/sell">
        <rdf:type rdf:resource="http://www.w3.org/2004/02/skos/core#Concept"/>
        <rdf:type rdf:resource="http://www.w3.org/ns/odrl/2/Action"/>
        <odrl:includedIn rdf:resource="http://www.w3.org/ns/odrl/2/transfer"/>
        <rdfs:isDefinedBy rdf:resource="http://www.w3.org/ns/odrl/2/"/>
        <rdfs:label xml:lang="en">Sell</rdfs:label>
        <skos:definition xml:lang="en">To transfer the ownership of the Asset to a third party with compensation and while deleting the original asset.</skos:definition>
        <skos:scopeNote xml:lang="en">Non-Normative</skos:scopeNote>
    </owl:NamedIndividual>
    


    <!-- http://www.w3.org/ns/odrl/2/share -->

    <owl:NamedIndividual rdf:about="http://www.w3.org/ns/odrl/2/share">
        <rdf:type rdf:resource="http://www.w3.org/2004/02/skos/core#Concept"/>
        <rdf:type rdf:resource="http://www.w3.org/ns/odrl/2/Action"/>
        <rdfs:isDefinedBy rdf:resource="http://www.w3.org/ns/odrl/2/"/>
        <rdfs:label xml:lang="en">Share</rdfs:label>
        <owl:deprecated rdf:datatype="http://www.w3.org/2001/XMLSchema#boolean">true</owl:deprecated>
        <skos:definition xml:lang="en">The act of the non-commercial reproduction and distribution of the asset to third-parties.</skos:definition>
        <skos:exactMatch rdf:resource="http://creativecommons.org/ns#Sharing"/>
    </owl:NamedIndividual>
    


    <!-- http://www.w3.org/ns/odrl/2/shareAlike -->

    <owl:NamedIndividual rdf:about="http://www.w3.org/ns/odrl/2/shareAlike">
        <rdf:type rdf:resource="http://www.w3.org/2004/02/skos/core#Concept"/>
        <rdf:type rdf:resource="http://www.w3.org/ns/odrl/2/Action"/>
        <rdfs:isDefinedBy rdf:resource="http://www.w3.org/ns/odrl/2/"/>
        <rdfs:label xml:lang="en">Share-alike</rdfs:label>
        <owl:deprecated rdf:datatype="http://www.w3.org/2001/XMLSchema#boolean">true</owl:deprecated>
        <skos:definition xml:lang="en">The act of distributing any derivative asset under the same terms as the original asset.</skos:definition>
        <skos:exactMatch rdf:resource="http://creativecommons.org/ns#ShareAlike"/>
    </owl:NamedIndividual>
    


    <!-- http://www.w3.org/ns/odrl/2/source -->

    <owl:NamedIndividual rdf:about="http://www.w3.org/ns/odrl/2/source">
        <rdf:type rdf:resource="http://www.w3.org/2004/02/skos/core#Concept"/>
        <rdfs:isDefinedBy rdf:resource="http://www.w3.org/ns/odrl/2/"/>
        <rdfs:label xml:lang="en">Source</rdfs:label>
        <skos:definition xml:lang="en">Reference to a Asset/PartyCollection</skos:definition>
        <skos:note xml:lang="en">Used by AssetCollection and PartyCollection when constraints are applied.</skos:note>
    </owl:NamedIndividual>
    


    <!-- http://www.w3.org/ns/odrl/2/spatial -->

    <owl:NamedIndividual rdf:about="http://www.w3.org/ns/odrl/2/spatial">
        <rdf:type rdf:resource="http://www.w3.org/2004/02/skos/core#Concept"/>
        <rdf:type rdf:resource="http://www.w3.org/ns/odrl/2/LeftOperand"/>
        <rdfs:isDefinedBy rdf:resource="http://www.w3.org/ns/odrl/2/"/>
        <rdfs:label xml:lang="en">Geospatial Named Area</rdfs:label>
        <skos:definition xml:lang="en">A named and identified geospatial area with defined borders which is used for exercising the action of the Rule. An IRI MUST be used to represent this value.</skos:definition>
        <skos:note xml:lang="en">A code value for the area and source of the code must be presented in the Right Operand. &lt;br /&gt;Example: the [[iso3166]] Country Codes or the Getty Thesaurus of Geographic Names. </skos:note>
        <skos:scopeNote xml:lang="en">Non-Normative</skos:scopeNote>
    </owl:NamedIndividual>
    


    <!-- http://www.w3.org/ns/odrl/2/spatialCoordinates -->

    <owl:NamedIndividual rdf:about="http://www.w3.org/ns/odrl/2/spatialCoordinates">
        <rdf:type rdf:resource="http://www.w3.org/2004/02/skos/core#Concept"/>
        <rdf:type rdf:resource="http://www.w3.org/ns/odrl/2/LeftOperand"/>
        <rdfs:isDefinedBy rdf:resource="http://www.w3.org/ns/odrl/2/"/>
        <rdfs:label xml:lang="en">Geospatial Coordinates</rdfs:label>
        <skos:broader rdf:resource="http://www.w3.org/ns/odrl/2/spatial"/>
        <skos:definition xml:lang="en">A set of coordinates setting the borders of a geospatial area used for exercising the action of the Rule. The coordinates MUST include longitude and latitude, they MAY include altitude and the geodetic datum.</skos:definition>
        <skos:note xml:lang="en">The default values are the altitude of earth&apos;s surface at this location and the WGS 84 datum.</skos:note>
        <skos:scopeNote xml:lang="en">Non-Normative</skos:scopeNote>
    </owl:NamedIndividual>
    


    <!-- http://www.w3.org/ns/odrl/2/status -->

    <owl:NamedIndividual rdf:about="http://www.w3.org/ns/odrl/2/status">
        <rdf:type rdf:resource="http://www.w3.org/2004/02/skos/core#Concept"/>
        <rdfs:isDefinedBy rdf:resource="http://www.w3.org/ns/odrl/2/"/>
        <rdfs:label xml:lang="en">Status</rdfs:label>
        <skos:definition xml:lang="en">the value generated from the leftOperand action or a value related to the leftOperand set as the reference for the comparison.</skos:definition>
    </owl:NamedIndividual>
    


    <!-- http://www.w3.org/ns/odrl/2/stream -->

    <owl:NamedIndividual rdf:about="http://www.w3.org/ns/odrl/2/stream">
        <rdf:type rdf:resource="http://www.w3.org/2004/02/skos/core#Concept"/>
        <rdf:type rdf:resource="http://www.w3.org/ns/odrl/2/Action"/>
        <odrl:includedIn rdf:resource="http://www.w3.org/ns/odrl/2/use"/>
        <rdfs:isDefinedBy rdf:resource="http://www.w3.org/ns/odrl/2/"/>
        <rdfs:label xml:lang="en">Stream</rdfs:label>
        <skos:definition xml:lang="en">To deliver the Asset in real-time.</skos:definition>
        <skos:note>The Asset maybe utilised in real-time as it is being delivered. If the action is to be performed to a wider audience than just the Assignees, then the Recipient constraint is recommended to be used.</skos:note>
        <skos:scopeNote xml:lang="en">Non-Normative</skos:scopeNote>
    </owl:NamedIndividual>
    


    <!-- http://www.w3.org/ns/odrl/2/support -->

    <owl:NamedIndividual rdf:about="http://www.w3.org/ns/odrl/2/support">
        <rdf:type rdf:resource="http://www.w3.org/2004/02/skos/core#Concept"/>
        <rdf:type rdf:resource="http://www.w3.org/ns/odrl/2/UndefinedTerm"/>
        <rdfs:isDefinedBy rdf:resource="http://www.w3.org/ns/odrl/2/"/>
        <rdfs:label xml:lang="en">Support Undefined Actions</rdfs:label>
        <owl:deprecated rdf:datatype="http://www.w3.org/2001/XMLSchema#boolean">true</owl:deprecated>
        <skos:definition xml:lang="en">The Action is to be supported as part of the policy – and the policy remains valid.</skos:definition>
        <skos:note xml:lang="en">Used to support actions not known to the policy system.</skos:note>
    </owl:NamedIndividual>
    


    <!-- http://www.w3.org/ns/odrl/2/synchronize -->

    <owl:NamedIndividual rdf:about="http://www.w3.org/ns/odrl/2/synchronize">
        <rdf:type rdf:resource="http://www.w3.org/2004/02/skos/core#Concept"/>
        <rdf:type rdf:resource="http://www.w3.org/ns/odrl/2/Action"/>
        <odrl:includedIn rdf:resource="http://www.w3.org/ns/odrl/2/use"/>
        <rdfs:isDefinedBy rdf:resource="http://www.w3.org/ns/odrl/2/"/>
        <rdfs:label xml:lang="en">Synchronize</rdfs:label>
        <skos:definition xml:lang="en">To use the Asset in timed relations with media (audio/visual) elements of another Asset.</skos:definition>
        <skos:scopeNote xml:lang="en">Non-Normative</skos:scopeNote>
    </owl:NamedIndividual>
    


    <!-- http://www.w3.org/ns/odrl/2/system -->

    <owl:NamedIndividual rdf:about="http://www.w3.org/ns/odrl/2/system">
        <rdf:type rdf:resource="http://www.w3.org/2004/02/skos/core#Concept"/>
        <rdf:type rdf:resource="http://www.w3.org/ns/odrl/2/LeftOperand"/>
        <rdfs:isDefinedBy rdf:resource="http://www.w3.org/ns/odrl/2/"/>
        <rdfs:label xml:lang="en">System</rdfs:label>
        <owl:deprecated rdf:datatype="http://www.w3.org/2001/XMLSchema#boolean">true</owl:deprecated>
        <skos:definition xml:lang="en">An identified computing system used for exercising the action of the Rule.</skos:definition>
        <skos:exactMatch rdf:resource="http://www.w3.org/ns/odrl/2/systemDevice"/>
        <skos:note>See System Device</skos:note>
    </owl:NamedIndividual>
    


    <!-- http://www.w3.org/ns/odrl/2/systemDevice -->

    <owl:NamedIndividual rdf:about="http://www.w3.org/ns/odrl/2/systemDevice">
        <rdf:type rdf:resource="http://www.w3.org/2004/02/skos/core#Concept"/>
        <rdf:type rdf:resource="http://www.w3.org/ns/odrl/2/LeftOperand"/>
        <rdfs:isDefinedBy rdf:resource="http://www.w3.org/ns/odrl/2/"/>
        <rdfs:label xml:lang="en">System Device</rdfs:label>
        <skos:definition xml:lang="en">An identified computing system or computing device used for exercising the action of the Rule.</skos:definition>
        <skos:exactMatch rdf:resource="http://www.w3.org/ns/odrl/2/device"/>
        <skos:exactMatch rdf:resource="http://www.w3.org/ns/odrl/2/system"/>
        <skos:note xml:lang="en">Example: The system device can be identified by a unique code created from the used hardware.</skos:note>
        <skos:scopeNote xml:lang="en">Non-Normative</skos:scopeNote>
    </owl:NamedIndividual>
    


    <!-- http://www.w3.org/ns/odrl/2/target -->

    <owl:NamedIndividual rdf:about="http://www.w3.org/ns/odrl/2/target">
        <rdf:type rdf:resource="http://www.w3.org/2004/02/skos/core#Concept"/>
    </owl:NamedIndividual>
    


    <!-- http://www.w3.org/ns/odrl/2/textToSpeech -->

    <owl:NamedIndividual rdf:about="http://www.w3.org/ns/odrl/2/textToSpeech">
        <rdf:type rdf:resource="http://www.w3.org/2004/02/skos/core#Concept"/>
        <rdf:type rdf:resource="http://www.w3.org/ns/odrl/2/Action"/>
        <odrl:includedIn rdf:resource="http://www.w3.org/ns/odrl/2/use"/>
        <rdfs:isDefinedBy rdf:resource="http://www.w3.org/ns/odrl/2/"/>
        <rdfs:label xml:lang="en">Text-to-speech</rdfs:label>
        <skos:definition xml:lang="en">To have a text Asset read out loud.</skos:definition>
        <skos:note>If the action is to be performed to a wider audience than just the Assignees, then the recipient constraint is recommended to be used.</skos:note>
        <skos:scopeNote xml:lang="en">Non-Normative</skos:scopeNote>
    </owl:NamedIndividual>
    


    <!-- http://www.w3.org/ns/odrl/2/timeInterval -->

    <owl:NamedIndividual rdf:about="http://www.w3.org/ns/odrl/2/timeInterval">
        <rdf:type rdf:resource="http://www.w3.org/2004/02/skos/core#Concept"/>
        <rdf:type rdf:resource="http://www.w3.org/ns/odrl/2/LeftOperand"/>
        <rdfs:isDefinedBy rdf:resource="http://www.w3.org/ns/odrl/2/"/>
        <rdfs:label xml:lang="en">Recurring Time Interval</rdfs:label>
        <skos:definition xml:lang="en">A recurring period of time before the next execution of the action of the Rule. Right operand value MUST be an xsd:duration as defined by [[xmlschema11-2]].</skos:definition>
        <skos:note>Only the eq operator SHOULD be used. &lt;br /&gt;Example: &lt;code&gt;timeInterval eq P7D&lt;/code&gt; indicates a recurring 7 day period.</skos:note>
        <skos:scopeNote xml:lang="en">Non-Normative</skos:scopeNote>
    </owl:NamedIndividual>
    


    <!-- http://www.w3.org/ns/odrl/2/timedCount -->

    <owl:NamedIndividual rdf:about="http://www.w3.org/ns/odrl/2/timedCount">
        <rdf:type rdf:resource="http://www.w3.org/2004/02/skos/core#Concept"/>
        <rdfs:isDefinedBy rdf:resource="http://www.w3.org/ns/odrl/2/"/>
        <rdfs:label xml:lang="en">Timed Count</rdfs:label>
        <owl:deprecated rdf:datatype="http://www.w3.org/2001/XMLSchema#boolean">true</owl:deprecated>
        <skos:definition xml:lang="en">The number of seconds after which timed metering use of the asset begins.</skos:definition>
        <skos:note xml:lang="en">This original term and URI from the OMA specification should be used: http://www.openmobilealliance.com/oma-dd/timed-count .</skos:note>
    </owl:NamedIndividual>
    


    <!-- http://www.w3.org/ns/odrl/2/trackedParty -->

    <owl:NamedIndividual rdf:about="http://www.w3.org/ns/odrl/2/trackedParty">
        <rdf:type rdf:resource="http://www.w3.org/2004/02/skos/core#Concept"/>
    </owl:NamedIndividual>
    


    <!-- http://www.w3.org/ns/odrl/2/trackingParty -->

    <owl:NamedIndividual rdf:about="http://www.w3.org/ns/odrl/2/trackingParty">
        <rdf:type rdf:resource="http://www.w3.org/2004/02/skos/core#Concept"/>
    </owl:NamedIndividual>
    


    <!-- http://www.w3.org/ns/odrl/2/transfer -->

    <owl:NamedIndividual rdf:about="http://www.w3.org/ns/odrl/2/transfer">
        <rdf:type rdf:resource="http://www.w3.org/2004/02/skos/core#Concept"/>
        <rdf:type rdf:resource="http://www.w3.org/ns/odrl/2/Action"/>
        <rdfs:isDefinedBy rdf:resource="http://www.w3.org/ns/odrl/2/"/>
        <rdfs:label xml:lang="en">Transfer Ownership</rdfs:label>
        <skos:definition xml:lang="en">To transfer the ownership of the Asset in perpetuity.</skos:definition>
    </owl:NamedIndividual>
    


    <!-- http://www.w3.org/ns/odrl/2/transform -->

    <owl:NamedIndividual rdf:about="http://www.w3.org/ns/odrl/2/transform">
        <rdf:type rdf:resource="http://www.w3.org/2004/02/skos/core#Concept"/>
        <rdf:type rdf:resource="http://www.w3.org/ns/odrl/2/Action"/>
        <odrl:includedIn rdf:resource="http://www.w3.org/ns/odrl/2/use"/>
        <rdfs:isDefinedBy rdf:resource="http://www.w3.org/ns/odrl/2/"/>
        <rdfs:label xml:lang="en">Transform</rdfs:label>
        <skos:definition xml:lang="en">To convert the Asset into a different format.</skos:definition>
        <skos:note xml:lang="en">Typically used to convert the Asset into a different format for consumption on/transfer to a third party system.</skos:note>
        <skos:scopeNote xml:lang="en">Non-Normative</skos:scopeNote>
    </owl:NamedIndividual>
    


    <!-- http://www.w3.org/ns/odrl/2/translate -->

    <owl:NamedIndividual rdf:about="http://www.w3.org/ns/odrl/2/translate">
        <rdf:type rdf:resource="http://www.w3.org/2004/02/skos/core#Concept"/>
        <rdf:type rdf:resource="http://www.w3.org/ns/odrl/2/Action"/>
        <odrl:includedIn rdf:resource="http://www.w3.org/ns/odrl/2/use"/>
        <rdfs:isDefinedBy rdf:resource="http://www.w3.org/ns/odrl/2/"/>
        <rdfs:label xml:lang="en">Translate</rdfs:label>
        <skos:definition xml:lang="en">To translate the original natural language of an Asset into another natural language.</skos:definition>
        <skos:note xml:lang="en">A new derivative Asset is created by that action.</skos:note>
        <skos:scopeNote xml:lang="en">Non-Normative</skos:scopeNote>
    </owl:NamedIndividual>
    


    <!-- http://www.w3.org/ns/odrl/2/uid -->

    <owl:NamedIndividual rdf:about="http://www.w3.org/ns/odrl/2/uid">
        <rdf:type rdf:resource="http://www.w3.org/2004/02/skos/core#Concept"/>
        <rdfs:isDefinedBy rdf:resource="http://www.w3.org/ns/odrl/2/"/>
        <rdfs:label xml:lang="en">Unique Identifier</rdfs:label>
        <skos:definition xml:lang="en">An unambiguous identifier</skos:definition>
        <skos:note xml:lang="en">Used by the Policy, Rule, Asset, Party, Constraint, and Logical Constraint Classes.</skos:note>
    </owl:NamedIndividual>
    


    <!-- http://www.w3.org/ns/odrl/2/undefined -->

    <owl:NamedIndividual rdf:about="http://www.w3.org/ns/odrl/2/undefined">
        <rdf:type rdf:resource="http://www.w3.org/2004/02/skos/core#Concept"/>
        <rdfs:isDefinedBy rdf:resource="http://www.w3.org/ns/odrl/2/"/>
        <rdfs:label xml:lang="en">Handle Undefined Term</rdfs:label>
        <owl:deprecated rdf:datatype="http://www.w3.org/2001/XMLSchema#boolean">true</owl:deprecated>
        <skos:definition xml:lang="en">Relates the strategy used for handling undefined actions to a Policy.</skos:definition>
        <skos:note xml:lang="en">If no strategy is specified, the default is invalid.</skos:note>
    </owl:NamedIndividual>
    


    <!-- http://www.w3.org/ns/odrl/2/uninstall -->

    <owl:NamedIndividual rdf:about="http://www.w3.org/ns/odrl/2/uninstall">
        <rdf:type rdf:resource="http://www.w3.org/2004/02/skos/core#Concept"/>
        <rdf:type rdf:resource="http://www.w3.org/ns/odrl/2/Action"/>
        <odrl:includedIn rdf:resource="http://www.w3.org/ns/odrl/2/use"/>
        <rdfs:isDefinedBy rdf:resource="http://www.w3.org/ns/odrl/2/"/>
        <rdfs:label xml:lang="en">Uninstall</rdfs:label>
        <skos:definition xml:lang="en">To unload and delete the computer program Asset from a storage device and disable its readiness for operation.</skos:definition>
        <skos:note xml:lang="en">The Asset is no longer accessible to the assignees after it has been used.</skos:note>
        <skos:scopeNote xml:lang="en">Non-Normative</skos:scopeNote>
    </owl:NamedIndividual>
    


    <!-- http://www.w3.org/ns/odrl/2/unitOfCount -->

    <owl:NamedIndividual rdf:about="http://www.w3.org/ns/odrl/2/unitOfCount">
        <rdf:type rdf:resource="http://www.w3.org/2004/02/skos/core#Concept"/>
        <rdf:type rdf:resource="http://www.w3.org/ns/odrl/2/LeftOperand"/>
        <rdfs:isDefinedBy rdf:resource="http://www.w3.org/ns/odrl/2/"/>
        <rdfs:label xml:lang="en">Unit Of Count</rdfs:label>
        <skos:definition xml:lang="en">The unit of measure used for counting the executions of the action of the Rule.</skos:definition>
        <skos:note xml:lang="en">Note: Typically used with Duties to indicate the unit entity to be counted of the Action. &lt;br /&gt;Example: A duty to compensate and a unitOfCount constraint of &apos;perUser&apos; would indicate that the compensation by multiplied by the &apos;number of users&apos;.</skos:note>
        <skos:scopeNote xml:lang="en">Non-Normative</skos:scopeNote>
    </owl:NamedIndividual>
    


    <!-- http://www.w3.org/ns/odrl/2/use -->

    <owl:NamedIndividual rdf:about="http://www.w3.org/ns/odrl/2/use">
        <rdf:type rdf:resource="http://www.w3.org/2004/02/skos/core#Concept"/>
        <rdf:type rdf:resource="http://www.w3.org/ns/odrl/2/Action"/>
        <rdfs:isDefinedBy rdf:resource="http://www.w3.org/ns/odrl/2/"/>
        <rdfs:label xml:lang="en">Use</rdfs:label>
        <skos:definition xml:lang="en">To use the Asset</skos:definition>
        <skos:note xml:lang="en">Use is the most generic action for all non-third-party usage. More specific types of the use action can be expressed by more targetted actions.</skos:note>
    </owl:NamedIndividual>
    


    <!-- http://www.w3.org/ns/odrl/2/version -->

    <owl:NamedIndividual rdf:about="http://www.w3.org/ns/odrl/2/version">
        <rdf:type rdf:resource="http://www.w3.org/2004/02/skos/core#Concept"/>
        <rdf:type rdf:resource="http://www.w3.org/ns/odrl/2/LeftOperand"/>
        <rdfs:isDefinedBy rdf:resource="http://www.w3.org/ns/odrl/2/"/>
        <rdfs:label xml:lang="en">Version</rdfs:label>
        <skos:definition xml:lang="en">The version of the target Asset.</skos:definition>
        <skos:note xml:lang="en">Example: Single Paperback or Multiple Issues or version 2.0 or higher.</skos:note>
        <skos:scopeNote xml:lang="en">Non-Normative</skos:scopeNote>
    </owl:NamedIndividual>
    


    <!-- http://www.w3.org/ns/odrl/2/virtualLocation -->

    <owl:NamedIndividual rdf:about="http://www.w3.org/ns/odrl/2/virtualLocation">
        <rdf:type rdf:resource="http://www.w3.org/2004/02/skos/core#Concept"/>
        <rdf:type rdf:resource="http://www.w3.org/ns/odrl/2/LeftOperand"/>
        <rdfs:isDefinedBy rdf:resource="http://www.w3.org/ns/odrl/2/"/>
        <rdfs:label xml:lang="en">Virtual IT Communication Location</rdfs:label>
        <skos:definition xml:lang="en">An identified location of the IT communication space which is relevant for exercising the action of the Rule.</skos:definition>
        <skos:note xml:lang="en">Example: an Internet domain or IP address range.</skos:note>
        <skos:scopeNote xml:lang="en">Non-Normative</skos:scopeNote>
    </owl:NamedIndividual>
    


    <!-- http://www.w3.org/ns/odrl/2/watermark -->

    <owl:NamedIndividual rdf:about="http://www.w3.org/ns/odrl/2/watermark">
        <rdf:type rdf:resource="http://www.w3.org/2004/02/skos/core#Concept"/>
        <rdf:type rdf:resource="http://www.w3.org/ns/odrl/2/Action"/>
        <odrl:includedIn rdf:resource="http://www.w3.org/ns/odrl/2/use"/>
        <rdfs:isDefinedBy rdf:resource="http://www.w3.org/ns/odrl/2/"/>
        <rdfs:label xml:lang="en">Watermark</rdfs:label>
        <skos:definition xml:lang="en">To apply a watermark to the Asset.</skos:definition>
        <skos:scopeNote xml:lang="en">Non-Normative</skos:scopeNote>
    </owl:NamedIndividual>
    


    <!-- http://www.w3.org/ns/odrl/2/write -->

    <owl:NamedIndividual rdf:about="http://www.w3.org/ns/odrl/2/write">
        <rdf:type rdf:resource="http://www.w3.org/2004/02/skos/core#Concept"/>
        <rdf:type rdf:resource="http://www.w3.org/ns/odrl/2/Action"/>
        <rdfs:isDefinedBy rdf:resource="http://www.w3.org/ns/odrl/2/"/>
        <rdfs:label xml:lang="en">Write</rdfs:label>
        <owl:deprecated rdf:datatype="http://www.w3.org/2001/XMLSchema#boolean">true</owl:deprecated>
        <skos:definition xml:lang="en">The act of writing to the Asset.</skos:definition>
        <skos:exactMatch rdf:resource="http://www.w3.org/ns/odrl/2/modify"/>
    </owl:NamedIndividual>
    


    <!-- http://www.w3.org/ns/odrl/2/writeTo -->

    <owl:NamedIndividual rdf:about="http://www.w3.org/ns/odrl/2/writeTo">
        <rdf:type rdf:resource="http://www.w3.org/2004/02/skos/core#Concept"/>
        <rdf:type rdf:resource="http://www.w3.org/ns/odrl/2/Action"/>
        <rdfs:isDefinedBy rdf:resource="http://www.w3.org/ns/odrl/2/"/>
        <rdfs:label xml:lang="en">Write to</rdfs:label>
        <owl:deprecated rdf:datatype="http://www.w3.org/2001/XMLSchema#boolean">true</owl:deprecated>
        <skos:definition xml:lang="en">The act of adding data to the Asset.</skos:definition>
        <skos:exactMatch rdf:resource="http://www.w3.org/ns/odrl/2/modify"/>
    </owl:NamedIndividual>
    


    <!-- http://www.w3.org/ns/odrl/2/xone -->

    <owl:NamedIndividual rdf:about="http://www.w3.org/ns/odrl/2/xone">
        <rdf:type rdf:resource="http://www.w3.org/2004/02/skos/core#Concept"/>
    </owl:NamedIndividual>
    


    <!-- http://www.w3.org/ns/odrl/2/#actionConcepts -->

    <owl:NamedIndividual rdf:about="http://www.w3.org/ns/odrl/2/#actionConcepts">
        <rdf:type rdf:resource="http://www.w3.org/2004/02/skos/core#Collection"/>
        <skos:member rdf:resource="http://www.w3.org/ns/odrl/2/Action"/>
        <skos:member rdf:resource="http://www.w3.org/ns/odrl/2/action"/>
        <skos:member rdf:resource="http://www.w3.org/ns/odrl/2/implies"/>
        <skos:member rdf:resource="http://www.w3.org/ns/odrl/2/includedIn"/>
        <skos:prefLabel xml:lang="en">Action</skos:prefLabel>
        <skos:scopeNote xml:lang="en">ODRL Core Vocabulary Terms</skos:scopeNote>
    </owl:NamedIndividual>
    


    <!-- http://www.w3.org/ns/odrl/2/#actions -->

    <owl:NamedIndividual rdf:about="http://www.w3.org/ns/odrl/2/#actions">
        <rdf:type rdf:resource="http://www.w3.org/2004/02/skos/core#Collection"/>
        <skos:member rdf:resource="http://www.w3.org/ns/odrl/2/transfer"/>
        <skos:member rdf:resource="http://www.w3.org/ns/odrl/2/use"/>
        <skos:prefLabel xml:lang="en">Actions for Rules</skos:prefLabel>
        <skos:scopeNote xml:lang="en">ODRL Core Vocabulary Terms</skos:scopeNote>
    </owl:NamedIndividual>
    


    <!-- http://www.w3.org/ns/odrl/2/#actionsCommon -->

    <owl:NamedIndividual rdf:about="http://www.w3.org/ns/odrl/2/#actionsCommon">
        <rdf:type rdf:resource="http://www.w3.org/2004/02/skos/core#Collection"/>
        <skos:member rdf:resource="http://creativecommons.org/ns#Attribution"/>
        <skos:member rdf:resource="http://creativecommons.org/ns#CommercialUse"/>
        <skos:member rdf:resource="http://creativecommons.org/ns#DerivativeWorks"/>
        <skos:member rdf:resource="http://creativecommons.org/ns#Distribution"/>
        <skos:member rdf:resource="http://creativecommons.org/ns#Notice"/>
        <skos:member rdf:resource="http://creativecommons.org/ns#Reproduction"/>
        <skos:member rdf:resource="http://creativecommons.org/ns#ShareAlike"/>
        <skos:member rdf:resource="http://creativecommons.org/ns#Sharing"/>
        <skos:member rdf:resource="http://creativecommons.org/ns#SourceCode"/>
        <skos:member rdf:resource="http://www.w3.org/ns/odrl/2/acceptTracking"/>
        <skos:member rdf:resource="http://www.w3.org/ns/odrl/2/aggregate"/>
        <skos:member rdf:resource="http://www.w3.org/ns/odrl/2/annotate"/>
        <skos:member rdf:resource="http://www.w3.org/ns/odrl/2/anonymize"/>
        <skos:member rdf:resource="http://www.w3.org/ns/odrl/2/archive"/>
        <skos:member rdf:resource="http://www.w3.org/ns/odrl/2/attribute"/>
        <skos:member rdf:resource="http://www.w3.org/ns/odrl/2/compensate"/>
        <skos:member rdf:resource="http://www.w3.org/ns/odrl/2/concurrentUse"/>
        <skos:member rdf:resource="http://www.w3.org/ns/odrl/2/delete"/>
        <skos:member rdf:resource="http://www.w3.org/ns/odrl/2/derive"/>
        <skos:member rdf:resource="http://www.w3.org/ns/odrl/2/digitize"/>
        <skos:member rdf:resource="http://www.w3.org/ns/odrl/2/display"/>
        <skos:member rdf:resource="http://www.w3.org/ns/odrl/2/distribute"/>
        <skos:member rdf:resource="http://www.w3.org/ns/odrl/2/ensureExclusivity"/>
        <skos:member rdf:resource="http://www.w3.org/ns/odrl/2/execute"/>
        <skos:member rdf:resource="http://www.w3.org/ns/odrl/2/extract"/>
        <skos:member rdf:resource="http://www.w3.org/ns/odrl/2/give"/>
        <skos:member rdf:resource="http://www.w3.org/ns/odrl/2/grantUse"/>
        <skos:member rdf:resource="http://www.w3.org/ns/odrl/2/include"/>
        <skos:member rdf:resource="http://www.w3.org/ns/odrl/2/index"/>
        <skos:member rdf:resource="http://www.w3.org/ns/odrl/2/inform"/>
        <skos:member rdf:resource="http://www.w3.org/ns/odrl/2/install"/>
        <skos:member rdf:resource="http://www.w3.org/ns/odrl/2/modify"/>
        <skos:member rdf:resource="http://www.w3.org/ns/odrl/2/move"/>
        <skos:member rdf:resource="http://www.w3.org/ns/odrl/2/nextPolicy"/>
        <skos:member rdf:resource="http://www.w3.org/ns/odrl/2/obtainConsent"/>
        <skos:member rdf:resource="http://www.w3.org/ns/odrl/2/play"/>
        <skos:member rdf:resource="http://www.w3.org/ns/odrl/2/present"/>
        <skos:member rdf:resource="http://www.w3.org/ns/odrl/2/print"/>
        <skos:member rdf:resource="http://www.w3.org/ns/odrl/2/read"/>
        <skos:member rdf:resource="http://www.w3.org/ns/odrl/2/reproduce"/>
        <skos:member rdf:resource="http://www.w3.org/ns/odrl/2/reviewPolicy"/>
        <skos:member rdf:resource="http://www.w3.org/ns/odrl/2/sell"/>
        <skos:member rdf:resource="http://www.w3.org/ns/odrl/2/stream"/>
        <skos:member rdf:resource="http://www.w3.org/ns/odrl/2/synchronize"/>
        <skos:member rdf:resource="http://www.w3.org/ns/odrl/2/textToSpeech"/>
        <skos:member rdf:resource="http://www.w3.org/ns/odrl/2/transform"/>
        <skos:member rdf:resource="http://www.w3.org/ns/odrl/2/translate"/>
        <skos:member rdf:resource="http://www.w3.org/ns/odrl/2/uninstall"/>
        <skos:member rdf:resource="http://www.w3.org/ns/odrl/2/watermark"/>
        <skos:prefLabel xml:lang="en">Actions for Rules</skos:prefLabel>
        <skos:scopeNote xml:lang="en">ODRL Common Vocabulary Terms</skos:scopeNote>
    </owl:NamedIndividual>
    


    <!-- http://www.w3.org/ns/odrl/2/#assetConcepts -->

    <owl:NamedIndividual rdf:about="http://www.w3.org/ns/odrl/2/#assetConcepts">
        <rdf:type rdf:resource="http://www.w3.org/2004/02/skos/core#Collection"/>
        <skos:member rdf:resource="http://www.w3.org/ns/odrl/2/Asset"/>
        <skos:member rdf:resource="http://www.w3.org/ns/odrl/2/AssetCollection"/>
        <skos:prefLabel xml:lang="en">Asset</skos:prefLabel>
        <skos:scopeNote xml:lang="en">ODRL Core Vocabulary Terms</skos:scopeNote>
    </owl:NamedIndividual>
    


    <!-- http://www.w3.org/ns/odrl/2/#assetParty -->

    <owl:NamedIndividual rdf:about="http://www.w3.org/ns/odrl/2/#assetParty">
        <rdf:type rdf:resource="http://www.w3.org/2004/02/skos/core#Collection"/>
        <skos:member rdf:resource="http://www.w3.org/ns/odrl/2/partOf"/>
        <skos:member rdf:resource="http://www.w3.org/ns/odrl/2/source"/>
        <skos:prefLabel xml:lang="en">Asset and Party</skos:prefLabel>
        <skos:scopeNote xml:lang="en">ODRL Core Vocabulary Terms</skos:scopeNote>
    </owl:NamedIndividual>
    


    <!-- http://www.w3.org/ns/odrl/2/#assetRelations -->

    <owl:NamedIndividual rdf:about="http://www.w3.org/ns/odrl/2/#assetRelations">
        <rdf:type rdf:resource="http://www.w3.org/2004/02/skos/core#Collection"/>
        <skos:member rdf:resource="http://www.w3.org/ns/odrl/2/hasPolicy"/>
        <skos:member rdf:resource="http://www.w3.org/ns/odrl/2/target"/>
        <skos:prefLabel xml:lang="en">Asset Relations</skos:prefLabel>
        <skos:scopeNote xml:lang="en">ODRL Core Vocabulary Terms</skos:scopeNote>
    </owl:NamedIndividual>
    


    <!-- http://www.w3.org/ns/odrl/2/#assetRelationsCommon -->

    <owl:NamedIndividual rdf:about="http://www.w3.org/ns/odrl/2/#assetRelationsCommon">
        <rdf:type rdf:resource="http://www.w3.org/2004/02/skos/core#Collection"/>
        <skos:member rdf:resource="http://www.w3.org/ns/odrl/2/output"/>
        <skos:prefLabel xml:lang="en">Asset Relations</skos:prefLabel>
        <skos:scopeNote xml:lang="en">ODRL Common Vocabulary Terms</skos:scopeNote>
    </owl:NamedIndividual>
    


    <!-- http://www.w3.org/ns/odrl/2/#conflictConcepts -->

    <owl:NamedIndividual rdf:about="http://www.w3.org/ns/odrl/2/#conflictConcepts">
        <rdf:type rdf:resource="http://www.w3.org/2004/02/skos/core#Collection"/>
        <skos:member rdf:resource="http://www.w3.org/ns/odrl/2/ConflictTerm"/>
        <skos:member rdf:resource="http://www.w3.org/ns/odrl/2/conflict"/>
        <skos:member rdf:resource="http://www.w3.org/ns/odrl/2/invalid"/>
        <skos:member rdf:resource="http://www.w3.org/ns/odrl/2/perm"/>
        <skos:member rdf:resource="http://www.w3.org/ns/odrl/2/prohibit"/>
        <skos:prefLabel xml:lang="en">Policy Conflict Strategy</skos:prefLabel>
        <skos:scopeNote xml:lang="en">ODRL Core Vocabulary Terms</skos:scopeNote>
    </owl:NamedIndividual>
    


    <!-- http://www.w3.org/ns/odrl/2/#constraintLeftOperandCommon -->

    <owl:NamedIndividual rdf:about="http://www.w3.org/ns/odrl/2/#constraintLeftOperandCommon">
        <rdf:type rdf:resource="http://www.w3.org/2004/02/skos/core#Collection"/>
        <skos:member rdf:resource="http://www.w3.org/ns/odrl/2/absolutePosition"/>
        <skos:member rdf:resource="http://www.w3.org/ns/odrl/2/absoluteSize"/>
        <skos:member rdf:resource="http://www.w3.org/ns/odrl/2/absoluteSpatialPosition"/>
        <skos:member rdf:resource="http://www.w3.org/ns/odrl/2/absoluteTemporalPosition"/>
        <skos:member rdf:resource="http://www.w3.org/ns/odrl/2/count"/>
        <skos:member rdf:resource="http://www.w3.org/ns/odrl/2/dateTime"/>
        <skos:member rdf:resource="http://www.w3.org/ns/odrl/2/delayPeriod"/>
        <skos:member rdf:resource="http://www.w3.org/ns/odrl/2/deliveryChannel"/>
        <skos:member rdf:resource="http://www.w3.org/ns/odrl/2/elapsedTime"/>
        <skos:member rdf:resource="http://www.w3.org/ns/odrl/2/event"/>
        <skos:member rdf:resource="http://www.w3.org/ns/odrl/2/fileFormat"/>
        <skos:member rdf:resource="http://www.w3.org/ns/odrl/2/industry"/>
        <skos:member rdf:resource="http://www.w3.org/ns/odrl/2/language"/>
        <skos:member rdf:resource="http://www.w3.org/ns/odrl/2/media"/>
        <skos:member rdf:resource="http://www.w3.org/ns/odrl/2/meteredTime"/>
        <skos:member rdf:resource="http://www.w3.org/ns/odrl/2/payAmount"/>
        <skos:member rdf:resource="http://www.w3.org/ns/odrl/2/percentage"/>
        <skos:member rdf:resource="http://www.w3.org/ns/odrl/2/product"/>
        <skos:member rdf:resource="http://www.w3.org/ns/odrl/2/purpose"/>
        <skos:member rdf:resource="http://www.w3.org/ns/odrl/2/recipient"/>
        <skos:member rdf:resource="http://www.w3.org/ns/odrl/2/relativePosition"/>
        <skos:member rdf:resource="http://www.w3.org/ns/odrl/2/relativeSize"/>
        <skos:member rdf:resource="http://www.w3.org/ns/odrl/2/relativeSpatialPosition"/>
        <skos:member rdf:resource="http://www.w3.org/ns/odrl/2/relativeTemporalPosition"/>
        <skos:member rdf:resource="http://www.w3.org/ns/odrl/2/resolution"/>
        <skos:member rdf:resource="http://www.w3.org/ns/odrl/2/spatial"/>
        <skos:member rdf:resource="http://www.w3.org/ns/odrl/2/spatialCoordinates"/>
        <skos:member rdf:resource="http://www.w3.org/ns/odrl/2/systemDevice"/>
        <skos:member rdf:resource="http://www.w3.org/ns/odrl/2/timeInterval"/>
        <skos:member rdf:resource="http://www.w3.org/ns/odrl/2/unitOfCount"/>
        <skos:member rdf:resource="http://www.w3.org/ns/odrl/2/version"/>
        <skos:member rdf:resource="http://www.w3.org/ns/odrl/2/virtualLocation"/>
        <skos:prefLabel xml:lang="en">Constraint Left Operands</skos:prefLabel>
        <skos:scopeNote xml:lang="en">ODRL Common Vocabulary Terms</skos:scopeNote>
    </owl:NamedIndividual>
    


    <!-- http://www.w3.org/ns/odrl/2/#constraintLogicalOperands -->

    <owl:NamedIndividual rdf:about="http://www.w3.org/ns/odrl/2/#constraintLogicalOperands">
        <rdf:type rdf:resource="http://www.w3.org/2004/02/skos/core#Collection"/>
        <skos:member rdf:resource="http://www.w3.org/ns/odrl/2/and"/>
        <skos:member rdf:resource="http://www.w3.org/ns/odrl/2/andSequence"/>
        <skos:member rdf:resource="http://www.w3.org/ns/odrl/2/or"/>
        <skos:member rdf:resource="http://www.w3.org/ns/odrl/2/xone"/>
        <skos:prefLabel xml:lang="en">Logical Constraint Operands</skos:prefLabel>
        <skos:scopeNote xml:lang="en">ODRL Core Vocabulary Terms</skos:scopeNote>
    </owl:NamedIndividual>
    


    <!-- http://www.w3.org/ns/odrl/2/#constraintRelationalOperators -->

    <owl:NamedIndividual rdf:about="http://www.w3.org/ns/odrl/2/#constraintRelationalOperators">
        <rdf:type rdf:resource="http://www.w3.org/2004/02/skos/core#Collection"/>
        <skos:member rdf:resource="http://www.w3.org/ns/odrl/2/eq"/>
        <skos:member rdf:resource="http://www.w3.org/ns/odrl/2/gt"/>
        <skos:member rdf:resource="http://www.w3.org/ns/odrl/2/gteq"/>
        <skos:member rdf:resource="http://www.w3.org/ns/odrl/2/hasPart"/>
        <skos:member rdf:resource="http://www.w3.org/ns/odrl/2/isA"/>
        <skos:member rdf:resource="http://www.w3.org/ns/odrl/2/isAllOf"/>
        <skos:member rdf:resource="http://www.w3.org/ns/odrl/2/isAnyOf"/>
        <skos:member rdf:resource="http://www.w3.org/ns/odrl/2/isNoneOf"/>
        <skos:member rdf:resource="http://www.w3.org/ns/odrl/2/isPartOf"/>
        <skos:member rdf:resource="http://www.w3.org/ns/odrl/2/lt"/>
        <skos:member rdf:resource="http://www.w3.org/ns/odrl/2/lteq"/>
        <skos:member rdf:resource="http://www.w3.org/ns/odrl/2/neq"/>
        <skos:prefLabel xml:lang="en">Constraint Operators</skos:prefLabel>
        <skos:scopeNote xml:lang="en">ODRL Core Vocabulary Terms</skos:scopeNote>
    </owl:NamedIndividual>
    


    <!-- http://www.w3.org/ns/odrl/2/#constraintRightOpCommon -->

    <owl:NamedIndividual rdf:about="http://www.w3.org/ns/odrl/2/#constraintRightOpCommon">
        <rdf:type rdf:resource="http://www.w3.org/2004/02/skos/core#Collection"/>
        <skos:member rdf:resource="http://www.w3.org/ns/odrl/2/policyUsage"/>
        <skos:prefLabel xml:lang="en">Constraint Right Operands</skos:prefLabel>
        <skos:scopeNote xml:lang="en">ODRL Common Vocabulary Terms</skos:scopeNote>
    </owl:NamedIndividual>
    


    <!-- http://www.w3.org/ns/odrl/2/#constraints -->

    <owl:NamedIndividual rdf:about="http://www.w3.org/ns/odrl/2/#constraints">
        <rdf:type rdf:resource="http://www.w3.org/2004/02/skos/core#Collection"/>
        <skos:member rdf:resource="http://www.w3.org/ns/odrl/2/Constraint"/>
        <skos:member rdf:resource="http://www.w3.org/ns/odrl/2/LeftOperand"/>
        <skos:member rdf:resource="http://www.w3.org/ns/odrl/2/Operator"/>
        <skos:member rdf:resource="http://www.w3.org/ns/odrl/2/RightOperand"/>
        <skos:member rdf:resource="http://www.w3.org/ns/odrl/2/constraint"/>
        <skos:member rdf:resource="http://www.w3.org/ns/odrl/2/dataType"/>
        <skos:member rdf:resource="http://www.w3.org/ns/odrl/2/leftOperand"/>
        <skos:member rdf:resource="http://www.w3.org/ns/odrl/2/operator"/>
        <skos:member rdf:resource="http://www.w3.org/ns/odrl/2/refinement"/>
        <skos:member rdf:resource="http://www.w3.org/ns/odrl/2/rightOperand"/>
        <skos:member rdf:resource="http://www.w3.org/ns/odrl/2/rightOperandReference"/>
        <skos:member rdf:resource="http://www.w3.org/ns/odrl/2/status"/>
        <skos:member rdf:resource="http://www.w3.org/ns/odrl/2/unit"/>
        <skos:prefLabel xml:lang="en">Constraint</skos:prefLabel>
        <skos:scopeNote xml:lang="en">ODRL Core Vocabulary Terms</skos:scopeNote>
    </owl:NamedIndividual>
    


    <!-- http://www.w3.org/ns/odrl/2/#deprecatedTerms -->

    <owl:NamedIndividual rdf:about="http://www.w3.org/ns/odrl/2/#deprecatedTerms">
        <rdf:type rdf:resource="http://www.w3.org/2004/02/skos/core#Collection"/>
        <skos:member rdf:resource="http://www.w3.org/ns/odrl/2/All"/>
        <skos:member rdf:resource="http://www.w3.org/ns/odrl/2/All2ndConnections"/>
        <skos:member rdf:resource="http://www.w3.org/ns/odrl/2/AllConnections"/>
        <skos:member rdf:resource="http://www.w3.org/ns/odrl/2/AllGroups"/>
        <skos:member rdf:resource="http://www.w3.org/ns/odrl/2/AssetScope"/>
        <skos:member rdf:resource="http://www.w3.org/ns/odrl/2/Group"/>
        <skos:member rdf:resource="http://www.w3.org/ns/odrl/2/Individual"/>
        <skos:member rdf:resource="http://www.w3.org/ns/odrl/2/PartyScope"/>
        <skos:member rdf:resource="http://www.w3.org/ns/odrl/2/UndefinedTerm"/>
        <skos:member rdf:resource="http://www.w3.org/ns/odrl/2/adHocShare"/>
        <skos:member rdf:resource="http://www.w3.org/ns/odrl/2/append"/>
        <skos:member rdf:resource="http://www.w3.org/ns/odrl/2/appendTo"/>
        <skos:member rdf:resource="http://www.w3.org/ns/odrl/2/attachPolicy"/>
        <skos:member rdf:resource="http://www.w3.org/ns/odrl/2/attachSource"/>
        <skos:member rdf:resource="http://www.w3.org/ns/odrl/2/commercialize"/>
        <skos:member rdf:resource="http://www.w3.org/ns/odrl/2/copy"/>
        <skos:member rdf:resource="http://www.w3.org/ns/odrl/2/device"/>
        <skos:member rdf:resource="http://www.w3.org/ns/odrl/2/export"/>
        <skos:member rdf:resource="http://www.w3.org/ns/odrl/2/extractChar"/>
        <skos:member rdf:resource="http://www.w3.org/ns/odrl/2/extractPage"/>
        <skos:member rdf:resource="http://www.w3.org/ns/odrl/2/extractWord"/>
        <skos:member rdf:resource="http://www.w3.org/ns/odrl/2/ignore"/>
        <skos:member rdf:resource="http://www.w3.org/ns/odrl/2/inheritAllowed"/>
        <skos:member rdf:resource="http://www.w3.org/ns/odrl/2/inheritRelation"/>
        <skos:member rdf:resource="http://www.w3.org/ns/odrl/2/lease"/>
        <skos:member rdf:resource="http://www.w3.org/ns/odrl/2/lend"/>
        <skos:member rdf:resource="http://www.w3.org/ns/odrl/2/license"/>
        <skos:member rdf:resource="http://www.w3.org/ns/odrl/2/pay"/>
        <skos:member rdf:resource="http://www.w3.org/ns/odrl/2/payeeParty"/>
        <skos:member rdf:resource="http://www.w3.org/ns/odrl/2/preview"/>
        <skos:member rdf:resource="http://www.w3.org/ns/odrl/2/proximity"/>
        <skos:member rdf:resource="http://www.w3.org/ns/odrl/2/scope"/>
        <skos:member rdf:resource="http://www.w3.org/ns/odrl/2/secondaryUse"/>
        <skos:member rdf:resource="http://www.w3.org/ns/odrl/2/share"/>
        <skos:member rdf:resource="http://www.w3.org/ns/odrl/2/shareAlike"/>
        <skos:member rdf:resource="http://www.w3.org/ns/odrl/2/support"/>
        <skos:member rdf:resource="http://www.w3.org/ns/odrl/2/system"/>
        <skos:member rdf:resource="http://www.w3.org/ns/odrl/2/timedCount"/>
        <skos:member rdf:resource="http://www.w3.org/ns/odrl/2/undefined"/>
        <skos:member rdf:resource="http://www.w3.org/ns/odrl/2/write"/>
        <skos:member rdf:resource="http://www.w3.org/ns/odrl/2/writeTo"/>
        <skos:prefLabel xml:lang="en">Deprecated Terms</skos:prefLabel>
    </owl:NamedIndividual>
    


    <!-- http://www.w3.org/ns/odrl/2/#duties -->

    <owl:NamedIndividual rdf:about="http://www.w3.org/ns/odrl/2/#duties">
        <rdf:type rdf:resource="http://www.w3.org/2004/02/skos/core#Collection"/>
        <skos:member rdf:resource="http://www.w3.org/ns/odrl/2/Duty"/>
        <skos:member rdf:resource="http://www.w3.org/ns/odrl/2/consequence"/>
        <skos:member rdf:resource="http://www.w3.org/ns/odrl/2/duty"/>
        <skos:member rdf:resource="http://www.w3.org/ns/odrl/2/obligation"/>
        <skos:member rdf:resource="http://www.w3.org/ns/odrl/2/remedy"/>
        <skos:prefLabel xml:lang="en">Duty</skos:prefLabel>
        <skos:scopeNote xml:lang="en">ODRL Core Vocabulary Terms</skos:scopeNote>
    </owl:NamedIndividual>
    


    <!-- http://www.w3.org/ns/odrl/2/#logicalConstraints -->

    <owl:NamedIndividual rdf:about="http://www.w3.org/ns/odrl/2/#logicalConstraints">
        <rdf:type rdf:resource="http://www.w3.org/2004/02/skos/core#Collection"/>
        <skos:member rdf:resource="http://www.w3.org/ns/odrl/2/LogicalConstraint"/>
        <skos:member rdf:resource="http://www.w3.org/ns/odrl/2/operand"/>
        <skos:prefLabel xml:lang="en">Logical Constraint</skos:prefLabel>
        <skos:scopeNote xml:lang="en">ODRL Core Vocabulary Terms</skos:scopeNote>
    </owl:NamedIndividual>
    


    <!-- http://www.w3.org/ns/odrl/2/#partyConcepts -->

    <owl:NamedIndividual rdf:about="http://www.w3.org/ns/odrl/2/#partyConcepts">
        <rdf:type rdf:resource="http://www.w3.org/2004/02/skos/core#Collection"/>
        <skos:member rdf:resource="http://www.w3.org/ns/odrl/2/Party"/>
        <skos:member rdf:resource="http://www.w3.org/ns/odrl/2/PartyCollection"/>
        <skos:prefLabel xml:lang="en">Party</skos:prefLabel>
        <skos:scopeNote xml:lang="en">ODRL Core Vocabulary Terms</skos:scopeNote>
    </owl:NamedIndividual>
    


    <!-- http://www.w3.org/ns/odrl/2/#partyRoles -->

    <owl:NamedIndividual rdf:about="http://www.w3.org/ns/odrl/2/#partyRoles">
        <rdf:type rdf:resource="http://www.w3.org/2004/02/skos/core#Collection"/>
        <skos:member rdf:resource="http://www.w3.org/ns/odrl/2/assignee"/>
        <skos:member rdf:resource="http://www.w3.org/ns/odrl/2/assigneeOf"/>
        <skos:member rdf:resource="http://www.w3.org/ns/odrl/2/assigner"/>
        <skos:member rdf:resource="http://www.w3.org/ns/odrl/2/assignerOf"/>
        <skos:prefLabel xml:lang="en">Party Functions</skos:prefLabel>
        <skos:scopeNote xml:lang="en">ODRL Core Vocabulary Terms</skos:scopeNote>
    </owl:NamedIndividual>
    


    <!-- http://www.w3.org/ns/odrl/2/#partyRolesCommon -->

    <owl:NamedIndividual rdf:about="http://www.w3.org/ns/odrl/2/#partyRolesCommon">
        <rdf:type rdf:resource="http://www.w3.org/2004/02/skos/core#Collection"/>
        <skos:member rdf:resource="http://www.w3.org/ns/odrl/2/attributedParty"/>
        <skos:member rdf:resource="http://www.w3.org/ns/odrl/2/attributingParty"/>
        <skos:member rdf:resource="http://www.w3.org/ns/odrl/2/compensatedParty"/>
        <skos:member rdf:resource="http://www.w3.org/ns/odrl/2/compensatingParty"/>
        <skos:member rdf:resource="http://www.w3.org/ns/odrl/2/consentedParty"/>
        <skos:member rdf:resource="http://www.w3.org/ns/odrl/2/consentingParty"/>
        <skos:member rdf:resource="http://www.w3.org/ns/odrl/2/contractedParty"/>
        <skos:member rdf:resource="http://www.w3.org/ns/odrl/2/contractingParty"/>
        <skos:member rdf:resource="http://www.w3.org/ns/odrl/2/informedParty"/>
        <skos:member rdf:resource="http://www.w3.org/ns/odrl/2/informingParty"/>
        <skos:member rdf:resource="http://www.w3.org/ns/odrl/2/trackedParty"/>
        <skos:member rdf:resource="http://www.w3.org/ns/odrl/2/trackingParty"/>
        <skos:prefLabel xml:lang="en">Party Functions</skos:prefLabel>
        <skos:scopeNote xml:lang="en">ODRL Common Vocabulary Terms</skos:scopeNote>
    </owl:NamedIndividual>
    


    <!-- http://www.w3.org/ns/odrl/2/#permissions -->

    <owl:NamedIndividual rdf:about="http://www.w3.org/ns/odrl/2/#permissions">
        <rdf:type rdf:resource="http://www.w3.org/2004/02/skos/core#Collection"/>
        <skos:member rdf:resource="http://www.w3.org/ns/odrl/2/Permission"/>
        <skos:member rdf:resource="http://www.w3.org/ns/odrl/2/permission"/>
        <skos:prefLabel xml:lang="en">Permission</skos:prefLabel>
        <skos:scopeNote xml:lang="en">ODRL Core Vocabulary Terms</skos:scopeNote>
    </owl:NamedIndividual>
    


    <!-- http://www.w3.org/ns/odrl/2/#policyConcepts -->

    <owl:NamedIndividual rdf:about="http://www.w3.org/ns/odrl/2/#policyConcepts">
        <rdf:type rdf:resource="http://www.w3.org/2004/02/skos/core#Collection"/>
        <skos:member rdf:resource="http://www.w3.org/ns/odrl/2/Policy"/>
        <skos:member rdf:resource="http://www.w3.org/ns/odrl/2/inheritFrom"/>
        <skos:member rdf:resource="http://www.w3.org/ns/odrl/2/profile"/>
        <skos:member rdf:resource="http://www.w3.org/ns/odrl/2/uid"/>
        <skos:prefLabel xml:lang="en">Policy</skos:prefLabel>
        <skos:scopeNote xml:lang="en">ODRL Core Vocabulary Terms</skos:scopeNote>
    </owl:NamedIndividual>
    


    <!-- http://www.w3.org/ns/odrl/2/#policySubClasses -->

    <owl:NamedIndividual rdf:about="http://www.w3.org/ns/odrl/2/#policySubClasses">
        <rdf:type rdf:resource="http://www.w3.org/2004/02/skos/core#Collection"/>
        <skos:member rdf:resource="http://www.w3.org/ns/odrl/2/Agreement"/>
        <skos:member rdf:resource="http://www.w3.org/ns/odrl/2/Offer"/>
        <skos:member rdf:resource="http://www.w3.org/ns/odrl/2/Set"/>
        <skos:prefLabel xml:lang="en">Policy Subclasses</skos:prefLabel>
        <skos:scopeNote xml:lang="en">ODRL Core Vocabulary Terms</skos:scopeNote>
    </owl:NamedIndividual>
    


    <!-- http://www.w3.org/ns/odrl/2/#policySubClassesCommon -->

    <owl:NamedIndividual rdf:about="http://www.w3.org/ns/odrl/2/#policySubClassesCommon">
        <rdf:type rdf:resource="http://www.w3.org/2004/02/skos/core#Collection"/>
        <skos:member rdf:resource="http://www.w3.org/ns/odrl/2/Assertion"/>
        <skos:member rdf:resource="http://www.w3.org/ns/odrl/2/Privacy"/>
        <skos:member rdf:resource="http://www.w3.org/ns/odrl/2/Request"/>
        <skos:member rdf:resource="http://www.w3.org/ns/odrl/2/Ticket"/>
        <skos:prefLabel xml:lang="en">Policy Subclasses</skos:prefLabel>
        <skos:scopeNote xml:lang="en">ODRL Common Vocabulary Terms</skos:scopeNote>
    </owl:NamedIndividual>
    


    <!-- http://www.w3.org/ns/odrl/2/#prohibitions -->

    <owl:NamedIndividual rdf:about="http://www.w3.org/ns/odrl/2/#prohibitions">
        <rdf:type rdf:resource="http://www.w3.org/2004/02/skos/core#Collection"/>
        <skos:member rdf:resource="http://www.w3.org/ns/odrl/2/Prohibition"/>
        <skos:member rdf:resource="http://www.w3.org/ns/odrl/2/prohibition"/>
        <skos:prefLabel xml:lang="en">Prohibition</skos:prefLabel>
        <skos:scopeNote xml:lang="en">ODRL Core Vocabulary Terms</skos:scopeNote>
    </owl:NamedIndividual>
    


    <!-- http://www.w3.org/ns/odrl/2/#ruleConcepts -->

    <owl:NamedIndividual rdf:about="http://www.w3.org/ns/odrl/2/#ruleConcepts">
        <rdf:type rdf:resource="http://www.w3.org/2004/02/skos/core#Collection"/>
        <skos:member rdf:resource="http://www.w3.org/ns/odrl/2/Rule"/>
        <skos:member rdf:resource="http://www.w3.org/ns/odrl/2/failure"/>
        <skos:member rdf:resource="http://www.w3.org/ns/odrl/2/function"/>
        <skos:member rdf:resource="http://www.w3.org/ns/odrl/2/relation"/>
        <skos:prefLabel xml:lang="en">Rule</skos:prefLabel>
        <skos:scopeNote xml:lang="en">ODRL Core Vocabulary Terms</skos:scopeNote>
    </owl:NamedIndividual>
    


    <!-- https://schema.org/actionApplication -->

    <owl:NamedIndividual rdf:about="https://schema.org/actionApplication">
        <rdfs:comment xml:lang="en">An application that can complete the request.</rdfs:comment>
        <rdfs:isDefinedBy rdf:resource="https://schema.org/actionApplication"/>
        <rdfs:label xml:lang="en">actionApplication</rdfs:label>
    </owl:NamedIndividual>
    


    <!-- https://schema.org/actionOption -->

    <owl:NamedIndividual rdf:about="https://schema.org/actionOption">
        <rdfs:comment xml:lang="en">A sub property of object. The options subject to this action.</rdfs:comment>
        <rdfs:isDefinedBy rdf:resource="https://schema.org/actionOption"/>
        <rdfs:label xml:lang="en">actionOption</rdfs:label>
    </owl:NamedIndividual>
    


    <!-- https://schema.org/actor -->

    <owl:NamedIndividual rdf:about="https://schema.org/actor">
        <rdfs:comment xml:lang="en">An actor (individual or a group), e.g. in TV, radio, movie, video games etc., or in an event. Actors can be associated with individual items or with a series, episode, clip.</rdfs:comment>
        <rdfs:isDefinedBy rdf:resource="https://schema.org/actor"/>
        <rdfs:label xml:lang="en">actor</rdfs:label>
    </owl:NamedIndividual>
    


    <!-- https://schema.org/actors -->

    <owl:NamedIndividual rdf:about="https://schema.org/actors">
        <schema:supersededBy rdf:resource="https://schema.org/actor"/>
        <rdfs:comment xml:lang="en">An actor, e.g. in TV, radio, movie, video games etc. Actors can be associated with individual items or with a series, episode, clip.</rdfs:comment>
        <rdfs:isDefinedBy rdf:resource="https://schema.org/actors"/>
        <rdfs:label xml:lang="en">actors</rdfs:label>
    </owl:NamedIndividual>
    


    <!-- https://schema.org/album -->

    <owl:NamedIndividual rdf:about="https://schema.org/album">
        <rdfs:comment xml:lang="en">A music album.</rdfs:comment>
        <rdfs:isDefinedBy rdf:resource="https://schema.org/album"/>
        <rdfs:label xml:lang="en">album</rdfs:label>
    </owl:NamedIndividual>
    


    <!-- https://schema.org/albums -->

    <owl:NamedIndividual rdf:about="https://schema.org/albums">
        <schema:supersededBy rdf:resource="https://schema.org/album"/>
        <rdfs:comment xml:lang="en">A collection of music albums.</rdfs:comment>
        <rdfs:isDefinedBy rdf:resource="https://schema.org/albums"/>
        <rdfs:label xml:lang="en">albums</rdfs:label>
    </owl:NamedIndividual>
    


    <!-- https://schema.org/application -->

    <owl:NamedIndividual rdf:about="https://schema.org/application">
        <schema:supersededBy rdf:resource="https://schema.org/actionApplication"/>
        <rdfs:comment xml:lang="en">An application that can complete the request.</rdfs:comment>
        <rdfs:isDefinedBy rdf:resource="https://schema.org/application"/>
        <rdfs:label xml:lang="en">application</rdfs:label>
    </owl:NamedIndividual>
    


    <!-- https://schema.org/area -->

    <owl:NamedIndividual rdf:about="https://schema.org/area">
        <schema:supersededBy rdf:resource="https://schema.org/serviceArea"/>
        <rdfs:comment xml:lang="en">The area within which users can expect to reach the broadcast service.</rdfs:comment>
        <rdfs:isDefinedBy rdf:resource="https://schema.org/area"/>
        <rdfs:label xml:lang="en">area</rdfs:label>
    </owl:NamedIndividual>
    


    <!-- https://schema.org/areaServed -->

    <owl:NamedIndividual rdf:about="https://schema.org/areaServed">
        <rdfs:comment xml:lang="en">The geographic area where a service or offered item is provided.</rdfs:comment>
        <rdfs:isDefinedBy rdf:resource="https://schema.org/areaServed"/>
        <rdfs:label xml:lang="en">areaServed</rdfs:label>
    </owl:NamedIndividual>
    


    <!-- https://schema.org/arterialBranch -->

    <owl:NamedIndividual rdf:about="https://schema.org/arterialBranch">
        <rdfs:comment xml:lang="en">The branches that comprise the arterial structure.</rdfs:comment>
        <rdfs:isDefinedBy rdf:resource="https://health-lifesci.schema.org/arterialBranch"/>
        <rdfs:label xml:lang="en">arterialBranch</rdfs:label>
    </owl:NamedIndividual>
    


    <!-- https://schema.org/artworkSurface -->

    <owl:NamedIndividual rdf:about="https://schema.org/artworkSurface">
        <rdfs:comment xml:lang="en">The supporting materials for the artwork, e.g. Canvas, Paper, Wood, Board, etc.</rdfs:comment>
        <rdfs:isDefinedBy rdf:resource="https://schema.org/artworkSurface"/>
        <rdfs:label xml:lang="en">artworkSurface</rdfs:label>
    </owl:NamedIndividual>
    


    <!-- https://schema.org/aspect -->

    <owl:NamedIndividual rdf:about="https://schema.org/aspect">
        <schema:supersededBy rdf:resource="https://schema.org/mainContentOfPage"/>
        <rdfs:comment xml:lang="en">An aspect of medical practice that is considered on the page, such as &apos;diagnosis&apos;, &apos;treatment&apos;, &apos;causes&apos;, &apos;prognosis&apos;, &apos;etiology&apos;, &apos;epidemiology&apos;, etc.</rdfs:comment>
        <rdfs:isDefinedBy rdf:resource="https://health-lifesci.schema.org/aspect"/>
        <rdfs:label xml:lang="en">aspect</rdfs:label>
    </owl:NamedIndividual>
    


    <!-- https://schema.org/assembly -->

    <owl:NamedIndividual rdf:about="https://schema.org/assembly">
        <schema:supersededBy rdf:resource="https://schema.org/executableLibraryName"/>
        <rdfs:comment xml:lang="en">Library file name, e.g., mscorlib.dll, system.web.dll.</rdfs:comment>
        <rdfs:isDefinedBy rdf:resource="https://schema.org/assembly"/>
        <rdfs:label xml:lang="en">assembly</rdfs:label>
    </owl:NamedIndividual>
    


    <!-- https://schema.org/attendee -->

    <owl:NamedIndividual rdf:about="https://schema.org/attendee">
        <rdfs:comment xml:lang="en">A person or organization attending the event.</rdfs:comment>
        <rdfs:isDefinedBy rdf:resource="https://schema.org/attendee"/>
        <rdfs:label xml:lang="en">attendee</rdfs:label>
    </owl:NamedIndividual>
    


    <!-- https://schema.org/attendees -->

    <owl:NamedIndividual rdf:about="https://schema.org/attendees">
        <schema:supersededBy rdf:resource="https://schema.org/attendee"/>
        <rdfs:comment xml:lang="en">A person attending the event.</rdfs:comment>
        <rdfs:isDefinedBy rdf:resource="https://schema.org/attendees"/>
        <rdfs:label xml:lang="en">attendees</rdfs:label>
    </owl:NamedIndividual>
    


    <!-- https://schema.org/audience -->

    <owl:NamedIndividual rdf:about="https://schema.org/audience">
        <rdfs:comment xml:lang="en">An intended audience, i.e. a group for whom something was created.</rdfs:comment>
        <rdfs:isDefinedBy rdf:resource="https://schema.org/audience"/>
        <rdfs:label xml:lang="en">audience</rdfs:label>
    </owl:NamedIndividual>
    


    <!-- https://schema.org/availableOnDevice -->

    <owl:NamedIndividual rdf:about="https://schema.org/availableOnDevice">
        <rdfs:comment xml:lang="en">Device required to run the application. Used in cases where a specific make/model is required to run the application.</rdfs:comment>
        <rdfs:isDefinedBy rdf:resource="https://schema.org/availableOnDevice"/>
        <rdfs:label xml:lang="en">availableOnDevice</rdfs:label>
    </owl:NamedIndividual>
    


    <!-- https://schema.org/award -->

    <owl:NamedIndividual rdf:about="https://schema.org/award">
        <rdfs:comment xml:lang="en">An award won by or for this item.</rdfs:comment>
        <rdfs:isDefinedBy rdf:resource="https://schema.org/award"/>
        <rdfs:label xml:lang="en">award</rdfs:label>
    </owl:NamedIndividual>
    


    <!-- https://schema.org/awards -->

    <owl:NamedIndividual rdf:about="https://schema.org/awards">
        <schema:supersededBy rdf:resource="https://schema.org/award"/>
        <rdfs:comment xml:lang="en">Awards won by or for this item.</rdfs:comment>
        <rdfs:isDefinedBy rdf:resource="https://schema.org/awards"/>
        <rdfs:label xml:lang="en">awards</rdfs:label>
    </owl:NamedIndividual>
    


    <!-- https://schema.org/benefits -->

    <owl:NamedIndividual rdf:about="https://schema.org/benefits">
        <schema:supersededBy rdf:resource="https://schema.org/jobBenefits"/>
        <rdfs:comment xml:lang="en">Description of benefits associated with the job.</rdfs:comment>
        <rdfs:isDefinedBy rdf:resource="https://schema.org/benefits"/>
        <rdfs:label xml:lang="en">benefits</rdfs:label>
    </owl:NamedIndividual>
    


    <!-- https://schema.org/blogPost -->

    <owl:NamedIndividual rdf:about="https://schema.org/blogPost">
        <rdfs:comment xml:lang="en">A posting that is part of this blog.</rdfs:comment>
        <rdfs:isDefinedBy rdf:resource="https://schema.org/blogPost"/>
        <rdfs:label xml:lang="en">blogPost</rdfs:label>
    </owl:NamedIndividual>
    


    <!-- https://schema.org/blogPosts -->

    <owl:NamedIndividual rdf:about="https://schema.org/blogPosts">
        <schema:supersededBy rdf:resource="https://schema.org/blogPost"/>
        <rdfs:comment xml:lang="en">Indicates a post that is part of a &lt;a class=&quot;localLink&quot; href=&quot;/Blog&quot;&gt;Blog&lt;/a&gt;. Note that historically, what we term a &quot;Blog&quot; was once known as a &quot;weblog&quot;, and that what we term a &quot;BlogPosting&quot; is now often colloquially referred to as a &quot;blog&quot;.</rdfs:comment>
        <rdfs:isDefinedBy rdf:resource="https://schema.org/blogPosts"/>
        <rdfs:label xml:lang="en">blogPosts</rdfs:label>
    </owl:NamedIndividual>
    


    <!-- https://schema.org/bookingAgent -->

    <owl:NamedIndividual rdf:about="https://schema.org/bookingAgent">
        <schema:supersededBy rdf:resource="https://schema.org/broker"/>
        <rdfs:comment xml:lang="en">&apos;bookingAgent&apos; is an out-dated term indicating a &apos;broker&apos; that serves as a booking agent.</rdfs:comment>
        <rdfs:isDefinedBy rdf:resource="https://schema.org/bookingAgent"/>
        <rdfs:label xml:lang="en">bookingAgent</rdfs:label>
    </owl:NamedIndividual>
    


    <!-- https://schema.org/branch -->

    <owl:NamedIndividual rdf:about="https://schema.org/branch">
        <schema:supersededBy rdf:resource="https://schema.org/arterialBranch"/>
        <rdfs:comment xml:lang="en">The branches that delineate from the nerve bundle. Not to be confused with &lt;a class=&quot;localLink&quot; href=&quot;/branchOf&quot;&gt;branchOf&lt;/a&gt;.</rdfs:comment>
        <rdfs:isDefinedBy rdf:resource="https://health-lifesci.schema.org/branch"/>
        <rdfs:label xml:lang="en">branch</rdfs:label>
    </owl:NamedIndividual>
    


    <!-- https://schema.org/branchOf -->

    <owl:NamedIndividual rdf:about="https://schema.org/branchOf">
        <schema:supersededBy rdf:resource="https://schema.org/parentOrganization"/>
        <rdfs:comment xml:lang="en">The larger organization that this local business is a branch of, if any. Not to be confused with (anatomical) &lt;a class=&quot;localLink&quot; href=&quot;/branch&quot;&gt;branch&lt;/a&gt;.</rdfs:comment>
        <rdfs:isDefinedBy rdf:resource="https://schema.org/branchOf"/>
        <rdfs:label xml:lang="en">branchOf</rdfs:label>
    </owl:NamedIndividual>
    


    <!-- https://schema.org/broker -->

    <owl:NamedIndividual rdf:about="https://schema.org/broker">
        <rdfs:comment xml:lang="en">An entity that arranges for an exchange between a buyer and a seller.  In most cases a broker never acquires or releases ownership of a product or service involved in an exchange.  If it is not clear whether an entity is a broker, seller, or buyer, the latter two terms are preferred.</rdfs:comment>
        <rdfs:isDefinedBy rdf:resource="https://schema.org/broker"/>
        <rdfs:label xml:lang="en">broker</rdfs:label>
    </owl:NamedIndividual>
    


    <!-- https://schema.org/carrier -->

    <owl:NamedIndividual rdf:about="https://schema.org/carrier">
        <schema:supersededBy rdf:resource="https://schema.org/provider"/>
        <rdfs:comment xml:lang="en">&apos;carrier&apos; is an out-dated term indicating the &apos;provider&apos; for parcel delivery and flights.</rdfs:comment>
        <rdfs:isDefinedBy rdf:resource="https://schema.org/carrier"/>
        <rdfs:label xml:lang="en">carrier</rdfs:label>
    </owl:NamedIndividual>
    


    <!-- https://schema.org/catalog -->

    <owl:NamedIndividual rdf:about="https://schema.org/catalog">
        <schema:supersededBy rdf:resource="https://schema.org/includedInDataCatalog"/>
        <rdfs:comment xml:lang="en">A data catalog which contains this dataset.</rdfs:comment>
        <rdfs:isDefinedBy rdf:resource="https://schema.org/catalog"/>
        <rdfs:label xml:lang="en">catalog</rdfs:label>
    </owl:NamedIndividual>
    


    <!-- https://schema.org/clincalPharmacology -->

    <owl:NamedIndividual rdf:about="https://schema.org/clincalPharmacology">
        <schema:supersededBy rdf:resource="https://schema.org/clinicalPharmacology"/>
        <rdfs:comment xml:lang="en">Description of the absorption and elimination of drugs, including their concentration (pharmacokinetics, pK) and biological effects (pharmacodynamics, pD).</rdfs:comment>
        <rdfs:isDefinedBy rdf:resource="https://health-lifesci.schema.org/clincalPharmacology"/>
        <rdfs:label xml:lang="en">clincalPharmacology</rdfs:label>
    </owl:NamedIndividual>
    


    <!-- https://schema.org/clinicalPharmacology -->

    <owl:NamedIndividual rdf:about="https://schema.org/clinicalPharmacology">
        <rdfs:comment xml:lang="en">Description of the absorption and elimination of drugs, including their concentration (pharmacokinetics, pK) and biological effects (pharmacodynamics, pD).</rdfs:comment>
        <rdfs:isDefinedBy rdf:resource="https://health-lifesci.schema.org/clinicalPharmacology"/>
        <rdfs:label xml:lang="en">clinicalPharmacology</rdfs:label>
    </owl:NamedIndividual>
    


    <!-- https://schema.org/codeSampleType -->

    <owl:NamedIndividual rdf:about="https://schema.org/codeSampleType">
        <rdfs:comment xml:lang="en">What type of code sample: full (compile ready) solution, code snippet, inline code, scripts, template.</rdfs:comment>
        <rdfs:isDefinedBy rdf:resource="https://schema.org/codeSampleType"/>
        <rdfs:label xml:lang="en">codeSampleType</rdfs:label>
    </owl:NamedIndividual>
    


    <!-- https://schema.org/colleague -->

    <owl:NamedIndividual rdf:about="https://schema.org/colleague">
        <rdfs:comment xml:lang="en">A colleague of the person.</rdfs:comment>
        <rdfs:isDefinedBy rdf:resource="https://schema.org/colleague"/>
        <rdfs:label xml:lang="en">colleague</rdfs:label>
    </owl:NamedIndividual>
    


    <!-- https://schema.org/colleagues -->

    <owl:NamedIndividual rdf:about="https://schema.org/colleagues">
        <schema:supersededBy rdf:resource="https://schema.org/colleague"/>
        <rdfs:comment xml:lang="en">A colleague of the person.</rdfs:comment>
        <rdfs:isDefinedBy rdf:resource="https://schema.org/colleagues"/>
        <rdfs:label xml:lang="en">colleagues</rdfs:label>
    </owl:NamedIndividual>
    


    <!-- https://schema.org/collection -->

    <owl:NamedIndividual rdf:about="https://schema.org/collection">
        <schema:supersededBy rdf:resource="https://schema.org/targetCollection"/>
        <rdfs:comment xml:lang="en">A sub property of object. The collection target of the action.</rdfs:comment>
        <rdfs:isDefinedBy rdf:resource="https://schema.org/collection"/>
        <rdfs:label xml:lang="en">collection</rdfs:label>
    </owl:NamedIndividual>
    


    <!-- https://schema.org/contactPoint -->

    <owl:NamedIndividual rdf:about="https://schema.org/contactPoint">
        <rdfs:comment xml:lang="en">A contact point for a person or organization.</rdfs:comment>
        <rdfs:isDefinedBy rdf:resource="https://schema.org/contactPoint"/>
        <rdfs:label xml:lang="en">contactPoint</rdfs:label>
    </owl:NamedIndividual>
    


    <!-- https://schema.org/contactPoints -->

    <owl:NamedIndividual rdf:about="https://schema.org/contactPoints">
        <schema:supersededBy rdf:resource="https://schema.org/contactPoint"/>
        <rdfs:comment xml:lang="en">A contact point for a person or organization.</rdfs:comment>
        <rdfs:isDefinedBy rdf:resource="https://schema.org/contactPoints"/>
        <rdfs:label xml:lang="en">contactPoints</rdfs:label>
    </owl:NamedIndividual>
    


    <!-- https://schema.org/containedIn -->

    <owl:NamedIndividual rdf:about="https://schema.org/containedIn">
        <schema:supersededBy rdf:resource="https://schema.org/containedInPlace"/>
        <rdfs:comment xml:lang="en">The basic containment relation between a place and one that contains it.</rdfs:comment>
        <rdfs:isDefinedBy rdf:resource="https://schema.org/containedIn"/>
        <rdfs:label xml:lang="en">containedIn</rdfs:label>
    </owl:NamedIndividual>
    


    <!-- https://schema.org/containedInPlace -->

    <owl:NamedIndividual rdf:about="https://schema.org/containedInPlace">
        <rdfs:comment xml:lang="en">The basic containment relation between a place and one that contains it.</rdfs:comment>
        <rdfs:isDefinedBy rdf:resource="https://schema.org/containedInPlace"/>
        <rdfs:label xml:lang="en">containedInPlace</rdfs:label>
    </owl:NamedIndividual>
    


    <!-- https://schema.org/containsSeason -->

    <owl:NamedIndividual rdf:about="https://schema.org/containsSeason">
        <rdfs:comment xml:lang="en">A season that is part of the media series.</rdfs:comment>
        <rdfs:isDefinedBy rdf:resource="https://schema.org/containsSeason"/>
        <rdfs:label xml:lang="en">containsSeason</rdfs:label>
    </owl:NamedIndividual>
    


    <!-- https://schema.org/course -->

    <owl:NamedIndividual rdf:about="https://schema.org/course">
        <schema:supersededBy rdf:resource="https://schema.org/exerciseCourse"/>
        <rdfs:comment xml:lang="en">A sub property of location. The course where this action was taken.</rdfs:comment>
        <rdfs:isDefinedBy rdf:resource="https://schema.org/course"/>
        <rdfs:label xml:lang="en">course</rdfs:label>
    </owl:NamedIndividual>
    


    <!-- https://schema.org/datasetTimeInterval -->

    <owl:NamedIndividual rdf:about="https://schema.org/datasetTimeInterval">
        <schema:supersededBy rdf:resource="https://schema.org/temporalCoverage"/>
        <rdfs:comment xml:lang="en">The range of temporal applicability of a dataset, e.g. for a 2011 census dataset, the year 2011 (in ISO 8601 time interval format).</rdfs:comment>
        <rdfs:isDefinedBy rdf:resource="https://schema.org/datasetTimeInterval"/>
        <rdfs:label xml:lang="en">datasetTimeInterval</rdfs:label>
    </owl:NamedIndividual>
    


    <!-- https://schema.org/device -->

    <owl:NamedIndividual rdf:about="https://schema.org/device">
        <schema:supersededBy rdf:resource="https://schema.org/availableOnDevice"/>
        <rdfs:comment xml:lang="en">Device required to run the application. Used in cases where a specific make/model is required to run the application.</rdfs:comment>
        <rdfs:isDefinedBy rdf:resource="https://schema.org/device"/>
        <rdfs:label xml:lang="en">device</rdfs:label>
    </owl:NamedIndividual>
    


    <!-- https://schema.org/director -->

    <owl:NamedIndividual rdf:about="https://schema.org/director">
        <rdfs:comment xml:lang="en">A director of e.g. TV, radio, movie, video gaming etc. content, or of an event. Directors can be associated with individual items or with a series, episode, clip.</rdfs:comment>
        <rdfs:isDefinedBy rdf:resource="https://schema.org/director"/>
        <rdfs:label xml:lang="en">director</rdfs:label>
    </owl:NamedIndividual>
    


    <!-- https://schema.org/directors -->

    <owl:NamedIndividual rdf:about="https://schema.org/directors">
        <schema:supersededBy rdf:resource="https://schema.org/director"/>
        <rdfs:comment xml:lang="en">A director of e.g. TV, radio, movie, video games etc. content. Directors can be associated with individual items or with a series, episode, clip.</rdfs:comment>
        <rdfs:isDefinedBy rdf:resource="https://schema.org/directors"/>
        <rdfs:label xml:lang="en">directors</rdfs:label>
    </owl:NamedIndividual>
    


    <!-- https://schema.org/employee -->

    <owl:NamedIndividual rdf:about="https://schema.org/employee">
        <rdfs:comment xml:lang="en">Someone working for this organization.</rdfs:comment>
        <rdfs:isDefinedBy rdf:resource="https://schema.org/employee"/>
        <rdfs:label xml:lang="en">employee</rdfs:label>
    </owl:NamedIndividual>
    


    <!-- https://schema.org/employees -->

    <owl:NamedIndividual rdf:about="https://schema.org/employees">
        <schema:supersededBy rdf:resource="https://schema.org/employee"/>
        <rdfs:comment xml:lang="en">People working for this organization.</rdfs:comment>
        <rdfs:isDefinedBy rdf:resource="https://schema.org/employees"/>
        <rdfs:label xml:lang="en">employees</rdfs:label>
    </owl:NamedIndividual>
    


    <!-- https://schema.org/encoding -->

    <owl:NamedIndividual rdf:about="https://schema.org/encoding">
        <rdfs:comment xml:lang="en">A media object that encodes this CreativeWork. This property is a synonym for associatedMedia.</rdfs:comment>
        <rdfs:isDefinedBy rdf:resource="https://schema.org/encoding"/>
        <rdfs:label xml:lang="en">encoding</rdfs:label>
    </owl:NamedIndividual>
    


    <!-- https://schema.org/encodingFormat -->

    <owl:NamedIndividual rdf:about="https://schema.org/encodingFormat">
        <rdfs:comment xml:lang="en">Media type typically expressed using a MIME format (see &lt;a href=&quot;http://www.iana.org/assignments/media-types/media-types.xhtml&quot;&gt;IANA site&lt;/a&gt; and &lt;a href=&quot;https://developer.mozilla.org/en-US/docs/Web/HTTP/Basics_of_HTTP/MIME_types&quot;&gt;MDN reference&lt;/a&gt;), e.g. application/zip for a SoftwareApplication binary, audio/mpeg for .mp3 etc.&lt;br/&gt;&lt;br/&gt;

In cases where a &lt;a class=&quot;localLink&quot; href=&quot;/CreativeWork&quot;&gt;CreativeWork&lt;/a&gt; has several media type representations, &lt;a class=&quot;localLink&quot; href=&quot;/encoding&quot;&gt;encoding&lt;/a&gt; can be used to indicate each &lt;a class=&quot;localLink&quot; href=&quot;/MediaObject&quot;&gt;MediaObject&lt;/a&gt; alongside particular &lt;a class=&quot;localLink&quot; href=&quot;/encodingFormat&quot;&gt;encodingFormat&lt;/a&gt; information.&lt;br/&gt;&lt;br/&gt;

Unregistered or niche encoding and file formats can be indicated instead via the most appropriate URL, e.g. defining Web page or a Wikipedia/Wikidata entry.</rdfs:comment>
        <rdfs:isDefinedBy rdf:resource="https://schema.org/encodingFormat"/>
        <rdfs:label xml:lang="en">encodingFormat</rdfs:label>
    </owl:NamedIndividual>
    


    <!-- https://schema.org/encodings -->

    <owl:NamedIndividual rdf:about="https://schema.org/encodings">
        <schema:supersededBy rdf:resource="https://schema.org/encoding"/>
        <rdfs:comment xml:lang="en">A media object that encodes this CreativeWork.</rdfs:comment>
        <rdfs:isDefinedBy rdf:resource="https://schema.org/encodings"/>
        <rdfs:label xml:lang="en">encodings</rdfs:label>
    </owl:NamedIndividual>
    


    <!-- https://schema.org/episode -->

    <owl:NamedIndividual rdf:about="https://schema.org/episode">
        <rdfs:comment xml:lang="en">An episode of a TV, radio or game media within a series or season.</rdfs:comment>
        <rdfs:isDefinedBy rdf:resource="https://schema.org/episode"/>
        <rdfs:label xml:lang="en">episode</rdfs:label>
    </owl:NamedIndividual>
    


    <!-- https://schema.org/episodes -->

    <owl:NamedIndividual rdf:about="https://schema.org/episodes">
        <schema:supersededBy rdf:resource="https://schema.org/episode"/>
        <rdfs:comment xml:lang="en">An episode of a TV/radio series or season.</rdfs:comment>
        <rdfs:isDefinedBy rdf:resource="https://schema.org/episodes"/>
        <rdfs:label xml:lang="en">episodes</rdfs:label>
    </owl:NamedIndividual>
    


    <!-- https://schema.org/event -->

    <owl:NamedIndividual rdf:about="https://schema.org/event">
        <rdfs:comment xml:lang="en">Upcoming or past event associated with this place, organization, or action.</rdfs:comment>
        <rdfs:isDefinedBy rdf:resource="https://schema.org/event"/>
        <rdfs:label xml:lang="en">event</rdfs:label>
    </owl:NamedIndividual>
    


    <!-- https://schema.org/events -->

    <owl:NamedIndividual rdf:about="https://schema.org/events">
        <schema:supersededBy rdf:resource="https://schema.org/event"/>
        <rdfs:comment xml:lang="en">Upcoming or past events associated with this place or organization.</rdfs:comment>
        <rdfs:isDefinedBy rdf:resource="https://schema.org/events"/>
        <rdfs:label xml:lang="en">events</rdfs:label>
    </owl:NamedIndividual>
    


    <!-- https://schema.org/executableLibraryName -->

    <owl:NamedIndividual rdf:about="https://schema.org/executableLibraryName">
        <rdfs:comment xml:lang="en">Library file name, e.g., mscorlib.dll, system.web.dll.</rdfs:comment>
        <rdfs:isDefinedBy rdf:resource="https://schema.org/executableLibraryName"/>
        <rdfs:label xml:lang="en">executableLibraryName</rdfs:label>
    </owl:NamedIndividual>
    


    <!-- https://schema.org/exerciseCourse -->

    <owl:NamedIndividual rdf:about="https://schema.org/exerciseCourse">
        <rdfs:comment xml:lang="en">A sub property of location. The course where this action was taken.</rdfs:comment>
        <rdfs:isDefinedBy rdf:resource="https://schema.org/exerciseCourse"/>
        <rdfs:label xml:lang="en">exerciseCourse</rdfs:label>
    </owl:NamedIndividual>
    


    <!-- https://schema.org/fileFormat -->

    <owl:NamedIndividual rdf:about="https://schema.org/fileFormat">
        <schema:supersededBy rdf:resource="https://schema.org/encodingFormat"/>
        <rdfs:comment xml:lang="en">Media type, typically MIME format (see &lt;a href=&quot;http://www.iana.org/assignments/media-types/media-types.xhtml&quot;&gt;IANA site&lt;/a&gt;) of the content, e.g. application/zip of a SoftwareApplication binary. In cases where a CreativeWork has several media type representations, &apos;encoding&apos; can be used to indicate each MediaObject alongside particular fileFormat information. Unregistered or niche file formats can be indicated instead via the most appropriate URL, e.g. defining Web page or a Wikipedia entry.</rdfs:comment>
        <rdfs:isDefinedBy rdf:resource="https://schema.org/fileFormat"/>
        <rdfs:label xml:lang="en">fileFormat</rdfs:label>
    </owl:NamedIndividual>
    


    <!-- https://schema.org/founder -->

    <owl:NamedIndividual rdf:about="https://schema.org/founder">
        <rdfs:comment xml:lang="en">A person or organization who founded this organization.</rdfs:comment>
        <rdfs:isDefinedBy rdf:resource="https://schema.org/founder"/>
        <rdfs:label xml:lang="en">founder</rdfs:label>
    </owl:NamedIndividual>
    


    <!-- https://schema.org/founders -->

    <owl:NamedIndividual rdf:about="https://schema.org/founders">
        <schema:supersededBy rdf:resource="https://schema.org/founder"/>
        <rdfs:comment xml:lang="en">A person who founded this organization.</rdfs:comment>
        <rdfs:isDefinedBy rdf:resource="https://schema.org/founders"/>
        <rdfs:label xml:lang="en">founders</rdfs:label>
    </owl:NamedIndividual>
    


    <!-- https://schema.org/free -->

    <owl:NamedIndividual rdf:about="https://schema.org/free">
        <schema:supersededBy rdf:resource="https://schema.org/isAccessibleForFree"/>
        <rdfs:comment xml:lang="en">A flag to signal that the item, event, or place is accessible for free.</rdfs:comment>
        <rdfs:isDefinedBy rdf:resource="https://schema.org/free"/>
        <rdfs:label xml:lang="en">free</rdfs:label>
    </owl:NamedIndividual>
    


    <!-- https://schema.org/hasMap -->

    <owl:NamedIndividual rdf:about="https://schema.org/hasMap">
        <rdfs:comment xml:lang="en">A URL to a map of the place.</rdfs:comment>
        <rdfs:isDefinedBy rdf:resource="https://schema.org/hasMap"/>
        <rdfs:label xml:lang="en">hasMap</rdfs:label>
    </owl:NamedIndividual>
    


    <!-- https://schema.org/hasMenu -->

    <owl:NamedIndividual rdf:about="https://schema.org/hasMenu">
        <rdfs:comment xml:lang="en">Either the actual menu as a structured representation, as text, or a URL of the menu.</rdfs:comment>
        <rdfs:isDefinedBy rdf:resource="https://schema.org/hasMenu"/>
        <rdfs:label xml:lang="en">hasMenu</rdfs:label>
    </owl:NamedIndividual>
    


    <!-- https://schema.org/hasMerchantReturnPolicy -->

    <owl:NamedIndividual rdf:about="https://schema.org/hasMerchantReturnPolicy">
        <rdfs:comment xml:lang="en">Specifies a MerchantReturnPolicy that may be applicable.</rdfs:comment>
        <rdfs:isDefinedBy rdf:resource="https://pending.schema.org/hasMerchantReturnPolicy"/>
        <rdfs:label xml:lang="en">hasMerchantReturnPolicy</rdfs:label>
    </owl:NamedIndividual>
    


    <!-- https://schema.org/hasProductReturnPolicy -->

    <owl:NamedIndividual rdf:about="https://schema.org/hasProductReturnPolicy">
        <schema:supersededBy rdf:resource="https://schema.org/hasMerchantReturnPolicy"/>
        <rdfs:comment xml:lang="en">Indicates a ProductReturnPolicy that may be applicable.</rdfs:comment>
        <rdfs:isDefinedBy rdf:resource="https://attic.schema.org/hasProductReturnPolicy"/>
        <rdfs:label xml:lang="en">hasProductReturnPolicy</rdfs:label>
    </owl:NamedIndividual>
    


    <!-- https://schema.org/inLanguage -->

    <owl:NamedIndividual rdf:about="https://schema.org/inLanguage">
        <rdfs:comment xml:lang="en">The language of the content or performance or used in an action. Please use one of the language codes from the &lt;a href=&quot;http://tools.ietf.org/html/bcp47&quot;&gt;IETF BCP 47 standard&lt;/a&gt;. See also &lt;a class=&quot;localLink&quot; href=&quot;/availableLanguage&quot;&gt;availableLanguage&lt;/a&gt;.</rdfs:comment>
        <rdfs:isDefinedBy rdf:resource="https://schema.org/inLanguage"/>
        <rdfs:label xml:lang="en">inLanguage</rdfs:label>
    </owl:NamedIndividual>
    


    <!-- https://schema.org/incentiveCompensation -->

    <owl:NamedIndividual rdf:about="https://schema.org/incentiveCompensation">
        <rdfs:comment xml:lang="en">Description of bonus and commission compensation aspects of the job.</rdfs:comment>
        <rdfs:isDefinedBy rdf:resource="https://schema.org/incentiveCompensation"/>
        <rdfs:label xml:lang="en">incentiveCompensation</rdfs:label>
    </owl:NamedIndividual>
    


    <!-- https://schema.org/incentives -->

    <owl:NamedIndividual rdf:about="https://schema.org/incentives">
        <schema:supersededBy rdf:resource="https://schema.org/incentiveCompensation"/>
        <rdfs:comment xml:lang="en">Description of bonus and commission compensation aspects of the job.</rdfs:comment>
        <rdfs:isDefinedBy rdf:resource="https://schema.org/incentives"/>
        <rdfs:label xml:lang="en">incentives</rdfs:label>
    </owl:NamedIndividual>
    


    <!-- https://schema.org/includedDataCatalog -->

    <owl:NamedIndividual rdf:about="https://schema.org/includedDataCatalog">
        <schema:supersededBy rdf:resource="https://schema.org/includedInDataCatalog"/>
        <rdfs:comment xml:lang="en">A data catalog which contains this dataset (this property was previously &apos;catalog&apos;, preferred name is now &apos;includedInDataCatalog&apos;).</rdfs:comment>
        <rdfs:isDefinedBy rdf:resource="https://schema.org/includedDataCatalog"/>
        <rdfs:label xml:lang="en">includedDataCatalog</rdfs:label>
    </owl:NamedIndividual>
    


    <!-- https://schema.org/includedInDataCatalog -->

    <owl:NamedIndividual rdf:about="https://schema.org/includedInDataCatalog">
        <rdfs:comment xml:lang="en">A data catalog which contains this dataset.</rdfs:comment>
        <rdfs:isDefinedBy rdf:resource="https://schema.org/includedInDataCatalog"/>
        <rdfs:label xml:lang="en">includedInDataCatalog</rdfs:label>
    </owl:NamedIndividual>
    


    <!-- https://schema.org/ingredients -->

    <owl:NamedIndividual rdf:about="https://schema.org/ingredients">
        <schema:supersededBy rdf:resource="https://schema.org/recipeIngredient"/>
        <rdfs:comment xml:lang="en">A single ingredient used in the recipe, e.g. sugar, flour or garlic.</rdfs:comment>
        <rdfs:isDefinedBy rdf:resource="https://schema.org/ingredients"/>
        <rdfs:label xml:lang="en">ingredients</rdfs:label>
    </owl:NamedIndividual>
    


    <!-- https://schema.org/interactionCount -->

    <owl:NamedIndividual rdf:about="https://schema.org/interactionCount">
        <schema:supersededBy rdf:resource="https://schema.org/interactionStatistic"/>
        <rdfs:comment xml:lang="en">This property is deprecated, alongside the UserInteraction types on which it depended.</rdfs:comment>
        <rdfs:isDefinedBy rdf:resource="https://schema.org/interactionCount"/>
        <rdfs:label xml:lang="en">interactionCount</rdfs:label>
    </owl:NamedIndividual>
    


    <!-- https://schema.org/interactionStatistic -->

    <owl:NamedIndividual rdf:about="https://schema.org/interactionStatistic">
        <rdfs:comment xml:lang="en">The number of interactions for the CreativeWork using the WebSite or SoftwareApplication. The most specific child type of InteractionCounter should be used.</rdfs:comment>
        <rdfs:isDefinedBy rdf:resource="https://schema.org/interactionStatistic"/>
        <rdfs:label xml:lang="en">interactionStatistic</rdfs:label>
    </owl:NamedIndividual>
    


    <!-- https://schema.org/isAccessibleForFree -->

    <owl:NamedIndividual rdf:about="https://schema.org/isAccessibleForFree">
        <rdfs:comment xml:lang="en">A flag to signal that the item, event, or place is accessible for free.</rdfs:comment>
        <rdfs:isDefinedBy rdf:resource="https://schema.org/isAccessibleForFree"/>
        <rdfs:label xml:lang="en">isAccessibleForFree</rdfs:label>
    </owl:NamedIndividual>
    


    <!-- https://schema.org/isBasedOn -->

    <owl:NamedIndividual rdf:about="https://schema.org/isBasedOn">
        <rdfs:comment xml:lang="en">A resource from which this work is derived or from which it is a modification or adaptation.</rdfs:comment>
        <rdfs:isDefinedBy rdf:resource="https://schema.org/isBasedOn"/>
        <rdfs:label xml:lang="en">isBasedOn</rdfs:label>
    </owl:NamedIndividual>
    


    <!-- https://schema.org/isBasedOnUrl -->

    <owl:NamedIndividual rdf:about="https://schema.org/isBasedOnUrl">
        <schema:supersededBy rdf:resource="https://schema.org/isBasedOn"/>
        <rdfs:comment xml:lang="en">A resource that was used in the creation of this resource. This term can be repeated for multiple sources. For example, http://example.com/great-multiplication-intro.html.</rdfs:comment>
        <rdfs:isDefinedBy rdf:resource="https://schema.org/isBasedOnUrl"/>
        <rdfs:label xml:lang="en">isBasedOnUrl</rdfs:label>
    </owl:NamedIndividual>
    


    <!-- https://schema.org/jobBenefits -->

    <owl:NamedIndividual rdf:about="https://schema.org/jobBenefits">
        <rdfs:comment xml:lang="en">Description of benefits associated with the job.</rdfs:comment>
        <rdfs:isDefinedBy rdf:resource="https://schema.org/jobBenefits"/>
        <rdfs:label xml:lang="en">jobBenefits</rdfs:label>
    </owl:NamedIndividual>
    


    <!-- https://schema.org/language -->

    <owl:NamedIndividual rdf:about="https://schema.org/language">
        <schema:supersededBy rdf:resource="https://schema.org/inLanguage"/>
        <rdfs:comment xml:lang="en">A sub property of instrument. The language used on this action.</rdfs:comment>
        <rdfs:isDefinedBy rdf:resource="https://schema.org/language"/>
        <rdfs:label xml:lang="en">language</rdfs:label>
    </owl:NamedIndividual>
    


    <!-- https://schema.org/mainContentOfPage -->

    <owl:NamedIndividual rdf:about="https://schema.org/mainContentOfPage">
        <rdfs:comment xml:lang="en">Indicates if this web page element is the main subject of the page.</rdfs:comment>
        <rdfs:isDefinedBy rdf:resource="https://schema.org/mainContentOfPage"/>
        <rdfs:label xml:lang="en">mainContentOfPage</rdfs:label>
    </owl:NamedIndividual>
    


    <!-- https://schema.org/map -->

    <owl:NamedIndividual rdf:about="https://schema.org/map">
        <schema:supersededBy rdf:resource="https://schema.org/hasMap"/>
        <rdfs:comment xml:lang="en">A URL to a map of the place.</rdfs:comment>
        <rdfs:isDefinedBy rdf:resource="https://schema.org/map"/>
        <rdfs:label xml:lang="en">map</rdfs:label>
    </owl:NamedIndividual>
    


    <!-- https://schema.org/maps -->

    <owl:NamedIndividual rdf:about="https://schema.org/maps">
        <schema:supersededBy rdf:resource="https://schema.org/hasMap"/>
        <rdfs:comment xml:lang="en">A URL to a map of the place.</rdfs:comment>
        <rdfs:isDefinedBy rdf:resource="https://schema.org/maps"/>
        <rdfs:label xml:lang="en">maps</rdfs:label>
    </owl:NamedIndividual>
    


    <!-- https://schema.org/member -->

    <owl:NamedIndividual rdf:about="https://schema.org/member">
        <rdfs:comment xml:lang="en">A member of an Organization or a ProgramMembership. Organizations can be members of organizations; ProgramMembership is typically for individuals.</rdfs:comment>
        <rdfs:isDefinedBy rdf:resource="https://schema.org/member"/>
        <rdfs:label xml:lang="en">member</rdfs:label>
    </owl:NamedIndividual>
    


    <!-- https://schema.org/members -->

    <owl:NamedIndividual rdf:about="https://schema.org/members">
        <schema:supersededBy rdf:resource="https://schema.org/member"/>
        <rdfs:comment xml:lang="en">A member of this organization.</rdfs:comment>
        <rdfs:isDefinedBy rdf:resource="https://schema.org/members"/>
        <rdfs:label xml:lang="en">members</rdfs:label>
    </owl:NamedIndividual>
    


    <!-- https://schema.org/menu -->

    <owl:NamedIndividual rdf:about="https://schema.org/menu">
        <schema:supersededBy rdf:resource="https://schema.org/hasMenu"/>
        <rdfs:comment xml:lang="en">Either the actual menu as a structured representation, as text, or a URL of the menu.</rdfs:comment>
        <rdfs:isDefinedBy rdf:resource="https://schema.org/menu"/>
        <rdfs:label xml:lang="en">menu</rdfs:label>
    </owl:NamedIndividual>
    


    <!-- https://schema.org/merchant -->

    <owl:NamedIndividual rdf:about="https://schema.org/merchant">
        <schema:supersededBy rdf:resource="https://schema.org/seller"/>
        <rdfs:comment xml:lang="en">&apos;merchant&apos; is an out-dated term for &apos;seller&apos;.</rdfs:comment>
        <rdfs:isDefinedBy rdf:resource="https://schema.org/merchant"/>
        <rdfs:label xml:lang="en">merchant</rdfs:label>
    </owl:NamedIndividual>
    


    <!-- https://schema.org/merchantReturnDays -->

    <owl:NamedIndividual rdf:about="https://schema.org/merchantReturnDays">
        <rdfs:comment xml:lang="en">Specifies either a fixed return date or the number of days (from the delivery date) that a product can be returned. Used when the &lt;a class=&quot;localLink&quot; href=&quot;/returnPolicyCategory&quot;&gt;returnPolicyCategory&lt;/a&gt; property is specified as &lt;a class=&quot;localLink&quot; href=&quot;/MerchantReturnFiniteReturnWindow&quot;&gt;MerchantReturnFiniteReturnWindow&lt;/a&gt;.</rdfs:comment>
        <rdfs:isDefinedBy rdf:resource="https://pending.schema.org/merchantReturnDays"/>
        <rdfs:label xml:lang="en">merchantReturnDays</rdfs:label>
    </owl:NamedIndividual>
    


    <!-- https://schema.org/merchantReturnLink -->

    <owl:NamedIndividual rdf:about="https://schema.org/merchantReturnLink">
        <rdfs:comment xml:lang="en">Specifies a Web page or service by URL, for product returns.</rdfs:comment>
        <rdfs:isDefinedBy rdf:resource="https://pending.schema.org/merchantReturnLink"/>
        <rdfs:label xml:lang="en">merchantReturnLink</rdfs:label>
    </owl:NamedIndividual>
    


    <!-- https://schema.org/musicGroupMember -->

    <owl:NamedIndividual rdf:about="https://schema.org/musicGroupMember">
        <schema:supersededBy rdf:resource="https://schema.org/member"/>
        <rdfs:comment xml:lang="en">A member of a music group&amp;#x2014;for example, John, Paul, George, or Ringo.</rdfs:comment>
        <rdfs:isDefinedBy rdf:resource="https://schema.org/musicGroupMember"/>
        <rdfs:label xml:lang="en">musicGroupMember</rdfs:label>
    </owl:NamedIndividual>
    


    <!-- https://schema.org/namedPosition -->

    <owl:NamedIndividual rdf:about="https://schema.org/namedPosition">
        <schema:supersededBy rdf:resource="https://schema.org/roleName"/>
        <rdfs:comment xml:lang="en">A position played, performed or filled by a person or organization, as part of an organization. For example, an athlete in a SportsTeam might play in the position named &apos;Quarterback&apos;.</rdfs:comment>
        <rdfs:isDefinedBy rdf:resource="https://schema.org/namedPosition"/>
        <rdfs:label xml:lang="en">namedPosition</rdfs:label>
    </owl:NamedIndividual>
    


    <!-- https://schema.org/option -->

    <owl:NamedIndividual rdf:about="https://schema.org/option">
        <schema:supersededBy rdf:resource="https://schema.org/actionOption"/>
        <rdfs:comment xml:lang="en">A sub property of object. The options subject to this action.</rdfs:comment>
        <rdfs:isDefinedBy rdf:resource="https://schema.org/option"/>
        <rdfs:label xml:lang="en">option</rdfs:label>
    </owl:NamedIndividual>
    


    <!-- https://schema.org/parent -->

    <owl:NamedIndividual rdf:about="https://schema.org/parent">
        <rdfs:comment xml:lang="en">A parent of this person.</rdfs:comment>
        <rdfs:isDefinedBy rdf:resource="https://schema.org/parent"/>
        <rdfs:label xml:lang="en">parent</rdfs:label>
    </owl:NamedIndividual>
    


    <!-- https://schema.org/parentOrganization -->

    <owl:NamedIndividual rdf:about="https://schema.org/parentOrganization">
        <rdfs:comment xml:lang="en">The larger organization that this organization is a &lt;a class=&quot;localLink&quot; href=&quot;/subOrganization&quot;&gt;subOrganization&lt;/a&gt; of, if any.</rdfs:comment>
        <rdfs:isDefinedBy rdf:resource="https://schema.org/parentOrganization"/>
        <rdfs:label xml:lang="en">parentOrganization</rdfs:label>
    </owl:NamedIndividual>
    


    <!-- https://schema.org/parents -->

    <owl:NamedIndividual rdf:about="https://schema.org/parents">
        <schema:supersededBy rdf:resource="https://schema.org/parent"/>
        <rdfs:comment xml:lang="en">A parents of the person.</rdfs:comment>
        <rdfs:isDefinedBy rdf:resource="https://schema.org/parents"/>
        <rdfs:label xml:lang="en">parents</rdfs:label>
    </owl:NamedIndividual>
    


    <!-- https://schema.org/partOfSeries -->

    <owl:NamedIndividual rdf:about="https://schema.org/partOfSeries">
        <rdfs:comment xml:lang="en">The series to which this episode or season belongs.</rdfs:comment>
        <rdfs:isDefinedBy rdf:resource="https://schema.org/partOfSeries"/>
        <rdfs:label xml:lang="en">partOfSeries</rdfs:label>
    </owl:NamedIndividual>
    


    <!-- https://schema.org/partOfTVSeries -->

    <owl:NamedIndividual rdf:about="https://schema.org/partOfTVSeries">
        <schema:supersededBy rdf:resource="https://schema.org/partOfSeries"/>
        <rdfs:comment xml:lang="en">The TV series to which this episode or season belongs.</rdfs:comment>
        <rdfs:isDefinedBy rdf:resource="https://schema.org/partOfTVSeries"/>
        <rdfs:label xml:lang="en">partOfTVSeries</rdfs:label>
    </owl:NamedIndividual>
    


    <!-- https://schema.org/paymentDue -->

    <owl:NamedIndividual rdf:about="https://schema.org/paymentDue">
        <schema:supersededBy rdf:resource="https://schema.org/paymentDueDate"/>
        <rdfs:comment xml:lang="en">The date that payment is due.</rdfs:comment>
        <rdfs:isDefinedBy rdf:resource="https://schema.org/paymentDue"/>
        <rdfs:label xml:lang="en">paymentDue</rdfs:label>
    </owl:NamedIndividual>
    


    <!-- https://schema.org/paymentDueDate -->

    <owl:NamedIndividual rdf:about="https://schema.org/paymentDueDate">
        <rdfs:comment xml:lang="en">The date that payment is due.</rdfs:comment>
        <rdfs:isDefinedBy rdf:resource="https://schema.org/paymentDueDate"/>
        <rdfs:label xml:lang="en">paymentDueDate</rdfs:label>
    </owl:NamedIndividual>
    


    <!-- https://schema.org/performer -->

    <owl:NamedIndividual rdf:about="https://schema.org/performer">
        <rdfs:comment xml:lang="en">A performer at the event&amp;#x2014;for example, a presenter, musician, musical group or actor.</rdfs:comment>
        <rdfs:isDefinedBy rdf:resource="https://schema.org/performer"/>
        <rdfs:label xml:lang="en">performer</rdfs:label>
    </owl:NamedIndividual>
    


    <!-- https://schema.org/performers -->

    <owl:NamedIndividual rdf:about="https://schema.org/performers">
        <schema:supersededBy rdf:resource="https://schema.org/performer"/>
        <rdfs:comment xml:lang="en">The main performer or performers of the event&amp;#x2014;for example, a presenter, musician, or actor.</rdfs:comment>
        <rdfs:isDefinedBy rdf:resource="https://schema.org/performers"/>
        <rdfs:label xml:lang="en">performers</rdfs:label>
    </owl:NamedIndividual>
    


    <!-- https://schema.org/photo -->

    <owl:NamedIndividual rdf:about="https://schema.org/photo">
        <rdfs:comment xml:lang="en">A photograph of this place.</rdfs:comment>
        <rdfs:isDefinedBy rdf:resource="https://schema.org/photo"/>
        <rdfs:label xml:lang="en">photo</rdfs:label>
    </owl:NamedIndividual>
    


    <!-- https://schema.org/photos -->

    <owl:NamedIndividual rdf:about="https://schema.org/photos">
        <schema:supersededBy rdf:resource="https://schema.org/photo"/>
        <rdfs:comment xml:lang="en">Photographs of this place.</rdfs:comment>
        <rdfs:isDefinedBy rdf:resource="https://schema.org/photos"/>
        <rdfs:label xml:lang="en">photos</rdfs:label>
    </owl:NamedIndividual>
    


    <!-- https://schema.org/produces -->

    <owl:NamedIndividual rdf:about="https://schema.org/produces">
        <schema:supersededBy rdf:resource="https://schema.org/serviceOutput"/>
        <rdfs:comment xml:lang="en">The tangible thing generated by the service, e.g. a passport, permit, etc.</rdfs:comment>
        <rdfs:isDefinedBy rdf:resource="https://schema.org/produces"/>
        <rdfs:label xml:lang="en">produces</rdfs:label>
    </owl:NamedIndividual>
    


    <!-- https://schema.org/productReturnDays -->

    <owl:NamedIndividual rdf:about="https://schema.org/productReturnDays">
        <schema:supersededBy rdf:resource="https://schema.org/merchantReturnDays"/>
        <rdfs:comment xml:lang="en">The productReturnDays property indicates the number of days (from purchase) within which relevant product return policy is applicable.</rdfs:comment>
        <rdfs:isDefinedBy rdf:resource="https://attic.schema.org/productReturnDays"/>
        <rdfs:label xml:lang="en">productReturnDays</rdfs:label>
    </owl:NamedIndividual>
    


    <!-- https://schema.org/productReturnLink -->

    <owl:NamedIndividual rdf:about="https://schema.org/productReturnLink">
        <schema:supersededBy rdf:resource="https://schema.org/merchantReturnLink"/>
        <rdfs:comment xml:lang="en">Indicates a Web page or service by URL, for product return.</rdfs:comment>
        <rdfs:isDefinedBy rdf:resource="https://attic.schema.org/productReturnLink"/>
        <rdfs:label xml:lang="en">productReturnLink</rdfs:label>
    </owl:NamedIndividual>
    


    <!-- https://schema.org/provider -->

    <owl:NamedIndividual rdf:about="https://schema.org/provider">
        <rdfs:comment xml:lang="en">The service provider, service operator, or service performer; the goods producer. Another party (a seller) may offer those services or goods on behalf of the provider. A provider may also serve as the seller.</rdfs:comment>
        <rdfs:isDefinedBy rdf:resource="https://pending.schema.org/provider"/>
        <rdfs:label xml:lang="en">provider</rdfs:label>
    </owl:NamedIndividual>
    


    <!-- https://schema.org/recipeIngredient -->

    <owl:NamedIndividual rdf:about="https://schema.org/recipeIngredient">
        <rdfs:comment xml:lang="en">A single ingredient used in the recipe, e.g. sugar, flour or garlic.</rdfs:comment>
        <rdfs:isDefinedBy rdf:resource="https://schema.org/recipeIngredient"/>
        <rdfs:label xml:lang="en">recipeIngredient</rdfs:label>
    </owl:NamedIndividual>
    


    <!-- https://schema.org/requirements -->

    <owl:NamedIndividual rdf:about="https://schema.org/requirements">
        <schema:supersededBy rdf:resource="https://schema.org/softwareRequirements"/>
        <rdfs:comment xml:lang="en">Component dependency requirements for application. This includes runtime environments and shared libraries that are not included in the application distribution package, but required to run the application (examples: DirectX, Java or .NET runtime).</rdfs:comment>
        <rdfs:isDefinedBy rdf:resource="https://schema.org/requirements"/>
        <rdfs:label xml:lang="en">requirements</rdfs:label>
    </owl:NamedIndividual>
    


    <!-- https://schema.org/review -->

    <owl:NamedIndividual rdf:about="https://schema.org/review">
        <rdfs:comment xml:lang="en">A review of the item.</rdfs:comment>
        <rdfs:isDefinedBy rdf:resource="https://schema.org/review"/>
        <rdfs:label xml:lang="en">review</rdfs:label>
    </owl:NamedIndividual>
    


    <!-- https://schema.org/reviews -->

    <owl:NamedIndividual rdf:about="https://schema.org/reviews">
        <schema:supersededBy rdf:resource="https://schema.org/review"/>
        <rdfs:comment xml:lang="en">Review of the item.</rdfs:comment>
        <rdfs:isDefinedBy rdf:resource="https://schema.org/reviews"/>
        <rdfs:label xml:lang="en">reviews</rdfs:label>
    </owl:NamedIndividual>
    


    <!-- https://schema.org/roleName -->

    <owl:NamedIndividual rdf:about="https://schema.org/roleName">
        <rdfs:comment xml:lang="en">A role played, performed or filled by a person or organization. For example, the team of creators for a comic book might fill the roles named &apos;inker&apos;, &apos;penciller&apos;, and &apos;letterer&apos;; or an athlete in a SportsTeam might play in the position named &apos;Quarterback&apos;.</rdfs:comment>
        <rdfs:isDefinedBy rdf:resource="https://schema.org/roleName"/>
        <rdfs:label xml:lang="en">roleName</rdfs:label>
    </owl:NamedIndividual>
    


    <!-- https://schema.org/runtime -->

    <owl:NamedIndividual rdf:about="https://schema.org/runtime">
        <schema:supersededBy rdf:resource="https://schema.org/runtimePlatform"/>
        <rdfs:comment xml:lang="en">Runtime platform or script interpreter dependencies (example: Java v1, Python 2.3, .NET Framework 3.0).</rdfs:comment>
        <rdfs:isDefinedBy rdf:resource="https://schema.org/runtime"/>
        <rdfs:label xml:lang="en">runtime</rdfs:label>
    </owl:NamedIndividual>
    


    <!-- https://schema.org/runtimePlatform -->

    <owl:NamedIndividual rdf:about="https://schema.org/runtimePlatform">
        <rdfs:comment xml:lang="en">Runtime platform or script interpreter dependencies (example: Java v1, Python 2.3, .NET Framework 3.0).</rdfs:comment>
        <rdfs:isDefinedBy rdf:resource="https://schema.org/runtimePlatform"/>
        <rdfs:label xml:lang="en">runtimePlatform</rdfs:label>
    </owl:NamedIndividual>
    


    <!-- https://schema.org/sampleType -->

    <owl:NamedIndividual rdf:about="https://schema.org/sampleType">
        <schema:supersededBy rdf:resource="https://schema.org/codeSampleType"/>
        <rdfs:comment xml:lang="en">What type of code sample: full (compile ready) solution, code snippet, inline code, scripts, template.</rdfs:comment>
        <rdfs:isDefinedBy rdf:resource="https://schema.org/sampleType"/>
        <rdfs:label xml:lang="en">sampleType</rdfs:label>
    </owl:NamedIndividual>
    


    <!-- https://schema.org/season -->

    <owl:NamedIndividual rdf:about="https://schema.org/season">
        <schema:supersededBy rdf:resource="https://schema.org/containsSeason"/>
        <rdfs:comment xml:lang="en">A season in a media series.</rdfs:comment>
        <rdfs:isDefinedBy rdf:resource="https://schema.org/season"/>
        <rdfs:label xml:lang="en">season</rdfs:label>
    </owl:NamedIndividual>
    


    <!-- https://schema.org/seasons -->

    <owl:NamedIndividual rdf:about="https://schema.org/seasons">
        <schema:supersededBy rdf:resource="https://schema.org/season"/>
        <rdfs:comment xml:lang="en">A season in a media series.</rdfs:comment>
        <rdfs:isDefinedBy rdf:resource="https://schema.org/seasons"/>
        <rdfs:label xml:lang="en">seasons</rdfs:label>
    </owl:NamedIndividual>
    


    <!-- https://schema.org/seller -->

    <owl:NamedIndividual rdf:about="https://schema.org/seller">
        <rdfs:comment xml:lang="en">An entity which offers (sells / leases / lends / loans) the services / goods.  A seller may also be a provider.</rdfs:comment>
        <rdfs:isDefinedBy rdf:resource="https://schema.org/seller"/>
        <rdfs:label xml:lang="en">seller</rdfs:label>
    </owl:NamedIndividual>
    


    <!-- https://schema.org/serviceArea -->

    <owl:NamedIndividual rdf:about="https://schema.org/serviceArea">
        <schema:supersededBy rdf:resource="https://schema.org/areaServed"/>
        <rdfs:comment xml:lang="en">The geographic area where the service is provided.</rdfs:comment>
        <rdfs:isDefinedBy rdf:resource="https://schema.org/serviceArea"/>
        <rdfs:label xml:lang="en">serviceArea</rdfs:label>
    </owl:NamedIndividual>
    


    <!-- https://schema.org/serviceAudience -->

    <owl:NamedIndividual rdf:about="https://schema.org/serviceAudience">
        <schema:supersededBy rdf:resource="https://schema.org/audience"/>
        <rdfs:comment xml:lang="en">The audience eligible for this service.</rdfs:comment>
        <rdfs:isDefinedBy rdf:resource="https://schema.org/serviceAudience"/>
        <rdfs:label xml:lang="en">serviceAudience</rdfs:label>
    </owl:NamedIndividual>
    


    <!-- https://schema.org/serviceOutput -->

    <owl:NamedIndividual rdf:about="https://schema.org/serviceOutput">
        <rdfs:comment xml:lang="en">The tangible thing generated by the service, e.g. a passport, permit, etc.</rdfs:comment>
        <rdfs:isDefinedBy rdf:resource="https://schema.org/serviceOutput"/>
        <rdfs:label xml:lang="en">serviceOutput</rdfs:label>
    </owl:NamedIndividual>
    


    <!-- https://schema.org/sibling -->

    <owl:NamedIndividual rdf:about="https://schema.org/sibling">
        <rdfs:comment xml:lang="en">A sibling of the person.</rdfs:comment>
        <rdfs:isDefinedBy rdf:resource="https://schema.org/sibling"/>
        <rdfs:label xml:lang="en">sibling</rdfs:label>
    </owl:NamedIndividual>
    


    <!-- https://schema.org/siblings -->

    <owl:NamedIndividual rdf:about="https://schema.org/siblings">
        <schema:supersededBy rdf:resource="https://schema.org/sibling"/>
        <rdfs:comment xml:lang="en">A sibling of the person.</rdfs:comment>
        <rdfs:isDefinedBy rdf:resource="https://schema.org/siblings"/>
        <rdfs:label xml:lang="en">siblings</rdfs:label>
    </owl:NamedIndividual>
    


    <!-- https://schema.org/significantLink -->

    <owl:NamedIndividual rdf:about="https://schema.org/significantLink">
        <rdfs:comment xml:lang="en">One of the more significant URLs on the page. Typically, these are the non-navigation links that are clicked on the most.</rdfs:comment>
        <rdfs:isDefinedBy rdf:resource="https://schema.org/significantLink"/>
        <rdfs:label xml:lang="en">significantLink</rdfs:label>
    </owl:NamedIndividual>
    


    <!-- https://schema.org/significantLinks -->

    <owl:NamedIndividual rdf:about="https://schema.org/significantLinks">
        <schema:supersededBy rdf:resource="https://schema.org/significantLink"/>
        <rdfs:comment xml:lang="en">The most significant URLs on the page. Typically, these are the non-navigation links that are clicked on the most.</rdfs:comment>
        <rdfs:isDefinedBy rdf:resource="https://schema.org/significantLinks"/>
        <rdfs:label xml:lang="en">significantLinks</rdfs:label>
    </owl:NamedIndividual>
    


    <!-- https://schema.org/softwareRequirements -->

    <owl:NamedIndividual rdf:about="https://schema.org/softwareRequirements">
        <rdfs:comment xml:lang="en">Component dependency requirements for application. This includes runtime environments and shared libraries that are not included in the application distribution package, but required to run the application (examples: DirectX, Java or .NET runtime).</rdfs:comment>
        <rdfs:isDefinedBy rdf:resource="https://schema.org/softwareRequirements"/>
        <rdfs:label xml:lang="en">softwareRequirements</rdfs:label>
    </owl:NamedIndividual>
    


    <!-- https://schema.org/step -->

    <owl:NamedIndividual rdf:about="https://schema.org/step">
        <rdfs:comment xml:lang="en">A single step item (as HowToStep, text, document, video, etc.) or a HowToSection.</rdfs:comment>
        <rdfs:isDefinedBy rdf:resource="https://schema.org/step"/>
        <rdfs:label xml:lang="en">step</rdfs:label>
    </owl:NamedIndividual>
    


    <!-- https://schema.org/steps -->

    <owl:NamedIndividual rdf:about="https://schema.org/steps">
        <schema:supersededBy rdf:resource="https://schema.org/step"/>
        <rdfs:comment xml:lang="en">A single step item (as HowToStep, text, document, video, etc.) or a HowToSection (originally misnamed &apos;steps&apos;; &apos;step&apos; is preferred).</rdfs:comment>
        <rdfs:isDefinedBy rdf:resource="https://schema.org/steps"/>
        <rdfs:label xml:lang="en">steps</rdfs:label>
    </owl:NamedIndividual>
    


    <!-- https://schema.org/subEvent -->

    <owl:NamedIndividual rdf:about="https://schema.org/subEvent">
        <rdfs:comment xml:lang="en">An Event that is part of this event. For example, a conference event includes many presentations, each of which is a subEvent of the conference.</rdfs:comment>
        <rdfs:isDefinedBy rdf:resource="https://schema.org/subEvent"/>
        <rdfs:label xml:lang="en">subEvent</rdfs:label>
    </owl:NamedIndividual>
    


    <!-- https://schema.org/subEvents -->

    <owl:NamedIndividual rdf:about="https://schema.org/subEvents">
        <schema:supersededBy rdf:resource="https://schema.org/subEvent"/>
        <rdfs:comment xml:lang="en">Events that are a part of this event. For example, a conference event includes many presentations, each subEvents of the conference.</rdfs:comment>
        <rdfs:isDefinedBy rdf:resource="https://schema.org/subEvents"/>
        <rdfs:label xml:lang="en">subEvents</rdfs:label>
    </owl:NamedIndividual>
    


    <!-- https://schema.org/surface -->

    <owl:NamedIndividual rdf:about="https://schema.org/surface">
        <schema:supersededBy rdf:resource="https://schema.org/artworkSurface"/>
        <rdfs:comment xml:lang="en">A material used as a surface in some artwork, e.g. Canvas, Paper, Wood, Board, etc.</rdfs:comment>
        <rdfs:isDefinedBy rdf:resource="https://schema.org/surface"/>
        <rdfs:label xml:lang="en">surface</rdfs:label>
    </owl:NamedIndividual>
    


    <!-- https://schema.org/targetCollection -->

    <owl:NamedIndividual rdf:about="https://schema.org/targetCollection">
        <rdfs:comment xml:lang="en">A sub property of object. The collection target of the action.</rdfs:comment>
        <rdfs:isDefinedBy rdf:resource="https://schema.org/targetCollection"/>
        <rdfs:label xml:lang="en">targetCollection</rdfs:label>
    </owl:NamedIndividual>
    


    <!-- https://schema.org/temporalCoverage -->

    <owl:NamedIndividual rdf:about="https://schema.org/temporalCoverage">
        <rdfs:comment xml:lang="en">The temporalCoverage of a CreativeWork indicates the period that the content applies to, i.e. that it describes, either as a DateTime or as a textual string indicating a time period in &lt;a href=&quot;https://en.wikipedia.org/wiki/ISO_8601#Time_intervals&quot;&gt;ISO 8601 time interval format&lt;/a&gt;. In
      the case of a Dataset it will typically indicate the relevant time period in a precise notation (e.g. for a 2011 census dataset, the year 2011 would be written &quot;2011/2012&quot;). Other forms of content, e.g. ScholarlyArticle, Book, TVSeries or TVEpisode, may indicate their temporalCoverage in broader terms - textually or via well-known URL.
      Written works such as books may sometimes have precise temporal coverage too, e.g. a work set in 1939 - 1945 can be indicated in ISO 8601 interval format format via &quot;1939/1945&quot;.&lt;br/&gt;&lt;br/&gt;

Open-ended date ranges can be written with &quot;..&quot; in place of the end date. For example, &quot;2015-11/..&quot; indicates a range beginning in November 2015 and with no specified final date. This is tentative and might be updated in future when ISO 8601 is officially updated.</rdfs:comment>
        <rdfs:isDefinedBy rdf:resource="https://schema.org/temporalCoverage"/>
        <rdfs:label xml:lang="en">temporalCoverage</rdfs:label>
    </owl:NamedIndividual>
    


    <!-- https://schema.org/track -->

    <owl:NamedIndividual rdf:about="https://schema.org/track">
        <rdfs:comment xml:lang="en">A music recording (track)&amp;#x2014;usually a single song. If an ItemList is given, the list should contain items of type MusicRecording.</rdfs:comment>
        <rdfs:isDefinedBy rdf:resource="https://schema.org/track"/>
        <rdfs:label xml:lang="en">track</rdfs:label>
    </owl:NamedIndividual>
    


    <!-- https://schema.org/tracks -->

    <owl:NamedIndividual rdf:about="https://schema.org/tracks">
        <schema:supersededBy rdf:resource="https://schema.org/track"/>
        <rdfs:comment xml:lang="en">A music recording (track)&amp;#x2014;usually a single song.</rdfs:comment>
        <rdfs:isDefinedBy rdf:resource="https://schema.org/tracks"/>
        <rdfs:label xml:lang="en">tracks</rdfs:label>
    </owl:NamedIndividual>
    


    <!-- https://schema.org/vendor -->

    <owl:NamedIndividual rdf:about="https://schema.org/vendor">
        <schema:supersededBy rdf:resource="https://schema.org/seller"/>
        <rdfs:comment xml:lang="en">&apos;vendor&apos; is an earlier term for &apos;seller&apos;.</rdfs:comment>
        <rdfs:isDefinedBy rdf:resource="https://schema.org/vendor"/>
        <rdfs:label xml:lang="en">vendor</rdfs:label>
    </owl:NamedIndividual>
    


    <!-- https://schema.org/warranty -->

    <owl:NamedIndividual rdf:about="https://schema.org/warranty">
        <rdfs:comment xml:lang="en">The warranty promise(s) included in the offer.</rdfs:comment>
        <rdfs:isDefinedBy rdf:resource="https://schema.org/warranty"/>
        <rdfs:label xml:lang="en">warranty</rdfs:label>
    </owl:NamedIndividual>
    


    <!-- https://schema.org/warrantyPromise -->

    <owl:NamedIndividual rdf:about="https://schema.org/warrantyPromise">
        <schema:supersededBy rdf:resource="https://schema.org/warranty"/>
        <rdfs:comment xml:lang="en">The warranty promise(s) included in the offer.</rdfs:comment>
        <rdfs:isDefinedBy rdf:resource="https://schema.org/warrantyPromise"/>
        <rdfs:label xml:lang="en">warrantyPromise</rdfs:label>
    </owl:NamedIndividual>
    


    <!-- 
    ///////////////////////////////////////////////////////////////////////////////////////
    //
    // Annotations
    //
    ///////////////////////////////////////////////////////////////////////////////////////
     -->

    <rdf:Description rdf:about="http://www.w3.org/ns/odrl/2/Action">
        <rdfs:isDefinedBy rdf:resource="http://www.w3.org/ns/odrl/2/"/>
        <rdfs:label xml:lang="en">Action</rdfs:label>
        <skos:definition xml:lang="en">An operation on an Asset.</skos:definition>
        <skos:note xml:lang="en">Actions may be allowed by Permissions, disallowed by Prohibitions, or made mandatory by Duties.</skos:note>
    </rdf:Description>
    <rdf:Description rdf:about="http://www.w3.org/ns/odrl/2/Agreement">
        <rdfs:isDefinedBy rdf:resource="http://www.w3.org/ns/odrl/2/"/>
        <rdfs:label xml:lang="en">Agreement</rdfs:label>
        <skos:definition xml:lang="en">A Policy that grants the assignee a Rule over an Asset from an assigner.</skos:definition>
        <skos:note xml:lang="en">An Agreement Policy MUST contain at least one Permission or Prohibition rule, a Party with Assigner function, and a Party with Assignee function (in the same Permission or Prohibition). The Agreement Policy will grant the terms of the Policy from the Assigner to the Assignee.</skos:note>
    </rdf:Description>
    <rdf:Description rdf:about="http://www.w3.org/ns/odrl/2/Assertion">
        <rdfs:isDefinedBy rdf:resource="http://www.w3.org/ns/odrl/2/"/>
        <rdfs:label xml:lang="en">Assertion</rdfs:label>
        <skos:definition xml:lang="en">A Policy that asserts a Rule over an Asset from parties.</skos:definition>
        <skos:note xml:lang="en">For example, a party (an assignee or assigner) can claim what terms they have over an Asset. An Assertion Policy does not grant such permissions/prohibitions but only asserts the parties claims. An Assetion Policy  MUST contain a target Asset, a Party with any functional role, and at least one of a Permission or Prohibition rule.</skos:note>
        <skos:scopeNote xml:lang="en">Non-Normative</skos:scopeNote>
    </rdf:Description>
    <rdf:Description rdf:about="http://www.w3.org/ns/odrl/2/Asset">
        <rdfs:isDefinedBy rdf:resource="http://www.w3.org/ns/odrl/2/"/>
        <rdfs:label xml:lang="en">Asset</rdfs:label>
        <skos:definition xml:lang="en">A resource or a collection of resources that are the subject of a Rule.</skos:definition>
        <skos:note xml:lang="en">The Asset entity can be any form of identifiable resource, such as data/information, content/media, applications, or services. Furthermore, it can be used to represent other Asset entities that are needed to undertake the Policy expression, such as with the Duty entity. To describe more details about the Asset, it is recommended to use Dublin Core [[dcterms]] elements or other content metadata.</skos:note>
    </rdf:Description>
    <rdf:Description rdf:about="http://www.w3.org/ns/odrl/2/AssetCollection">
        <rdfs:isDefinedBy rdf:resource="http://www.w3.org/ns/odrl/2/"/>
        <rdfs:label xml:lang="en">Asset Collection</rdfs:label>
        <skos:definition xml:lang="en">An Asset that is collection of individual resources</skos:definition>
    </rdf:Description>
    <rdf:Description rdf:about="http://www.w3.org/ns/odrl/2/ConflictTerm">
        <rdfs:isDefinedBy rdf:resource="http://www.w3.org/ns/odrl/2/"/>
        <rdfs:label xml:lang="en">Conflict Strategy Preference</rdfs:label>
        <skos:definition xml:lang="en">Used to establish strategies to resolve conflicts that arise from the merging of Policies or conflicts between Permissions and Prohibitions in the same Policy.</skos:definition>
        <skos:note xml:lang="en">Instances of ConflictTerm describe strategies for resolving conflicts.</skos:note>
    </rdf:Description>
    <rdf:Description rdf:about="http://www.w3.org/ns/odrl/2/Constraint">
        <rdfs:isDefinedBy rdf:resource="http://www.w3.org/ns/odrl/2/"/>
        <rdfs:label xml:lang="en">Constraint</rdfs:label>
        <skos:definition xml:lang="en">A boolean expression that refines the semantics of an Action and Party/Asset Collection or declare the conditions applicable to a Rule.</skos:definition>
    </rdf:Description>
    <rdf:Description rdf:about="http://www.w3.org/ns/odrl/2/Duty">
        <rdfs:isDefinedBy rdf:resource="http://www.w3.org/ns/odrl/2/"/>
        <rdfs:label xml:lang="en">Duty</rdfs:label>
        <skos:definition xml:lang="en">The obligation to perform an Action</skos:definition>
    </rdf:Description>
    <rdf:Description rdf:about="http://www.w3.org/ns/odrl/2/LeftOperand">
        <rdfs:isDefinedBy rdf:resource="http://www.w3.org/ns/odrl/2/"/>
        <rdfs:label xml:lang="en">Left Operand</rdfs:label>
        <skos:definition xml:lang="en">Left operand for a constraint expression.</skos:definition>
        <skos:note xml:lang="en">Instances of the LeftOperand class are used as the leftOperand of a Constraint.</skos:note>
    </rdf:Description>
    <rdf:Description rdf:about="http://www.w3.org/ns/odrl/2/LogicalConstraint">
        <rdfs:isDefinedBy rdf:resource="http://www.w3.org/ns/odrl/2/"/>
        <rdfs:label xml:lang="en">Logical Constraint</rdfs:label>
        <skos:definition xml:lang="en">A logical expression that refines the semantics of an Action and Party/Asset Collection or declare the conditions applicable to a Rule.</skos:definition>
    </rdf:Description>
    <rdf:Description rdf:about="http://www.w3.org/ns/odrl/2/Offer">
        <rdfs:isDefinedBy rdf:resource="http://www.w3.org/ns/odrl/2/"/>
        <rdfs:label xml:lang="en">Offer</rdfs:label>
        <skos:definition xml:lang="en">A Policy that proposes a Rule over an Asset from an assigner.</skos:definition>
        <skos:note xml:lang="en">An Offer Policy MUST contain at least one Permission or Prohibition rule and a Party with Assigner function (in the same Permission or Prohibition). The Offer Policy MAY contain a Party with Assignee function, but MUST not grant any privileges to that Party.</skos:note>
    </rdf:Description>
    <rdf:Description rdf:about="http://www.w3.org/ns/odrl/2/Operator">
        <rdfs:isDefinedBy rdf:resource="http://www.w3.org/ns/odrl/2/"/>
        <rdfs:label xml:lang="en">Operator</rdfs:label>
        <skos:definition xml:lang="en">Operator for constraint expression.</skos:definition>
        <skos:note xml:lang="en">Instances of the Operator class representing relational operators.</skos:note>
    </rdf:Description>
    <rdf:Description rdf:about="http://www.w3.org/ns/odrl/2/Party">
        <rdfs:isDefinedBy rdf:resource="http://www.w3.org/ns/odrl/2/"/>
        <rdfs:label xml:lang="en">Party</rdfs:label>
        <skos:definition xml:lang="en">An entity or a collection of entities that undertake Roles in a Rule.</skos:definition>
        <skos:note xml:lang="en">The Party entity could be a person, group of people, organisation, or agent. An agent is a person or thing that takes an active role or produces a specified effect. To describe more details about the Party, it is recommended to use W3C vCard Ontology [[vcard-rdf]] or FOAF Vocabulary [[foaf]].</skos:note>
    </rdf:Description>
    <rdf:Description rdf:about="http://www.w3.org/ns/odrl/2/PartyCollection">
        <rdfs:isDefinedBy rdf:resource="http://www.w3.org/ns/odrl/2/"/>
        <rdfs:label xml:lang="en">Party Collection</rdfs:label>
        <skos:definition xml:lang="en">A Party that is a group of individual entities</skos:definition>
    </rdf:Description>
    <rdf:Description rdf:about="http://www.w3.org/ns/odrl/2/PartyScope">
        <rdfs:isDefinedBy rdf:resource="http://www.w3.org/ns/odrl/2/"/>
        <rdfs:label xml:lang="en">Party Scope</rdfs:label>
        <owl:deprecated rdf:datatype="http://www.w3.org/2001/XMLSchema#boolean">true</owl:deprecated>
        <skos:definition xml:lang="en">Scopes for Party Scope expressions.</skos:definition>
        <skos:note xml:lang="en">Instances of the PartyScope class represent the terms for the scope property of Parties.</skos:note>
    </rdf:Description>
    <rdf:Description rdf:about="http://www.w3.org/ns/odrl/2/Permission">
        <rdfs:isDefinedBy rdf:resource="http://www.w3.org/ns/odrl/2/"/>
        <rdfs:label xml:lang="en">Permission</rdfs:label>
        <skos:definition xml:lang="en">The ability to perform an Action over an Asset.</skos:definition>
    </rdf:Description>
    <rdf:Description rdf:about="http://www.w3.org/ns/odrl/2/Policy">
        <rdfs:isDefinedBy rdf:resource="http://www.w3.org/ns/odrl/2/"/>
        <rdfs:label xml:lang="en">Policy</rdfs:label>
        <skos:definition xml:lang="en">A non-empty group of Permissions and/or Prohibitions.</skos:definition>
        <skos:note xml:lang="en">A Policy may contain multiple Rules.</skos:note>
    </rdf:Description>
    <rdf:Description rdf:about="http://www.w3.org/ns/odrl/2/Privacy">
        <rdfs:isDefinedBy rdf:resource="http://www.w3.org/ns/odrl/2/"/>
        <rdfs:label xml:lang="en">Privacy Policy</rdfs:label>
        <skos:definition xml:lang="en">A Policy that expresses a Rule over an Asset containing personal information.</skos:definition>
        <skos:note xml:lang="en">A Privacy Policy  MUST contain a target Asset, a Party with Assigner  is, a Party with Assignee function, and at least one of a Permission or Prohibition rule that MUST include a Duty. The target Asset SHOULD contain or relate to personal information about the Assignee. The Duty MUST describe obligations on the Assigner about managing the Asset. The Assignee is being granted the terms of the Privacy policy from the Assigner.</skos:note>
        <skos:scopeNote xml:lang="en">Non-Normative</skos:scopeNote>
    </rdf:Description>
    <rdf:Description rdf:about="http://www.w3.org/ns/odrl/2/Prohibition">
        <rdfs:isDefinedBy rdf:resource="http://www.w3.org/ns/odrl/2/"/>
        <rdfs:label xml:lang="en">Prohibition</rdfs:label>
        <skos:definition xml:lang="en">The inability to perform an Action over an Asset.</skos:definition>
    </rdf:Description>
    <rdf:Description rdf:about="http://www.w3.org/ns/odrl/2/Request">
        <rdfs:isDefinedBy rdf:resource="http://www.w3.org/ns/odrl/2/"/>
        <rdfs:label xml:lang="en">Request</rdfs:label>
        <skos:definition xml:lang="en">A Policy that proposes a Rule over an Asset from an assignee.</skos:definition>
        <skos:note xml:lang="en">A Request Policy  MUST contain a target Asset, a Party with Assignee function, and at least one of a Permission or Prohibition rule. The Request MAY also contain the Party with Assigner function if this is known. No privileges are granted to any Party.</skos:note>
        <skos:scopeNote xml:lang="en">Non-Normative</skos:scopeNote>
    </rdf:Description>
    <rdf:Description rdf:about="http://www.w3.org/ns/odrl/2/RightOperand">
        <rdfs:isDefinedBy rdf:resource="http://www.w3.org/ns/odrl/2/"/>
        <rdfs:label xml:lang="en">Right Operand</rdfs:label>
        <skos:definition xml:lang="en">Right operand for constraint expression.</skos:definition>
        <skos:note xml:lang="en">Instances of the RightOperand class are used as the rightOperand of a Constraint.</skos:note>
    </rdf:Description>
    <rdf:Description rdf:about="http://www.w3.org/ns/odrl/2/Rule">
        <rdfs:isDefinedBy rdf:resource="http://www.w3.org/ns/odrl/2/"/>
        <rdfs:label xml:lang="en">Rule</rdfs:label>
        <skos:definition xml:lang="en">An abstract concept that represents the common characteristics of Permissions, Prohibitions, and Duties.</skos:definition>
        <skos:note xml:lang="en">Rule is an abstract concept.</skos:note>
    </rdf:Description>
    <rdf:Description rdf:about="http://www.w3.org/ns/odrl/2/Set">
        <rdfs:isDefinedBy rdf:resource="http://www.w3.org/ns/odrl/2/"/>
        <rdfs:label xml:lang="en">Set</rdfs:label>
        <skos:definition xml:lang="en">A Policy that expresses a Rule over an Asset.</skos:definition>
        <skos:note xml:lang="en">A Set Policy MUST contain a target Asset, and at least one Rule. A Set Policy is the default Policy subclass. The Set is aimed at scenarios where there is an open criteria for the semantics of the policy expressions and typically refined by other systems/profiles that process the information at a later time. No privileges are granted to any Party (if defined).</skos:note>
    </rdf:Description>
    <rdf:Description rdf:about="http://www.w3.org/ns/odrl/2/Ticket">
        <rdfs:isDefinedBy rdf:resource="http://www.w3.org/ns/odrl/2/"/>
        <rdfs:label xml:lang="en">Ticket</rdfs:label>
        <skos:definition xml:lang="en">A Policy that grants the holder a Rule over an Asset from an assigner.</skos:definition>
        <skos:note xml:lang="en">A Ticket Policy MUST contain a target Asset and at least one of a Permission or Prohibition rule.  The Ticket MAY contain the Party with Assigner function and MUST NOT contain an Assignee. The Ticket Policy will grant the terms of the Policy to the holder of that Ticket. The holder of the Ticket MAY remain unknown or MAY have to be identified at some later stage.</skos:note>
        <skos:scopeNote xml:lang="en">Non-Normative</skos:scopeNote>
    </rdf:Description>
    <rdf:Description rdf:about="http://www.w3.org/ns/odrl/2/UndefinedTerm">
        <rdfs:isDefinedBy rdf:resource="http://www.w3.org/ns/odrl/2/"/>
        <rdfs:label xml:lang="en">Undefined Term</rdfs:label>
        <owl:deprecated rdf:datatype="http://www.w3.org/2001/XMLSchema#boolean">true</owl:deprecated>
        <skos:definition xml:lang="en">Is used to indicate how to support Actions that are not part of any vocabulary or profile in the policy expression system.</skos:definition>
        <skos:note xml:lang="en">Instances of UndefinedTerm describe strategies for processing unsupported actions.</skos:note>
    </rdf:Description>
    <rdf:Description rdf:about="http://www.w3.org/ns/odrl/2/action">
        <rdfs:isDefinedBy rdf:resource="http://www.w3.org/ns/odrl/2/"/>
        <rdfs:label xml:lang="en">Has Action</rdfs:label>
        <skos:definition xml:lang="en">The operation relating to the Asset for which the Rule is being subjected.</skos:definition>
    </rdf:Description>
    <rdf:Description rdf:about="http://www.w3.org/ns/odrl/2/and">
        <rdfs:isDefinedBy rdf:resource="http://www.w3.org/ns/odrl/2/"/>
        <rdfs:label xml:lang="en">And</rdfs:label>
        <skos:definition xml:lang="en">The relation is satisfied when all of the Constraints are satisfied.</skos:definition>
        <skos:note xml:lang="en">This property MUST only be used for Logical Constraints, and the list of operand values MUST be Constraint instances.</skos:note>
    </rdf:Description>
    <rdf:Description rdf:about="http://www.w3.org/ns/odrl/2/andSequence">
        <rdfs:isDefinedBy rdf:resource="http://www.w3.org/ns/odrl/2/"/>
        <rdfs:label xml:lang="en">And Sequence</rdfs:label>
        <skos:definition xml:lang="en">The relation is satisfied when each of the Constraints are satisfied in the order specified.</skos:definition>
        <skos:note xml:lang="en">This property MUST only be used for Logical Constraints, and the list of operand values MUST be Constraint instances. The order of the list MUST be preserved. The andSequence operator is an example where there may be temporal conditional requirements between the operands. This may lead to situations where the outcome is unresolvable, such as deadlock if one of the Constraints is unable to be satisfied. ODRL Processing systems SHOULD plan for these scenarios and implement mechanisms to resolve them.</skos:note>
    </rdf:Description>
    <rdf:Description rdf:about="http://www.w3.org/ns/odrl/2/assignee">
        <rdfs:isDefinedBy rdf:resource="http://www.w3.org/ns/odrl/2/"/>
        <rdfs:label xml:lang="en">Assignee</rdfs:label>
        <skos:definition xml:lang="en">The Party is the recipient of the Rule.</skos:definition>
    </rdf:Description>
    <rdf:Description rdf:about="http://www.w3.org/ns/odrl/2/assigneeOf">
        <rdfs:isDefinedBy rdf:resource="http://www.w3.org/ns/odrl/2/"/>
        <rdfs:label xml:lang="en">Assignee Of</rdfs:label>
        <skos:definition xml:lang="en">Identifies an ODRL Policy for which the identified Party undertakes the assignee functional role.</skos:definition>
        <skos:note xml:lang="en">When assigneeOf has been asserted between a metadata expression and an ODRL Policy, the Party being identified MUST be inferred to undertake the assignee functional role of all the Rules of that Policy.</skos:note>
    </rdf:Description>
    <rdf:Description rdf:about="http://www.w3.org/ns/odrl/2/assigner">
        <rdfs:isDefinedBy rdf:resource="http://www.w3.org/ns/odrl/2/"/>
        <rdfs:label xml:lang="en">Assigner</rdfs:label>
        <skos:definition xml:lang="en">The Party is the issuer of the Rule.</skos:definition>
    </rdf:Description>
    <rdf:Description rdf:about="http://www.w3.org/ns/odrl/2/assignerOf">
        <rdfs:isDefinedBy rdf:resource="http://www.w3.org/ns/odrl/2/"/>
        <rdfs:label xml:lang="en">Assigner Of</rdfs:label>
        <skos:definition xml:lang="en">Identifies an ODRL Policy for which the identified Party undertakes the assigner functional role.</skos:definition>
        <skos:note xml:lang="en">When assignerOf has been asserted between a metadata expression and an ODRL Policy, the Party being identified MUST be inferred to undertake the assigner functional role of all the Rules of that Policy.</skos:note>
    </rdf:Description>
    <rdf:Description rdf:about="http://www.w3.org/ns/odrl/2/attributedParty">
        <rdfs:isDefinedBy rdf:resource="http://www.w3.org/ns/odrl/2/"/>
        <rdfs:label xml:lang="en">Attributed Party</rdfs:label>
        <skos:definition xml:lang="en">The Party to be attributed.</skos:definition>
        <skos:note xml:lang="en">Maybe specified as part of the attribute action.</skos:note>
        <skos:scopeNote xml:lang="en">Non-Normative</skos:scopeNote>
    </rdf:Description>
    <rdf:Description rdf:about="http://www.w3.org/ns/odrl/2/attributingParty">
        <rdfs:isDefinedBy rdf:resource="http://www.w3.org/ns/odrl/2/"/>
        <rdfs:label xml:lang="en">Attributing Party</rdfs:label>
        <skos:definition xml:lang="en">The Party who undertakes the attribution.</skos:definition>
        <skos:note xml:lang="en">Maybe specified as part of the attribute action.</skos:note>
        <skos:scopeNote xml:lang="en">Non-Normative</skos:scopeNote>
    </rdf:Description>
    <rdf:Description rdf:about="http://www.w3.org/ns/odrl/2/compensatedParty">
        <rdfs:isDefinedBy rdf:resource="http://www.w3.org/ns/odrl/2/"/>
        <rdfs:label xml:lang="en">Compensated Party</rdfs:label>
        <skos:definition xml:lang="en">The Party is the recipient of the compensation.</skos:definition>
        <skos:note xml:lang="en">Maybe specified as part of the compensate duty action.</skos:note>
        <skos:scopeNote xml:lang="en">Non-Normative</skos:scopeNote>
    </rdf:Description>
    <rdf:Description rdf:about="http://www.w3.org/ns/odrl/2/compensatingParty">
        <rdfs:isDefinedBy rdf:resource="http://www.w3.org/ns/odrl/2/"/>
        <rdfs:label xml:lang="en">Compensating Party</rdfs:label>
        <skos:definition xml:lang="en">The Party that is the provider of the compensation.</skos:definition>
        <skos:note xml:lang="en">Maybe specified as part of the compensate duty action.</skos:note>
        <skos:scopeNote xml:lang="en">Non-Normative</skos:scopeNote>
    </rdf:Description>
    <rdf:Description rdf:about="http://www.w3.org/ns/odrl/2/conflict">
        <rdfs:isDefinedBy rdf:resource="http://www.w3.org/ns/odrl/2/"/>
        <rdfs:label xml:lang="en">Handle Policy Conflicts</rdfs:label>
        <skos:definition xml:lang="en">The conflict-resolution strategy for a Policy.</skos:definition>
        <skos:note xml:lang="en">If no strategy is specified, the default is invalid.</skos:note>
    </rdf:Description>
    <rdf:Description rdf:about="http://www.w3.org/ns/odrl/2/consentedParty">
        <rdfs:isDefinedBy rdf:resource="http://www.w3.org/ns/odrl/2/"/>
        <rdfs:label xml:lang="en">Consented Party</rdfs:label>
        <skos:definition xml:lang="en">The Party who obtains the consent.</skos:definition>
        <skos:note xml:lang="en">Maybe specified as part of the obtainConsent action.</skos:note>
        <skos:scopeNote xml:lang="en">Non-Normative</skos:scopeNote>
    </rdf:Description>
    <rdf:Description rdf:about="http://www.w3.org/ns/odrl/2/consentingParty">
        <rdfs:isDefinedBy rdf:resource="http://www.w3.org/ns/odrl/2/"/>
        <rdfs:label xml:lang="en">Consenting Party</rdfs:label>
        <skos:definition xml:lang="en">The Party to obtain consent from.</skos:definition>
        <skos:note xml:lang="en">Maybe specified as part of the obtainConsent action.</skos:note>
        <skos:scopeNote xml:lang="en">Non-Normative</skos:scopeNote>
    </rdf:Description>
    <rdf:Description rdf:about="http://www.w3.org/ns/odrl/2/consequence">
        <rdfs:isDefinedBy rdf:resource="http://www.w3.org/ns/odrl/2/"/>
        <rdfs:label xml:lang="en">Consequence</rdfs:label>
        <skos:definition xml:lang="en">Relates a Duty to another Duty, the latter being a consequence of not fulfilling the former.</skos:definition>
        <skos:note xml:lang="en">The consequence property is utilised to express the repercussions of not fulfilling an agreed Policy obligation or duty for a Permission. If either of these fails to be fulfilled, then this will result in the consequence Duty also becoming a new requirement, meaning that the original obligation or duty, as well as the consequence Duty must all be fulfilled</skos:note>
    </rdf:Description>
    <rdf:Description rdf:about="http://www.w3.org/ns/odrl/2/constraint">
        <rdfs:isDefinedBy rdf:resource="http://www.w3.org/ns/odrl/2/"/>
        <rdfs:label xml:lang="en">Has Constraint</rdfs:label>
        <skos:definition xml:lang="en">Constraint applied to a Rule</skos:definition>
        <skos:note xml:lang="en">Constraints on Rules are used to determine if a rule is Active or not. Example: the Permission rule is only active during the year 2018.</skos:note>
    </rdf:Description>
    <rdf:Description rdf:about="http://www.w3.org/ns/odrl/2/contractedParty">
        <rdfs:isDefinedBy rdf:resource="http://www.w3.org/ns/odrl/2/"/>
        <rdfs:label xml:lang="en">Contracted Party</rdfs:label>
        <skos:definition xml:lang="en">The Party who is being contracted.</skos:definition>
        <skos:scopeNote xml:lang="en">Non-Normative</skos:scopeNote>
    </rdf:Description>
    <rdf:Description rdf:about="http://www.w3.org/ns/odrl/2/contractingParty">
        <rdfs:isDefinedBy rdf:resource="http://www.w3.org/ns/odrl/2/"/>
        <rdfs:label xml:lang="en">Contracting Party</rdfs:label>
        <skos:definition xml:lang="en">The Party who is offering the contract.</skos:definition>
        <skos:scopeNote xml:lang="en">Non-Normative</skos:scopeNote>
    </rdf:Description>
    <rdf:Description rdf:about="http://www.w3.org/ns/odrl/2/dataType">
        <rdfs:isDefinedBy rdf:resource="http://www.w3.org/ns/odrl/2/"/>
        <rdfs:label xml:lang="en">Datatype</rdfs:label>
        <skos:definition xml:lang="en">The datatype of the value of the rightOperand or rightOperandReference of a Constraint.</skos:definition>
        <skos:note xml:lang="en">In RDF encodings, use of the rdf:datatype MUST be used. In JSON-LD encoding, the use of @type MUST be used.</skos:note>
    </rdf:Description>
    <rdf:Description rdf:about="http://www.w3.org/ns/odrl/2/duty">
        <rdfs:isDefinedBy rdf:resource="http://www.w3.org/ns/odrl/2/"/>
        <rdfs:label xml:lang="en">Has Duty</rdfs:label>
        <skos:definition xml:lang="en">Relates an individual Duty to a Permission.</skos:definition>
        <skos:note xml:lang="en">A Duty is a pre-condition which must be fulfilled in order to receive the Permission.</skos:note>
    </rdf:Description>
    <rdf:Description rdf:about="http://www.w3.org/ns/odrl/2/failure">
        <rdfs:isDefinedBy rdf:resource="http://www.w3.org/ns/odrl/2/"/>
        <rdfs:label xml:lang="en">Failure</rdfs:label>
        <skos:definition xml:lang="en">Failure is an abstract property that defines the violation (or unmet) relationship between Rules.</skos:definition>
        <skos:note xml:lang="en">The parent property to sub-properties that express explicit failure contexts.</skos:note>
    </rdf:Description>
    <rdf:Description rdf:about="http://www.w3.org/ns/odrl/2/function">
        <rdfs:isDefinedBy rdf:resource="http://www.w3.org/ns/odrl/2/"/>
        <rdfs:label xml:lang="en">Function</rdfs:label>
        <skos:definition xml:lang="en">Function is an abstract property whose sub-properties define the functional roles which may be fulfilled by a party in relation to a Rule.</skos:definition>
    </rdf:Description>
    <rdf:Description rdf:about="http://www.w3.org/ns/odrl/2/hasPolicy">
        <rdfs:isDefinedBy rdf:resource="http://www.w3.org/ns/odrl/2/"/>
        <rdfs:label xml:lang="en">Target Policy</rdfs:label>
        <skos:definition xml:lang="en">Identifies an ODRL Policy for which the identified Asset is the target Asset to all the Rules.</skos:definition>
        <skos:note xml:lang="en">The Asset being identified MUST be inferred to be the target Asset of all of the Rules of the Policy.</skos:note>
    </rdf:Description>
    <rdf:Description rdf:about="http://www.w3.org/ns/odrl/2/implies">
        <rdfs:isDefinedBy rdf:resource="http://www.w3.org/ns/odrl/2/"/>
        <rdfs:label xml:lang="en">Implies</rdfs:label>
        <skos:definition xml:lang="en">An Action asserts that another Action is not prohibited to enable its operational semantics.</skos:definition>
        <skos:note xml:lang="en">The property asserts that an instance of Action entails that the other instance of Action is not prohibited.</skos:note>
    </rdf:Description>
    <rdf:Description rdf:about="http://www.w3.org/ns/odrl/2/includedIn">
        <rdfs:isDefinedBy rdf:resource="http://www.w3.org/ns/odrl/2/"/>
        <rdfs:label xml:lang="en">Included In</rdfs:label>
        <skos:definition xml:lang="en">An Action transitively asserts that another Action that encompasses its operational semantics.</skos:definition>
        <skos:note xml:lang="en">The purpose is to explicitly assert that the semantics of the referenced instance of an other Action encompasses (includes) the semantics of this instance of Action. The includedIn property is transitive, and as such, the Actions form ancestor relationships.</skos:note>
    </rdf:Description>
    <rdf:Description rdf:about="http://www.w3.org/ns/odrl/2/informedParty">
        <rdfs:isDefinedBy rdf:resource="http://www.w3.org/ns/odrl/2/"/>
        <rdfs:label xml:lang="en">Informed Party</rdfs:label>
        <skos:definition xml:lang="en">The Party to be informed of all uses.</skos:definition>
        <skos:note xml:lang="en">Maybe specified as part of the inform action.</skos:note>
        <skos:scopeNote xml:lang="en">Non-Normative</skos:scopeNote>
    </rdf:Description>
    <rdf:Description rdf:about="http://www.w3.org/ns/odrl/2/inheritFrom">
        <rdfs:isDefinedBy rdf:resource="http://www.w3.org/ns/odrl/2/"/>
        <rdfs:label xml:lang="en">Inherits From</rdfs:label>
        <skos:definition xml:lang="en">Relates a (child) policy to another (parent) policy from which terms are inherited.</skos:definition>
        <skos:note xml:lang="en">The child policy will inherit Rules from the parent policy</skos:note>
    </rdf:Description>
    <rdf:Description rdf:about="http://www.w3.org/ns/odrl/2/leftOperand">
        <rdfs:isDefinedBy rdf:resource="http://www.w3.org/ns/odrl/2/"/>
        <rdfs:label xml:lang="en">Has Left Operand</rdfs:label>
        <skos:definition xml:lang="en">The left operand in a constraint expression.</skos:definition>
    </rdf:Description>
    <rdf:Description rdf:about="http://www.w3.org/ns/odrl/2/obligation">
        <rdfs:isDefinedBy rdf:resource="http://www.w3.org/ns/odrl/2/"/>
        <rdfs:label xml:lang="en">Obligation</rdfs:label>
        <skos:definition xml:lang="en">Relates an individual Duty to a Policy.</skos:definition>
        <skos:note xml:lang="en">The Duty is a requirement which must be fulfilled.</skos:note>
    </rdf:Description>
    <rdf:Description rdf:about="http://www.w3.org/ns/odrl/2/operand">
        <rdfs:isDefinedBy rdf:resource="http://www.w3.org/ns/odrl/2/"/>
        <rdfs:label xml:lang="en">Operand</rdfs:label>
        <skos:definition xml:lang="en">Operand is an abstract property for a logical relationship.</skos:definition>
        <skos:note xml:lang="en">Sub-properties of operand are used for Logical Constraints.</skos:note>
    </rdf:Description>
    <rdf:Description rdf:about="http://www.w3.org/ns/odrl/2/operator">
        <rdfs:isDefinedBy rdf:resource="http://www.w3.org/ns/odrl/2/"/>
        <rdfs:label xml:lang="en">Has Operator</rdfs:label>
        <skos:definition xml:lang="en">The operator function applied to operands of a Constraint</skos:definition>
    </rdf:Description>
    <rdf:Description rdf:about="http://www.w3.org/ns/odrl/2/or">
        <rdfs:isDefinedBy rdf:resource="http://www.w3.org/ns/odrl/2/"/>
        <rdfs:label xml:lang="en">Or</rdfs:label>
        <skos:definition xml:lang="en">The relation is satisfied when at least one of the Constraints is satisfied.</skos:definition>
        <skos:note xml:lang="en">This property MUST only be used for Logical Constraints, and the list of operand values MUST be Constraint instances.</skos:note>
    </rdf:Description>
    <rdf:Description rdf:about="http://www.w3.org/ns/odrl/2/output">
        <rdfs:isDefinedBy rdf:resource="http://www.w3.org/ns/odrl/2/"/>
        <rdfs:label xml:lang="en">Output</rdfs:label>
        <skos:definition xml:lang="en">The output property specifies the Asset which is created from the output of the Action.</skos:definition>
        <skos:scopeNote xml:lang="en">Non-Normative</skos:scopeNote>
    </rdf:Description>
    <rdf:Description rdf:about="http://www.w3.org/ns/odrl/2/partOf">
        <rdfs:isDefinedBy rdf:resource="http://www.w3.org/ns/odrl/2/"/>
        <rdfs:label xml:lang="en">Part Of</rdfs:label>
        <skos:definition xml:lang="en">Identifies an Asset/PartyCollection that the Asset/Party is a member of.</skos:definition>
    </rdf:Description>
    <rdf:Description rdf:about="http://www.w3.org/ns/odrl/2/permission">
        <rdfs:isDefinedBy rdf:resource="http://www.w3.org/ns/odrl/2/"/>
        <rdfs:label xml:lang="en">Has Permission</rdfs:label>
        <skos:definition xml:lang="en">Relates an individual Permission to a Policy.</skos:definition>
    </rdf:Description>
    <rdf:Description rdf:about="http://www.w3.org/ns/odrl/2/prohibition">
        <rdfs:isDefinedBy rdf:resource="http://www.w3.org/ns/odrl/2/"/>
        <rdfs:label xml:lang="en">Has Prohibition</rdfs:label>
        <skos:definition xml:lang="en">Relates an individual Prohibition to a Policy.</skos:definition>
    </rdf:Description>
    <rdf:Description rdf:about="http://www.w3.org/ns/odrl/2/refinement">
        <rdfs:isDefinedBy rdf:resource="http://www.w3.org/ns/odrl/2/"/>
        <rdfs:label xml:lang="en">Refinement</rdfs:label>
        <skos:definition xml:lang="en">Constraint used to refine the semantics of an Action, or Party/Asset Collection</skos:definition>
        <skos:note xml:lang="en">Example: the Action print is only permitted on 50% of the asset.</skos:note>
    </rdf:Description>
    <rdf:Description rdf:about="http://www.w3.org/ns/odrl/2/relation">
        <rdfs:isDefinedBy rdf:resource="http://www.w3.org/ns/odrl/2/"/>
        <rdfs:label xml:lang="en">Relation</rdfs:label>
        <skos:definition xml:lang="en">Relation is an abstract property which creates an explicit link between an Action and an Asset.</skos:definition>
        <skos:note xml:lang="en">Sub-properties of relation are used to define the nature of that link.</skos:note>
    </rdf:Description>
    <rdf:Description rdf:about="http://www.w3.org/ns/odrl/2/remedy">
        <rdfs:isDefinedBy rdf:resource="http://www.w3.org/ns/odrl/2/"/>
        <rdfs:label xml:lang="en">Remedy</rdfs:label>
        <skos:definition xml:lang="en">Relates an individual remedy Duty to a Prohibition.</skos:definition>
        <skos:note xml:lang="en">The remedy property expresses an agreed Duty that must be fulfilled in case that a Prohibition has been violated by being exercised.</skos:note>
    </rdf:Description>
    <rdf:Description rdf:about="http://www.w3.org/ns/odrl/2/rightOperand">
        <rdfs:isDefinedBy rdf:resource="http://www.w3.org/ns/odrl/2/"/>
        <rdfs:label xml:lang="en">Has Right Operand</rdfs:label>
        <skos:definition xml:lang="en">The value of the right operand in a constraint expression.</skos:definition>
        <skos:note xml:lang="en">When used with set-based operators, a list of values may be used.</skos:note>
    </rdf:Description>
    <rdf:Description rdf:about="http://www.w3.org/ns/odrl/2/target">
        <rdfs:isDefinedBy rdf:resource="http://www.w3.org/ns/odrl/2/"/>
        <rdfs:label xml:lang="en">Target</rdfs:label>
        <skos:definition xml:lang="en">The target property indicates the Asset that is the primary subject to which the Rule action directly applies.</skos:definition>
    </rdf:Description>
    <rdf:Description rdf:about="http://www.w3.org/ns/odrl/2/trackedParty">
        <rdfs:isDefinedBy rdf:resource="http://www.w3.org/ns/odrl/2/"/>
        <rdfs:label xml:lang="en">Tracked Party</rdfs:label>
        <skos:definition xml:lang="en">The Party whose usage is being tracked.</skos:definition>
        <skos:note xml:lang="en">May be specified as part of the acceptTracking action.</skos:note>
        <skos:scopeNote xml:lang="en">Non-Normative</skos:scopeNote>
    </rdf:Description>
    <rdf:Description rdf:about="http://www.w3.org/ns/odrl/2/trackingParty">
        <rdfs:isDefinedBy rdf:resource="http://www.w3.org/ns/odrl/2/"/>
        <rdfs:label xml:lang="en">Tracking Party</rdfs:label>
        <skos:definition xml:lang="en">The Party who is tracking usage.</skos:definition>
        <skos:note xml:lang="en">May be specified as part of the acceptTracking action.</skos:note>
        <skos:scopeNote xml:lang="en">Non-Normative</skos:scopeNote>
    </rdf:Description>
    <rdf:Description rdf:about="http://www.w3.org/ns/odrl/2/xone">
        <rdfs:isDefinedBy rdf:resource="http://www.w3.org/ns/odrl/2/"/>
        <rdfs:label xml:lang="en">Only One</rdfs:label>
        <skos:definition xml:lang="en">The relation is satisfied when only one, and not more, of the Constaints is satisfied</skos:definition>
        <skos:note xml:lang="en">This property MUST only be used for Logical Constraints, and the list of operand values MUST be Constraint instances.</skos:note>
    </rdf:Description>
</rdf:RDF>



<!-- Generated by the OWL API (version 4.5.29) https://github.com/owlcs/owlapi -->

